<?xml version="1.0" encoding="utf-8"?>
<rdf:RDF
   xmlns:ex="http://transience.eu/ontologies/"
   xmlns:rdf="http://www.w3.org/1999/02/22-rdf-syntax-ns#"
   xmlns:rdfs="http://www.w3.org/2000/01/rdf-schema#"
>
  <rdf:Description rdf:about="http://transience.eu/ontologies/Efficiency_Electricity_Biomass_w__CCS">
    <rdf:type rdf:resource="http://www.w3.org/2002/07/owl#Class"/>
    <rdfs:subClassOf rdf:resource="http://transience.eu/ontologies/Variable"/>
    <rdfs:label>Efficiency|Electricity|Biomass|w/ CCS</rdfs:label>
    <rdfs:comment>Conversion efficiency (electricity produced per unit of primary energy input) of a new biomass power plant with CCS. The efficiency should refer to the plant type(s) for which capital costs have been reported. If capital cost for more than one plant type has been reported, modellers should report efficiency for the additional plant types by adding variables Efficiency|Electricity| Biomass|w/ CCS|2, ... Efficiency|Electricity|Biomass|w/ CCS|N (matching the assignment of plant types to technologies in the reporting of capital costs as documented in the comments sheet). </rdfs:comment>
    <ex:unit>%</ex:unit>
  </rdf:Description>
  <rdf:Description rdf:about="http://transience.eu/ontologies/Production_Non-Metallic_Minerals_Limestone_Volume">
    <rdf:type rdf:resource="http://www.w3.org/2002/07/owl#Class"/>
    <rdfs:subClassOf rdf:resource="http://transience.eu/ontologies/Variable"/>
    <rdfs:label>Production|Non-Metallic Minerals|Limestone|Volume</rdfs:label>
    <rdfs:comment>production of limestone (raw material for the production of cement)</rdfs:comment>
    <ex:unit>Mt/yr</ex:unit>
  </rdf:Description>
  <rdf:Description rdf:about="http://transience.eu/ontologies/OM_Cost_Fixed_Liquids_Oil">
    <rdf:type rdf:resource="http://www.w3.org/2002/07/owl#Class"/>
    <rdfs:subClassOf rdf:resource="http://transience.eu/ontologies/Variable"/>
    <rdfs:label>OM Cost|Fixed|Liquids|Oil</rdfs:label>
    <rdfs:comment>Annual fixed operation &amp; maintainance cost of a new oil refining plant. If more than one refinery technology is modelled, modellers should report fixed O&amp;M costs  for each represented refinery technology by adding variables OM Cost|Fixed|Liquids|Oil|2, ... OM Cost|Fixed|Liquids|Oil|N (with N = number of represented technologies) (matching the assignment of plant types to technologies in the reporting of capital costs as documented in the comments sheet).</rdfs:comment>
    <ex:unit>US$2010/kW/yr</ex:unit>
  </rdf:Description>
  <rdf:Description rdf:about="http://transience.eu/ontologies/Trade_Primary_Energy_Coal_Value">
    <rdf:type rdf:resource="http://www.w3.org/2002/07/owl#Class"/>
    <rdfs:subClassOf rdf:resource="http://transience.eu/ontologies/Variable"/>
    <rdfs:label>Trade|Primary Energy|Coal|Value</rdfs:label>
    <rdfs:comment>value of net exports of coal, at the global level these should add up to the trade losses only</rdfs:comment>
    <ex:unit>billion US$2010/yr</ex:unit>
  </rdf:Description>
  <rdf:Description rdf:about="http://transience.eu/ontologies/Total_Scrap_Iron_and_Steel_Other">
    <rdf:type rdf:resource="http://www.w3.org/2002/07/owl#Class"/>
    <rdfs:subClassOf rdf:resource="http://transience.eu/ontologies/Variable"/>
    <rdfs:label>Total Scrap|Iron and Steel|Other</rdfs:label>
    <rdfs:comment>Total potential of iron &amp; steel scrap material as a result of end of life products (before collection)</rdfs:comment>
    <ex:unit>Mt/yr</ex:unit>
  </rdf:Description>
  <rdf:Description rdf:about="http://transience.eu/ontologies/Lifetime_Liquids_Biomass_w_o_CCS">
    <rdf:type rdf:resource="http://www.w3.org/2002/07/owl#Class"/>
    <rdfs:subClassOf rdf:resource="http://transience.eu/ontologies/Variable"/>
    <rdfs:label>Lifetime|Liquids|Biomass|w/o CCS</rdfs:label>
    <rdfs:comment>Lifetime of a new biomass to liquids plant w/o CCS. Lifetime should be calculated by summing all vintages of a  capacity unit (e.g. (1+1+0.9+0.7+0.5) * 10 years = 41 years) or by the e-folding time for exponential capacity depreciation.  The lifetime should refer to the plant type(s) for which capital costs have been reported. If capital cost for more than one plant type has been reported, modellers should report lifetime for the additional plant types by adding variables Lifetime|Liquids|Biomass|w/o CCS|2, ... Lifetime|Liquids|Biomass|w/o CCS|N (matching the assignment of plant types to technologies in the reporting of capital costs as documented in the comments sheet). </rdfs:comment>
    <ex:unit>years</ex:unit>
  </rdf:Description>
  <rdf:Description rdf:about="http://transience.eu/ontologies/Capacity_Electricity_Wind_Offshore">
    <rdf:type rdf:resource="http://www.w3.org/2002/07/owl#Class"/>
    <rdfs:subClassOf rdf:resource="http://transience.eu/ontologies/Variable"/>
    <rdfs:label>Capacity|Electricity|Wind|Offshore</rdfs:label>
    <rdfs:comment>Total installed (available) capacity of offshore wind power plants. The installed (available) capacity of offshore wind power plants by plant type for which capital costs are reported should be reported by adding variables Capacity|Electricity|Wind|Offshore|1, ..., Capacity|Electricity|Wind|Offshore|N (matching the assignment of plant types to technologies in the reporting of capital costs as documented in the comments sheet). </rdfs:comment>
    <ex:unit>GW</ex:unit>
  </rdf:Description>
  <rdf:Description rdf:about="http://transience.eu/ontologies/Final_Energy_Industry_Iron_and_Steel">
    <rdf:type rdf:resource="http://www.w3.org/2002/07/owl#Class"/>
    <rdfs:subClassOf rdf:resource="http://transience.eu/ontologies/Variable"/>
    <rdfs:label>Final Energy|Industry|Iron and Steel</rdfs:label>
    <rdfs:comment>Final energy consumed by the iron and steel sector, excluding feedstocks</rdfs:comment>
    <ex:unit>EJ/yr</ex:unit>
  </rdf:Description>
  <rdf:Description rdf:about="http://transience.eu/ontologies/Final_Energy_Industry_Chemicals_Geothermal">
    <rdf:type rdf:resource="http://www.w3.org/2002/07/owl#Class"/>
    <rdfs:subClassOf rdf:resource="http://transience.eu/ontologies/Variable"/>
    <rdfs:label>Final Energy|Industry|Chemicals|Geothermal</rdfs:label>
    <rdfs:comment>Final energy consumption of geothermal heat by the chemicals sector</rdfs:comment>
    <ex:unit>EJ/yr</ex:unit>
  </rdf:Description>
  <rdf:Description rdf:about="http://transience.eu/ontologies/Secondary_Energy_Hydrogen_Coal_w_o_CCS">
    <rdf:type rdf:resource="http://www.w3.org/2002/07/owl#Class"/>
    <rdfs:subClassOf rdf:resource="http://transience.eu/ontologies/Variable"/>
    <rdfs:label>Secondary Energy|Hydrogen|Coal|w/o CCS</rdfs:label>
    <rdfs:comment>hydrogen production from coal with freely vented CO2 emissions</rdfs:comment>
    <ex:unit>EJ/yr</ex:unit>
  </rdf:Description>
  <rdf:Description rdf:about="http://transience.eu/ontologies/Efficiency_Liquids_Coal_w__CCS">
    <rdf:type rdf:resource="http://www.w3.org/2002/07/owl#Class"/>
    <rdfs:subClassOf rdf:resource="http://transience.eu/ontologies/Variable"/>
    <rdfs:label>Efficiency|Liquids|Coal|w/ CCS</rdfs:label>
    <rdfs:comment>Conversion efficiency (energy content of liquids produced per unit of primary energy input) of a new coal to liquids plant with CCS. The efficiency should refer to the plant type(s) for which capital costs have been reported. If capital cost for more than one plant type has been reported, modellers should report efficiency for the additional plant types by adding variables Efficiency|Liquids|Coal|w/ CCS|2, ... Efficiency|Liquids|Coal|w/ CCS|N (matching the assignment of plant types to technologies in the reporting of capital costs as documented in the comments sheet). </rdfs:comment>
    <ex:unit>%</ex:unit>
  </rdf:Description>
  <rdf:Description rdf:about="http://transience.eu/ontologies/Investment_Energy_Supply_Liquids">
    <rdf:type rdf:resource="http://www.w3.org/2002/07/owl#Class"/>
    <rdfs:subClassOf rdf:resource="http://transience.eu/ontologies/Variable"/>
    <rdfs:label>Investment|Energy Supply|Liquids</rdfs:label>
    <rdfs:comment>investments for the production of liquid fuels. For plants equipped with CCS, the investment in the capturing equipment should be included but not the one on transport and storage.</rdfs:comment>
    <ex:unit>billion US$2010/yr</ex:unit>
  </rdf:Description>
  <rdf:Description rdf:about="http://transience.eu/ontologies/Carbon_Capture_Storage_Fossil_Energy_Supply">
    <rdf:type rdf:resource="http://www.w3.org/2002/07/owl#Class"/>
    <rdfs:subClassOf rdf:resource="http://transience.eu/ontologies/Variable"/>
    <rdfs:label>Carbon Capture|Storage|Fossil|Energy|Supply</rdfs:label>
    <rdfs:comment>total carbon dioxide emissions captured from fossil fuel use in energy supply (IPCC category 1A) and stored in geological deposits (e.g. in depleted oil and gas fields, unmined coal seams, saline aquifers) and the deep ocean, stored amounts should be reported as positive numbers</rdfs:comment>
    <ex:unit>Mt CO2/yr</ex:unit>
  </rdf:Description>
  <rdf:Description rdf:about="http://transience.eu/ontologies/Final_Energy_Non-Energy_Use_Gases_Electricity">
    <rdf:type rdf:resource="http://www.w3.org/2002/07/owl#Class"/>
    <rdfs:subClassOf rdf:resource="http://transience.eu/ontologies/Variable"/>
    <rdfs:label>Final Energy|Non-Energy Use|Gases|Electricity</rdfs:label>
    <rdfs:comment>Final energy consumption of synthetic e-fuel gas ("power-to-gas") by the non-combustion processes</rdfs:comment>
    <ex:unit>EJ/yr</ex:unit>
  </rdf:Description>
  <rdf:Description rdf:about="http://transience.eu/ontologies/Final_Energy_Industry_Chemicals_Hydrogen">
    <rdf:type rdf:resource="http://www.w3.org/2002/07/owl#Class"/>
    <rdfs:subClassOf rdf:resource="http://transience.eu/ontologies/Variable"/>
    <rdfs:label>Final Energy|Industry|Chemicals|Hydrogen</rdfs:label>
    <rdfs:comment>Final energy consumption of hydrogen by the chemicals sector</rdfs:comment>
    <ex:unit>EJ/yr</ex:unit>
  </rdf:Description>
  <rdf:Description rdf:about="http://transience.eu/ontologies/Final_Energy_Industry_Other_Sector_Geothermal">
    <rdf:type rdf:resource="http://www.w3.org/2002/07/owl#Class"/>
    <rdfs:subClassOf rdf:resource="http://transience.eu/ontologies/Variable"/>
    <rdfs:label>Final Energy|Industry|Other Sector|Geothermal</rdfs:label>
    <rdfs:comment>Final energy consumption of geothermal heat by other industry sectors</rdfs:comment>
    <ex:unit>EJ/yr</ex:unit>
  </rdf:Description>
  <rdf:Description rdf:about="http://transience.eu/ontologies/OM_Cost_Fixed_Electricity_Biomass_w_o_CCS">
    <rdf:type rdf:resource="http://www.w3.org/2002/07/owl#Class"/>
    <rdfs:subClassOf rdf:resource="http://transience.eu/ontologies/Variable"/>
    <rdfs:label>OM Cost|Fixed|Electricity|Biomass|w/o CCS</rdfs:label>
    <rdfs:comment>Annual fixed operation &amp; maintainance cost of a new biomass power plant w/o CCS. If more than one biomass power technology is modelled, modellers should report fixed O&amp;M costs  for each represented biomass power technology by adding variables OM Cost|Fixed|Electricity|Biomass|w/o CCS|2, ... OM Cost|Fixed|Electricity|Biomass|w/o CCS|N (with N = number of represented technologies) (matching the assignment of plant types to technologies in the reporting of capital costs as documented in the comments sheet).</rdfs:comment>
    <ex:unit>US$2010/kW/yr</ex:unit>
  </rdf:Description>
  <rdf:Description rdf:about="http://transience.eu/ontologies/Final_Energy_Residential_Gases">
    <rdf:type rdf:resource="http://www.w3.org/2002/07/owl#Class"/>
    <rdfs:subClassOf rdf:resource="http://transience.eu/ontologies/Variable"/>
    <rdfs:label>Final Energy|Residential|Gases</rdfs:label>
    <rdfs:comment>final energy consumption by the residential sector of gases (natural gas, biogas, coal-gas), excluding transmission/distribution losses</rdfs:comment>
    <ex:unit>EJ/yr</ex:unit>
  </rdf:Description>
  <rdf:Description rdf:about="http://transience.eu/ontologies/Primary_Energy_Biomass_Electricity">
    <rdf:type rdf:resource="http://www.w3.org/2002/07/owl#Class"/>
    <rdfs:subClassOf rdf:resource="http://transience.eu/ontologies/Variable"/>
    <rdfs:label>Primary Energy|Biomass|Electricity</rdfs:label>
    <rdfs:comment>primary energy input to electricity generation of purpose-grown bioenergy crops, crop and forestry residue bioenergy, municipal solid waste bioenergy, traditional biomass</rdfs:comment>
    <ex:unit>EJ/yr</ex:unit>
  </rdf:Description>
  <rdf:Description rdf:about="http://transience.eu/ontologies/Final_Energy_Industry_Non-Ferrous_Metals_Geothermal">
    <rdf:type rdf:resource="http://www.w3.org/2002/07/owl#Class"/>
    <rdfs:subClassOf rdf:resource="http://transience.eu/ontologies/Variable"/>
    <rdfs:label>Final Energy|Industry|Non-Ferrous Metals|Geothermal</rdfs:label>
    <rdfs:comment>Final energy consumption of geothermal heat by the non-ferrous metals sector</rdfs:comment>
    <ex:unit>EJ/yr</ex:unit>
  </rdf:Description>
  <rdf:Description rdf:about="http://transience.eu/ontologies/Production_Chemicals_Plastics_Primary_Plastics_Volume">
    <rdf:type rdf:resource="http://www.w3.org/2002/07/owl#Class"/>
    <rdfs:subClassOf rdf:resource="http://transience.eu/ontologies/Variable"/>
    <rdfs:label>Production|Chemicals|Plastics|Primary Plastics|Volume</rdfs:label>
    <rdfs:comment>production of primary plastics </rdfs:comment>
    <ex:unit>Mt/yr</ex:unit>
  </rdf:Description>
  <rdf:Description rdf:about="http://transience.eu/ontologies/Lifetime_Electricity_Biomass_w__CCS">
    <rdf:type rdf:resource="http://www.w3.org/2002/07/owl#Class"/>
    <rdfs:subClassOf rdf:resource="http://transience.eu/ontologies/Variable"/>
    <rdfs:label>Lifetime|Electricity|Biomass|w/ CCS</rdfs:label>
    <rdfs:comment>Lifetime of a new biomass power plant with CCS. Lifetime should be calculated by summing all vintages of a  capacity unit (e.g. (1+1+0.9+0.7+0.5) * 10 years = 41 years) or by the e-folding time for exponential capacity depreciation.  The lifetime should refer to the plant type(s) for which capital costs have been reported. If capital cost for more than one plant type has been reported, modellers should report lifetime for the additional plant types by adding variables Lifetime|Electricity|Biomass|w/ CCS|2, ... Lifetime|Electricity|Biomass|w/ CCS|N (matching the assignment of plant types to technologies in the reporting of capital costs as documented in the comments sheet). </rdfs:comment>
    <ex:unit>years</ex:unit>
  </rdf:Description>
  <rdf:Description rdf:about="http://transience.eu/ontologies/Capital_Stock">
    <rdf:type rdf:resource="http://www.w3.org/2002/07/owl#Class"/>
    <rdfs:subClassOf rdf:resource="http://transience.eu/ontologies/Variable"/>
    <rdfs:label>Capital Stock</rdfs:label>
    <rdfs:comment>Macroeconomic capital stock</rdfs:comment>
    <ex:unit>billion US$2010/yr</ex:unit>
  </rdf:Description>
  <rdf:Description rdf:about="http://transience.eu/ontologies/Production_Steel_DRI_DRI_biogenic_syngas_Volume">
    <rdf:type rdf:resource="http://www.w3.org/2002/07/owl#Class"/>
    <rdfs:subClassOf rdf:resource="http://transience.eu/ontologies/Variable"/>
    <rdfs:label>Production|Steel|DRI|DRI biogenic syngas|Volume</rdfs:label>
    <rdfs:comment>Production of DRI using biogenic syngas as reducing gas (including DRI which is processed into steel)</rdfs:comment>
    <ex:unit>Mt/yr</ex:unit>
  </rdf:Description>
  <rdf:Description rdf:about="http://transience.eu/ontologies/Collected_Scrap_Non-Ferrous_Metals_Residential_and_Commercial">
    <rdf:type rdf:resource="http://www.w3.org/2002/07/owl#Class"/>
    <rdfs:subClassOf rdf:resource="http://transience.eu/ontologies/Variable"/>
    <rdfs:label>Collected Scrap|Non-Ferrous Metals|Residential and Commercial</rdfs:label>
    <rdfs:comment>Collected non-ferrous metals scrap coming from residential and commercial sector (available to be used in recycling)</rdfs:comment>
    <ex:unit>Mt/yr</ex:unit>
  </rdf:Description>
  <rdf:Description rdf:about="http://transience.eu/ontologies/Policy_Cost_Area_under_MAC_Curve">
    <rdf:type rdf:resource="http://www.w3.org/2002/07/owl#Class"/>
    <rdfs:subClassOf rdf:resource="http://transience.eu/ontologies/Variable"/>
    <rdfs:label>Policy Cost|Area under MAC Curve</rdfs:label>
    <rdfs:comment>total costs of the policy, i.e. the area under the Marginal Abatement Cost (MAC) curve</rdfs:comment>
    <ex:unit>billion US$2010/yr</ex:unit>
  </rdf:Description>
  <rdf:Description rdf:about="http://transience.eu/ontologies/Capacity_Petrochemicals_Chemical_Recycling_Pyrolysis">
    <rdf:type rdf:resource="http://www.w3.org/2002/07/owl#Class"/>
    <rdfs:subClassOf rdf:resource="http://transience.eu/ontologies/Variable"/>
    <rdfs:label>Capacity|Petrochemicals|Chemical Recycling|Pyrolysis</rdfs:label>
    <rdfs:comment>Capacity for chemical recycling of plastic wastes via pyrolysis; the value refers to the amount of plastic waste input that can be processed per year</rdfs:comment>
    <ex:unit>Mt plastic waste input / yr</ex:unit>
  </rdf:Description>
  <rdf:Description rdf:about="http://transience.eu/ontologies/Investment_Petrochemicals_Chemical_Reycling">
    <rdf:type rdf:resource="http://www.w3.org/2002/07/owl#Class"/>
    <rdfs:subClassOf rdf:resource="http://transience.eu/ontologies/Variable"/>
    <rdfs:label>Investment|Petrochemicals|Chemical Reycling</rdfs:label>
    <rdfs:comment>Investment in plants for chemical recycling, including both pyrolysis and gasification plants</rdfs:comment>
    <ex:unit>Mio â‚¬_2022/yr</ex:unit>
  </rdf:Description>
  <rdf:Description rdf:about="http://transience.eu/ontologies/Gross_Emissions_CO2_Industrial_Processes">
    <rdf:type rdf:resource="http://www.w3.org/2002/07/owl#Class"/>
    <rdfs:subClassOf rdf:resource="http://transience.eu/ontologies/Variable"/>
    <rdfs:label>Gross Emissions|CO2|Industrial Processes</rdfs:label>
    <rdfs:comment>Gross CO2 emissions from industrial processes (IPCC categories 2A, B, C, E), not accounting for negative emissions from BECCS</rdfs:comment>
    <ex:unit>Mt CO2/yr</ex:unit>
  </rdf:Description>
  <rdf:Description rdf:about="http://transience.eu/ontologies/Trade_Secondary_Energy_Electricity_Value">
    <rdf:type rdf:resource="http://www.w3.org/2002/07/owl#Class"/>
    <rdfs:subClassOf rdf:resource="http://transience.eu/ontologies/Variable"/>
    <rdfs:label>Trade|Secondary Energy|Electricity|Value</rdfs:label>
    <rdfs:comment>value of net exports of electricity, at the global level these should add up to the trade losses only</rdfs:comment>
    <ex:unit>EJ/yr</ex:unit>
  </rdf:Description>
  <rdf:Description rdf:about="http://transience.eu/ontologies/Final_Energy_Industry_Iron_and_Steel_Geothermal">
    <rdf:type rdf:resource="http://www.w3.org/2002/07/owl#Class"/>
    <rdfs:subClassOf rdf:resource="http://transience.eu/ontologies/Variable"/>
    <rdfs:label>Final Energy|Industry|Iron and Steel|Geothermal</rdfs:label>
    <rdfs:comment>Final energy consumption of geothermal heat by the iron and steel sector</rdfs:comment>
    <ex:unit>EJ/yr</ex:unit>
  </rdf:Description>
  <rdf:Description rdf:about="http://transience.eu/ontologies/Carbon_Capture_Storage_Biomass">
    <rdf:type rdf:resource="http://www.w3.org/2002/07/owl#Class"/>
    <rdfs:subClassOf rdf:resource="http://transience.eu/ontologies/Variable"/>
    <rdfs:label>Carbon Capture|Storage|Biomass</rdfs:label>
    <rdfs:comment>total carbon dioxide emissions captured  from bioenergy use and stored in geological deposits (e.g. in depleted oil and gas fields, unmined coal seams, saline aquifers) and the deep ocean, stored amounts should be reported as positive numbers</rdfs:comment>
    <ex:unit>Mt CO2/yr</ex:unit>
  </rdf:Description>
  <rdf:Description rdf:about="http://transience.eu/ontologies/Emissions_CO2_Industry_Petrochemicals">
    <rdf:type rdf:resource="http://www.w3.org/2002/07/owl#Class"/>
    <rdfs:subClassOf rdf:resource="http://transience.eu/ontologies/Variable"/>
    <rdfs:label>Emissions|CO2|Industry|Petrochemicals</rdfs:label>
    <rdfs:comment>Net direct CO2 emissions from petrochemical processes (excluding heat provision), including both fossil and biogenic CO2, after CCS</rdfs:comment>
    <ex:unit>Mt CO2/yr</ex:unit>
  </rdf:Description>
  <rdf:Description rdf:about="http://transience.eu/ontologies/Capacity_Petrochemicals_Organosolv">
    <rdf:type rdf:resource="http://www.w3.org/2002/07/owl#Class"/>
    <rdfs:subClassOf rdf:resource="http://transience.eu/ontologies/Variable"/>
    <rdfs:label>Capacity|Petrochemicals|Organosolv</rdfs:label>
    <rdfs:comment>Capacity for dissolving biomass into cellulose+lignocellulose+lignin via Organosolv process; the value refers to the amount of biomass input that can be processed per year</rdfs:comment>
    <ex:unit>Mt biomass input / yr</ex:unit>
  </rdf:Description>
  <rdf:Description rdf:about="http://transience.eu/ontologies/Emissions_CO2_Energy_Demand_Transportation_(w__bunkers)">
    <rdf:type rdf:resource="http://www.w3.org/2002/07/owl#Class"/>
    <rdfs:subClassOf rdf:resource="http://transience.eu/ontologies/Variable"/>
    <rdfs:label>Emissions|CO2|Energy|Demand|Transportation (w/ bunkers)</rdfs:label>
    <rdfs:comment>Fossil CO2 emissions from fuel combustion in transportation sector (IPCC category 1A3), excluding pipeline emissions (IPCC category 1A3ei), including emissions from international bunkers (IPCC category 1A3ai and 1A3di) </rdfs:comment>
    <ex:unit>Mt CO2/yr</ex:unit>
  </rdf:Description>
  <rdf:Description rdf:about="http://transience.eu/ontologies/Capital_Cost_Electricity_Nuclear">
    <rdf:type rdf:resource="http://www.w3.org/2002/07/owl#Class"/>
    <rdfs:subClassOf rdf:resource="http://transience.eu/ontologies/Variable"/>
    <rdfs:label>Capital Cost|Electricity|Nuclear</rdfs:label>
    <rdfs:comment>Capital cost of a new nuclear power plants. If more than one nuclear power plant technology is modelled (e.g., Gen II, III, IV; LWR, thermal reactors with other moderator materials, fast breeders), modellers should report capital costs for each represented nuclear power technology by adding variables Capital Cost|Electricity|Nuclear|2, ... Capital|Cost|Electricity|Nuclear|N (with N = number of represented nuclear power technologies). It is modeller's choice which nuclear power technologies to assign to type 1 (assigned to the variable without number suffix),2,...,N. The assignment should be documented in the comments sheet. </rdfs:comment>
    <ex:unit>US$2010/kW</ex:unit>
  </rdf:Description>
  <rdf:Description rdf:about="http://transience.eu/ontologies/OM_Cost_Fixed_Hydrogen_Gas_w_o_CCS">
    <rdf:type rdf:resource="http://www.w3.org/2002/07/owl#Class"/>
    <rdfs:subClassOf rdf:resource="http://transience.eu/ontologies/Variable"/>
    <rdfs:label>OM Cost|Fixed|Hydrogen|Gas|w/o CCS</rdfs:label>
    <rdfs:comment>Annual fixed operation &amp; maintainance cost of a new gas to hydrogen plant w/o CCS. If more than one gas to hydrogen technology is modelled, modellers should report fixed O&amp;M costs  for each represented gas to hydrogen technology by adding variables OM Cost|Fixed|Hydrogen|Gas|w/o CCS|2, ... OM Cost|Fixed|Hydrogen|Gas|w/o CCS|N (with N = number of represented technologies) (matching the assignment of plant types to technologies in the reporting of capital costs as documented in the comments sheet).</rdfs:comment>
    <ex:unit>US$2010/kW/yr</ex:unit>
  </rdf:Description>
  <rdf:Description rdf:about="http://transience.eu/ontologies/Secondary_Energy_Heat_Geothermal">
    <rdf:type rdf:resource="http://www.w3.org/2002/07/owl#Class"/>
    <rdfs:subClassOf rdf:resource="http://transience.eu/ontologies/Variable"/>
    <rdfs:label>Secondary Energy|Heat|Geothermal</rdfs:label>
    <rdfs:comment>centralized heat generation from geothermal energy EXCLUDING geothermal heat pumps</rdfs:comment>
    <ex:unit>EJ/yr</ex:unit>
  </rdf:Description>
  <rdf:Description rdf:about="http://transience.eu/ontologies/Capacity_Electricity_Wind_Onshore">
    <rdf:type rdf:resource="http://www.w3.org/2002/07/owl#Class"/>
    <rdfs:subClassOf rdf:resource="http://transience.eu/ontologies/Variable"/>
    <rdfs:label>Capacity|Electricity|Wind|Onshore</rdfs:label>
    <rdfs:comment>Total installed (available) capacity of onshore wind power plants. The installed (available) capacity of onshore wind power plants by plant type for which capital costs are reported should be reported by adding variables Capacity|Electricity|Wind|Onshore|1, ..., Capacity|Electricity|Wind|Onshore|N (matching the assignment of plant types to technologies in the reporting of capital costs as documented in the comments sheet). </rdfs:comment>
    <ex:unit>GW</ex:unit>
  </rdf:Description>
  <rdf:Description rdf:about="http://transience.eu/ontologies/Final_Energy_Non-Energy_Use_Chemicals_Gases_Electricity">
    <rdf:type rdf:resource="http://www.w3.org/2002/07/owl#Class"/>
    <rdfs:subClassOf rdf:resource="http://transience.eu/ontologies/Variable"/>
    <rdfs:label>Final Energy|Non-Energy Use|Chemicals|Gases|Electricity</rdfs:label>
    <rdfs:comment>Final energy consumption of synthetic e-fuel gas ("power-to-gas") by the chemical sector by the non-combustion processes</rdfs:comment>
    <ex:unit>EJ/yr</ex:unit>
  </rdf:Description>
  <rdf:Description rdf:about="http://transience.eu/ontologies/Final_Energy_Commercial_Solids">
    <rdf:type rdf:resource="http://www.w3.org/2002/07/owl#Class"/>
    <rdfs:subClassOf rdf:resource="http://transience.eu/ontologies/Variable"/>
    <rdfs:label>Final Energy|Commercial|Solids</rdfs:label>
    <rdfs:comment>final energy solid fuel consumption by the commercial sector (including coal and solid biomass)</rdfs:comment>
    <ex:unit>EJ/yr</ex:unit>
  </rdf:Description>
  <rdf:Description rdf:about="http://transience.eu/ontologies/Investment_Energy_Supply">
    <rdf:type rdf:resource="http://www.w3.org/2002/07/owl#Class"/>
    <rdfs:subClassOf rdf:resource="http://transience.eu/ontologies/Variable"/>
    <rdfs:label>Investment|Energy Supply</rdfs:label>
    <rdfs:comment>Investments into the energy supply system</rdfs:comment>
    <ex:unit>billion US$2010/yr</ex:unit>
  </rdf:Description>
  <rdf:Description rdf:about="http://transience.eu/ontologies/Final_Energy_Other">
    <rdf:type rdf:resource="http://www.w3.org/2002/07/owl#Class"/>
    <rdfs:subClassOf rdf:resource="http://transience.eu/ontologies/Variable"/>
    <rdfs:label>Final Energy|Other</rdfs:label>
    <rdfs:comment>final energy consumption of other sources that do not fit to any other category (please provide a definition of the sources in this category in the 'comments' tab)</rdfs:comment>
    <ex:unit>EJ/yr</ex:unit>
  </rdf:Description>
  <rdf:Description rdf:about="http://transience.eu/ontologies/Emissions_CO2_Waste_Fossil">
    <rdf:type rdf:resource="http://www.w3.org/2002/07/owl#Class"/>
    <rdfs:subClassOf rdf:resource="http://transience.eu/ontologies/Variable"/>
    <rdfs:label>Emissions|CO2|Waste|Fossil</rdfs:label>
    <rdfs:comment>CO2 emissions from waste of fossil origin</rdfs:comment>
    <ex:unit>Mt CO2/yr</ex:unit>
  </rdf:Description>
  <rdf:Description rdf:about="http://transience.eu/ontologies/Investment_Steel_DRI-EAF_SAF_routes">
    <rdf:type rdf:resource="http://www.w3.org/2002/07/owl#Class"/>
    <rdfs:subClassOf rdf:resource="http://transience.eu/ontologies/Variable"/>
    <rdfs:label>Investment|Steel|DRI-EAF/SAF routes</rdfs:label>
    <rdfs:comment>Investment in DRI routes, including DRI shaft furnaces, electric arc furnaces and electric smelters</rdfs:comment>
    <ex:unit>Mio â‚¬_2022 / year</ex:unit>
  </rdf:Description>
  <rdf:Description rdf:about="http://transience.eu/ontologies/Outflow_Plastics_Recyclate_Types">
    <rdf:type rdf:resource="http://www.w3.org/2002/07/owl#Class"/>
    <rdfs:subClassOf rdf:resource="http://transience.eu/ontologies/ParameterOutput"/>
    <rdfs:label>Outflow|Plastics|Recyclate|[Types]</rdfs:label>
    <rdfs:comment>RecyclatesÂ </rdfs:comment>
    <ex:unit>t/yr</ex:unit>
  </rdf:Description>
  <rdf:Description rdf:about="http://transience.eu/ontologies/Secondary_Energy_Electricity_Gas_w__CCS">
    <rdf:type rdf:resource="http://www.w3.org/2002/07/owl#Class"/>
    <rdfs:subClassOf rdf:resource="http://transience.eu/ontologies/Variable"/>
    <rdfs:label>Secondary Energy|Electricity|Gas|w/ CCS</rdfs:label>
    <rdfs:comment>net electricity production from natural gas with a CO2 capture component</rdfs:comment>
    <ex:unit>EJ/yr</ex:unit>
  </rdf:Description>
  <rdf:Description rdf:about="http://transience.eu/ontologies/Investment_Infrastructure_Residential_and_Commercial_Building_Retrofits">
    <rdf:type rdf:resource="http://www.w3.org/2002/07/owl#Class"/>
    <rdfs:subClassOf rdf:resource="http://transience.eu/ontologies/Variable"/>
    <rdfs:label>Investment|Infrastructure|Residential and Commercial|Building Retrofits</rdfs:label>
    <rdfs:comment>investment into residential and commercial buildings infrastructure (all types of existing buildings that have been retrofitted to become more energy efficient)</rdfs:comment>
    <ex:unit>billion US$2010/yr</ex:unit>
  </rdf:Description>
  <rdf:Description rdf:about="http://transience.eu/ontologies/Final_Energy_Industry_Iron_and_Steel_Waste">
    <rdf:type rdf:resource="http://www.w3.org/2002/07/owl#Class"/>
    <rdfs:subClassOf rdf:resource="http://transience.eu/ontologies/Variable"/>
    <rdfs:label>Final Energy|Industry|Iron and Steel|Waste</rdfs:label>
    <rdfs:comment>Final energy consumption of non-renewable waste by the iron and steel sector</rdfs:comment>
    <ex:unit>EJ/yr</ex:unit>
  </rdf:Description>
  <rdf:Description rdf:about="http://transience.eu/ontologies/Energy_Service_Residential_Floor_Space">
    <rdf:type rdf:resource="http://www.w3.org/2002/07/owl#Class"/>
    <rdfs:subClassOf rdf:resource="http://transience.eu/ontologies/Variable"/>
    <rdfs:label>Energy Service|Residential|Floor Space</rdfs:label>
    <rdfs:comment>energy service demand for conditioned floor space in residential buildings</rdfs:comment>
    <ex:unit>bn m2</ex:unit>
  </rdf:Description>
  <rdf:Description rdf:about="http://transience.eu/ontologies/Price_Final_Energy_Residential_and_Commercial_Electricity">
    <rdf:type rdf:resource="http://www.w3.org/2002/07/owl#Class"/>
    <rdfs:subClassOf rdf:resource="http://transience.eu/ontologies/Variable"/>
    <rdfs:label>Price|Final Energy|Residential and Commercial|Electricity</rdfs:label>
    <rdfs:comment>electricity price at the final level in the residential and commercial sector. Prices should include the effect of carbon prices.</rdfs:comment>
    <ex:unit>US$2010/GJ</ex:unit>
  </rdf:Description>
  <rdf:Description rdf:about="http://transience.eu/ontologies/Subsidies_Energy">
    <rdf:type rdf:resource="http://www.w3.org/2002/07/owl#Class"/>
    <rdfs:subClassOf rdf:resource="http://transience.eu/ontologies/Variable"/>
    <rdfs:label>Subsidies|Energy</rdfs:label>
    <rdfs:comment>Total energy-related subsidies</rdfs:comment>
    <ex:unit>billion US$2010/yr</ex:unit>
  </rdf:Description>
  <rdf:Description rdf:about="http://transience.eu/ontologies/Emissions_CO2_Energy_Demand_Industry_Non-Metallic_Minerals">
    <rdf:type rdf:resource="http://www.w3.org/2002/07/owl#Class"/>
    <rdfs:subClassOf rdf:resource="http://transience.eu/ontologies/Variable"/>
    <rdfs:label>Emissions|CO2|Energy|Demand|Industry|Non-Metallic Minerals</rdfs:label>
    <rdfs:comment>Fossil CO2 emissions from fuel combustion in industry in the non-metallic minerals sector</rdfs:comment>
    <ex:unit>Mt CO2/yr</ex:unit>
  </rdf:Description>
  <rdf:Description rdf:about="http://transience.eu/ontologies/Final_Energy_Industry_Pulp_and_Paper_Solar">
    <rdf:type rdf:resource="http://www.w3.org/2002/07/owl#Class"/>
    <rdfs:subClassOf rdf:resource="http://transience.eu/ontologies/Variable"/>
    <rdfs:label>Final Energy|Industry|Pulp and Paper|Solar</rdfs:label>
    <rdfs:comment>Final energy consumption of solar thermal heat by the pulp and paper sector</rdfs:comment>
    <ex:unit>EJ/yr</ex:unit>
  </rdf:Description>
  <rdf:Description rdf:about="http://transience.eu/ontologies/Final_Energy_Residential_and_Commercial_Gases">
    <rdf:type rdf:resource="http://www.w3.org/2002/07/owl#Class"/>
    <rdfs:subClassOf rdf:resource="http://transience.eu/ontologies/Variable"/>
    <rdfs:label>Final Energy|Residential and Commercial|Gases</rdfs:label>
    <rdfs:comment>final energy consumption by the residential &amp; commercial sector of gases (natural gas, biogas, coal-gas), excluding transmission/distribution losses</rdfs:comment>
    <ex:unit>EJ/yr</ex:unit>
  </rdf:Description>
  <rdf:Description rdf:about="http://transience.eu/ontologies/Final_Energy_Transportation_Gases_Electricity">
    <rdf:type rdf:resource="http://www.w3.org/2002/07/owl#Class"/>
    <rdfs:subClassOf rdf:resource="http://transience.eu/ontologies/Variable"/>
    <rdfs:label>Final Energy|Transportation|Gases|Electricity</rdfs:label>
    <rdfs:comment>final energy consumption by the transportation sector of e-fuel gas ("power-to-gas")</rdfs:comment>
    <ex:unit>EJ/yr</ex:unit>
  </rdf:Description>
  <rdf:Description rdf:about="http://transience.eu/ontologies/Production_Chemicals_Value">
    <rdf:type rdf:resource="http://www.w3.org/2002/07/owl#Class"/>
    <rdfs:subClassOf rdf:resource="http://transience.eu/ontologies/Variable"/>
    <rdfs:label>Production|Chemicals|Value</rdfs:label>
    <rdfs:comment>production of chemicals (e.g. sulfuric acid)</rdfs:comment>
    <ex:unit>billion US$2010/yr</ex:unit>
  </rdf:Description>
  <rdf:Description rdf:about="http://transience.eu/ontologies/Final_Energy_Residential_Solids_Biomass_Traditional">
    <rdf:type rdf:resource="http://www.w3.org/2002/07/owl#Class"/>
    <rdfs:subClassOf rdf:resource="http://transience.eu/ontologies/Variable"/>
    <rdfs:label>Final Energy|Residential|Solids|Biomass|Traditional</rdfs:label>
    <rdfs:comment>final energy solid traditional biomass consumption by the residential sector</rdfs:comment>
    <ex:unit>EJ/yr</ex:unit>
  </rdf:Description>
  <rdf:Description rdf:about="http://transience.eu/ontologies/Secondary_Energy_Hydrogen_Other">
    <rdf:type rdf:resource="http://www.w3.org/2002/07/owl#Class"/>
    <rdfs:subClassOf rdf:resource="http://transience.eu/ontologies/Variable"/>
    <rdfs:label>Secondary Energy|Hydrogen|Other</rdfs:label>
    <rdfs:comment>hydrogen production from other sources that do not fit to any other category (please provide a definition of the sources in this category in the 'comments' tab)</rdfs:comment>
    <ex:unit>EJ/yr</ex:unit>
  </rdf:Description>
  <rdf:Description rdf:about="http://transience.eu/ontologies/Investment_Energy_Supply_Electricity_Coal_w__CCS">
    <rdf:type rdf:resource="http://www.w3.org/2002/07/owl#Class"/>
    <rdfs:subClassOf rdf:resource="http://transience.eu/ontologies/Variable"/>
    <rdfs:label>Investment|Energy Supply|Electricity|Coal|w/ CCS</rdfs:label>
    <rdfs:comment>investments in new power generation for the specified power plant category. If the model features several sub-categories, the total investments should be reported. For plants equipped with CCS, the investment in the capturing equipment should be included but not the one on transport and storage.</rdfs:comment>
    <ex:unit>billion US$2010/yr</ex:unit>
  </rdf:Description>
  <rdf:Description rdf:about="http://transience.eu/ontologies/Emissions_CO2_Energy_Demand_Residential_and_Commercial">
    <rdf:type rdf:resource="http://www.w3.org/2002/07/owl#Class"/>
    <rdfs:subClassOf rdf:resource="http://transience.eu/ontologies/Variable"/>
    <rdfs:label>Emissions|CO2|Energy|Demand|Residential and Commercial</rdfs:label>
    <rdfs:comment>Fossil CO2 emissions from fuel combustion in residential, commercial, institutional sectors (IPCC category 1A4a, 1A4b)</rdfs:comment>
    <ex:unit>Mt CO2/yr</ex:unit>
  </rdf:Description>
  <rdf:Description rdf:about="http://transience.eu/ontologies/Emissions_CO2_Industrial_Processes_Non-Ferrous_Metals">
    <rdf:type rdf:resource="http://www.w3.org/2002/07/owl#Class"/>
    <rdfs:subClassOf rdf:resource="http://transience.eu/ontologies/Variable"/>
    <rdfs:label>Emissions|CO2|Industrial Processes|Non-Ferrous Metals</rdfs:label>
    <rdfs:comment>CO2 emissions from industrial processes from non-ferrous minerals</rdfs:comment>
    <ex:unit>Mt CO2/yr</ex:unit>
  </rdf:Description>
  <rdf:Description rdf:about="http://transience.eu/ontologies/Import_Industry_Chemicals_Plastics_Volume">
    <rdf:type rdf:resource="http://www.w3.org/2002/07/owl#Class"/>
    <rdfs:subClassOf rdf:resource="http://transience.eu/ontologies/Variable"/>
    <rdfs:label>Import|Industry|Chemicals|Plastics|Volume</rdfs:label>
    <rdfs:comment>Import of plastics</rdfs:comment>
    <ex:unit>Mt/yr</ex:unit>
  </rdf:Description>
  <rdf:Description rdf:about="http://transience.eu/ontologies/Total_Scrap_Non-Ferrous_Metals_Power_Sector">
    <rdf:type rdf:resource="http://www.w3.org/2002/07/owl#Class"/>
    <rdfs:subClassOf rdf:resource="http://transience.eu/ontologies/Variable"/>
    <rdfs:label>Total Scrap|Non-Ferrous Metals|Power Sector</rdfs:label>
    <rdfs:comment>Total potential of non-ferrous metals scrap material as a result of end of life products (before collection)</rdfs:comment>
    <ex:unit>Mt/yr</ex:unit>
  </rdf:Description>
  <rdf:Description rdf:about="http://transience.eu/ontologies/Emissions_CO2_Energy_and_Industrial_Processes">
    <rdf:type rdf:resource="http://www.w3.org/2002/07/owl#Class"/>
    <rdfs:subClassOf rdf:resource="http://transience.eu/ontologies/Variable"/>
    <rdfs:label>Emissions|CO2|Energy and Industrial Processes</rdfs:label>
    <rdfs:comment>Fossil CO2 emissions from energy use on supply and demand side (IPCC category 1A, 1B) and from industrial processes (IPCC categories 2A, B, C, E), including emissions from international bunkers, net of negative emissions from Bioenergy with CCS (BECCS)</rdfs:comment>
    <ex:unit>Mt CO2/yr</ex:unit>
  </rdf:Description>
  <rdf:Description rdf:about="http://transience.eu/ontologies/Final_Energy_Residential_and_Commercial_Solids_Biomass_Traditional">
    <rdf:type rdf:resource="http://www.w3.org/2002/07/owl#Class"/>
    <rdfs:subClassOf rdf:resource="http://transience.eu/ontologies/Variable"/>
    <rdfs:label>Final Energy|Residential and Commercial|Solids|Biomass|Traditional</rdfs:label>
    <rdfs:comment>final energy consumed in the residential &amp; commercial sector of solid biomass (traditional)</rdfs:comment>
    <ex:unit>EJ/yr</ex:unit>
  </rdf:Description>
  <rdf:Description rdf:about="http://transience.eu/ontologies/Carbon_Capture_Usage_Materials_Long-lived">
    <rdf:type rdf:resource="http://www.w3.org/2002/07/owl#Class"/>
    <rdfs:subClassOf rdf:resource="http://transience.eu/ontologies/Variable"/>
    <rdfs:label>Carbon Capture|Usage|Materials|Long-lived</rdfs:label>
    <rdfs:comment>total carbon dioxide captured and used in long-lived materials (e.g. carbon fibers)</rdfs:comment>
    <ex:unit>Mt CO2/yr</ex:unit>
  </rdf:Description>
  <rdf:Description rdf:about="http://transience.eu/ontologies/Energy_Use_Industry_Petrochemicals_FT-Naphtha">
    <rdf:type rdf:resource="http://www.w3.org/2002/07/owl#Class"/>
    <rdfs:subClassOf rdf:resource="http://transience.eu/ontologies/Variable"/>
    <rdfs:label>Energy Use|Industry|Petrochemicals|FT-Naphtha</rdfs:label>
    <rdfs:comment>Use of Fischer-Tropsch naphtha, including both, non-energetic  use and energetic use  of by-products of FT-naphtha processing</rdfs:comment>
    <ex:unit>Mt/yr</ex:unit>
  </rdf:Description>
  <rdf:Description rdf:about="http://transience.eu/ontologies/Final_Energy_Industry_Steel_Hard_coal">
    <rdf:type rdf:resource="http://www.w3.org/2002/07/owl#Class"/>
    <rdfs:subClassOf rdf:resource="http://transience.eu/ontologies/Variable"/>
    <rdfs:label>Final Energy|Industry|Steel|Hard coal</rdfs:label>
    <rdfs:comment>Final energy. System boundaries in line with energy accounting</rdfs:comment>
    <ex:unit>PJ/yr</ex:unit>
  </rdf:Description>
  <rdf:Description rdf:about="http://transience.eu/ontologies/Final_Energy_Industry_Other_Sector_Solids">
    <rdf:type rdf:resource="http://www.w3.org/2002/07/owl#Class"/>
    <rdfs:subClassOf rdf:resource="http://transience.eu/ontologies/Variable"/>
    <rdfs:label>Final Energy|Industry|Other Sector|Solids</rdfs:label>
    <rdfs:comment>Final energy solid fuel consumption by other industry sectors (including coal and solid biomass)</rdfs:comment>
    <ex:unit>EJ/yr</ex:unit>
  </rdf:Description>
  <rdf:Description rdf:about="http://transience.eu/ontologies/Investment_Energy_Supply_Other">
    <rdf:type rdf:resource="http://www.w3.org/2002/07/owl#Class"/>
    <rdfs:subClassOf rdf:resource="http://transience.eu/ontologies/Variable"/>
    <rdfs:label>Investment|Energy Supply|Other</rdfs:label>
    <rdfs:comment>investments in other types of energy conversion facilities</rdfs:comment>
    <ex:unit>billion US$2010/yr</ex:unit>
  </rdf:Description>
  <rdf:Description rdf:about="http://transience.eu/ontologies/Lifetime_Hydrogen_Biomass_w__CCS">
    <rdf:type rdf:resource="http://www.w3.org/2002/07/owl#Class"/>
    <rdfs:subClassOf rdf:resource="http://transience.eu/ontologies/Variable"/>
    <rdfs:label>Lifetime|Hydrogen|Biomass|w/ CCS</rdfs:label>
    <rdfs:comment>Lifetime of a new biomass to hydrogen plant with CCS. Lifetime should be calculated by summing all vintages of a  capacity unit (e.g. (1+1+0.9+0.7+0.5) * 10 years = 41 years) or by the e-folding time for exponential capacity depreciation.  The lifetime should refer to the plant type(s) for which capital costs have been reported. If capital cost for more than one plant type has been reported, modellers should report lifetime for the additional plant types by adding variables Lifetime|Hydrogen|Biomass|w/ CCS|2, ... Lifetime|Hydrogen|Biomass|w/ CCS|N (matching the assignment of plant types to technologies in the reporting of capital costs as documented in the comments sheet). </rdfs:comment>
    <ex:unit>years</ex:unit>
  </rdf:Description>
  <rdf:Description rdf:about="http://transience.eu/ontologies/Primary_Energy_Gas_w__CCS">
    <rdf:type rdf:resource="http://www.w3.org/2002/07/owl#Class"/>
    <rdfs:subClassOf rdf:resource="http://transience.eu/ontologies/Variable"/>
    <rdfs:label>Primary Energy|Gas|w/ CCS</rdfs:label>
    <rdfs:comment>gas primary energy consumption used in combination with CCS</rdfs:comment>
    <ex:unit>EJ/yr</ex:unit>
  </rdf:Description>
  <rdf:Description rdf:about="http://transience.eu/ontologies/Carbon_Capture_Storage_Direct_Air_Capture">
    <rdf:type rdf:resource="http://www.w3.org/2002/07/owl#Class"/>
    <rdfs:subClassOf rdf:resource="http://transience.eu/ontologies/Variable"/>
    <rdfs:label>Carbon Capture|Storage|Direct Air Capture</rdfs:label>
    <rdfs:comment>total carbon dioxide sequestered through direct air capture</rdfs:comment>
    <ex:unit>Mt CO2/yr</ex:unit>
  </rdf:Description>
  <rdf:Description rdf:about="http://transience.eu/ontologies/Carbon_Capture_Storage_Biomass_Energy_Supply_Hydrogen">
    <rdf:type rdf:resource="http://www.w3.org/2002/07/owl#Class"/>
    <rdfs:subClassOf rdf:resource="http://transience.eu/ontologies/Variable"/>
    <rdfs:label>Carbon Capture|Storage|Biomass|Energy|Supply|Hydrogen</rdfs:label>
    <rdfs:comment>total carbon dioxide emissions captured from bioenergy use in hydrogen production (part of IPCC category 1A) and stored in geological deposits (e.g. in depleted oil and gas fields, unmined coal seams, saline aquifers) and the deep ocean, stored amounts should be reported as positive numbers</rdfs:comment>
    <ex:unit>Mt CO2/yr</ex:unit>
  </rdf:Description>
  <rdf:Description rdf:about="http://transience.eu/ontologies/Employment_Agriculture">
    <rdf:type rdf:resource="http://www.w3.org/2002/07/owl#Class"/>
    <rdfs:subClassOf rdf:resource="http://transience.eu/ontologies/Variable"/>
    <rdfs:label>Employment|Agriculture</rdfs:label>
    <rdfs:comment>Number of employed inhabitants (payrolls) in agriculture (based on ILO classification)</rdfs:comment>
    <ex:unit>million</ex:unit>
  </rdf:Description>
  <rdf:Description rdf:about="http://transience.eu/ontologies/Trade_Secondary_Energy_Liquids_Coal_Value">
    <rdf:type rdf:resource="http://www.w3.org/2002/07/owl#Class"/>
    <rdfs:subClassOf rdf:resource="http://transience.eu/ontologies/Variable"/>
    <rdfs:label>Trade|Secondary Energy|Liquids|Coal|Value</rdfs:label>
    <rdfs:comment>value of net exports of fossil liquid synfuels from coal-to-liquids (CTL) technologies, at the global level these should add up to the trade losses only</rdfs:comment>
    <ex:unit>EJ/yr</ex:unit>
  </rdf:Description>
  <rdf:Description rdf:about="http://transience.eu/ontologies/Primary_Energy_Biomass_Energy_Crops">
    <rdf:type rdf:resource="http://www.w3.org/2002/07/owl#Class"/>
    <rdfs:subClassOf rdf:resource="http://transience.eu/ontologies/Variable"/>
    <rdfs:label>Primary Energy|Biomass|Energy Crops</rdfs:label>
    <rdfs:comment>biomass primary energy from purpose-grown bioenergy crops</rdfs:comment>
    <ex:unit>EJ/yr</ex:unit>
  </rdf:Description>
  <rdf:Description rdf:about="http://transience.eu/ontologies/Conversion_Input_Electricity_Hydrogen">
    <rdf:type rdf:resource="http://www.w3.org/2002/07/owl#Class"/>
    <rdfs:subClassOf rdf:resource="http://transience.eu/ontologies/Variable"/>
    <rdfs:label>Conversion Input|Electricity|Hydrogen</rdfs:label>
    <rdfs:comment>secondary energy consumption of electricity for the production of hydrogen</rdfs:comment>
    <ex:unit>EJ/yr</ex:unit>
  </rdf:Description>
  <rdf:Description rdf:about="http://transience.eu/ontologies/Final_Energy_Transportation_Hydrogen_Fossil">
    <rdf:type rdf:resource="http://www.w3.org/2002/07/owl#Class"/>
    <rdfs:subClassOf rdf:resource="http://transience.eu/ontologies/Variable"/>
    <rdfs:label>Final Energy|Transportation|Hydrogen|Fossil</rdfs:label>
    <rdfs:comment>final energy consumption by the transportation sector of synthetic or derived Hydrogen of fossil origin</rdfs:comment>
    <ex:unit>EJ/yr</ex:unit>
  </rdf:Description>
  <rdf:Description rdf:about="http://transience.eu/ontologies/Secondary_Energy_Hydrogen_Coal">
    <rdf:type rdf:resource="http://www.w3.org/2002/07/owl#Class"/>
    <rdfs:subClassOf rdf:resource="http://transience.eu/ontologies/Variable"/>
    <rdfs:label>Secondary Energy|Hydrogen|Coal</rdfs:label>
    <rdfs:comment>hydrogen production from coal</rdfs:comment>
    <ex:unit>EJ/yr</ex:unit>
  </rdf:Description>
  <rdf:Description rdf:about="http://transience.eu/ontologies/Capital_Cost_Electricity_Coal_w_o_CCS">
    <rdf:type rdf:resource="http://www.w3.org/2002/07/owl#Class"/>
    <rdfs:subClassOf rdf:resource="http://transience.eu/ontologies/Variable"/>
    <rdfs:label>Capital Cost|Electricity|Coal|w/o CCS</rdfs:label>
    <rdfs:comment>Capital cost of a new coal power plant w/o CCS. If more than one coal power technology is modelled (e.g. subcritical PC, supercritical PC, IGCC), modellers should report capital costs for each represented coal power technology by adding variables Capital Cost|Electricity|Coal|w/o CCS|2, ... Capital Cost|Electricity|Coal|w/o CCS|N (with N = number of represented technologies). It is modeller's choice which coal power technologies to assign to type 1 (assigned to the variable without number suffix),2,...,N. The assignment should be documented in the comments sheet. </rdfs:comment>
    <ex:unit>US$2010/kW</ex:unit>
  </rdf:Description>
  <rdf:Description rdf:about="http://transience.eu/ontologies/Final_Energy_Non-Energy_Use_Chemicals_Hydrogen">
    <rdf:type rdf:resource="http://www.w3.org/2002/07/owl#Class"/>
    <rdfs:subClassOf rdf:resource="http://transience.eu/ontologies/Variable"/>
    <rdfs:label>Final Energy|Non-Energy Use|Chemicals|Hydrogen</rdfs:label>
    <rdfs:comment>Final energy consumption of hydrogen by the chemical sector by the non-combustion processes</rdfs:comment>
    <ex:unit>EJ/yr</ex:unit>
  </rdf:Description>
  <rdf:Description rdf:about="http://transience.eu/ontologies/OM_Cost_Fixed_Liquids_Gas_w_o_CCS">
    <rdf:type rdf:resource="http://www.w3.org/2002/07/owl#Class"/>
    <rdfs:subClassOf rdf:resource="http://transience.eu/ontologies/Variable"/>
    <rdfs:label>OM Cost|Fixed|Liquids|Gas|w/o CCS</rdfs:label>
    <rdfs:comment>Annual fixed operation &amp; maintainance cost of a new gas to liquids plant w/o CCS. If more than one GTL technology is modelled, modellers should report fixed O&amp;M costs  for each represented GTL technology by adding variables OM Cost|Fixed|Liquids|Gas|w/o CCS|2, ... OM Cost|Fixed|Liquids|Gas|w/o CCS|N (with N = number of represented technologies) (matching the assignment of plant types to technologies in the reporting of capital costs as documented in the comments sheet).</rdfs:comment>
    <ex:unit>US$2010/kW/yr</ex:unit>
  </rdf:Description>
  <rdf:Description rdf:about="http://transience.eu/ontologies/Final_Energy_Industry_Other_Sector_Solids_Coal">
    <rdf:type rdf:resource="http://www.w3.org/2002/07/owl#Class"/>
    <rdfs:subClassOf rdf:resource="http://transience.eu/ontologies/Variable"/>
    <rdfs:label>Final Energy|Industry|Other Sector|Solids|Coal</rdfs:label>
    <rdfs:comment>Final energy consumption of coal by other industry sectors</rdfs:comment>
    <ex:unit>EJ/yr</ex:unit>
  </rdf:Description>
  <rdf:Description rdf:about="http://transience.eu/ontologies/Export_Industry_Non-Metallic_Minerals">
    <rdf:type rdf:resource="http://www.w3.org/2002/07/owl#Class"/>
    <rdfs:subClassOf rdf:resource="http://transience.eu/ontologies/Variable"/>
    <rdfs:label>Export|Industry|Non-Metallic Minerals</rdfs:label>
    <rdfs:comment>Export of non-metallic minerals measured in monetary units</rdfs:comment>
    <ex:unit>billion US$2010/yr</ex:unit>
  </rdf:Description>
  <rdf:Description rdf:about="http://transience.eu/ontologies/Secondary_Energy_Electricity_Transmission_Losses">
    <rdf:type rdf:resource="http://www.w3.org/2002/07/owl#Class"/>
    <rdfs:subClassOf rdf:resource="http://transience.eu/ontologies/Variable"/>
    <rdfs:label>Secondary Energy|Electricity|Transmission Losses</rdfs:label>
    <rdfs:comment>electricity losses from long-range high-voltage transmission</rdfs:comment>
    <ex:unit>EJ/yr</ex:unit>
  </rdf:Description>
  <rdf:Description rdf:about="http://transience.eu/ontologies/Trade_Secondary_Energy_Liquids_Coal_Volume">
    <rdf:type rdf:resource="http://www.w3.org/2002/07/owl#Class"/>
    <rdfs:subClassOf rdf:resource="http://transience.eu/ontologies/Variable"/>
    <rdfs:label>Trade|Secondary Energy|Liquids|Coal|Volume</rdfs:label>
    <rdfs:comment>net exports of fossil liquid synfuels from coal-to-liquids (CTL) technologies, at the global level these should add up to the trade losses only</rdfs:comment>
    <ex:unit>EJ/yr</ex:unit>
  </rdf:Description>
  <rdf:Description rdf:about="http://transience.eu/ontologies/Final_Energy_Industry_Pulp_and_Paper_Solids">
    <rdf:type rdf:resource="http://www.w3.org/2002/07/owl#Class"/>
    <rdfs:subClassOf rdf:resource="http://transience.eu/ontologies/Variable"/>
    <rdfs:label>Final Energy|Industry|Pulp and Paper|Solids</rdfs:label>
    <rdfs:comment>Final energy consumption of solid fuels of the pulp and paper sector (including coal and solid biomass)</rdfs:comment>
    <ex:unit>EJ/yr</ex:unit>
  </rdf:Description>
  <rdf:Description rdf:about="http://transience.eu/ontologies/Final_Energy_Residential_and_Commercial_Solids">
    <rdf:type rdf:resource="http://www.w3.org/2002/07/owl#Class"/>
    <rdfs:subClassOf rdf:resource="http://transience.eu/ontologies/Variable"/>
    <rdfs:label>Final Energy|Residential and Commercial|Solids</rdfs:label>
    <rdfs:comment>final energy solid fuel consumption by the residential &amp; commercial sector (including coal and solid biomass)</rdfs:comment>
    <ex:unit>EJ/yr</ex:unit>
  </rdf:Description>
  <rdf:Description rdf:about="http://transience.eu/ontologies/Export_Industry_Non-Metallic_Minerals_Cement_Volume">
    <rdf:type rdf:resource="http://www.w3.org/2002/07/owl#Class"/>
    <rdfs:subClassOf rdf:resource="http://transience.eu/ontologies/Variable"/>
    <rdfs:label>Export|Industry|Non-Metallic Minerals|Cement|Volume</rdfs:label>
    <rdfs:comment>Export of cement</rdfs:comment>
    <ex:unit>Mt/yr</ex:unit>
  </rdf:Description>
  <rdf:Description rdf:about="http://transience.eu/ontologies/Collected_Scrap_Iron_and_Steel_Residential_and_Commercial">
    <rdf:type rdf:resource="http://www.w3.org/2002/07/owl#Class"/>
    <rdfs:subClassOf rdf:resource="http://transience.eu/ontologies/Variable"/>
    <rdfs:label>Collected Scrap|Iron and Steel|Residential and Commercial</rdfs:label>
    <rdfs:comment>Collected iron &amp; steel scrap coming from residential and commercial sector (available to be used in recycling)</rdfs:comment>
    <ex:unit>Mt/yr</ex:unit>
  </rdf:Description>
  <rdf:Description rdf:about="http://transience.eu/ontologies/Final_Energy_Industry_Pulp_and_Paper_Liquids_Biomass">
    <rdf:type rdf:resource="http://www.w3.org/2002/07/owl#Class"/>
    <rdfs:subClassOf rdf:resource="http://transience.eu/ontologies/Variable"/>
    <rdfs:label>Final Energy|Industry|Pulp and Paper|Liquids|Biomass</rdfs:label>
    <rdfs:comment>Final energy consumption of liquid biofuels by the pulp and paper sector</rdfs:comment>
    <ex:unit>EJ/yr</ex:unit>
  </rdf:Description>
  <rdf:Description rdf:about="http://transience.eu/ontologies/Capacity_Petrochemicals_Steamcracker">
    <rdf:type rdf:resource="http://www.w3.org/2002/07/owl#Class"/>
    <rdfs:subClassOf rdf:resource="http://transience.eu/ontologies/Variable"/>
    <rdfs:label>Capacity|Petrochemicals|Steamcracker</rdfs:label>
    <rdfs:comment>Capacity for HVC production in steamcrackers, the value refers to the amount of feedstock input that can be processed per year</rdfs:comment>
    <ex:unit>Mt feedstock input / yr</ex:unit>
  </rdf:Description>
  <rdf:Description rdf:about="http://transience.eu/ontologies/Final_Energy_Transportation_Hydrogen">
    <rdf:type rdf:resource="http://www.w3.org/2002/07/owl#Class"/>
    <rdfs:subClassOf rdf:resource="http://transience.eu/ontologies/Variable"/>
    <rdfs:label>Final Energy|Transportation|Hydrogen</rdfs:label>
    <rdfs:comment>final energy consumption by the transportation sector of hydrogen</rdfs:comment>
    <ex:unit>EJ/yr</ex:unit>
  </rdf:Description>
  <rdf:Description rdf:about="http://transience.eu/ontologies/Outflow_Steel_Product_categories">
    <rdf:type rdf:resource="http://www.w3.org/2002/07/owl#Class"/>
    <rdfs:subClassOf rdf:resource="http://transience.eu/ontologies/Variable"/>
    <rdfs:label>Outflow|Steel|[Product categories]</rdfs:label>
    <rdfs:comment>Steel outflowÂ </rdfs:comment>
    <ex:unit>t/yr</ex:unit>
  </rdf:Description>
  <rdf:Description rdf:about="http://transience.eu/ontologies/Emissions_CO2_Energy_Demand_AFOFI">
    <rdf:type rdf:resource="http://www.w3.org/2002/07/owl#Class"/>
    <rdfs:subClassOf rdf:resource="http://transience.eu/ontologies/Variable"/>
    <rdfs:label>Emissions|CO2|Energy|Demand|AFOFI</rdfs:label>
    <rdfs:comment>CO2 emissions from fuel combustion in agriculture, forestry, fishing (AFOFI) (IPCC category 1A4c)</rdfs:comment>
    <ex:unit>Mt CO2/yr</ex:unit>
  </rdf:Description>
  <rdf:Description rdf:about="http://transience.eu/ontologies/Resource_use_Scrap_Industry_Steel">
    <rdf:type rdf:resource="http://www.w3.org/2002/07/owl#Class"/>
    <rdfs:subClassOf rdf:resource="http://transience.eu/ontologies/Variable"/>
    <rdfs:label>Resource use|Scrap|Industry|Steel</rdfs:label>
    <rdfs:comment>Total use of scrap, including scrap used in primary routes</rdfs:comment>
    <ex:unit>Mt/yr</ex:unit>
  </rdf:Description>
  <rdf:Description rdf:about="http://transience.eu/ontologies/OM_Cost_Fixed_Liquids_Coal_w_o_CCS">
    <rdf:type rdf:resource="http://www.w3.org/2002/07/owl#Class"/>
    <rdfs:subClassOf rdf:resource="http://transience.eu/ontologies/Variable"/>
    <rdfs:label>OM Cost|Fixed|Liquids|Coal|w/o CCS</rdfs:label>
    <rdfs:comment>Annual fixed operation &amp; maintainance cost of a new coal to liquids plant w/o CCS. If more than one CTL technology is modelled, modellers should report fixed O&amp;M costs  for each represented CTL technology by adding variables OM Cost|Fixed|Liquids|Coal|w/o CCS|2, ... OM Cost|Fixed|Liquids|Coal|w/o CCS|N (with N = number of represented technologies) (matching the assignment of plant types to technologies in the reporting of capital costs as documented in the comments sheet).</rdfs:comment>
    <ex:unit>US$2010/kW/yr</ex:unit>
  </rdf:Description>
  <rdf:Description rdf:about="http://transience.eu/ontologies/Final_Energy_Carbon_Removal_Electricity">
    <rdf:type rdf:resource="http://www.w3.org/2002/07/owl#Class"/>
    <rdfs:subClassOf rdf:resource="http://transience.eu/ontologies/Variable"/>
    <rdfs:label>Final Energy|Carbon Removal|Electricity</rdfs:label>
    <rdfs:comment>Final energy consumption of electricity by carbon dioxide removal processes</rdfs:comment>
    <ex:unit>EJ/yr</ex:unit>
  </rdf:Description>
  <rdf:Description rdf:about="http://transience.eu/ontologies/Lifetime_Electricity_Solar_PV">
    <rdf:type rdf:resource="http://www.w3.org/2002/07/owl#Class"/>
    <rdfs:subClassOf rdf:resource="http://transience.eu/ontologies/Variable"/>
    <rdfs:label>Lifetime|Electricity|Solar|PV</rdfs:label>
    <rdfs:comment>Lifetime of a new PV unit. Lifetime should be calculated by summing all vintages of a  capacity unit (e.g. (1+1+0.9+0.7+0.5) * 10 years = 41 years) or by the e-folding time for exponential capacity depreciation.  The lifetime should refer to the plant type(s) for which capital costs have been reported. If capital cost for more than one plant type has been reported, modellers should report lifetime for the additional plant types by adding variables Lifetime|Electricity|Solar|PV|2, ... Lifetime|Electricity|Solar|PV|N (matching the assignment of plant types to technologies in the reporting of capital costs as documented in the comments sheet). </rdfs:comment>
    <ex:unit>years</ex:unit>
  </rdf:Description>
  <rdf:Description rdf:about="http://transience.eu/ontologies/Trade_Primary_Energy_Biomass_Volume">
    <rdf:type rdf:resource="http://www.w3.org/2002/07/owl#Class"/>
    <rdfs:subClassOf rdf:resource="http://transience.eu/ontologies/Variable"/>
    <rdfs:label>Trade|Primary Energy|Biomass|Volume</rdfs:label>
    <rdfs:comment>net exports of solid, unprocessed biomass, at the global level these should add up to the trade losses only</rdfs:comment>
    <ex:unit>EJ/yr</ex:unit>
  </rdf:Description>
  <rdf:Description rdf:about="http://transience.eu/ontologies/Carbon_Capture_Storage_Biomass_Energy_Supply_Gases">
    <rdf:type rdf:resource="http://www.w3.org/2002/07/owl#Class"/>
    <rdfs:subClassOf rdf:resource="http://transience.eu/ontologies/Variable"/>
    <rdfs:label>Carbon Capture|Storage|Biomass|Energy|Supply|Gases</rdfs:label>
    <rdfs:comment>total carbon dioxide emissions captured from bioenergy use in gaseous fuel production, excl. hydrogen (part of IPCC category 1A) and stored in geological deposits (e.g. in depleted oil and gas fields, unmined coal seams, saline aquifers) and the deep ocean, stored amounts should be reported as positive numbers</rdfs:comment>
    <ex:unit>Mt CO2/yr</ex:unit>
  </rdf:Description>
  <rdf:Description rdf:about="http://transience.eu/ontologies/Subsidies_Energy_Fossil">
    <rdf:type rdf:resource="http://www.w3.org/2002/07/owl#Class"/>
    <rdfs:subClassOf rdf:resource="http://transience.eu/ontologies/Variable"/>
    <rdfs:label>Subsidies|Energy|Fossil</rdfs:label>
    <rdfs:comment>Fossil fuel subsidies</rdfs:comment>
    <ex:unit>billion US$2010/yr</ex:unit>
  </rdf:Description>
  <rdf:Description rdf:about="http://transience.eu/ontologies/Efficiency_Gases_Coal_w__CCS">
    <rdf:type rdf:resource="http://www.w3.org/2002/07/owl#Class"/>
    <rdfs:subClassOf rdf:resource="http://transience.eu/ontologies/Variable"/>
    <rdfs:label>Efficiency|Gases|Coal|w/ CCS</rdfs:label>
    <rdfs:comment>Conversion efficiency (energy content of gases produced per unit of primary energy input) of a new coal to gas plant with CCS. The efficiency should refer to the plant type(s) for which capital costs have been reported. If capital cost for more than one plant type has been reported, modellers should report efficiency for the additional plant types by adding variables Efficiency|Gases|Coal|w/ CCS|2, ... Efficiency|Gases|Coal|w/ CCS|N (matching the assignment of plant types to technologies in the reporting of capital costs as documented in the comments sheet). </rdfs:comment>
    <ex:unit>%</ex:unit>
  </rdf:Description>
  <rdf:Description rdf:about="http://transience.eu/ontologies/Production_Petrochemicals_High_Value_Chemicals">
    <rdf:type rdf:resource="http://www.w3.org/2002/07/owl#Class"/>
    <rdfs:subClassOf rdf:resource="http://transience.eu/ontologies/Variable"/>
    <rdfs:label>Production|Petrochemicals|High Value Chemicals</rdfs:label>
    <rdfs:comment>Production of olefins and aromatics</rdfs:comment>
    <ex:unit>Mt/yr</ex:unit>
  </rdf:Description>
  <rdf:Description rdf:about="http://transience.eu/ontologies/Final_Energy_Commercial_Liquids_Electricity">
    <rdf:type rdf:resource="http://www.w3.org/2002/07/owl#Class"/>
    <rdfs:subClassOf rdf:resource="http://transience.eu/ontologies/Variable"/>
    <rdfs:label>Final Energy|Commercial|Liquids|Electricity</rdfs:label>
    <rdfs:comment>final energy consumption by the commercial sector of liquid efuels ("power-to-liquid")</rdfs:comment>
    <ex:unit>EJ/yr</ex:unit>
  </rdf:Description>
  <rdf:Description rdf:about="http://transience.eu/ontologies/Energy_Service_Transportation_Freight_Domestic_Aviation">
    <rdf:type rdf:resource="http://www.w3.org/2002/07/owl#Class"/>
    <rdfs:subClassOf rdf:resource="http://transience.eu/ontologies/Variable"/>
    <rdfs:label>Energy Service|Transportation|Freight|Domestic Aviation</rdfs:label>
    <rdfs:comment>energy service demand for freight transport on domestic aircrafts</rdfs:comment>
    <ex:unit>bn tkm/yr</ex:unit>
  </rdf:Description>
  <rdf:Description rdf:about="http://transience.eu/ontologies/Secondary_Energy_Heat_Biomass">
    <rdf:type rdf:resource="http://www.w3.org/2002/07/owl#Class"/>
    <rdfs:subClassOf rdf:resource="http://transience.eu/ontologies/Variable"/>
    <rdfs:label>Secondary Energy|Heat|Biomass</rdfs:label>
    <rdfs:comment>centralized heat generation from biomass</rdfs:comment>
    <ex:unit>EJ/yr</ex:unit>
  </rdf:Description>
  <rdf:Description rdf:about="http://transience.eu/ontologies/Export_Industry_Non-Ferrous_Metals_Aluminum_Volume">
    <rdf:type rdf:resource="http://www.w3.org/2002/07/owl#Class"/>
    <rdfs:subClassOf rdf:resource="http://transience.eu/ontologies/Variable"/>
    <rdfs:label>Export|Industry|Non-Ferrous Metals|Aluminum|Volume</rdfs:label>
    <rdfs:comment>Export of aluminium</rdfs:comment>
    <ex:unit>Mt/yr</ex:unit>
  </rdf:Description>
  <rdf:Description rdf:about="http://transience.eu/ontologies/Primary_Energy_Industry_Steel_Electricity_(autoproduction)">
    <rdf:type rdf:resource="http://www.w3.org/2002/07/owl#Class"/>
    <rdfs:subClassOf rdf:resource="http://transience.eu/ontologies/Variable"/>
    <rdfs:label>Primary Energy|Industry|Steel|Electricity (autoproduction)</rdfs:label>
    <rdfs:comment>Energy demand including own coke ovens and autoproduction of electricity</rdfs:comment>
    <ex:unit>PJ/yr</ex:unit>
  </rdf:Description>
  <rdf:Description rdf:about="http://transience.eu/ontologies/Energy_Service_Commercial_Floor_Space">
    <rdf:type rdf:resource="http://www.w3.org/2002/07/owl#Class"/>
    <rdfs:subClassOf rdf:resource="http://transience.eu/ontologies/Variable"/>
    <rdfs:label>Energy Service|Commercial|Floor Space</rdfs:label>
    <rdfs:comment>energy service demand for conditioned floor space in commercial buildings</rdfs:comment>
    <ex:unit>bn m2</ex:unit>
  </rdf:Description>
  <rdf:Description rdf:about="http://transience.eu/ontologies/Investment_Infrastructure_Transport">
    <rdf:type rdf:resource="http://www.w3.org/2002/07/owl#Class"/>
    <rdfs:subClassOf rdf:resource="http://transience.eu/ontologies/Variable"/>
    <rdfs:label>Investment|Infrastructure|Transport</rdfs:label>
    <rdfs:comment>investment into transport infrastructure - both newly constructed and maintenance of existing (all types: roads, bridges, ports, railways, refueling stations and charging infrastructure, etc.). Please specify in the comments section the type of infastructure that is being referred to here.</rdfs:comment>
    <ex:unit>billion US$2010/yr</ex:unit>
  </rdf:Description>
  <rdf:Description rdf:about="http://transience.eu/ontologies/Production_Non-Metallic_Minerals_Value">
    <rdf:type rdf:resource="http://www.w3.org/2002/07/owl#Class"/>
    <rdfs:subClassOf rdf:resource="http://transience.eu/ontologies/Variable"/>
    <rdfs:label>Production|Non-Metallic Minerals|Value</rdfs:label>
    <rdfs:comment>Production of non-metallic minerals</rdfs:comment>
    <ex:unit>billion US$2010/yr</ex:unit>
  </rdf:Description>
  <rdf:Description rdf:about="http://transience.eu/ontologies/Secondary_Energy_Electricity_Storage_Losses">
    <rdf:type rdf:resource="http://www.w3.org/2002/07/owl#Class"/>
    <rdfs:subClassOf rdf:resource="http://transience.eu/ontologies/Variable"/>
    <rdfs:label>Secondary Energy|Electricity|Storage Losses</rdfs:label>
    <rdfs:comment>losses from electricity storage</rdfs:comment>
    <ex:unit>EJ/yr</ex:unit>
  </rdf:Description>
  <rdf:Description rdf:about="http://transience.eu/ontologies/Carbon_Sequestration_CCS_Biomass_Industry_Steel">
    <rdf:type rdf:resource="http://www.w3.org/2002/07/owl#Class"/>
    <rdfs:subClassOf rdf:resource="http://transience.eu/ontologies/Variable"/>
    <rdfs:label>Carbon Sequestration|CCS|Biomass|Industry|Steel</rdfs:label>
    <rdfs:comment>Biogenic CO2 captured and stored</rdfs:comment>
    <ex:unit>Mt CO2/yr</ex:unit>
  </rdf:Description>
  <rdf:Description rdf:about="http://transience.eu/ontologies/Secondary_Energy_Heat_Gas">
    <rdf:type rdf:resource="http://www.w3.org/2002/07/owl#Class"/>
    <rdfs:subClassOf rdf:resource="http://transience.eu/ontologies/Variable"/>
    <rdfs:label>Secondary Energy|Heat|Gas</rdfs:label>
    <rdfs:comment>centralized heat generation from gases</rdfs:comment>
    <ex:unit>EJ/yr</ex:unit>
  </rdf:Description>
  <rdf:Description rdf:about="http://transience.eu/ontologies/Final_Energy_Residential_and_Commercial_Liquids_Fossil">
    <rdf:type rdf:resource="http://www.w3.org/2002/07/owl#Class"/>
    <rdfs:subClassOf rdf:resource="http://transience.eu/ontologies/Variable"/>
    <rdfs:label>Final Energy|Residential and Commercial|Liquids|Fossil</rdfs:label>
    <rdfs:comment>final energy consumption by the residential &amp; commercial sector of liquids from fossil origin (conventional &amp; unconventional petroleum, coal-to-liquids, gas-to-liquids)</rdfs:comment>
    <ex:unit>EJ/yr</ex:unit>
  </rdf:Description>
  <rdf:Description rdf:about="http://transience.eu/ontologies/Final_Energy_Transportation_Liquids_Biomass">
    <rdf:type rdf:resource="http://www.w3.org/2002/07/owl#Class"/>
    <rdfs:subClassOf rdf:resource="http://transience.eu/ontologies/Variable"/>
    <rdfs:label>Final Energy|Transportation|Liquids|Biomass</rdfs:label>
    <rdfs:comment>final energy consumption by the transportation sector of liquid biofuels</rdfs:comment>
    <ex:unit>EJ/yr</ex:unit>
  </rdf:Description>
  <rdf:Description rdf:about="http://transience.eu/ontologies/Trade_Emissions_Allowances_Value">
    <rdf:type rdf:resource="http://www.w3.org/2002/07/owl#Class"/>
    <rdfs:subClassOf rdf:resource="http://transience.eu/ontologies/Variable"/>
    <rdfs:label>Trade|Emissions Allowances|Value</rdfs:label>
    <rdfs:comment>value of trade in GHG emission allowances</rdfs:comment>
    <ex:unit>billion US$2010/yr</ex:unit>
  </rdf:Description>
  <rdf:Description rdf:about="http://transience.eu/ontologies/Capital_Cost_Hydrogen_Gas_w__CCS">
    <rdf:type rdf:resource="http://www.w3.org/2002/07/owl#Class"/>
    <rdfs:subClassOf rdf:resource="http://transience.eu/ontologies/Variable"/>
    <rdfs:label>Capital Cost|Hydrogen|Gas|w/ CCS</rdfs:label>
    <rdfs:comment>Capital cost of a new gas to hydrogen plant with CCS. If more than one CCS gas to hydrogen technology is modelled, modellers should report capital costs for each represented CCS gas to hydrogen technology by adding variables Capital Cost|Hydrogen|Gas|w/ CCS|2, ... Capital Cost|Hydrogen|Gas|w/ CCS|N (with N = number of represented technologies). It is modeller's choice which CCS gas to hydrogen technologies to assign to type 1 (assigned to the variable without number suffix),2,...,N. The assignment should be documented in the comments sheet. </rdfs:comment>
    <ex:unit>US$2010/kW</ex:unit>
  </rdf:Description>
  <rdf:Description rdf:about="http://transience.eu/ontologies/OM_Cost_Fixed_Liquids_Gas_w__CCS">
    <rdf:type rdf:resource="http://www.w3.org/2002/07/owl#Class"/>
    <rdfs:subClassOf rdf:resource="http://transience.eu/ontologies/Variable"/>
    <rdfs:label>OM Cost|Fixed|Liquids|Gas|w/ CCS</rdfs:label>
    <rdfs:comment>Annual fixed operation &amp; maintainance cost of a new gas to liquids plant with CCS. If more than one CCS GTL technology is modelled, modellers should report fixed O&amp;M costs  for each represented CCS GTL technology by adding variables OM Cost|Fixed|Liquids|Gas|w/ CCS|2, ... OM Cost|Fixed|Liquids|Gas|w/ CCS|N (with N = number of represented technologies) (matching the assignment of plant types to technologies in the reporting of capital costs as documented in the comments sheet).</rdfs:comment>
    <ex:unit>US$2010/kW/yr</ex:unit>
  </rdf:Description>
  <rdf:Description rdf:about="http://transience.eu/ontologies/Materials_Demand_Non-Ferrous_Metals_Transportation">
    <rdf:type rdf:resource="http://www.w3.org/2002/07/owl#Class"/>
    <rdfs:subClassOf rdf:resource="http://transience.eu/ontologies/Variable"/>
    <rdfs:label>Materials Demand|Non-Ferrous Metals|Transportation</rdfs:label>
    <rdfs:comment>Non-ferrous metals requirments from a certain end-use sector</rdfs:comment>
    <ex:unit>Mt/yr</ex:unit>
  </rdf:Description>
  <rdf:Description rdf:about="http://transience.eu/ontologies/Inflow_Plastics_Product_categories_">
    <rdf:type rdf:resource="http://www.w3.org/2002/07/owl#Class"/>
    <rdfs:subClassOf rdf:resource="http://transience.eu/ontologies/Variable"/>
    <rdfs:label>Inflow|Plastics|[Product categories] </rdfs:label>
    <rdfs:comment>Plastics inflowÂ </rdfs:comment>
    <ex:unit>t/yr</ex:unit>
  </rdf:Description>
  <rdf:Description rdf:about="http://transience.eu/ontologies/Policy_Cost_GDP_Loss">
    <rdf:type rdf:resource="http://www.w3.org/2002/07/owl#Class"/>
    <rdfs:subClassOf rdf:resource="http://transience.eu/ontologies/Variable"/>
    <rdfs:label>Policy Cost|GDP Loss</rdfs:label>
    <rdfs:comment>GDP loss in a policy scenario compared to the corresponding baseline (losses should be reported as positive numbers)</rdfs:comment>
    <ex:unit>billion US$2010/yr</ex:unit>
  </rdf:Description>
  <rdf:Description rdf:about="http://transience.eu/ontologies/Carbon_Capture_Industry_Biomass">
    <rdf:type rdf:resource="http://www.w3.org/2002/07/owl#Class"/>
    <rdfs:subClassOf rdf:resource="http://transience.eu/ontologies/Variable"/>
    <rdfs:label>Carbon Capture|Industry|Biomass</rdfs:label>
    <rdfs:comment>total carbon dioxide emissions from biomass captured in industry sector</rdfs:comment>
    <ex:unit>Mt CO2/yr</ex:unit>
  </rdf:Description>
  <rdf:Description rdf:about="http://transience.eu/ontologies/Capacity_Electricity_Hydrogen">
    <rdf:type rdf:resource="http://www.w3.org/2002/07/owl#Class"/>
    <rdfs:subClassOf rdf:resource="http://transience.eu/ontologies/Variable"/>
    <rdfs:label>Capacity|Electricity|Hydrogen</rdfs:label>
    <rdfs:comment>Total installed (available) capacity of hydrogen power plants. The installed (available) capacity of hydrogen power plants by plant type for which capital costs are reported should be reported by adding variables Capacity|Electricity|Hydrogen|1, ..., Capacity|Electricity|Hydrogen|N (matching the assignment of plant types to technologies in the reporting of capital costs as documented in the comments sheet). </rdfs:comment>
    <ex:unit>GW</ex:unit>
  </rdf:Description>
  <rdf:Description rdf:about="http://transience.eu/ontologies/Production_Steel_Primary_crude_steel_DRI_biomass_route">
    <rdf:type rdf:resource="http://www.w3.org/2002/07/owl#Class"/>
    <rdfs:subClassOf rdf:resource="http://transience.eu/ontologies/Variable"/>
    <rdfs:label>Production|Steel|Primary crude steel|DRI biomass route</rdfs:label>
    <rdfs:comment>Production of primary crude steel in DRI route with biogenic syngas as reducing gas (including both: processing of DRI into steel in EAF and in Smelter/BOF)</rdfs:comment>
    <ex:unit>Mt/yr</ex:unit>
  </rdf:Description>
  <rdf:Description rdf:about="http://transience.eu/ontologies/Investment_Energy_Efficiency">
    <rdf:type rdf:resource="http://www.w3.org/2002/07/owl#Class"/>
    <rdfs:subClassOf rdf:resource="http://transience.eu/ontologies/Variable"/>
    <rdfs:label>Investment|Energy Efficiency</rdfs:label>
    <rdfs:comment>investments into the efficiency-increasing components of energy demand technologies</rdfs:comment>
    <ex:unit>billion US$2010/yr</ex:unit>
  </rdf:Description>
  <rdf:Description rdf:about="http://transience.eu/ontologies/Secondary_Energy_Hydrogen_Biomass">
    <rdf:type rdf:resource="http://www.w3.org/2002/07/owl#Class"/>
    <rdfs:subClassOf rdf:resource="http://transience.eu/ontologies/Variable"/>
    <rdfs:label>Secondary Energy|Hydrogen|Biomass</rdfs:label>
    <rdfs:comment>hydrogen production from biomass</rdfs:comment>
    <ex:unit>EJ/yr</ex:unit>
  </rdf:Description>
  <rdf:Description rdf:about="http://transience.eu/ontologies/Investment_Energy_Demand_Transportation_Freight_Road_HDT_FCV">
    <rdf:type rdf:resource="http://www.w3.org/2002/07/owl#Class"/>
    <rdfs:subClassOf rdf:resource="http://transience.eu/ontologies/Variable"/>
    <rdfs:label>Investment|Energy Demand|Transportation|Freight|Road|HDT|FCV</rdfs:label>
    <rdfs:comment>investments into new vehicle technologies in the transport sector (heavy-duty freight trucks: fuel cell technologies running on hydrogen or another type of fuel)</rdfs:comment>
    <ex:unit>billion US$2010/yr</ex:unit>
  </rdf:Description>
  <rdf:Description rdf:about="http://transience.eu/ontologies/Production_Iron_and_Steel_Pig_Iron_Volume">
    <rdf:type rdf:resource="http://www.w3.org/2002/07/owl#Class"/>
    <rdfs:subClassOf rdf:resource="http://transience.eu/ontologies/Variable"/>
    <rdfs:label>Production|Iron and Steel|Pig Iron|Volume</rdfs:label>
    <rdfs:comment>production of pig iron (intermediate product for the production of primary steel)</rdfs:comment>
    <ex:unit>Mt/yr</ex:unit>
  </rdf:Description>
  <rdf:Description rdf:about="http://transience.eu/ontologies/Lifetime_Gases_Biomass_w__CCS">
    <rdf:type rdf:resource="http://www.w3.org/2002/07/owl#Class"/>
    <rdfs:subClassOf rdf:resource="http://transience.eu/ontologies/Variable"/>
    <rdfs:label>Lifetime|Gases|Biomass|w/ CCS</rdfs:label>
    <rdfs:comment>Lifetime of a new biomass to gas plant with CCS. Lifetime should be calculated by summing all vintages of a  capacity unit (e.g. (1+1+0.9+0.7+0.5) * 10 years = 41 years) or by the e-folding time for exponential capacity depreciation.  The lifetime should refer to the plant type(s) for which capital costs have been reported. If capital cost for more than one plant type has been reported, modellers should report lifetime for the additional plant types by adding variables Lifetime|Gases|Biomass|w/ CCS|2, ... Lifetime|Gases|Biomass|w/ CCS|N (matching the assignment of plant types to technologies in the reporting of capital costs as documented in the comments sheet). </rdfs:comment>
    <ex:unit>years</ex:unit>
  </rdf:Description>
  <rdf:Description rdf:about="http://transience.eu/ontologies/Employment_Service">
    <rdf:type rdf:resource="http://www.w3.org/2002/07/owl#Class"/>
    <rdfs:subClassOf rdf:resource="http://transience.eu/ontologies/Variable"/>
    <rdfs:label>Employment|Service</rdfs:label>
    <rdfs:comment>Number of employed inhabitants (payrolls) in the service sector (based on ILO classification)</rdfs:comment>
    <ex:unit>million</ex:unit>
  </rdf:Description>
  <rdf:Description rdf:about="http://transience.eu/ontologies/Secondary_Energy_Liquids_Biomass_Other">
    <rdf:type rdf:resource="http://www.w3.org/2002/07/owl#Class"/>
    <rdfs:subClassOf rdf:resource="http://transience.eu/ontologies/Variable"/>
    <rdfs:label>Secondary Energy|Liquids|Biomass|Other</rdfs:label>
    <rdfs:comment>biofuel production from biomass that does not fit to any other category (please provide a definition of the sources in this category in the 'comments' tab)</rdfs:comment>
    <ex:unit>EJ/yr</ex:unit>
  </rdf:Description>
  <rdf:Description rdf:about="http://transience.eu/ontologies/Export_Industry_Iron_and_Steel_Primary">
    <rdf:type rdf:resource="http://www.w3.org/2002/07/owl#Class"/>
    <rdfs:subClassOf rdf:resource="http://transience.eu/ontologies/Variable"/>
    <rdfs:label>Export|Industry|Iron and Steel|Primary</rdfs:label>
    <rdfs:comment>Export of primary steel measured in monetary units</rdfs:comment>
    <ex:unit>billion US$2010/yr</ex:unit>
  </rdf:Description>
  <rdf:Description rdf:about="http://transience.eu/ontologies/Production_Chemicals_Plastics_Secondary_Plastics_Volume">
    <rdf:type rdf:resource="http://www.w3.org/2002/07/owl#Class"/>
    <rdfs:subClassOf rdf:resource="http://transience.eu/ontologies/Variable"/>
    <rdfs:label>Production|Chemicals|Plastics|Secondary Plastics|Volume</rdfs:label>
    <rdfs:comment>production of secondary plastics, i.e. plastics obtained from recycling of plastics</rdfs:comment>
    <ex:unit>Mt/yr</ex:unit>
  </rdf:Description>
  <rdf:Description rdf:about="http://transience.eu/ontologies/Primary_Energy_Biomass_Residues">
    <rdf:type rdf:resource="http://www.w3.org/2002/07/owl#Class"/>
    <rdfs:subClassOf rdf:resource="http://transience.eu/ontologies/Variable"/>
    <rdfs:label>Primary Energy|Biomass|Residues</rdfs:label>
    <rdfs:comment>biomass primary energy from residues</rdfs:comment>
    <ex:unit>EJ/yr</ex:unit>
  </rdf:Description>
  <rdf:Description rdf:about="http://transience.eu/ontologies/Energy_Service_Residential_and_Commercial_Floor_Space">
    <rdf:type rdf:resource="http://www.w3.org/2002/07/owl#Class"/>
    <rdfs:subClassOf rdf:resource="http://transience.eu/ontologies/Variable"/>
    <rdfs:label>Energy Service|Residential and Commercial|Floor Space</rdfs:label>
    <rdfs:comment>energy service demand for conditioned floor space in buildings</rdfs:comment>
    <ex:unit>bn m2</ex:unit>
  </rdf:Description>
  <rdf:Description rdf:about="http://transience.eu/ontologies/Production_Steel_Primary_crude_steel_DRI_imported_route">
    <rdf:type rdf:resource="http://www.w3.org/2002/07/owl#Class"/>
    <rdfs:subClassOf rdf:resource="http://transience.eu/ontologies/Variable"/>
    <rdfs:label>Production|Steel|Primary crude steel|DRI imported route</rdfs:label>
    <rdfs:comment>Production of primary crude steel from imported DRI (including both: processing of DRI into steel in EAF and in Smelter/BOF)</rdfs:comment>
    <ex:unit>Mt/yr</ex:unit>
  </rdf:Description>
  <rdf:Description rdf:about="http://transience.eu/ontologies/Policy_Cost_Default">
    <rdf:type rdf:resource="http://www.w3.org/2002/07/owl#Class"/>
    <rdfs:subClassOf rdf:resource="http://transience.eu/ontologies/Variable"/>
    <rdfs:label>Policy Cost|Default</rdfs:label>
    <rdfs:comment>total costs of the policy in the default metric (consumption losses for GE models, area under MAC curve for PE models if available) to be used for calculation of Cost over Abatement Value (CAV) indicator. Must be identical to the policy costs in one of the reported metrics. </rdfs:comment>
    <ex:unit>billion US$2010/yr</ex:unit>
  </rdf:Description>
  <rdf:Description rdf:about="http://transience.eu/ontologies/Investment_Energy_Supply_Electricity_Hydro">
    <rdf:type rdf:resource="http://www.w3.org/2002/07/owl#Class"/>
    <rdfs:subClassOf rdf:resource="http://transience.eu/ontologies/Variable"/>
    <rdfs:label>Investment|Energy Supply|Electricity|Hydro</rdfs:label>
    <rdfs:comment>investments in new power generation for the specified power plant category. If the model features several sub-categories, the total investments should be reported. For plants equipped with CCS, the investment in the capturing equipment should be included but not the one on transport and storage.</rdfs:comment>
    <ex:unit>billion US$2010/yr</ex:unit>
  </rdf:Description>
  <rdf:Description rdf:about="http://transience.eu/ontologies/Carbon_Capture_Industry">
    <rdf:type rdf:resource="http://www.w3.org/2002/07/owl#Class"/>
    <rdfs:subClassOf rdf:resource="http://transience.eu/ontologies/Variable"/>
    <rdfs:label>Carbon Capture|Industry</rdfs:label>
    <rdfs:comment>total carbon dioxide emissions captured from industrial energy use, should be reported as positive numbers</rdfs:comment>
    <ex:unit>Mt CO2/yr</ex:unit>
  </rdf:Description>
  <rdf:Description rdf:about="http://transience.eu/ontologies/Capacity_Steel_EAF">
    <rdf:type rdf:resource="http://www.w3.org/2002/07/owl#Class"/>
    <rdfs:subClassOf rdf:resource="http://transience.eu/ontologies/Variable"/>
    <rdfs:label>Capacity|Steel|EAF</rdfs:label>
    <rdfs:comment>Capacity of basic oxygen furnaces for crude steel production in Mt crude steel / year</rdfs:comment>
    <ex:unit>Mt/yr</ex:unit>
  </rdf:Description>
  <rdf:Description rdf:about="http://transience.eu/ontologies/Primary_Energy_Biomass">
    <rdf:type rdf:resource="http://www.w3.org/2002/07/owl#Class"/>
    <rdfs:subClassOf rdf:resource="http://transience.eu/ontologies/Variable"/>
    <rdfs:label>Primary Energy|Biomass</rdfs:label>
    <rdfs:comment>primary energy consumption of purpose-grown bioenergy crops, crop and forestry residue bioenergy, municipal solid waste bioenergy, traditional biomass</rdfs:comment>
    <ex:unit>EJ/yr</ex:unit>
  </rdf:Description>
  <rdf:Description rdf:about="http://transience.eu/ontologies/Parameter">
    <rdf:type rdf:resource="http://www.w3.org/2002/07/owl#Class"/>
    <rdfs:comment>Base class for all Parameters</rdfs:comment>
  </rdf:Description>
  <rdf:Description rdf:about="http://transience.eu/ontologies/Final_Energy_Industry_Chemicals_Heat">
    <rdf:type rdf:resource="http://www.w3.org/2002/07/owl#Class"/>
    <rdfs:subClassOf rdf:resource="http://transience.eu/ontologies/Variable"/>
    <rdfs:label>Final Energy|Industry|Chemicals|Heat</rdfs:label>
    <rdfs:comment>Final energy consumption of centrally supplied heat by the chemicals sector</rdfs:comment>
    <ex:unit>EJ/yr</ex:unit>
  </rdf:Description>
  <rdf:Description rdf:about="http://transience.eu/ontologies/Investment_Petrochemicals_CO2_capture">
    <rdf:type rdf:resource="http://www.w3.org/2002/07/owl#Class"/>
    <rdfs:subClassOf rdf:resource="http://transience.eu/ontologies/Variable"/>
    <rdfs:label>Investment|Petrochemicals|CO2 capture</rdfs:label>
    <rdfs:comment>Investment in CO2 capture plants</rdfs:comment>
    <ex:unit>Mio â‚¬_2022/yr</ex:unit>
  </rdf:Description>
  <rdf:Description rdf:about="http://transience.eu/ontologies/Production_Steel_Primary_crude_steel_blast_furnace_route">
    <rdf:type rdf:resource="http://www.w3.org/2002/07/owl#Class"/>
    <rdfs:subClassOf rdf:resource="http://transience.eu/ontologies/Variable"/>
    <rdfs:label>Production|Steel|Primary crude steel|blast furnace route</rdfs:label>
    <rdfs:comment>Production of primary crude steel in blast furnance route (blast furnace, basic oxygen furnace)</rdfs:comment>
    <ex:unit>Mt/yr</ex:unit>
  </rdf:Description>
  <rdf:Description rdf:about="http://transience.eu/ontologies/Import_Industry_Non-Ferrous_Metals_Volume">
    <rdf:type rdf:resource="http://www.w3.org/2002/07/owl#Class"/>
    <rdfs:subClassOf rdf:resource="http://transience.eu/ontologies/Variable"/>
    <rdfs:label>Import|Industry|Non-Ferrous Metals|Volume</rdfs:label>
    <rdfs:comment>Import of non-ferrous metals</rdfs:comment>
    <ex:unit>Mt/yr</ex:unit>
  </rdf:Description>
  <rdf:Description rdf:about="http://transience.eu/ontologies/Export_Industry_Iron_and_Steel_Secondary_Steel_Volume">
    <rdf:type rdf:resource="http://www.w3.org/2002/07/owl#Class"/>
    <rdfs:subClassOf rdf:resource="http://transience.eu/ontologies/Variable"/>
    <rdfs:label>Export|Industry|Iron and Steel|Secondary Steel|Volume</rdfs:label>
    <rdfs:comment>Export of secondary steel</rdfs:comment>
    <ex:unit>Mt/yr</ex:unit>
  </rdf:Description>
  <rdf:Description rdf:about="http://transience.eu/ontologies/Final_Energy_Industry_Other_Sector_Heat">
    <rdf:type rdf:resource="http://www.w3.org/2002/07/owl#Class"/>
    <rdfs:subClassOf rdf:resource="http://transience.eu/ontologies/Variable"/>
    <rdfs:label>Final Energy|Industry|Other Sector|Heat</rdfs:label>
    <rdfs:comment>Final energy consumption of centrally supplied heat by other industry sectors</rdfs:comment>
    <ex:unit>EJ/yr</ex:unit>
  </rdf:Description>
  <rdf:Description rdf:about="http://transience.eu/ontologies/Stock_Plastics_Other_demand_sectors_Product_categories">
    <rdf:type rdf:resource="http://www.w3.org/2002/07/owl#Class"/>
    <rdfs:subClassOf rdf:resource="http://transience.eu/ontologies/Variable"/>
    <rdfs:label>Stock|Plastics|Other|[demand sectors]|[Product categories]</rdfs:label>
    <rdfs:comment>Plastics stock in other sectorsÂ </rdfs:comment>
    <ex:unit>t/yr</ex:unit>
  </rdf:Description>
  <rdf:Description rdf:about="http://transience.eu/ontologies/Capital_Cost_Liquids_Coal_w__CCS">
    <rdf:type rdf:resource="http://www.w3.org/2002/07/owl#Class"/>
    <rdfs:subClassOf rdf:resource="http://transience.eu/ontologies/Variable"/>
    <rdfs:label>Capital Cost|Liquids|Coal|w/ CCS</rdfs:label>
    <rdfs:comment>Capital cost of a new coal to liquids plant with CCS. If more than one CCS CTL technology is modelled, modellers should report capital costs for each represented CCS CTL technology by adding variables Capital Cost|Liquids|Coal|w/ CCS|2, ... Capital Cost|Liquids|Coal|w/ CCS|N (with N = number of represented technologies). It is modeller's choice which CCS CTL technologies to assign to type 1 (assigned to the variable without number suffix),2,...,N. The assignment should be documented in the comments sheet. </rdfs:comment>
    <ex:unit>US$2010/kW</ex:unit>
  </rdf:Description>
  <rdf:Description rdf:about="http://transience.eu/ontologies/Final_Energy_Residential_Liquids_Biomass">
    <rdf:type rdf:resource="http://www.w3.org/2002/07/owl#Class"/>
    <rdfs:subClassOf rdf:resource="http://transience.eu/ontologies/Variable"/>
    <rdfs:label>Final Energy|Residential|Liquids|Biomass</rdfs:label>
    <rdfs:comment>final energy consumption by the residential sector of liquid biofuels</rdfs:comment>
    <ex:unit>EJ/yr</ex:unit>
  </rdf:Description>
  <rdf:Description rdf:about="http://transience.eu/ontologies/Cost_Production_Steel_DRI_EAF_NG">
    <rdf:type rdf:resource="http://www.w3.org/2002/07/owl#Class"/>
    <rdfs:subClassOf rdf:resource="http://transience.eu/ontologies/Variable"/>
    <rdfs:label>Cost|Production|Steel|DRI_EAF_NG</rdfs:label>
    <rdfs:comment>Specific production cost of crude steel in DRI/EAF route when using natural gas as reducing gas; including CAPEX (annuity), fixed and variable OPEX</rdfs:comment>
    <ex:unit>Mio â‚¬_2022 / t crude steel</ex:unit>
  </rdf:Description>
  <rdf:Description rdf:about="http://transience.eu/ontologies/Production_Non-Ferrous_Metals_Value">
    <rdf:type rdf:resource="http://www.w3.org/2002/07/owl#Class"/>
    <rdfs:subClassOf rdf:resource="http://transience.eu/ontologies/Variable"/>
    <rdfs:label>Production|Non-Ferrous Metals|Value</rdfs:label>
    <rdfs:comment>production of non-ferrous metals (e.g., aluminum)</rdfs:comment>
    <ex:unit>billion US$2010/yr</ex:unit>
  </rdf:Description>
  <rdf:Description rdf:about="http://transience.eu/ontologies/Collected_Scrap_Non-Ferrous_Metals_Power_Sector">
    <rdf:type rdf:resource="http://www.w3.org/2002/07/owl#Class"/>
    <rdfs:subClassOf rdf:resource="http://transience.eu/ontologies/Variable"/>
    <rdfs:label>Collected Scrap|Non-Ferrous Metals|Power Sector</rdfs:label>
    <rdfs:comment>Collected non-ferrous metals scrap coming from power sector (available to be used in recycling)</rdfs:comment>
    <ex:unit>Mt/yr</ex:unit>
  </rdf:Description>
  <rdf:Description rdf:about="http://transience.eu/ontologies/Capacity_Electricity_Biomass_w_o_CCS">
    <rdf:type rdf:resource="http://www.w3.org/2002/07/owl#Class"/>
    <rdfs:subClassOf rdf:resource="http://transience.eu/ontologies/Variable"/>
    <rdfs:label>Capacity|Electricity|Biomass|w/o CCS</rdfs:label>
    <rdfs:comment>Total installed (available) capacity of biomass power plants without CCS, including plants held in an operating reserve. The installed (available) capacity of biomass power plants by plant type for which capital costs are reported should be reported by adding variables Capacity|Electricity|Biomass|w/o CCS|1, ..., Capacity|Electricity|Biomass|w/o CCS|N (matching the assignment of plant types to technologies in the reporting of capital costs as documented in the comments sheet). </rdfs:comment>
    <ex:unit>GW</ex:unit>
  </rdf:Description>
  <rdf:Description rdf:about="http://transience.eu/ontologies/Export_Industry_Chemicals_High_Value_Chemicals">
    <rdf:type rdf:resource="http://www.w3.org/2002/07/owl#Class"/>
    <rdfs:subClassOf rdf:resource="http://transience.eu/ontologies/Variable"/>
    <rdfs:label>Export|Industry|Chemicals|High Value Chemicals</rdfs:label>
    <rdfs:comment>Export of high value chemicals measured in monetary units</rdfs:comment>
    <ex:unit>billion US$2010/yr</ex:unit>
  </rdf:Description>
  <rdf:Description rdf:about="http://transience.eu/ontologies/Emissions_CO2_Industrial_Processes_Iron_and_Steel">
    <rdf:type rdf:resource="http://www.w3.org/2002/07/owl#Class"/>
    <rdfs:subClassOf rdf:resource="http://transience.eu/ontologies/Variable"/>
    <rdfs:label>Emissions|CO2|Industrial Processes|Iron and Steel</rdfs:label>
    <rdfs:comment>CO2 emissions from industrial processes from iron &amp; steel</rdfs:comment>
    <ex:unit>Mt CO2/yr</ex:unit>
  </rdf:Description>
  <rdf:Description rdf:about="http://transience.eu/ontologies/Trade_Secondary_Energy_Hydrogen_Volume">
    <rdf:type rdf:resource="http://www.w3.org/2002/07/owl#Class"/>
    <rdfs:subClassOf rdf:resource="http://transience.eu/ontologies/Variable"/>
    <rdfs:label>Trade|Secondary Energy|Hydrogen|Volume</rdfs:label>
    <rdfs:comment>net exports of hydrogen, at the global level these should add up to the trade losses only</rdfs:comment>
    <ex:unit>EJ/yr</ex:unit>
  </rdf:Description>
  <rdf:Description rdf:about="http://transience.eu/ontologies/Energy_Service_Transportation_Passenger_Domestic_Aviation">
    <rdf:type rdf:resource="http://www.w3.org/2002/07/owl#Class"/>
    <rdfs:subClassOf rdf:resource="http://transience.eu/ontologies/Variable"/>
    <rdfs:label>Energy Service|Transportation|Passenger|Domestic Aviation</rdfs:label>
    <rdfs:comment>energy service demand for passenger transport on domestic aircrafts</rdfs:comment>
    <ex:unit>bn pkm/yr</ex:unit>
  </rdf:Description>
  <rdf:Description rdf:about="http://transience.eu/ontologies/Final_Energy_Residential_Solids_Fossil">
    <rdf:type rdf:resource="http://www.w3.org/2002/07/owl#Class"/>
    <rdfs:subClassOf rdf:resource="http://transience.eu/ontologies/Variable"/>
    <rdfs:label>Final Energy|Residential|Solids|Fossil</rdfs:label>
    <rdfs:comment>final energy consumption of fossil solids by the residential sector</rdfs:comment>
    <ex:unit>EJ/yr</ex:unit>
  </rdf:Description>
  <rdf:Description rdf:about="http://transience.eu/ontologies/Emissions_CO2_Energy_Demand_Industry_Pulp_and_Paper">
    <rdf:type rdf:resource="http://www.w3.org/2002/07/owl#Class"/>
    <rdfs:subClassOf rdf:resource="http://transience.eu/ontologies/Variable"/>
    <rdfs:label>Emissions|CO2|Energy|Demand|Industry|Pulp and Paper</rdfs:label>
    <rdfs:comment>Fossil CO2 emissions from fuel combustion in industry in the pulp and paper sector</rdfs:comment>
    <ex:unit>Mt CO2/yr</ex:unit>
  </rdf:Description>
  <rdf:Description rdf:about="http://transience.eu/ontologies/Secondary_Energy">
    <rdf:type rdf:resource="http://www.w3.org/2002/07/owl#Class"/>
    <rdfs:subClassOf rdf:resource="http://transience.eu/ontologies/Variable"/>
    <rdfs:label>Secondary Energy</rdfs:label>
    <rdfs:comment>total secondary energy - the sum of all secondary energy carrier production (for consistency checks)</rdfs:comment>
    <ex:unit>EJ/yr</ex:unit>
  </rdf:Description>
  <rdf:Description rdf:about="http://transience.eu/ontologies/Emissions_CO2_Energy_Demand_Commercial">
    <rdf:type rdf:resource="http://www.w3.org/2002/07/owl#Class"/>
    <rdfs:subClassOf rdf:resource="http://transience.eu/ontologies/Variable"/>
    <rdfs:label>Emissions|CO2|Energy|Demand|Commercial</rdfs:label>
    <rdfs:comment>Fossil CO2 emissions from fuel combustion in commercial and institutional sectors (IPCC category 1A4a)</rdfs:comment>
    <ex:unit>Mt CO2/yr</ex:unit>
  </rdf:Description>
  <rdf:Description rdf:about="http://transience.eu/ontologies/Lifetime_Electricity_Gas_w_o_CCS">
    <rdf:type rdf:resource="http://www.w3.org/2002/07/owl#Class"/>
    <rdfs:subClassOf rdf:resource="http://transience.eu/ontologies/Variable"/>
    <rdfs:label>Lifetime|Electricity|Gas|w/o CCS</rdfs:label>
    <rdfs:comment>Lifetime of a new gas power plant w/o CCS. Lifetime should be calculated by summing all vintages of a  capacity unit (e.g. (1+1+0.9+0.7+0.5) * 10 years = 41 years) or by the e-folding time for exponential capacity depreciation.  The lifetime should refer to the plant type(s) for which capital costs have been reported. If capital cost for more than one plant type has been reported, modellers should report lifetime for the additional plant types by adding variables Lifetime|Electricity|Gas|w/o CCS|2, ... Lifetime|Electricity|Gas|w/o CCS|N (matching the assignment of plant types to technologies in the reporting of capital costs as documented in the comments sheet). </rdfs:comment>
    <ex:unit>years</ex:unit>
  </rdf:Description>
  <rdf:Description rdf:about="http://transience.eu/ontologies/Secondary_Energy_Other_Carrier">
    <rdf:type rdf:resource="http://www.w3.org/2002/07/owl#Class"/>
    <rdfs:subClassOf rdf:resource="http://transience.eu/ontologies/Variable"/>
    <rdfs:label>Secondary Energy|Other Carrier</rdfs:label>
    <rdfs:comment>generation of other secondary energy carriers that do not fit any other category (please provide a definition of other energy carrier in this category in the 'comments' tab)</rdfs:comment>
    <ex:unit>EJ/yr</ex:unit>
  </rdf:Description>
  <rdf:Description rdf:about="http://transience.eu/ontologies/Final_Energy_Commercial_Hydrogen">
    <rdf:type rdf:resource="http://www.w3.org/2002/07/owl#Class"/>
    <rdfs:subClassOf rdf:resource="http://transience.eu/ontologies/Variable"/>
    <rdfs:label>Final Energy|Commercial|Hydrogen</rdfs:label>
    <rdfs:comment>final energy consumption by the commercial sector of hydrogen</rdfs:comment>
    <ex:unit>EJ/yr</ex:unit>
  </rdf:Description>
  <rdf:Description rdf:about="http://transience.eu/ontologies/Final_Energy_Industry_Chemicals_Solar">
    <rdf:type rdf:resource="http://www.w3.org/2002/07/owl#Class"/>
    <rdfs:subClassOf rdf:resource="http://transience.eu/ontologies/Variable"/>
    <rdfs:label>Final Energy|Industry|Chemicals|Solar</rdfs:label>
    <rdfs:comment>Final energy consumption of solar thermal heat by the chemicals sector</rdfs:comment>
    <ex:unit>EJ/yr</ex:unit>
  </rdf:Description>
  <rdf:Description rdf:about="http://transience.eu/ontologies/Secondary_Energy_Liquids_Fossil_w__CCS">
    <rdf:type rdf:resource="http://www.w3.org/2002/07/owl#Class"/>
    <rdfs:subClassOf rdf:resource="http://transience.eu/ontologies/Variable"/>
    <rdfs:label>Secondary Energy|Liquids|Fossil|w/ CCS</rdfs:label>
    <rdfs:comment>total production of fossil liquid synfuels from facilities with CCS</rdfs:comment>
    <ex:unit>EJ/yr</ex:unit>
  </rdf:Description>
  <rdf:Description rdf:about="http://transience.eu/ontologies/Production_Non-Ferrous_Metals_Volume">
    <rdf:type rdf:resource="http://www.w3.org/2002/07/owl#Class"/>
    <rdfs:subClassOf rdf:resource="http://transience.eu/ontologies/Variable"/>
    <rdfs:label>Production|Non-Ferrous Metals|Volume</rdfs:label>
    <rdfs:comment>production of non-ferrous metals (e.g. copper, lead, aluminum)</rdfs:comment>
    <ex:unit>Mt/yr</ex:unit>
  </rdf:Description>
  <rdf:Description rdf:about="http://transience.eu/ontologies/Secondary_Energy_Liquids_Fossil">
    <rdf:type rdf:resource="http://www.w3.org/2002/07/owl#Class"/>
    <rdfs:subClassOf rdf:resource="http://transience.eu/ontologies/Variable"/>
    <rdfs:label>Secondary Energy|Liquids|Fossil</rdfs:label>
    <rdfs:comment>total production of fossil liquid synfuels</rdfs:comment>
    <ex:unit>EJ/yr</ex:unit>
  </rdf:Description>
  <rdf:Description rdf:about="http://transience.eu/ontologies/Collected_Scrap_Iron_and_Steel_Transportation">
    <rdf:type rdf:resource="http://www.w3.org/2002/07/owl#Class"/>
    <rdfs:subClassOf rdf:resource="http://transience.eu/ontologies/Variable"/>
    <rdfs:label>Collected Scrap|Iron and Steel|Transportation</rdfs:label>
    <rdfs:comment>Collected iron &amp; steel scrap coming from transport sector (available to be used in recycling)</rdfs:comment>
    <ex:unit>Mt/yr</ex:unit>
  </rdf:Description>
  <rdf:Description rdf:about="http://transience.eu/ontologies/Final_Energy_Industry_Non-Ferrous_Metals_Liquids_Fossil">
    <rdf:type rdf:resource="http://www.w3.org/2002/07/owl#Class"/>
    <rdfs:subClassOf rdf:resource="http://transience.eu/ontologies/Variable"/>
    <rdfs:label>Final Energy|Industry|Non-Ferrous Metals|Liquids|Fossil</rdfs:label>
    <rdfs:comment>Final energy consumption of liquids of fossil origin (conventional &amp; unconventional petroleum, coal-to-liquids, gas-to-liquids)by the non-ferrous metals sector</rdfs:comment>
    <ex:unit>EJ/yr</ex:unit>
  </rdf:Description>
  <rdf:Description rdf:about="http://transience.eu/ontologies/Trade_Primary_Energy_Oil_Volume">
    <rdf:type rdf:resource="http://www.w3.org/2002/07/owl#Class"/>
    <rdfs:subClassOf rdf:resource="http://transience.eu/ontologies/Variable"/>
    <rdfs:label>Trade|Primary Energy|Oil|Volume</rdfs:label>
    <rdfs:comment>net exports of crude oil, at the global level these should add up to the trade losses only</rdfs:comment>
    <ex:unit>EJ/yr</ex:unit>
  </rdf:Description>
  <rdf:Description rdf:about="http://transience.eu/ontologies/Lifetime_Liquids_Coal_w_o_CCS">
    <rdf:type rdf:resource="http://www.w3.org/2002/07/owl#Class"/>
    <rdfs:subClassOf rdf:resource="http://transience.eu/ontologies/Variable"/>
    <rdfs:label>Lifetime|Liquids|Coal|w/o CCS</rdfs:label>
    <rdfs:comment>Lifetime of a new coal to liquids plant w/o CCS. Lifetime should be calculated by summing all vintages of a  capacity unit (e.g. (1+1+0.9+0.7+0.5) * 10 years = 41 years) or by the e-folding time for exponential capacity depreciation.  The lifetime should refer to the plant type(s) for which capital costs have been reported. If capital cost for more than one plant type has been reported, modellers should report lifetime for the additional plant types by adding variables Lifetime|Liquids|Coal|w/o CCS|2, ... Lifetime|Liquids|Coal|w/o CCS|N (matching the assignment of plant types to technologies in the reporting of capital costs as documented in the comments sheet). </rdfs:comment>
    <ex:unit>years</ex:unit>
  </rdf:Description>
  <rdf:Description rdf:about="http://transience.eu/ontologies/Final_Energy_Industry_Non-Ferrous_Metals_Electricity">
    <rdf:type rdf:resource="http://www.w3.org/2002/07/owl#Class"/>
    <rdfs:subClassOf rdf:resource="http://transience.eu/ontologies/Variable"/>
    <rdfs:label>Final Energy|Industry|Non-Ferrous Metals|Electricity</rdfs:label>
    <rdfs:comment>Final energy consumption of electricity of the non-ferrous metals sector</rdfs:comment>
    <ex:unit>EJ/yr</ex:unit>
  </rdf:Description>
  <rdf:Description rdf:about="http://transience.eu/ontologies/OM_Cost_Fixed_Gases_Coal_w_o_CCS">
    <rdf:type rdf:resource="http://www.w3.org/2002/07/owl#Class"/>
    <rdfs:subClassOf rdf:resource="http://transience.eu/ontologies/Variable"/>
    <rdfs:label>OM Cost|Fixed|Gases|Coal|w/o CCS</rdfs:label>
    <rdfs:comment>Annual fixed operation &amp; maintainance cost of a new coal to gas plant w/o CCS. If more than one coal to gas technology is modelled, modellers should report fixed O&amp;M costs  for each represented coal to gas technology by adding variables OM Cost|Fixed|Gases|Coal|w/o CCS|2, ... OM Cost|Fixed|Gases|Coal|w/o CCS|N (with N = number of represented technologies) (matching the assignment of plant types to technologies in the reporting of capital costs as documented in the comments sheet).</rdfs:comment>
    <ex:unit>US$2010/kW/yr</ex:unit>
  </rdf:Description>
  <rdf:Description rdf:about="http://transience.eu/ontologies/Capacity_Electricity_Gas_w__CCS">
    <rdf:type rdf:resource="http://www.w3.org/2002/07/owl#Class"/>
    <rdfs:subClassOf rdf:resource="http://transience.eu/ontologies/Variable"/>
    <rdfs:label>Capacity|Electricity|Gas|w/ CCS</rdfs:label>
    <rdfs:comment>Total installed (available) capacity of gas power plants with CCS, including plants held in an operating reserve. The installed (available) capacity of CCS gas power plants by plant type for which capital costs are reported should be reported by adding variables Capacity|Electricity|Gas|w/ CCS|1, ..., Capacity|Electricity|Gas|w/ CCS|N (matching the assignment of plant types to technologies in the reporting of capital costs as documented in the comments sheet). </rdfs:comment>
    <ex:unit>GW</ex:unit>
  </rdf:Description>
  <rdf:Description rdf:about="http://transience.eu/ontologies/Carbon_Capture_Biomass_Energy_Supply">
    <rdf:type rdf:resource="http://www.w3.org/2002/07/owl#Class"/>
    <rdfs:subClassOf rdf:resource="http://transience.eu/ontologies/Variable"/>
    <rdfs:label>Carbon Capture|Biomass|Energy|Supply</rdfs:label>
    <rdfs:comment>total carbon dioxide emissions captured  from bioenergy use, should be reported as positive numbers</rdfs:comment>
    <ex:unit>Mt CO2/yr</ex:unit>
  </rdf:Description>
  <rdf:Description rdf:about="http://transience.eu/ontologies/Emissions_CO2_AFOLU_Agriculture">
    <rdf:type rdf:resource="http://www.w3.org/2002/07/owl#Class"/>
    <rdfs:subClassOf rdf:resource="http://transience.eu/ontologies/Variable"/>
    <rdfs:label>Emissions|CO2|AFOLU|Agriculture</rdfs:label>
    <rdfs:comment>CO2 emissions from agriculture</rdfs:comment>
    <ex:unit>Mt CO2/yr</ex:unit>
  </rdf:Description>
  <rdf:Description rdf:about="http://transience.eu/ontologies/OM_Cost_Fixed_Electricity_Coal_w_o_CCS">
    <rdf:type rdf:resource="http://www.w3.org/2002/07/owl#Class"/>
    <rdfs:subClassOf rdf:resource="http://transience.eu/ontologies/Variable"/>
    <rdfs:label>OM Cost|Fixed|Electricity|Coal|w/o CCS</rdfs:label>
    <rdfs:comment>Annual fixed operation &amp; maintainance cost of a new coal power plant w/o CCS. If more than one coal power technology is modelled (e.g. subcritical PC, supercritical PC, IGCC), modellers should report fixed O&amp;M costs  for each represented coal power technology by adding variables OM Cost|Fixed|Electricity|Coal|w/o CCS|2, ... OM Cost|Fixed|Electricity|Coal|w/o CCS|N (with N = number of represented technologies) (matching the assignment of plant types to technologies in the reporting of capital costs as documented in the comments sheet).</rdfs:comment>
    <ex:unit>US$2010/kW/yr</ex:unit>
  </rdf:Description>
  <rdf:Description rdf:about="http://transience.eu/ontologies/Capacity_Electricity_Oil_w__CCS">
    <rdf:type rdf:resource="http://www.w3.org/2002/07/owl#Class"/>
    <rdfs:subClassOf rdf:resource="http://transience.eu/ontologies/Variable"/>
    <rdfs:label>Capacity|Electricity|Oil|w/ CCS</rdfs:label>
    <rdfs:comment>Total installed (available) capacity of oil power plants with CCS, including plants held in an operating reserve. The installed (available) capacity of CCS oil power plants by plant type for which capital costs are reported should be reported by adding variables Capacity|Electricity|Oil|w/ CCS|1, ..., Capacity|Electricity|Oil|w/ CCS|N (matching the assignment of plant types to technologies in the reporting of capital costs as documented in the comments sheet). </rdfs:comment>
    <ex:unit>GW</ex:unit>
  </rdf:Description>
  <rdf:Description rdf:about="http://transience.eu/ontologies/Secondary_Energy_Hydrogen_Oil">
    <rdf:type rdf:resource="http://www.w3.org/2002/07/owl#Class"/>
    <rdfs:subClassOf rdf:resource="http://transience.eu/ontologies/Variable"/>
    <rdfs:label>Secondary Energy|Hydrogen|Oil</rdfs:label>
    <rdfs:comment>hydrogen production from oil </rdfs:comment>
    <ex:unit>EJ/yr</ex:unit>
  </rdf:Description>
  <rdf:Description rdf:about="http://transience.eu/ontologies/Capital_Formation">
    <rdf:type rdf:resource="http://www.w3.org/2002/07/owl#Class"/>
    <rdfs:subClassOf rdf:resource="http://transience.eu/ontologies/Variable"/>
    <rdfs:label>Capital Formation</rdfs:label>
    <rdfs:comment>net additions to the physical capital stock</rdfs:comment>
    <ex:unit>billion US$2010/yr</ex:unit>
  </rdf:Description>
  <rdf:Description rdf:about="http://transience.eu/ontologies/Final_Energy_Transportation_Gases_Fossil">
    <rdf:type rdf:resource="http://www.w3.org/2002/07/owl#Class"/>
    <rdfs:subClassOf rdf:resource="http://transience.eu/ontologies/Variable"/>
    <rdfs:label>Final Energy|Transportation|Gases|Fossil</rdfs:label>
    <rdfs:comment>final energy consumption by the transportation sector of synthetic or derived gases of fossil origin</rdfs:comment>
    <ex:unit>EJ/yr</ex:unit>
  </rdf:Description>
  <rdf:Description rdf:about="http://transience.eu/ontologies/Final_Energy_Non-Energy_Use_Chemicals_Gases">
    <rdf:type rdf:resource="http://www.w3.org/2002/07/owl#Class"/>
    <rdfs:subClassOf rdf:resource="http://transience.eu/ontologies/Variable"/>
    <rdfs:label>Final Energy|Non-Energy Use|Chemicals|Gases</rdfs:label>
    <rdfs:comment>Final energy consumption of gases by the chemical sector by the non-combustion processes</rdfs:comment>
    <ex:unit>EJ/yr</ex:unit>
  </rdf:Description>
  <rdf:Description rdf:about="http://transience.eu/ontologies/Employment_Industry_Energy">
    <rdf:type rdf:resource="http://www.w3.org/2002/07/owl#Class"/>
    <rdfs:subClassOf rdf:resource="http://transience.eu/ontologies/Variable"/>
    <rdfs:label>Employment|Industry|Energy</rdfs:label>
    <rdfs:comment>Number of employed inhabitants (payrolls) in energy related industries (based on ILO classification)</rdfs:comment>
    <ex:unit>million</ex:unit>
  </rdf:Description>
  <rdf:Description rdf:about="http://transience.eu/ontologies/Secondary_Energy_Electricity_Biomass_w_o_CCS">
    <rdf:type rdf:resource="http://www.w3.org/2002/07/owl#Class"/>
    <rdfs:subClassOf rdf:resource="http://transience.eu/ontologies/Variable"/>
    <rdfs:label>Secondary Energy|Electricity|Biomass|w/o CCS</rdfs:label>
    <rdfs:comment>net electricity production from municipal solid waste, purpose-grown biomass, crop residues, forest industry waste with freely vented CO2 emissions</rdfs:comment>
    <ex:unit>EJ/yr</ex:unit>
  </rdf:Description>
  <rdf:Description rdf:about="http://transience.eu/ontologies/Material_Consumption_Domestic">
    <rdf:type rdf:resource="http://www.w3.org/2002/07/owl#Class"/>
    <rdfs:subClassOf rdf:resource="http://transience.eu/ontologies/Variable"/>
    <rdfs:label>Material Consumption|Domestic</rdfs:label>
    <rdfs:comment>Domestic material consumption</rdfs:comment>
    <ex:unit>Mt/year</ex:unit>
  </rdf:Description>
  <rdf:Description rdf:about="http://transience.eu/ontologies/Production_Iron_and_Steel_Secondary_Steel_Value">
    <rdf:type rdf:resource="http://www.w3.org/2002/07/owl#Class"/>
    <rdfs:subClassOf rdf:resource="http://transience.eu/ontologies/Variable"/>
    <rdfs:label>Production|Iron and Steel|Secondary Steel|Value</rdfs:label>
    <rdfs:comment>Production of secondary steel from recycling of scrap</rdfs:comment>
    <ex:unit>billion US$2010/yr</ex:unit>
  </rdf:Description>
  <rdf:Description rdf:about="http://transience.eu/ontologies/Final_Energy_Industry_Other_Sector_Liquids_Electricity">
    <rdf:type rdf:resource="http://www.w3.org/2002/07/owl#Class"/>
    <rdfs:subClassOf rdf:resource="http://transience.eu/ontologies/Variable"/>
    <rdfs:label>Final Energy|Industry|Other Sector|Liquids|Electricity</rdfs:label>
    <rdfs:comment>Final energy consumption of synthetic liquid efuels ("power-to-liquid") by other industry sectors</rdfs:comment>
    <ex:unit>EJ/yr</ex:unit>
  </rdf:Description>
  <rdf:Description rdf:about="http://transience.eu/ontologies/Lifetime_Liquids_Oil">
    <rdf:type rdf:resource="http://www.w3.org/2002/07/owl#Class"/>
    <rdfs:subClassOf rdf:resource="http://transience.eu/ontologies/Variable"/>
    <rdfs:label>Lifetime|Liquids|Oil</rdfs:label>
    <rdfs:comment>Lifetime of a new oil refining plant. Lifetime should be calculated by summing all vintages of a  capacity unit (e.g. (1+1+0.9+0.7+0.5) * 10 years = 41 years) or by the e-folding time for exponential capacity depreciation.  The lifetime should refer to the plant type(s) for which capital costs have been reported. If capital cost for more than one plant type has been reported, modellers should report lifetime for the additional plant types by adding variables Lifetime|Liquids|Oil|w/ CCS|2, ... Lifetime|Liquids|Oil|w/ CCS|N (matching the assignment of plant types to technologies in the reporting of capital costs as documented in the comments sheet). </rdfs:comment>
    <ex:unit>years</ex:unit>
  </rdf:Description>
  <rdf:Description rdf:about="http://transience.eu/ontologies/Final_Energy_Transportation_Hydrogen_Electricity">
    <rdf:type rdf:resource="http://www.w3.org/2002/07/owl#Class"/>
    <rdfs:subClassOf rdf:resource="http://transience.eu/ontologies/Variable"/>
    <rdfs:label>Final Energy|Transportation|Hydrogen|Electricity</rdfs:label>
    <rdfs:comment>final energy consumption by the transportation sector of green hydrogen</rdfs:comment>
    <ex:unit>EJ/yr</ex:unit>
  </rdf:Description>
  <rdf:Description rdf:about="http://transience.eu/ontologies/Total_Scrap_Iron_and_Steel">
    <rdf:type rdf:resource="http://www.w3.org/2002/07/owl#Class"/>
    <rdfs:subClassOf rdf:resource="http://transience.eu/ontologies/Variable"/>
    <rdfs:label>Total Scrap|Iron and Steel</rdfs:label>
    <rdfs:comment>Total potential of iron &amp; steel scrap material as a result of end of life products (before collection)</rdfs:comment>
    <ex:unit>Mt/yr</ex:unit>
  </rdf:Description>
  <rdf:Description rdf:about="http://transience.eu/ontologies/Investment_Energy_Demand_Transportation_Freight_Road_HDT_ICE">
    <rdf:type rdf:resource="http://www.w3.org/2002/07/owl#Class"/>
    <rdfs:subClassOf rdf:resource="http://transience.eu/ontologies/Variable"/>
    <rdfs:label>Investment|Energy Demand|Transportation|Freight|Road|HDT|ICE</rdfs:label>
    <rdfs:comment>investments into new vehicle technologies in the transport sector (heavy-duty freight trucks: internal combustion engine technologies running on any type of liquid or gaseous fuel)</rdfs:comment>
    <ex:unit>billion US$2010/yr</ex:unit>
  </rdf:Description>
  <rdf:Description rdf:about="http://transience.eu/ontologies/Energy_Service_Transportation_Passenger_Road_Bus">
    <rdf:type rdf:resource="http://www.w3.org/2002/07/owl#Class"/>
    <rdfs:subClassOf rdf:resource="http://transience.eu/ontologies/Variable"/>
    <rdfs:label>Energy Service|Transportation|Passenger|Road|Bus</rdfs:label>
    <rdfs:comment>energy service demand for passenger transport on roads (buses)</rdfs:comment>
    <ex:unit>bn pkm/yr</ex:unit>
  </rdf:Description>
  <rdf:Description rdf:about="http://transience.eu/ontologies/Final_Energy_Commercial_Electricity">
    <rdf:type rdf:resource="http://www.w3.org/2002/07/owl#Class"/>
    <rdfs:subClassOf rdf:resource="http://transience.eu/ontologies/Variable"/>
    <rdfs:label>Final Energy|Commercial|Electricity</rdfs:label>
    <rdfs:comment>final energy consumption by the commercial sector of electricity (including on-site solar PV), excluding transmission/distribution losses</rdfs:comment>
    <ex:unit>EJ/yr</ex:unit>
  </rdf:Description>
  <rdf:Description rdf:about="http://transience.eu/ontologies/Final_Energy_Residential_Gases_Fossil">
    <rdf:type rdf:resource="http://www.w3.org/2002/07/owl#Class"/>
    <rdfs:subClassOf rdf:resource="http://transience.eu/ontologies/Variable"/>
    <rdfs:label>Final Energy|Residential|Gases|Fossil</rdfs:label>
    <rdfs:comment>final energy consumption by the residential sector of  synthetic or derived gases of fossil origin, excluding transmission/distribution losses</rdfs:comment>
    <ex:unit>EJ/yr</ex:unit>
  </rdf:Description>
  <rdf:Description rdf:about="http://transience.eu/ontologies/Cost_Production_Steel_DRI_SAF_BOF_H2">
    <rdf:type rdf:resource="http://www.w3.org/2002/07/owl#Class"/>
    <rdfs:subClassOf rdf:resource="http://transience.eu/ontologies/Variable"/>
    <rdfs:label>Cost|Production|Steel|DRI_SAF_BOF_H2</rdfs:label>
    <rdfs:comment>Specific production cost of crude steel in DRI/Smelter/BOF route when using hydrogen as reducing gas; including CAPEX (annuity), fixed and variable OPEX</rdfs:comment>
    <ex:unit>Mio â‚¬_2022 / t crude steel</ex:unit>
  </rdf:Description>
  <rdf:Description rdf:about="http://transience.eu/ontologies/Secondary_Energy_Hydrogen_Electricity">
    <rdf:type rdf:resource="http://www.w3.org/2002/07/owl#Class"/>
    <rdfs:subClassOf rdf:resource="http://transience.eu/ontologies/Variable"/>
    <rdfs:label>Secondary Energy|Hydrogen|Electricity</rdfs:label>
    <rdfs:comment>hydrogen production from electricity via electrolysis</rdfs:comment>
    <ex:unit>EJ/yr</ex:unit>
  </rdf:Description>
  <rdf:Description rdf:about="http://transience.eu/ontologies/Price_Primary_Energy_Gas">
    <rdf:type rdf:resource="http://www.w3.org/2002/07/owl#Class"/>
    <rdfs:subClassOf rdf:resource="http://transience.eu/ontologies/Variable"/>
    <rdfs:label>Price|Primary Energy|Gas</rdfs:label>
    <rdfs:comment>natural gas price at the primary level (i.e. the spot price at the global or regional market)</rdfs:comment>
    <ex:unit>US$2010/GJ</ex:unit>
  </rdf:Description>
  <rdf:Description rdf:about="http://transience.eu/ontologies/Primary_Energy_Oil_w__CCS">
    <rdf:type rdf:resource="http://www.w3.org/2002/07/owl#Class"/>
    <rdfs:subClassOf rdf:resource="http://transience.eu/ontologies/Variable"/>
    <rdfs:label>Primary Energy|Oil|w/ CCS</rdfs:label>
    <rdfs:comment>conventional &amp; unconventional oil primary energy consumption used in combination with CCS</rdfs:comment>
    <ex:unit>EJ/yr</ex:unit>
  </rdf:Description>
  <rdf:Description rdf:about="http://transience.eu/ontologies/Trade_Primary_Energy_Gas_Value">
    <rdf:type rdf:resource="http://www.w3.org/2002/07/owl#Class"/>
    <rdfs:subClassOf rdf:resource="http://transience.eu/ontologies/Variable"/>
    <rdfs:label>Trade|Primary Energy|Gas|Value</rdfs:label>
    <rdfs:comment>value of net exports of natural gas, at the global level these should add up to the trade losses only</rdfs:comment>
    <ex:unit>billion US$2010/yr</ex:unit>
  </rdf:Description>
  <rdf:Description rdf:about="http://transience.eu/ontologies/Revenue_government_Tax">
    <rdf:type rdf:resource="http://www.w3.org/2002/07/owl#Class"/>
    <rdfs:subClassOf rdf:resource="http://transience.eu/ontologies/Variable"/>
    <rdfs:label>Revenue|government|Tax</rdfs:label>
    <rdfs:comment>government revenue from taxes</rdfs:comment>
    <ex:unit>billion US$2010/yr</ex:unit>
  </rdf:Description>
  <rdf:Description rdf:about="http://transience.eu/ontologies/Emissions_CO2_Industrial_Processes_Non-Metallic_Minerals">
    <rdf:type rdf:resource="http://www.w3.org/2002/07/owl#Class"/>
    <rdfs:subClassOf rdf:resource="http://transience.eu/ontologies/Variable"/>
    <rdfs:label>Emissions|CO2|Industrial Processes|Non-Metallic Minerals</rdfs:label>
    <rdfs:comment>CO2 emissions from industrial processes from non-metallic minerals</rdfs:comment>
    <ex:unit>Mt CO2/yr</ex:unit>
  </rdf:Description>
  <rdf:Description rdf:about="http://transience.eu/ontologies/Capital_Cost_Electricity_Coal_w__CCS">
    <rdf:type rdf:resource="http://www.w3.org/2002/07/owl#Class"/>
    <rdfs:subClassOf rdf:resource="http://transience.eu/ontologies/Variable"/>
    <rdfs:label>Capital Cost|Electricity|Coal|w/ CCS</rdfs:label>
    <rdfs:comment>Capital cost of a new coal power plant with CCS. If more than one CCS coal power technology is modelled (e.g. subcritical PC with post-combustion capture, supercritical PC with post-combustion capture, supercritical PC with oxyfuel combustion and capture, IGCC with pre-combustion capture), modellers should report capital costs for each represented CCS coal power technology by adding variables Capital Cost|Electricity|Coal|w/ CCS|2, ... Capital Cost|Electricity|Coal|w/ CCS|N (with N = number of represented technologies). It is modeller's choice which CCS coal power technologies to assign to type 1 (assigned to the variable without number suffix),2,...,N. The assignment should be documented in the comments sheet. </rdfs:comment>
    <ex:unit>US$2010/kW</ex:unit>
  </rdf:Description>
  <rdf:Description rdf:about="http://transience.eu/ontologies/Secondary_Energy_Hydrogen_Coal_w__CCS">
    <rdf:type rdf:resource="http://www.w3.org/2002/07/owl#Class"/>
    <rdfs:subClassOf rdf:resource="http://transience.eu/ontologies/Variable"/>
    <rdfs:label>Secondary Energy|Hydrogen|Coal|w/ CCS</rdfs:label>
    <rdfs:comment>hydrogen production from coal with a CO2 capture component</rdfs:comment>
    <ex:unit>EJ/yr</ex:unit>
  </rdf:Description>
  <rdf:Description rdf:about="http://transience.eu/ontologies/Production_Steel_DRI_DRI_natural_gas_Volume">
    <rdf:type rdf:resource="http://www.w3.org/2002/07/owl#Class"/>
    <rdfs:subClassOf rdf:resource="http://transience.eu/ontologies/Variable"/>
    <rdfs:label>Production|Steel|DRI|DRI natural gas|Volume</rdfs:label>
    <rdfs:comment>Production of DRI using natural gas as reducing gas (including DRI which is processed into steel)</rdfs:comment>
    <ex:unit>Mt/yr</ex:unit>
  </rdf:Description>
  <rdf:Description rdf:about="http://transience.eu/ontologies/Production_Iron_and_Steel_Primary_Steel_Volume">
    <rdf:type rdf:resource="http://www.w3.org/2002/07/owl#Class"/>
    <rdfs:subClassOf rdf:resource="http://transience.eu/ontologies/Variable"/>
    <rdfs:label>Production|Iron and Steel|Primary Steel|Volume</rdfs:label>
    <rdfs:comment>Production of primary / virgin steel</rdfs:comment>
    <ex:unit>Mt/yr</ex:unit>
  </rdf:Description>
  <rdf:Description rdf:about="http://transience.eu/ontologies/Outflow_Concrete_Other_demand_sectors_Product_categories">
    <rdf:type rdf:resource="http://www.w3.org/2002/07/owl#Class"/>
    <rdfs:subClassOf rdf:resource="http://transience.eu/ontologies/Variable"/>
    <rdfs:label>Outflow|Concrete|Other|[demand sectors]|[Product categories]</rdfs:label>
    <rdfs:comment>Concrete outflow from other sectorsÂ </rdfs:comment>
    <ex:unit>t/yr</ex:unit>
  </rdf:Description>
  <rdf:Description rdf:about="http://transience.eu/ontologies/Final_Energy_Industry_Non-Ferrous_Metals_Liquids">
    <rdf:type rdf:resource="http://www.w3.org/2002/07/owl#Class"/>
    <rdfs:subClassOf rdf:resource="http://transience.eu/ontologies/Variable"/>
    <rdfs:label>Final Energy|Industry|Non-Ferrous Metals|Liquids</rdfs:label>
    <rdfs:comment>Final energy consumption of refined liquids of the non-ferrous metals sector (conventional &amp; unconventional oil, biofuels, coal-to-liquids, gas-to-liquids, efuels)</rdfs:comment>
    <ex:unit>EJ/yr</ex:unit>
  </rdf:Description>
  <rdf:Description rdf:about="http://transience.eu/ontologies/Gross_Emissions_CO2">
    <rdf:type rdf:resource="http://www.w3.org/2002/07/owl#Class"/>
    <rdfs:subClassOf rdf:resource="http://transience.eu/ontologies/Variable"/>
    <rdfs:label>Gross Emissions|CO2</rdfs:label>
    <rdfs:comment>Gross CO2 emissions, not accounting for negative emissions e.g. from BECCS or AFOLU</rdfs:comment>
    <ex:unit>Mt CO2/yr</ex:unit>
  </rdf:Description>
  <rdf:Description rdf:about="http://transience.eu/ontologies/Capacity_Electricity_Coal_w_o_CCS">
    <rdf:type rdf:resource="http://www.w3.org/2002/07/owl#Class"/>
    <rdfs:subClassOf rdf:resource="http://transience.eu/ontologies/Variable"/>
    <rdfs:label>Capacity|Electricity|Coal|w/o CCS</rdfs:label>
    <rdfs:comment>Total installed (available) capacity of coal power plants without CCS, including plants held in an operating reserve. The installed (available) capacity of coal power plants by plant type for which capital costs are reported should be reported by adding variables Capacity|Electricity|Coal|w/o CCS|1, ..., Capacity|Electricity|Coal|w/o CCS|N (matching the assignment of plant types to technologies in the reporting of capital costs as documented in the comments sheet). </rdfs:comment>
    <ex:unit>GW</ex:unit>
  </rdf:Description>
  <rdf:Description rdf:about="http://transience.eu/ontologies/Production_Steel_DRI_DRI_hydrogen_Volume">
    <rdf:type rdf:resource="http://www.w3.org/2002/07/owl#Class"/>
    <rdfs:subClassOf rdf:resource="http://transience.eu/ontologies/Variable"/>
    <rdfs:label>Production|Steel|DRI|DRI hydrogen|Volume</rdfs:label>
    <rdfs:comment>Production of DRI using hydrogen as reducing gas (including DRI which is processed into steel)</rdfs:comment>
    <ex:unit>Mt/yr</ex:unit>
  </rdf:Description>
  <rdf:Description rdf:about="http://transience.eu/ontologies/Final_Energy_Industry_Chemicals">
    <rdf:type rdf:resource="http://www.w3.org/2002/07/owl#Class"/>
    <rdfs:subClassOf rdf:resource="http://transience.eu/ontologies/Variable"/>
    <rdfs:label>Final Energy|Industry|Chemicals</rdfs:label>
    <rdfs:comment>Final energy consumed by the chemicals sector, excluding feedstocks</rdfs:comment>
    <ex:unit>EJ/yr</ex:unit>
  </rdf:Description>
  <rdf:Description rdf:about="http://transience.eu/ontologies/Resource_use_Fossil_Hydrocarbons_Industry_Petrochemicals">
    <rdf:type rdf:resource="http://www.w3.org/2002/07/owl#Class"/>
    <rdfs:subClassOf rdf:resource="http://transience.eu/ontologies/Variable"/>
    <rdfs:label>Resource use|Fossil Hydrocarbons|Industry|Petrochemicals</rdfs:label>
    <rdfs:comment>Use of fossil hydrocarbons for non-energetic use including energetic use of by-products; C-content</rdfs:comment>
    <ex:unit>Mt C_eq/yr</ex:unit>
  </rdf:Description>
  <rdf:Description rdf:about="http://transience.eu/ontologies/Final_Energy_Residential_Gases_Electricity">
    <rdf:type rdf:resource="http://www.w3.org/2002/07/owl#Class"/>
    <rdfs:subClassOf rdf:resource="http://transience.eu/ontologies/Variable"/>
    <rdfs:label>Final Energy|Residential|Gases|Electricity</rdfs:label>
    <rdfs:comment>final energy consumption by the residential sector of synthetic e-fuel gas ("power-to-gas"), excluding transmission/distribution losses</rdfs:comment>
    <ex:unit>EJ/yr</ex:unit>
  </rdf:Description>
  <rdf:Description rdf:about="http://transience.eu/ontologies/Production_Chemicals_High_Value_Chemicals_Volume">
    <rdf:type rdf:resource="http://www.w3.org/2002/07/owl#Class"/>
    <rdfs:subClassOf rdf:resource="http://transience.eu/ontologies/Variable"/>
    <rdfs:label>Production|Chemicals|High Value Chemicals|Volume</rdfs:label>
    <rdfs:comment>production of high value chemicals (intermediate material for the production of plastics, high value chemicals include ethylene)</rdfs:comment>
    <ex:unit>Mt/yr</ex:unit>
  </rdf:Description>
  <rdf:Description rdf:about="http://transience.eu/ontologies/Primary_Energy_Industry_Steel_Natural_gas">
    <rdf:type rdf:resource="http://www.w3.org/2002/07/owl#Class"/>
    <rdfs:subClassOf rdf:resource="http://transience.eu/ontologies/Variable"/>
    <rdfs:label>Primary Energy|Industry|Steel|Natural gas</rdfs:label>
    <rdfs:comment>Energy demand including own coke ovens and autoproduction of electricity</rdfs:comment>
    <ex:unit>PJ/yr</ex:unit>
  </rdf:Description>
  <rdf:Description rdf:about="http://transience.eu/ontologies/Import_Other">
    <rdf:type rdf:resource="http://www.w3.org/2002/07/owl#Class"/>
    <rdfs:subClassOf rdf:resource="http://transience.eu/ontologies/Variable"/>
    <rdfs:label>Import|Other</rdfs:label>
    <rdfs:comment>import of other commodities measured in monetary units (please provide a definition of the sources in this category in the 'comments' tab).</rdfs:comment>
    <ex:unit>billion US$2010/yr</ex:unit>
  </rdf:Description>
  <rdf:Description rdf:about="http://transience.eu/ontologies/Emissions_CO2_Energy_Demand_Industry">
    <rdf:type rdf:resource="http://www.w3.org/2002/07/owl#Class"/>
    <rdfs:subClassOf rdf:resource="http://transience.eu/ontologies/Variable"/>
    <rdfs:label>Emissions|CO2|Energy|Demand|Industry</rdfs:label>
    <rdfs:comment>Fossil CO2 emissions from fuel combustion in industry (IPCC category 1A2), net of negative emissions from Bioenergy with CCS (BECCS), excluding emissions related to feedstocks</rdfs:comment>
    <ex:unit>Mt CO2/yr</ex:unit>
  </rdf:Description>
  <rdf:Description rdf:about="http://transience.eu/ontologies/Price_Secondary_Energy_Electricity">
    <rdf:type rdf:resource="http://www.w3.org/2002/07/owl#Class"/>
    <rdfs:subClassOf rdf:resource="http://transience.eu/ontologies/Variable"/>
    <rdfs:label>Price|Secondary Energy|Electricity</rdfs:label>
    <rdfs:comment>electricity price at the secondary level, i.e. for large scale consumers (e.g. aluminum production).  Prices should include the effect of carbon prices.</rdfs:comment>
    <ex:unit>US$2010/GJ</ex:unit>
  </rdf:Description>
  <rdf:Description rdf:about="http://transience.eu/ontologies/Primary_Energy_Oil_w_o_CCS">
    <rdf:type rdf:resource="http://www.w3.org/2002/07/owl#Class"/>
    <rdfs:subClassOf rdf:resource="http://transience.eu/ontologies/Variable"/>
    <rdfs:label>Primary Energy|Oil|w/o CCS</rdfs:label>
    <rdfs:comment>conventional &amp; unconventional oil primary energy consumption without CCS</rdfs:comment>
    <ex:unit>EJ/yr</ex:unit>
  </rdf:Description>
  <rdf:Description rdf:about="http://transience.eu/ontologies/Final_Energy_Industry_Iron_and_Steel_Liquids_Fossil">
    <rdf:type rdf:resource="http://www.w3.org/2002/07/owl#Class"/>
    <rdfs:subClassOf rdf:resource="http://transience.eu/ontologies/Variable"/>
    <rdfs:label>Final Energy|Industry|Iron and Steel|Liquids|Fossil</rdfs:label>
    <rdfs:comment>Final energy consumption of liquids of fossil origin by the iron and steel sector</rdfs:comment>
    <ex:unit>EJ/yr</ex:unit>
  </rdf:Description>
  <rdf:Description rdf:about="http://transience.eu/ontologies/Export_Industry_Iron_and_Steel_Primary_Steel_Volume">
    <rdf:type rdf:resource="http://www.w3.org/2002/07/owl#Class"/>
    <rdfs:subClassOf rdf:resource="http://transience.eu/ontologies/Variable"/>
    <rdfs:label>Export|Industry|Iron and Steel|Primary Steel|Volume</rdfs:label>
    <rdfs:comment>Export of primary steel</rdfs:comment>
    <ex:unit>Mt/yr</ex:unit>
  </rdf:Description>
  <rdf:Description rdf:about="http://transience.eu/ontologies/Carbon_Capture_Electricity">
    <rdf:type rdf:resource="http://www.w3.org/2002/07/owl#Class"/>
    <rdfs:subClassOf rdf:resource="http://transience.eu/ontologies/Variable"/>
    <rdfs:label>Carbon Capture|Electricity</rdfs:label>
    <rdfs:comment>total carbon dioxide emissions captured from hydrogen or synthetic fuel use, should be reported as positive numbers</rdfs:comment>
    <ex:unit>Mt CO2/yr</ex:unit>
  </rdf:Description>
  <rdf:Description rdf:about="http://transience.eu/ontologies/Primary_Energy_Fossil">
    <rdf:type rdf:resource="http://www.w3.org/2002/07/owl#Class"/>
    <rdfs:subClassOf rdf:resource="http://transience.eu/ontologies/Variable"/>
    <rdfs:label>Primary Energy|Fossil</rdfs:label>
    <rdfs:comment>coal, gas, conventional and unconventional oil primary energy consumption</rdfs:comment>
    <ex:unit>EJ/yr</ex:unit>
  </rdf:Description>
  <rdf:Description rdf:about="http://transience.eu/ontologies/Final_Energy_Carbon_Removal_Liquids">
    <rdf:type rdf:resource="http://www.w3.org/2002/07/owl#Class"/>
    <rdfs:subClassOf rdf:resource="http://transience.eu/ontologies/Variable"/>
    <rdfs:label>Final Energy|Carbon Removal|Liquids</rdfs:label>
    <rdfs:comment>Final energy consumption of liquids by carbon dioxide removal processes</rdfs:comment>
    <ex:unit>EJ/yr</ex:unit>
  </rdf:Description>
  <rdf:Description rdf:about="http://transience.eu/ontologies/Production_Chemicals_Plastics_Volume">
    <rdf:type rdf:resource="http://www.w3.org/2002/07/owl#Class"/>
    <rdfs:subClassOf rdf:resource="http://transience.eu/ontologies/Variable"/>
    <rdfs:label>Production|Chemicals|Plastics|Volume</rdfs:label>
    <rdfs:comment>production of plastics </rdfs:comment>
    <ex:unit>Mt/yr</ex:unit>
  </rdf:Description>
  <rdf:Description rdf:about="http://transience.eu/ontologies/Investment_Petrochemicals_Methanol_Synthesis">
    <rdf:type rdf:resource="http://www.w3.org/2002/07/owl#Class"/>
    <rdfs:subClassOf rdf:resource="http://transience.eu/ontologies/Variable"/>
    <rdfs:label>Investment|Petrochemicals|Methanol Synthesis</rdfs:label>
    <rdfs:comment>Investment in methanol synthesis (from syngas)</rdfs:comment>
    <ex:unit>Mio â‚¬_2022/yr</ex:unit>
  </rdf:Description>
  <rdf:Description rdf:about="http://transience.eu/ontologies/Production_Pulp_and_Paper_Value">
    <rdf:type rdf:resource="http://www.w3.org/2002/07/owl#Class"/>
    <rdfs:subClassOf rdf:resource="http://transience.eu/ontologies/Variable"/>
    <rdfs:label>Production|Pulp and Paper|Value</rdfs:label>
    <rdfs:comment>production of pulp and paper</rdfs:comment>
    <ex:unit>billion US$2010/yr</ex:unit>
  </rdf:Description>
  <rdf:Description rdf:about="http://transience.eu/ontologies/Final_Energy_Industry_Other_Sector_Solar">
    <rdf:type rdf:resource="http://www.w3.org/2002/07/owl#Class"/>
    <rdfs:subClassOf rdf:resource="http://transience.eu/ontologies/Variable"/>
    <rdfs:label>Final Energy|Industry|Other Sector|Solar</rdfs:label>
    <rdfs:comment>Final energy consumption of solar thermal heat by other industry sectors</rdfs:comment>
    <ex:unit>EJ/yr</ex:unit>
  </rdf:Description>
  <rdf:Description rdf:about="http://transience.eu/ontologies/Secondary_Energy_Heat_Nuclear">
    <rdf:type rdf:resource="http://www.w3.org/2002/07/owl#Class"/>
    <rdfs:subClassOf rdf:resource="http://transience.eu/ontologies/Variable"/>
    <rdfs:label>Secondary Energy|Heat|Nuclear</rdfs:label>
    <rdfs:comment>centralized heat generation from nuclear energy</rdfs:comment>
    <ex:unit>EJ/yr</ex:unit>
  </rdf:Description>
  <rdf:Description rdf:about="http://transience.eu/ontologies/OM_Cost_Fixed_Gases_Biomass_w_o_CCS">
    <rdf:type rdf:resource="http://www.w3.org/2002/07/owl#Class"/>
    <rdfs:subClassOf rdf:resource="http://transience.eu/ontologies/Variable"/>
    <rdfs:label>OM Cost|Fixed|Gases|Biomass|w/o CCS</rdfs:label>
    <rdfs:comment>Annual fixed operation &amp; maintainance cost of a new biomass to gas plant w/o CCS. If more than one biomass to gas technology is modelled, modellers should report fixed O&amp;M costs  for each represented biomass to gas technology by adding variables OM Cost|Fixed|Gases|Biomass|w/o CCS|2, ... OM Cost|Fixed|Gases|Biomass|w/o CCS|N (with N = number of represented technologies). (matching the assignment of plant types to technologies in the reporting of capital costs as documented in the comments sheet).</rdfs:comment>
    <ex:unit>US$2010/kW/yr</ex:unit>
  </rdf:Description>
  <rdf:Description rdf:about="http://transience.eu/ontologies/Import_Industry_Iron_and_Steel_Primary_Steel_Volume">
    <rdf:type rdf:resource="http://www.w3.org/2002/07/owl#Class"/>
    <rdfs:subClassOf rdf:resource="http://transience.eu/ontologies/Variable"/>
    <rdfs:label>Import|Industry|Iron and Steel|Primary Steel|Volume</rdfs:label>
    <rdfs:comment>Import of primary steel</rdfs:comment>
    <ex:unit>Mt/yr</ex:unit>
  </rdf:Description>
  <rdf:Description rdf:about="http://transience.eu/ontologies/Primary_Energy_Gas_Electricity">
    <rdf:type rdf:resource="http://www.w3.org/2002/07/owl#Class"/>
    <rdfs:subClassOf rdf:resource="http://transience.eu/ontologies/Variable"/>
    <rdfs:label>Primary Energy|Gas|Electricity</rdfs:label>
    <rdfs:comment>gas primary energy input to electricity generation </rdfs:comment>
    <ex:unit>EJ/yr</ex:unit>
  </rdf:Description>
  <rdf:Description rdf:about="http://transience.eu/ontologies/Lifetime_Liquids_Coal_w__CCS">
    <rdf:type rdf:resource="http://www.w3.org/2002/07/owl#Class"/>
    <rdfs:subClassOf rdf:resource="http://transience.eu/ontologies/Variable"/>
    <rdfs:label>Lifetime|Liquids|Coal|w/ CCS</rdfs:label>
    <rdfs:comment>Lifetime of a new coal to liquids plant with CCS. Lifetime should be calculated by summing all vintages of a  capacity unit (e.g. (1+1+0.9+0.7+0.5) * 10 years = 41 years) or by the e-folding time for exponential capacity depreciation.  The lifetime should refer to the plant type(s) for which capital costs have been reported. If capital cost for more than one plant type has been reported, modellers should report lifetime for the additional plant types by adding variables Lifetime|Liquids|Coal|w/ CCS|2, ... Lifetime|Liquids|Coal|w/ CCS|N (matching the assignment of plant types to technologies in the reporting of capital costs as documented in the comments sheet). </rdfs:comment>
    <ex:unit>years</ex:unit>
  </rdf:Description>
  <rdf:Description rdf:about="http://transience.eu/ontologies/Carbon_Capture_Fossil_Energy_Supply_Liquids">
    <rdf:type rdf:resource="http://www.w3.org/2002/07/owl#Class"/>
    <rdfs:subClassOf rdf:resource="http://transience.eu/ontologies/Variable"/>
    <rdfs:label>Carbon Capture|Fossil|Energy|Supply|Liquids</rdfs:label>
    <rdfs:comment>total carbon dioxide emissions captured from fossil fuel use in liquid fuel production (part of IPCC category 1A), should be reported as positive numbers</rdfs:comment>
    <ex:unit>Mt CO2/yr</ex:unit>
  </rdf:Description>
  <rdf:Description rdf:about="http://transience.eu/ontologies/Investment_Energy_Supply_Extraction_Coal">
    <rdf:type rdf:resource="http://www.w3.org/2002/07/owl#Class"/>
    <rdfs:subClassOf rdf:resource="http://transience.eu/ontologies/Variable"/>
    <rdfs:label>Investment|Energy Supply|Extraction|Coal</rdfs:label>
    <rdfs:comment>investments for extraction and conversion of coal. These should include mining, shipping and ports</rdfs:comment>
    <ex:unit>billion US$2010/yr</ex:unit>
  </rdf:Description>
  <rdf:Description rdf:about="http://transience.eu/ontologies/Emissions_CO2_Industrial_Processes">
    <rdf:type rdf:resource="http://www.w3.org/2002/07/owl#Class"/>
    <rdfs:subClassOf rdf:resource="http://transience.eu/ontologies/Variable"/>
    <rdfs:label>Emissions|CO2|Industrial Processes</rdfs:label>
    <rdfs:comment>CO2 emissions from industrial processes (IPCC categories 2A, B, C, E)</rdfs:comment>
    <ex:unit>Mt CO2/yr</ex:unit>
  </rdf:Description>
  <rdf:Description rdf:about="http://transience.eu/ontologies/Final_Energy_Industry_Non-Ferrous_Metals">
    <rdf:type rdf:resource="http://www.w3.org/2002/07/owl#Class"/>
    <rdfs:subClassOf rdf:resource="http://transience.eu/ontologies/Variable"/>
    <rdfs:label>Final Energy|Industry|Non-Ferrous Metals</rdfs:label>
    <rdfs:comment>Final energy consumption of the non-ferrous metals sector</rdfs:comment>
    <ex:unit>EJ/yr</ex:unit>
  </rdf:Description>
  <rdf:Description rdf:about="http://transience.eu/ontologies/Price_Final_Energy_Residential_Electricity">
    <rdf:type rdf:resource="http://www.w3.org/2002/07/owl#Class"/>
    <rdfs:subClassOf rdf:resource="http://transience.eu/ontologies/Variable"/>
    <rdfs:label>Price|Final Energy|Residential|Electricity</rdfs:label>
    <rdfs:comment>electricity price at the final level in the residential sector. Prices should include the effect of carbon prices.</rdfs:comment>
    <ex:unit>US$2010/GJ</ex:unit>
  </rdf:Description>
  <rdf:Description rdf:about="http://transience.eu/ontologies/Energy_Service_Transportation_Passenger_Road_2W_and_3W">
    <rdf:type rdf:resource="http://www.w3.org/2002/07/owl#Class"/>
    <rdfs:subClassOf rdf:resource="http://transience.eu/ontologies/Variable"/>
    <rdfs:label>Energy Service|Transportation|Passenger|Road|2W and 3W</rdfs:label>
    <rdfs:comment>energy service demand for passenger transport on roads (two- and three-wheel vehicles)</rdfs:comment>
    <ex:unit>bn pkm/yr</ex:unit>
  </rdf:Description>
  <rdf:Description rdf:about="http://transience.eu/ontologies/Investment_Energy_Supply_Liquids_Coal_and_Gas">
    <rdf:type rdf:resource="http://www.w3.org/2002/07/owl#Class"/>
    <rdfs:subClassOf rdf:resource="http://transience.eu/ontologies/Variable"/>
    <rdfs:label>Investment|Energy Supply|Liquids|Coal and Gas</rdfs:label>
    <rdfs:comment>investments for the production of fossil-based synfuels (coal and gas). For plants equipped with CCS, the investment in the capturing equipment should be included but not the one on transport and storage.</rdfs:comment>
    <ex:unit>billion US$2010/yr</ex:unit>
  </rdf:Description>
  <rdf:Description rdf:about="http://transience.eu/ontologies/Final_Energy_Industry_Pulp_and_Paper_Gases_Electricity">
    <rdf:type rdf:resource="http://www.w3.org/2002/07/owl#Class"/>
    <rdfs:subClassOf rdf:resource="http://transience.eu/ontologies/Variable"/>
    <rdfs:label>Final Energy|Industry|Pulp and Paper|Gases|Electricity</rdfs:label>
    <rdfs:comment>Final energy consumption of synthetic e-fuel gas ("power-to-gas") by the pulp and paper sector</rdfs:comment>
    <ex:unit>EJ/yr</ex:unit>
  </rdf:Description>
  <rdf:Description rdf:about="http://transience.eu/ontologies/Total_Scrap_Iron_and_Steel_Residential_and_Commercial">
    <rdf:type rdf:resource="http://www.w3.org/2002/07/owl#Class"/>
    <rdfs:subClassOf rdf:resource="http://transience.eu/ontologies/Variable"/>
    <rdfs:label>Total Scrap|Iron and Steel|Residential and Commercial</rdfs:label>
    <rdfs:comment>Total potential of iron &amp; steel scrap material as a result of end of life products (before collection)</rdfs:comment>
    <ex:unit>Mt/yr</ex:unit>
  </rdf:Description>
  <rdf:Description rdf:about="http://transience.eu/ontologies/Efficiency_Liquids_Biomass_w_o_CCS">
    <rdf:type rdf:resource="http://www.w3.org/2002/07/owl#Class"/>
    <rdfs:subClassOf rdf:resource="http://transience.eu/ontologies/Variable"/>
    <rdfs:label>Efficiency|Liquids|Biomass|w/o CCS</rdfs:label>
    <rdfs:comment>Conversion efficiency (energy content of liquids produced per unit of primary energy input) of a new biomass to liquids plant w/o CCS. The efficiency should refer to the plant type(s) for which capital costs have been reported. If capital cost for more than one plant type has been reported, modellers should report efficiency for the additional plant types by adding variables Efficiency|Liquids|Biomass|w/o CCS|2, ... Efficiency|Liquids|Biomass|w/o CCS|N (matching the assignment of plant types to technologies in the reporting of capital costs as documented in the comments sheet). </rdfs:comment>
    <ex:unit>%</ex:unit>
  </rdf:Description>
  <rdf:Description rdf:about="http://transience.eu/ontologies/Secondary_Energy_Electricity_Fossil_w__CCS">
    <rdf:type rdf:resource="http://www.w3.org/2002/07/owl#Class"/>
    <rdfs:subClassOf rdf:resource="http://transience.eu/ontologies/Variable"/>
    <rdfs:label>Secondary Energy|Electricity|Fossil|w/ CCS</rdfs:label>
    <rdfs:comment>net electricity production from coal, gas, conventional and unconventional oil used in combination with CCS</rdfs:comment>
    <ex:unit>EJ/yr</ex:unit>
  </rdf:Description>
  <rdf:Description rdf:about="http://transience.eu/ontologies/OM_Cost_Fixed_Liquids_Biomass_w__CCS">
    <rdf:type rdf:resource="http://www.w3.org/2002/07/owl#Class"/>
    <rdfs:subClassOf rdf:resource="http://transience.eu/ontologies/Variable"/>
    <rdfs:label>OM Cost|Fixed|Liquids|Biomass|w/ CCS</rdfs:label>
    <rdfs:comment>Annual fixed operation &amp; maintainance cost of a new biomass to liquids plant with CCS. If more than one CCS BTL technology is modelled, modellers should report fixed O&amp;M costs  for each represented CCS BTL technology by adding variables OM Cost|Fixed|Liquids|Biomass|w/ CCS|2, ... OM Cost|Fixed|Liquids|Biomass|w/ CCS|N (with N = number of represented technologies) (matching the assignment of plant types to technologies in the reporting of capital costs as documented in the comments sheet).</rdfs:comment>
    <ex:unit>US$2010/kW/yr</ex:unit>
  </rdf:Description>
  <rdf:Description rdf:about="http://transience.eu/ontologies/Final_Energy_Carbon_Removal_Enhanced_Weathering">
    <rdf:type rdf:resource="http://www.w3.org/2002/07/owl#Class"/>
    <rdfs:subClassOf rdf:resource="http://transience.eu/ontologies/Variable"/>
    <rdfs:label>Final Energy|Carbon Removal|Enhanced Weathering</rdfs:label>
    <rdfs:comment>Final energy consumption by enhanced weathering</rdfs:comment>
    <ex:unit>EJ/yr</ex:unit>
  </rdf:Description>
  <rdf:Description rdf:about="http://transience.eu/ontologies/OM_Cost_Fixed_Electricity_Biomass_w__CCS">
    <rdf:type rdf:resource="http://www.w3.org/2002/07/owl#Class"/>
    <rdfs:subClassOf rdf:resource="http://transience.eu/ontologies/Variable"/>
    <rdfs:label>OM Cost|Fixed|Electricity|Biomass|w/ CCS</rdfs:label>
    <rdfs:comment>Annual fixed operation &amp; maintainance cost of a new biomass power plant with CCS. If more than one CCS biomass power technology is modelled, modellers should report fixed O&amp;M costs  for each represented CCS biomass power technology by adding variables OM Cost|Fixed|Electricity|Biomass|w/ CCS|2, ... OM Cost|Fixed|Electricity|Biomass|w/ CCS|N (with N = number of represented technologies) (matching the assignment of plant types to technologies in the reporting of capital costs as documented in the comments sheet).</rdfs:comment>
    <ex:unit>US$2010/kW/yr</ex:unit>
  </rdf:Description>
  <rdf:Description rdf:about="http://transience.eu/ontologies/Production_Steel_Secondary_crude_steel_Volume">
    <rdf:type rdf:resource="http://www.w3.org/2002/07/owl#Class"/>
    <rdfs:subClassOf rdf:resource="http://transience.eu/ontologies/Variable"/>
    <rdfs:label>Production|Steel|Secondary crude steel|Volume</rdfs:label>
    <rdfs:comment>Production of secondary crude steel</rdfs:comment>
    <ex:unit>Mt/yr</ex:unit>
  </rdf:Description>
  <rdf:Description rdf:about="http://transience.eu/ontologies/Secondary_Energy_Electricity_Hydro">
    <rdf:type rdf:resource="http://www.w3.org/2002/07/owl#Class"/>
    <rdfs:subClassOf rdf:resource="http://transience.eu/ontologies/Variable"/>
    <rdfs:label>Secondary Energy|Electricity|Hydro</rdfs:label>
    <rdfs:comment>net hydroelectric production</rdfs:comment>
    <ex:unit>EJ/yr</ex:unit>
  </rdf:Description>
  <rdf:Description rdf:about="http://transience.eu/ontologies/Efficiency_Electricity_Gas_w_o_CCS">
    <rdf:type rdf:resource="http://www.w3.org/2002/07/owl#Class"/>
    <rdfs:subClassOf rdf:resource="http://transience.eu/ontologies/Variable"/>
    <rdfs:label>Efficiency|Electricity|Gas|w/o CCS</rdfs:label>
    <rdfs:comment>Conversion efficiency (electricity produced per unit of primary energy input) of a new gas power plant w/o CCS. The efficiency should refer to the plant type(s) for which capital costs have been reported. If capital cost for more than one plant type has been reported, modellers should report efficiency for the additional plant types by adding variables Efficiency|Electricity|Gas|w/o CCS|2, ... Efficiency|Electricity|Gas|w/o CCS|N (matching the assignment of plant types to technologies in the reporting of capital costs as documented in the comments sheet). </rdfs:comment>
    <ex:unit>%</ex:unit>
  </rdf:Description>
  <rdf:Description rdf:about="http://transience.eu/ontologies/Efficiency_Electricity_Coal_w_o_CCS">
    <rdf:type rdf:resource="http://www.w3.org/2002/07/owl#Class"/>
    <rdfs:subClassOf rdf:resource="http://transience.eu/ontologies/Variable"/>
    <rdfs:label>Efficiency|Electricity|Coal|w/o CCS</rdfs:label>
    <rdfs:comment>Conversion efficiency (electricity produced per unit of primary energy input) of a new coal power plant w/o CCS. The efficiency should refer to the plant type(s) for which capital costs have been reported. If capital cost for more than one plant type has been reported, modellers should report efficiency for the additional plant types by adding variables Efficiency|Electricity|Coal|w/o CCS|2, ... Efficiency|Electricity|Coal|w/o CCS|N (matching the assignment of plant types to technologies in the reporting of capital costs as documented in the comments sheet). </rdfs:comment>
    <ex:unit>%</ex:unit>
  </rdf:Description>
  <rdf:Description rdf:about="http://transience.eu/ontologies/Emissions_CO2_Energy_Demand_Industry_Steel">
    <rdf:type rdf:resource="http://www.w3.org/2002/07/owl#Class"/>
    <rdfs:subClassOf rdf:resource="http://transience.eu/ontologies/Variable"/>
    <rdfs:label>Emissions|CO2|Energy|Demand|Industry|Steel</rdfs:label>
    <rdfs:comment>Fossil CO2 emissions from fuel combustion in industry in the iron and steel sector</rdfs:comment>
    <ex:unit>Mt CO2/yr</ex:unit>
  </rdf:Description>
  <rdf:Description rdf:about="http://transience.eu/ontologies/Investment_Energy_Supply_Electricity_Nuclear">
    <rdf:type rdf:resource="http://www.w3.org/2002/07/owl#Class"/>
    <rdfs:subClassOf rdf:resource="http://transience.eu/ontologies/Variable"/>
    <rdfs:label>Investment|Energy Supply|Electricity|Nuclear</rdfs:label>
    <rdfs:comment>investments in new power generation for the specified power plant category. If the model features several sub-categories, the total investments should be reported. For plants equipped with CCS, the investment in the capturing equipment should be included but not the one on transport and storage.</rdfs:comment>
    <ex:unit>billion US$2010/yr</ex:unit>
  </rdf:Description>
  <rdf:Description rdf:about="http://transience.eu/ontologies/OM_Cost_Fixed_Electricity_Gas_w__CCS">
    <rdf:type rdf:resource="http://www.w3.org/2002/07/owl#Class"/>
    <rdfs:subClassOf rdf:resource="http://transience.eu/ontologies/Variable"/>
    <rdfs:label>OM Cost|Fixed|Electricity|Gas|w/ CCS</rdfs:label>
    <rdfs:comment>Annual fixed operation &amp; maintainance cost of a new gas power plant with CCS. If more than one CCS gas power technology is modelled, modellers should report fixed O&amp;M costs  for each represented CCS gas power technology by adding variables OM Cost|Fixed|Electricity|Gas|w/ CCS|2, ... OM Cost|Fixed|Electricity|Gas|w/ CCS|N (with N = number of represented technologies) (matching the assignment of plant types to technologies in the reporting of capital costs as documented in the comments sheet).</rdfs:comment>
    <ex:unit>US$2010/kW/yr</ex:unit>
  </rdf:Description>
  <rdf:Description rdf:about="http://transience.eu/ontologies/Export_Industry_Iron_and_Steel_Secondary">
    <rdf:type rdf:resource="http://www.w3.org/2002/07/owl#Class"/>
    <rdfs:subClassOf rdf:resource="http://transience.eu/ontologies/Variable"/>
    <rdfs:label>Export|Industry|Iron and Steel|Secondary</rdfs:label>
    <rdfs:comment>Export of secondary steel measured in monetary units</rdfs:comment>
    <ex:unit>billion US$2010/yr</ex:unit>
  </rdf:Description>
  <rdf:Description rdf:about="http://transience.eu/ontologies/Investment_Petrochemicals_Other_Biomass_to_Chemicals_Routes">
    <rdf:type rdf:resource="http://www.w3.org/2002/07/owl#Class"/>
    <rdfs:subClassOf rdf:resource="http://transience.eu/ontologies/Variable"/>
    <rdfs:label>Investment|Petrochemicals|Other Biomass to Chemicals Routes</rdfs:label>
    <rdfs:comment>Investments in plants to produce sugar from lignocellulosic biomass via Organosolv process</rdfs:comment>
    <ex:unit>Mio â‚¬_2022/yr</ex:unit>
  </rdf:Description>
  <rdf:Description rdf:about="http://transience.eu/ontologies/Final_Energy_Non-Energy_Use_Solids">
    <rdf:type rdf:resource="http://www.w3.org/2002/07/owl#Class"/>
    <rdfs:subClassOf rdf:resource="http://transience.eu/ontologies/Variable"/>
    <rdfs:label>Final Energy|Non-Energy Use|Solids</rdfs:label>
    <rdfs:comment>final energy consumption of solids by the non-combustion processes</rdfs:comment>
    <ex:unit>EJ/yr</ex:unit>
  </rdf:Description>
  <rdf:Description rdf:about="http://transience.eu/ontologies/Import_Industry_Chemicals_High_Value_Chemicals_Volume">
    <rdf:type rdf:resource="http://www.w3.org/2002/07/owl#Class"/>
    <rdfs:subClassOf rdf:resource="http://transience.eu/ontologies/Variable"/>
    <rdfs:label>Import|Industry|Chemicals|High Value Chemicals|Volume</rdfs:label>
    <rdfs:comment>Import of high value chemicals</rdfs:comment>
    <ex:unit>Mt/yr</ex:unit>
  </rdf:Description>
  <rdf:Description rdf:about="http://transience.eu/ontologies/Energy_Service_Transportation_Passenger_Domestic_Navigation">
    <rdf:type rdf:resource="http://www.w3.org/2002/07/owl#Class"/>
    <rdfs:subClassOf rdf:resource="http://transience.eu/ontologies/Variable"/>
    <rdfs:label>Energy Service|Transportation|Passenger|Domestic Navigation</rdfs:label>
    <rdfs:comment>energy service demand for passenger transport on domestic ships</rdfs:comment>
    <ex:unit>bn pkm/yr</ex:unit>
  </rdf:Description>
  <rdf:Description rdf:about="http://transience.eu/ontologies/Capacity_Electricity_Solar_PV">
    <rdf:type rdf:resource="http://www.w3.org/2002/07/owl#Class"/>
    <rdfs:subClassOf rdf:resource="http://transience.eu/ontologies/Variable"/>
    <rdfs:label>Capacity|Electricity|Solar|PV</rdfs:label>
    <rdfs:comment>Total installed (available) capacity of solar PV power plants. The installed (available) capacity of solar PV power plants by plant type for which capital costs are reported should be reported by adding variables Capacity|Electricity|Solar|PV|1, ..., Capacity|Electricity|Solar|PV|N (matching the assignment of plant types to technologies in the reporting of capital costs as documented in the comments sheet). </rdfs:comment>
    <ex:unit>GW</ex:unit>
  </rdf:Description>
  <rdf:Description rdf:about="http://transience.eu/ontologies/Final_Energy_Industry_Non-Ferrous_Metals_Gases_Electricity">
    <rdf:type rdf:resource="http://www.w3.org/2002/07/owl#Class"/>
    <rdfs:subClassOf rdf:resource="http://transience.eu/ontologies/Variable"/>
    <rdfs:label>Final Energy|Industry|Non-Ferrous Metals|Gases|Electricity</rdfs:label>
    <rdfs:comment>Final energy consumption of synthetic e-fuel gas ("power-to-gas") by the non-ferrous metals sector</rdfs:comment>
    <ex:unit>EJ/yr</ex:unit>
  </rdf:Description>
  <rdf:Description rdf:about="http://transience.eu/ontologies/Efficiency_Hydrogen_Biomass_w__CCS">
    <rdf:type rdf:resource="http://www.w3.org/2002/07/owl#Class"/>
    <rdfs:subClassOf rdf:resource="http://transience.eu/ontologies/Variable"/>
    <rdfs:label>Efficiency|Hydrogen|Biomass|w/ CCS</rdfs:label>
    <rdfs:comment>Conversion efficiency (energy content of hydrogen produced per unit of primary energy input) of a new biomass to hydrogen plant with CCS. The efficiency should refer to the plant type(s) for which capital costs have been reported. If capital cost for more than one plant type has been reported, modellers should report efficiency for the additional plant types by adding variables Efficiency|Hydrogen|Biomass|w/ CCS|2, ... Efficiency|Hydrogen|Biomass|w/ CCS|N (matching the assignment of plant types to technologies in the reporting of capital costs as documented in the comments sheet). </rdfs:comment>
    <ex:unit>%</ex:unit>
  </rdf:Description>
  <rdf:Description rdf:about="http://transience.eu/ontologies/Outflow_Plastics_Product_categories">
    <rdf:type rdf:resource="http://www.w3.org/2002/07/owl#Class"/>
    <rdfs:subClassOf rdf:resource="http://transience.eu/ontologies/Variable"/>
    <rdfs:label>Outflow|Plastics|[Product categories]</rdfs:label>
    <rdfs:comment>Plastics outflowÂ </rdfs:comment>
    <ex:unit>t/yr</ex:unit>
  </rdf:Description>
  <rdf:Description rdf:about="http://transience.eu/ontologies/Energy_Service_Transportation_Freight_Railways">
    <rdf:type rdf:resource="http://www.w3.org/2002/07/owl#Class"/>
    <rdfs:subClassOf rdf:resource="http://transience.eu/ontologies/Variable"/>
    <rdfs:label>Energy Service|Transportation|Freight|Railways</rdfs:label>
    <rdfs:comment>energy service demand for freight transport on railways</rdfs:comment>
    <ex:unit>bn tkm/yr</ex:unit>
  </rdf:Description>
  <rdf:Description rdf:about="http://transience.eu/ontologies/OM_Cost_Fixed_Liquids_Biomass_w_o_CCS">
    <rdf:type rdf:resource="http://www.w3.org/2002/07/owl#Class"/>
    <rdfs:subClassOf rdf:resource="http://transience.eu/ontologies/Variable"/>
    <rdfs:label>OM Cost|Fixed|Liquids|Biomass|w/o CCS</rdfs:label>
    <rdfs:comment>Annual fixed operation &amp; maintainance cost of a new biomass to liquids plant w/o CCS. If more than one BTL technology is modelled, modellers should report fixed O&amp;M costs  for each represented BTL technology by adding variables OM Cost|Fixed|Liquids|Biomass|w/o CCS|2, ... OM Cost|Fixed|Liquids|Biomass|w/o CCS|N (with N = number of represented technologies) (matching the assignment of plant types to technologies in the reporting of capital costs as documented in the comments sheet).</rdfs:comment>
    <ex:unit>US$2010/kW/yr</ex:unit>
  </rdf:Description>
  <rdf:Description rdf:about="http://transience.eu/ontologies/Efficiency_Hydrogen_Gas_w_o_CCS">
    <rdf:type rdf:resource="http://www.w3.org/2002/07/owl#Class"/>
    <rdfs:subClassOf rdf:resource="http://transience.eu/ontologies/Variable"/>
    <rdfs:label>Efficiency|Hydrogen|Gas|w/o CCS</rdfs:label>
    <rdfs:comment>Conversion efficiency (energy content of hydrogen produced per unit of primary energy input) of a new gas to hydrogen plant w/o CCS. The efficiency should refer to the plant type(s) for which capital costs have been reported. If capital cost for more than one plant type has been reported, modellers should report efficiency for the additional plant types by adding variables Efficiency|Hydrogen|Gas|w/o CCS|2, ... Efficiency|Hydrogen|Gas|w/o CCS|N (matching the assignment of plant types to technologies in the reporting of capital costs as documented in the comments sheet). </rdfs:comment>
    <ex:unit>%</ex:unit>
  </rdf:Description>
  <rdf:Description rdf:about="http://transience.eu/ontologies/Stock_Buildings_building_types_age_cohort">
    <rdf:type rdf:resource="http://www.w3.org/2002/07/owl#Class"/>
    <rdfs:subClassOf rdf:resource="http://transience.eu/ontologies/ParameterInput"/>
    <rdfs:label>Stock|Buildings|[building types]|[age cohort]</rdfs:label>
    <rdfs:comment>Building stock developmentÂ </rdfs:comment>
    <ex:unit>m2</ex:unit>
  </rdf:Description>
  <rdf:Description rdf:about="http://transience.eu/ontologies/Primary_Energy_Biomass_Modern">
    <rdf:type rdf:resource="http://www.w3.org/2002/07/owl#Class"/>
    <rdfs:subClassOf rdf:resource="http://transience.eu/ontologies/Variable"/>
    <rdfs:label>Primary Energy|Biomass|Modern</rdfs:label>
    <rdfs:comment>modern biomass primary energy consumption, including purpose-grown bioenergy crops, crop and forestry residue bioenergy and municipal solid waste bioenergy</rdfs:comment>
    <ex:unit>EJ/yr</ex:unit>
  </rdf:Description>
  <rdf:Description rdf:about="http://transience.eu/ontologies/Conversion_Input_Hydrogen_Gases">
    <rdf:type rdf:resource="http://www.w3.org/2002/07/owl#Class"/>
    <rdfs:subClassOf rdf:resource="http://transience.eu/ontologies/Variable"/>
    <rdfs:label>Conversion Input|Hydrogen|Gases</rdfs:label>
    <rdfs:comment>secondary energy consumption of hydrogen for the production of gases (syngases)</rdfs:comment>
    <ex:unit>EJ/yr</ex:unit>
  </rdf:Description>
  <rdf:Description rdf:about="http://transience.eu/ontologies/Final_Energy_Industry_Non-Ferrous_Metals_Waste">
    <rdf:type rdf:resource="http://www.w3.org/2002/07/owl#Class"/>
    <rdfs:subClassOf rdf:resource="http://transience.eu/ontologies/Variable"/>
    <rdfs:label>Final Energy|Industry|Non-Ferrous Metals|Waste</rdfs:label>
    <rdfs:comment>Final energy consumption of non-renewable waste by the non-ferrous metals sector</rdfs:comment>
    <ex:unit>EJ/yr</ex:unit>
  </rdf:Description>
  <rdf:Description rdf:about="http://transience.eu/ontologies/Secondary_Energy_Hydrogen_Solar">
    <rdf:type rdf:resource="http://www.w3.org/2002/07/owl#Class"/>
    <rdfs:subClassOf rdf:resource="http://transience.eu/ontologies/Variable"/>
    <rdfs:label>Secondary Energy|Hydrogen|Solar</rdfs:label>
    <rdfs:comment>total hydrogen production from solar energy (e.g. thermalchemical water splitting with solar heat)</rdfs:comment>
    <ex:unit>EJ/yr</ex:unit>
  </rdf:Description>
  <rdf:Description rdf:about="http://transience.eu/ontologies/Secondary_Energy_Electricity_Solar_PV_Commercial">
    <rdf:type rdf:resource="http://www.w3.org/2002/07/owl#Class"/>
    <rdfs:subClassOf rdf:resource="http://transience.eu/ontologies/Variable"/>
    <rdfs:label>Secondary Energy|Electricity|Solar|PV|Commercial</rdfs:label>
    <rdfs:comment>net electricity production from commercial rooftop PV</rdfs:comment>
    <ex:unit>EJ/yr</ex:unit>
  </rdf:Description>
  <rdf:Description rdf:about="http://transience.eu/ontologies/Final_Energy_Industry_Pulp_and_Paper_Electricity">
    <rdf:type rdf:resource="http://www.w3.org/2002/07/owl#Class"/>
    <rdfs:subClassOf rdf:resource="http://transience.eu/ontologies/Variable"/>
    <rdfs:label>Final Energy|Industry|Pulp and Paper|Electricity</rdfs:label>
    <rdfs:comment>Final energy consumption of electricity of the pulp and paper sector</rdfs:comment>
    <ex:unit>EJ/yr</ex:unit>
  </rdf:Description>
  <rdf:Description rdf:about="http://transience.eu/ontologies/Final_Energy_Residential_and_Commercial_Liquids_Biomass">
    <rdf:type rdf:resource="http://www.w3.org/2002/07/owl#Class"/>
    <rdfs:subClassOf rdf:resource="http://transience.eu/ontologies/Variable"/>
    <rdfs:label>Final Energy|Residential and Commercial|Liquids|Biomass</rdfs:label>
    <rdfs:comment>final energy consumption by the residential &amp; commercial sector of liquid biofuels</rdfs:comment>
    <ex:unit>EJ/yr</ex:unit>
  </rdf:Description>
  <rdf:Description rdf:about="http://transience.eu/ontologies/OM_Cost_Fixed_Electricity_Wind">
    <rdf:type rdf:resource="http://www.w3.org/2002/07/owl#Class"/>
    <rdfs:subClassOf rdf:resource="http://transience.eu/ontologies/Variable"/>
    <rdfs:label>OM Cost|Fixed|Electricity|Wind</rdfs:label>
    <rdfs:comment>Annual fixed operation &amp; maintainance cost of a new wind power plants. This variable should only be filled, if wind power is not separated into onshore and offshore. If more than one wind power technology is modelled (e.g., wind power units with different hub height and capacity), modellers should report fixed O&amp;M costs  for each represented wind power technology by adding variables OM Cost|Fixed|Electricity|Wind|2, ... Capital|Cost|Electricity|Wind|N (with N = number of represented wind power technologies) (matching the assignment of plant types to technologies in the reporting of capital costs as documented in the comments sheet).</rdfs:comment>
    <ex:unit>US$2010/kW/yr</ex:unit>
  </rdf:Description>
  <rdf:Description rdf:about="http://transience.eu/ontologies/Final_Energy_Industry_Pulp_and_Paper_Solids_Coal">
    <rdf:type rdf:resource="http://www.w3.org/2002/07/owl#Class"/>
    <rdfs:subClassOf rdf:resource="http://transience.eu/ontologies/Variable"/>
    <rdfs:label>Final Energy|Industry|Pulp and Paper|Solids|Coal</rdfs:label>
    <rdfs:comment>Final energy consumption of coal by the pulp and paper sector</rdfs:comment>
    <ex:unit>EJ/yr</ex:unit>
  </rdf:Description>
  <rdf:Description rdf:about="http://transience.eu/ontologies/Investment_Infrastructure_Water_Irrigation">
    <rdf:type rdf:resource="http://www.w3.org/2002/07/owl#Class"/>
    <rdfs:subClassOf rdf:resource="http://transience.eu/ontologies/Variable"/>
    <rdfs:label>Investment|Infrastructure|Water|Irrigation</rdfs:label>
    <rdfs:comment>investment into water-related infrastructure (conveyance of water via canals, aqueducts, irrigation ditches, pumps, etc.)</rdfs:comment>
    <ex:unit>billion US$2010/yr</ex:unit>
  </rdf:Description>
  <rdf:Description rdf:about="http://transience.eu/ontologies/Investment_Infrastructure_Residential_and_Commercial_Low-Efficiency_Buildings">
    <rdf:type rdf:resource="http://www.w3.org/2002/07/owl#Class"/>
    <rdfs:subClassOf rdf:resource="http://transience.eu/ontologies/Variable"/>
    <rdfs:label>Investment|Infrastructure|Residential and Commercial|Low-Efficiency Buildings</rdfs:label>
    <rdfs:comment>investment into residential and commercial buildings infrastructure (all types of new buildings that are relatively low in their energy efficiency)</rdfs:comment>
    <ex:unit>billion US$2010/yr</ex:unit>
  </rdf:Description>
  <rdf:Description rdf:about="http://transience.eu/ontologies/Final_Energy_Industry_Chemicals_Gases">
    <rdf:type rdf:resource="http://www.w3.org/2002/07/owl#Class"/>
    <rdfs:subClassOf rdf:resource="http://transience.eu/ontologies/Variable"/>
    <rdfs:label>Final Energy|Industry|Chemicals|Gases</rdfs:label>
    <rdfs:comment>Final energy consumption of gases by the chemicals sector (natural gas, biogas, coal-gas), excluding transmission/distribution losses</rdfs:comment>
    <ex:unit>EJ/yr</ex:unit>
  </rdf:Description>
  <rdf:Description rdf:about="http://transience.eu/ontologies/Trade_Primary_Energy_Biomass_Value">
    <rdf:type rdf:resource="http://www.w3.org/2002/07/owl#Class"/>
    <rdfs:subClassOf rdf:resource="http://transience.eu/ontologies/Variable"/>
    <rdfs:label>Trade|Primary Energy|Biomass|Value</rdfs:label>
    <rdfs:comment>value of net exports of solid, unprocessed biomass, at the global level these should add up to the trade losses only</rdfs:comment>
    <ex:unit>billion US$2010/yr</ex:unit>
  </rdf:Description>
  <rdf:Description rdf:about="http://transience.eu/ontologies/Import_Industry_Non-Metallic_Minerals_Cement">
    <rdf:type rdf:resource="http://www.w3.org/2002/07/owl#Class"/>
    <rdfs:subClassOf rdf:resource="http://transience.eu/ontologies/Variable"/>
    <rdfs:label>Import|Industry|Non-Metallic Minerals|Cement</rdfs:label>
    <rdfs:comment>Import of cement measured in monetary units</rdfs:comment>
    <ex:unit>billion US$2010/yr</ex:unit>
  </rdf:Description>
  <rdf:Description rdf:about="http://transience.eu/ontologies/Price_Final_Energy_Residential_Liquids_Biomass">
    <rdf:type rdf:resource="http://www.w3.org/2002/07/owl#Class"/>
    <rdfs:subClassOf rdf:resource="http://transience.eu/ontologies/Variable"/>
    <rdfs:label>Price|Final Energy|Residential|Liquids|Biomass</rdfs:label>
    <rdfs:comment>biofuel price at the final level in the residential sector. Prices should include the effect of carbon prices.</rdfs:comment>
    <ex:unit>US$2010/GJ</ex:unit>
  </rdf:Description>
  <rdf:Description rdf:about="http://transience.eu/ontologies/Stock_Concrete_Other_demand_sectors_Product_categories">
    <rdf:type rdf:resource="http://www.w3.org/2002/07/owl#Class"/>
    <rdfs:subClassOf rdf:resource="http://transience.eu/ontologies/Variable"/>
    <rdfs:label>Stock|Concrete|Other|[demand sectors]|[Product categories]</rdfs:label>
    <rdfs:comment>Concrete stock in other sectorsÂ </rdfs:comment>
    <ex:unit>t/yr</ex:unit>
  </rdf:Description>
  <rdf:Description rdf:about="http://transience.eu/ontologies/OM_Cost_Fixed_Liquids_Coal_w__CCS">
    <rdf:type rdf:resource="http://www.w3.org/2002/07/owl#Class"/>
    <rdfs:subClassOf rdf:resource="http://transience.eu/ontologies/Variable"/>
    <rdfs:label>OM Cost|Fixed|Liquids|Coal|w/ CCS</rdfs:label>
    <rdfs:comment>Annual fixed operation &amp; maintainance cost of a new coal to liquids plant with CCS. If more than one CCS CTL technology is modelled, modellers should report fixed O&amp;M costs  for each represented CCS CTL technology by adding variables OM Cost|Fixed|Liquids|Coal|w/ CCS|2, ... OM Cost|Fixed|Liquids|Coal|w/ CCS|N (with N = number of represented technologies) (matching the assignment of plant types to technologies in the reporting of capital costs as documented in the comments sheet).</rdfs:comment>
    <ex:unit>US$2010/kW/yr</ex:unit>
  </rdf:Description>
  <rdf:Description rdf:about="http://transience.eu/ontologies/Final_Energy_Industry_Pulp_and_Paper_Liquids_Electricity">
    <rdf:type rdf:resource="http://www.w3.org/2002/07/owl#Class"/>
    <rdfs:subClassOf rdf:resource="http://transience.eu/ontologies/Variable"/>
    <rdfs:label>Final Energy|Industry|Pulp and Paper|Liquids|Electricity</rdfs:label>
    <rdfs:comment>Final energy consumption of synthetic liquid efuels ("power-to-liquid") by the pulp and paper sector</rdfs:comment>
    <ex:unit>EJ/yr</ex:unit>
  </rdf:Description>
  <rdf:Description rdf:about="http://transience.eu/ontologies/Investment_Energy_Supply_Hydrogen_Other">
    <rdf:type rdf:resource="http://www.w3.org/2002/07/owl#Class"/>
    <rdfs:subClassOf rdf:resource="http://transience.eu/ontologies/Variable"/>
    <rdfs:label>Investment|Energy Supply|Hydrogen|Other</rdfs:label>
    <rdfs:comment>investments for the production of hydrogen from the specified source. For plants equipped with CCS, the investment in the capturing equipment should be included but not the one on transport and storage.</rdfs:comment>
    <ex:unit>billion US$2010/yr</ex:unit>
  </rdf:Description>
  <rdf:Description rdf:about="http://transience.eu/ontologies/Expenditure_household_Energy">
    <rdf:type rdf:resource="http://www.w3.org/2002/07/owl#Class"/>
    <rdfs:subClassOf rdf:resource="http://transience.eu/ontologies/Variable"/>
    <rdfs:label>Expenditure|household|Energy</rdfs:label>
    <rdfs:comment>expenditure of households for energy.</rdfs:comment>
    <ex:unit>billion US$2010/yr</ex:unit>
  </rdf:Description>
  <rdf:Description rdf:about="http://transience.eu/ontologies/Carbon_Capture_Storage_Fossil_Energy_Supply_Electricity">
    <rdf:type rdf:resource="http://www.w3.org/2002/07/owl#Class"/>
    <rdfs:subClassOf rdf:resource="http://transience.eu/ontologies/Variable"/>
    <rdfs:label>Carbon Capture|Storage|Fossil|Energy|Supply|Electricity</rdfs:label>
    <rdfs:comment>total carbon dioxide emissions captured from fossil fuel use in electricity production (part of IPCC category 1A1a) and stored in geological deposits (e.g. in depleted oil and gas fields, unmined coal seams, saline aquifers) and the deep ocean, stored amounts should be reported as positive numbers</rdfs:comment>
    <ex:unit>Mt CO2/yr</ex:unit>
  </rdf:Description>
  <rdf:Description rdf:about="http://transience.eu/ontologies/Final_Energy_Transportation_Liquids">
    <rdf:type rdf:resource="http://www.w3.org/2002/07/owl#Class"/>
    <rdfs:subClassOf rdf:resource="http://transience.eu/ontologies/Variable"/>
    <rdfs:label>Final Energy|Transportation|Liquids</rdfs:label>
    <rdfs:comment>final energy consumption by the transportation sector of refined liquids (conventional &amp; unconventional oil, biofuels, coal-to-liquids, gas-to-liquids)</rdfs:comment>
    <ex:unit>EJ/yr</ex:unit>
  </rdf:Description>
  <rdf:Description rdf:about="http://transience.eu/ontologies/Import_Industry_Non-Metallic_Minerals_Volume">
    <rdf:type rdf:resource="http://www.w3.org/2002/07/owl#Class"/>
    <rdfs:subClassOf rdf:resource="http://transience.eu/ontologies/Variable"/>
    <rdfs:label>Import|Industry|Non-Metallic Minerals|Volume</rdfs:label>
    <rdfs:comment>Import of non-metallic minerals</rdfs:comment>
    <ex:unit>Mt/yr</ex:unit>
  </rdf:Description>
  <rdf:Description rdf:about="http://transience.eu/ontologies/Final_Energy_Non-Energy_Use_Chemicals">
    <rdf:type rdf:resource="http://www.w3.org/2002/07/owl#Class"/>
    <rdfs:subClassOf rdf:resource="http://transience.eu/ontologies/Variable"/>
    <rdfs:label>Final Energy|Non-Energy Use|Chemicals</rdfs:label>
    <rdfs:comment>Final energy consumption in the chemical sector by the non-combustion processes</rdfs:comment>
    <ex:unit>EJ/yr</ex:unit>
  </rdf:Description>
  <rdf:Description rdf:about="http://transience.eu/ontologies/Final_Energy_Industry_Chemicals_Gases_Biomass">
    <rdf:type rdf:resource="http://www.w3.org/2002/07/owl#Class"/>
    <rdfs:subClassOf rdf:resource="http://transience.eu/ontologies/Variable"/>
    <rdfs:label>Final Energy|Industry|Chemicals|Gases|Biomass</rdfs:label>
    <rdfs:comment>Final energy consumption of biogas by the chemicals sector</rdfs:comment>
    <ex:unit>EJ/yr</ex:unit>
  </rdf:Description>
  <rdf:Description rdf:about="http://transience.eu/ontologies/Efficiency_Liquids_Biomass_w__CCS">
    <rdf:type rdf:resource="http://www.w3.org/2002/07/owl#Class"/>
    <rdfs:subClassOf rdf:resource="http://transience.eu/ontologies/Variable"/>
    <rdfs:label>Efficiency|Liquids|Biomass|w/ CCS</rdfs:label>
    <rdfs:comment>Conversion efficiency (energy content of liquids produced per unit of primary energy input) of a new biomass to liquids plant with CCS. The efficiency should refer to the plant type(s) for which capital costs have been reported. If capital cost for more than one plant type has been reported, modellers should report efficiency for the additional plant types by adding variables Efficiency|Liquids|Biomass|w/ CCS|2, ... Efficiency|Liquids|Biomass|w/ CCS|N (matching the assignment of plant types to technologies in the reporting of capital costs as documented in the comments sheet). </rdfs:comment>
    <ex:unit>%</ex:unit>
  </rdf:Description>
  <rdf:Description rdf:about="http://transience.eu/ontologies/Import_Agriculture">
    <rdf:type rdf:resource="http://www.w3.org/2002/07/owl#Class"/>
    <rdfs:subClassOf rdf:resource="http://transience.eu/ontologies/Variable"/>
    <rdfs:label>Import|Agriculture</rdfs:label>
    <rdfs:comment>import of agricultural commodities measured in monetary units.</rdfs:comment>
    <ex:unit>billion US$2010/yr</ex:unit>
  </rdf:Description>
  <rdf:Description rdf:about="http://transience.eu/ontologies/Secondary_Energy_Gases_Other">
    <rdf:type rdf:resource="http://www.w3.org/2002/07/owl#Class"/>
    <rdfs:subClassOf rdf:resource="http://transience.eu/ontologies/Variable"/>
    <rdfs:label>Secondary Energy|Gases|Other</rdfs:label>
    <rdfs:comment>total production of gases from sources that do not fit any other category</rdfs:comment>
    <ex:unit>EJ/yr</ex:unit>
  </rdf:Description>
  <rdf:Description rdf:about="http://transience.eu/ontologies/Final_Energy_Industry_Iron_and_Steel_Gases_Fossil">
    <rdf:type rdf:resource="http://www.w3.org/2002/07/owl#Class"/>
    <rdfs:subClassOf rdf:resource="http://transience.eu/ontologies/Variable"/>
    <rdfs:label>Final Energy|Industry|Iron and Steel|Gases|Fossil</rdfs:label>
    <rdfs:comment>Final energy consumption of synthetic or derived gases of fossil origin by the iron and steel sector</rdfs:comment>
    <ex:unit>EJ/yr</ex:unit>
  </rdf:Description>
  <rdf:Description rdf:about="http://transience.eu/ontologies/Lifetime_Electricity_Biomass_w_o_CCS">
    <rdf:type rdf:resource="http://www.w3.org/2002/07/owl#Class"/>
    <rdfs:subClassOf rdf:resource="http://transience.eu/ontologies/Variable"/>
    <rdfs:label>Lifetime|Electricity|Biomass|w/o CCS</rdfs:label>
    <rdfs:comment>Lifetime of a new biomass power plant w/o CCS. Lifetime should be calculated by summing all vintages of a  capacity unit (e.g. (1+1+0.9+0.7+0.5) * 10 years = 41 years) or by the e-folding time for exponential capacity depreciation.  The lifetime should refer to the plant type(s) for which capital costs have been reported. If capital cost for more than one plant type has been reported, modellers should report lifetime for the additional plant types by adding variables Lifetime|Electricity|Biomass|w/o CCS|2, ... Lifetime|Electricity|Biomass|w/o CCS|N (matching the assignment of plant types to technologies in the reporting of capital costs as documented in the comments sheet). </rdfs:comment>
    <ex:unit>years</ex:unit>
  </rdf:Description>
  <rdf:Description rdf:about="http://transience.eu/ontologies/Final_Energy_Non-Energy_Use_Chemicals_Gases_Biomass">
    <rdf:type rdf:resource="http://www.w3.org/2002/07/owl#Class"/>
    <rdfs:subClassOf rdf:resource="http://transience.eu/ontologies/Variable"/>
    <rdfs:label>Final Energy|Non-Energy Use|Chemicals|Gases|Biomass</rdfs:label>
    <rdfs:comment>Final energy consumption of biogas by the chemical sector by the non-combustion processes</rdfs:comment>
    <ex:unit>EJ/yr</ex:unit>
  </rdf:Description>
  <rdf:Description rdf:about="http://transience.eu/ontologies/Emissions_CO2_Other_Removal">
    <rdf:type rdf:resource="http://www.w3.org/2002/07/owl#Class"/>
    <rdfs:subClassOf rdf:resource="http://transience.eu/ontologies/Variable"/>
    <rdfs:label>Emissions|CO2|Other Removal</rdfs:label>
    <rdfs:comment>CO2 emissions from carbon removal not reported in the other categories (i.e. without BECCS and land use), should be reported as negative values</rdfs:comment>
    <ex:unit>Mt CO2/yr</ex:unit>
  </rdf:Description>
  <rdf:Description rdf:about="http://transience.eu/ontologies/Final_Energy_Non-Energy_Use_Chemicals_Liquids_Electricity">
    <rdf:type rdf:resource="http://www.w3.org/2002/07/owl#Class"/>
    <rdfs:subClassOf rdf:resource="http://transience.eu/ontologies/Variable"/>
    <rdfs:label>Final Energy|Non-Energy Use|Chemicals|Liquids|Electricity</rdfs:label>
    <rdfs:comment>Final energy consumption of synthetic liquid efuels ("power-to-liquid") by the chemical sector by the non-combustion processes</rdfs:comment>
    <ex:unit>EJ/yr</ex:unit>
  </rdf:Description>
  <rdf:Description rdf:about="http://transience.eu/ontologies/Primary_Energy_Geothermal">
    <rdf:type rdf:resource="http://www.w3.org/2002/07/owl#Class"/>
    <rdfs:subClassOf rdf:resource="http://transience.eu/ontologies/Variable"/>
    <rdfs:label>Primary Energy|Geothermal</rdfs:label>
    <rdfs:comment>total geothermal primary energy consumption</rdfs:comment>
    <ex:unit>EJ/yr</ex:unit>
  </rdf:Description>
  <rdf:Description rdf:about="http://transience.eu/ontologies/Secondary_Energy_Heat">
    <rdf:type rdf:resource="http://www.w3.org/2002/07/owl#Class"/>
    <rdfs:subClassOf rdf:resource="http://transience.eu/ontologies/Variable"/>
    <rdfs:label>Secondary Energy|Heat</rdfs:label>
    <rdfs:comment>total centralized heat generation</rdfs:comment>
    <ex:unit>EJ/yr</ex:unit>
  </rdf:Description>
  <rdf:Description rdf:about="http://transience.eu/ontologies/Capacity_Electricity_Hydro">
    <rdf:type rdf:resource="http://www.w3.org/2002/07/owl#Class"/>
    <rdfs:subClassOf rdf:resource="http://transience.eu/ontologies/Variable"/>
    <rdfs:label>Capacity|Electricity|Hydro</rdfs:label>
    <rdfs:comment>Total installed (available) capacity of hydropower plants. The installed (available) capacity of hydropower plants by plant type for which capital costs are reported should be reported by adding variables Capacity|Electricity|Hydro|1, ..., Capacity|Electricity|Hydro|N (matching the assignment of plant types to technologies in the reporting of capital costs as documented in the comments sheet). </rdfs:comment>
    <ex:unit>GW</ex:unit>
  </rdf:Description>
  <rdf:Description rdf:about="http://transience.eu/ontologies/Capacity_Electricity">
    <rdf:type rdf:resource="http://www.w3.org/2002/07/owl#Class"/>
    <rdfs:subClassOf rdf:resource="http://transience.eu/ontologies/Variable"/>
    <rdfs:label>Capacity|Electricity</rdfs:label>
    <rdfs:comment>Total installed (available) capacity of all operating power plants</rdfs:comment>
    <ex:unit>GW</ex:unit>
  </rdf:Description>
  <rdf:Description rdf:about="http://transience.eu/ontologies/Investment_Energy_Supply_Electricity_Biomass_w__CCS">
    <rdf:type rdf:resource="http://www.w3.org/2002/07/owl#Class"/>
    <rdfs:subClassOf rdf:resource="http://transience.eu/ontologies/Variable"/>
    <rdfs:label>Investment|Energy Supply|Electricity|Biomass|w/ CCS</rdfs:label>
    <rdfs:comment>investments in new power generation for the specified power plant category. If the model features several sub-categories, the total investments should be reported. For plants equipped with CCS, the investment in the capturing equipment should be included but not the one on transport and storage.</rdfs:comment>
    <ex:unit>billion US$2010/yr</ex:unit>
  </rdf:Description>
  <rdf:Description rdf:about="http://transience.eu/ontologies/Expenditure_household_Services">
    <rdf:type rdf:resource="http://www.w3.org/2002/07/owl#Class"/>
    <rdfs:subClassOf rdf:resource="http://transience.eu/ontologies/Variable"/>
    <rdfs:label>Expenditure|household|Services</rdfs:label>
    <rdfs:comment>expenditure of households for services.</rdfs:comment>
    <ex:unit>billion US$2010/yr</ex:unit>
  </rdf:Description>
  <rdf:Description rdf:about="http://transience.eu/ontologies/Export_Other">
    <rdf:type rdf:resource="http://www.w3.org/2002/07/owl#Class"/>
    <rdfs:subClassOf rdf:resource="http://transience.eu/ontologies/Variable"/>
    <rdfs:label>Export|Other</rdfs:label>
    <rdfs:comment>export of other commodities measured in monetary units (please provide a definition of the sources in this category in the 'comments' tab).</rdfs:comment>
    <ex:unit>billion US$2010/yr</ex:unit>
  </rdf:Description>
  <rdf:Description rdf:about="http://transience.eu/ontologies/Emissions_CO2_Energy_Demand_Other_Sector">
    <rdf:type rdf:resource="http://www.w3.org/2002/07/owl#Class"/>
    <rdfs:subClassOf rdf:resource="http://transience.eu/ontologies/Variable"/>
    <rdfs:label>Emissions|CO2|Energy|Demand|Other Sector</rdfs:label>
    <rdfs:comment>CO2 emissions from fuel combustion in other energy supply sectors (please provide a definition of other sources in this category in the 'comments' tab)</rdfs:comment>
    <ex:unit>Mt CO2/yr</ex:unit>
  </rdf:Description>
  <rdf:Description rdf:about="http://transience.eu/ontologies/Capacity_Steel_DRI">
    <rdf:type rdf:resource="http://www.w3.org/2002/07/owl#Class"/>
    <rdfs:subClassOf rdf:resource="http://transience.eu/ontologies/Variable"/>
    <rdfs:label>Capacity|Steel|DRI</rdfs:label>
    <rdfs:comment>Capacity of shaft furnaces for DRI production in Mt DRI / year</rdfs:comment>
    <ex:unit>Mt/yr</ex:unit>
  </rdf:Description>
  <rdf:Description rdf:about="http://transience.eu/ontologies/Energy_Service_Transportation_Passenger_Walking">
    <rdf:type rdf:resource="http://www.w3.org/2002/07/owl#Class"/>
    <rdfs:subClassOf rdf:resource="http://transience.eu/ontologies/Variable"/>
    <rdfs:label>Energy Service|Transportation|Passenger|Walking</rdfs:label>
    <rdfs:comment>energy service demand for passenger transport by foot</rdfs:comment>
    <ex:unit>bn pkm/yr</ex:unit>
  </rdf:Description>
  <rdf:Description rdf:about="http://transience.eu/ontologies/Final_Energy_Industry_Iron_and_Steel_Liquids_Electricity">
    <rdf:type rdf:resource="http://www.w3.org/2002/07/owl#Class"/>
    <rdfs:subClassOf rdf:resource="http://transience.eu/ontologies/Variable"/>
    <rdfs:label>Final Energy|Industry|Iron and Steel|Liquids|Electricity</rdfs:label>
    <rdfs:comment>Final energy consumption of synthetic liquid efuels ("power-to-liquid") by the iron and steel sector</rdfs:comment>
    <ex:unit>EJ/yr</ex:unit>
  </rdf:Description>
  <rdf:Description rdf:about="http://transience.eu/ontologies/Carbon_Capture_Storage_Fossil">
    <rdf:type rdf:resource="http://www.w3.org/2002/07/owl#Class"/>
    <rdfs:subClassOf rdf:resource="http://transience.eu/ontologies/Variable"/>
    <rdfs:label>Carbon Capture|Storage|Fossil</rdfs:label>
    <rdfs:comment>total carbon dioxide emissions captured from fossil fuel use and stored in geological deposits (e.g. in depleted oil and gas fields, unmined coal seams, saline aquifers) and the deep ocean, stored amounts should be reported as positive numbers</rdfs:comment>
    <ex:unit>Mt CO2/yr</ex:unit>
  </rdf:Description>
  <rdf:Description rdf:about="http://transience.eu/ontologies/Secondary_Energy_Electricity_Coal_w_o_CCS">
    <rdf:type rdf:resource="http://www.w3.org/2002/07/owl#Class"/>
    <rdfs:subClassOf rdf:resource="http://transience.eu/ontologies/Variable"/>
    <rdfs:label>Secondary Energy|Electricity|Coal|w/o CCS</rdfs:label>
    <rdfs:comment>net electricity production from coal with freely vented CO2 emissions</rdfs:comment>
    <ex:unit>EJ/yr</ex:unit>
  </rdf:Description>
  <rdf:Description rdf:about="http://transience.eu/ontologies/Primary_Energy_Industry_Steel_Electricity_(external)">
    <rdf:type rdf:resource="http://www.w3.org/2002/07/owl#Class"/>
    <rdfs:subClassOf rdf:resource="http://transience.eu/ontologies/Variable"/>
    <rdfs:label>Primary Energy|Industry|Steel|Electricity (external)</rdfs:label>
    <rdfs:comment>Energy demand including own coke ovens and autoproduction of electricity</rdfs:comment>
    <ex:unit>PJ/yr</ex:unit>
  </rdf:Description>
  <rdf:Description rdf:about="http://transience.eu/ontologies/Emissions_CO2_AFOLU_Land_Negative">
    <rdf:type rdf:resource="http://www.w3.org/2002/07/owl#Class"/>
    <rdfs:subClassOf rdf:resource="http://transience.eu/ontologies/Variable"/>
    <rdfs:label>Emissions|CO2|AFOLU|Land|Negative</rdfs:label>
    <rdfs:comment>negative CO2 emissions from Land Use, Land-Use Change and Forestry (LULUCF), e.g. from afforestation</rdfs:comment>
    <ex:unit>Mt CO2/yr</ex:unit>
  </rdf:Description>
  <rdf:Description rdf:about="http://transience.eu/ontologies/Emissions_CO2_Energy">
    <rdf:type rdf:resource="http://www.w3.org/2002/07/owl#Class"/>
    <rdfs:subClassOf rdf:resource="http://transience.eu/ontologies/Variable"/>
    <rdfs:label>Emissions|CO2|Energy</rdfs:label>
    <rdfs:comment>Fossil CO2 emissions from energy use on supply and demand side (IPCC category 1A, 1B), net of negative emissions from Bioenergy with CCS (BECCS), including emissions from international bunkers</rdfs:comment>
    <ex:unit>Mt CO2/yr</ex:unit>
  </rdf:Description>
  <rdf:Description rdf:about="http://transience.eu/ontologies/Final_Energy_Residential_Other">
    <rdf:type rdf:resource="http://www.w3.org/2002/07/owl#Class"/>
    <rdfs:subClassOf rdf:resource="http://transience.eu/ontologies/Variable"/>
    <rdfs:label>Final Energy|Residential|Other</rdfs:label>
    <rdfs:comment>final energy consumption by the residential sector of other sources that do not fit to any other category (please provide a definition of the sources in this category in the 'comments' tab)</rdfs:comment>
    <ex:unit>EJ/yr</ex:unit>
  </rdf:Description>
  <rdf:Description rdf:about="http://transience.eu/ontologies/Secondary_Energy_Gases_Biomass">
    <rdf:type rdf:resource="http://www.w3.org/2002/07/owl#Class"/>
    <rdfs:subClassOf rdf:resource="http://transience.eu/ontologies/Variable"/>
    <rdfs:label>Secondary Energy|Gases|Biomass</rdfs:label>
    <rdfs:comment>total production of biogas</rdfs:comment>
    <ex:unit>EJ/yr</ex:unit>
  </rdf:Description>
  <rdf:Description rdf:about="http://transience.eu/ontologies/Final_Energy_Commercial_Heat">
    <rdf:type rdf:resource="http://www.w3.org/2002/07/owl#Class"/>
    <rdfs:subClassOf rdf:resource="http://transience.eu/ontologies/Variable"/>
    <rdfs:label>Final Energy|Commercial|Heat</rdfs:label>
    <rdfs:comment>final energy consumption by the commercial sector of heat (e.g., district heat, process heat, solar heating and warm water), excluding transmission/distribution losses</rdfs:comment>
    <ex:unit>EJ/yr</ex:unit>
  </rdf:Description>
  <rdf:Description rdf:about="http://transience.eu/ontologies/Final_Energy_Industry_Pulp_and_Paper_Other">
    <rdf:type rdf:resource="http://www.w3.org/2002/07/owl#Class"/>
    <rdfs:subClassOf rdf:resource="http://transience.eu/ontologies/Variable"/>
    <rdfs:label>Final Energy|Industry|Pulp and Paper|Other</rdfs:label>
    <rdfs:comment>Final energy consumption of other energy carriers by the pulp and paper sector (please provide a definition of the energy carriers in this category in the 'comments' tab)</rdfs:comment>
    <ex:unit>EJ/yr</ex:unit>
  </rdf:Description>
  <rdf:Description rdf:about="http://transience.eu/ontologies/Lifetime_Electricity_Coal_w__CCS">
    <rdf:type rdf:resource="http://www.w3.org/2002/07/owl#Class"/>
    <rdfs:subClassOf rdf:resource="http://transience.eu/ontologies/Variable"/>
    <rdfs:label>Lifetime|Electricity|Coal|w/ CCS</rdfs:label>
    <rdfs:comment>Lifetime of a new coal power plant with CCS. Lifetime should be calculated by summing all vintages of a  capacity unit (e.g. (1+1+0.9+0.7+0.5) * 10 years = 41 years) or by the e-folding time for exponential capacity depreciation.  The lifetime should refer to the plant type(s) for which capital costs have been reported. If capital cost for more than one plant type has been reported, modellers should report lifetime for the additional plant types by adding variables Lifetime|Electricity|Coal|w/ CCS|2, ... Lifetime|Electricity|Coal|w/ CCS|N (matching the assignment of plant types to technologies in the reporting of capital costs as documented in the comments sheet). </rdfs:comment>
    <ex:unit>years</ex:unit>
  </rdf:Description>
  <rdf:Description rdf:about="http://transience.eu/ontologies/Carbon_Capture_Storage_Fossil_Energy_Supply_Liquids">
    <rdf:type rdf:resource="http://www.w3.org/2002/07/owl#Class"/>
    <rdfs:subClassOf rdf:resource="http://transience.eu/ontologies/Variable"/>
    <rdfs:label>Carbon Capture|Storage|Fossil|Energy|Supply|Liquids</rdfs:label>
    <rdfs:comment>total carbon dioxide emissions captured from fossil fuel use in liquid fuel production (part of IPCC category 1A) and stored in geological deposits (e.g. in depleted oil and gas fields, unmined coal seams, saline aquifers) and the deep ocean, stored amounts should be reported as positive numbers</rdfs:comment>
    <ex:unit>Mt CO2/yr</ex:unit>
  </rdf:Description>
  <rdf:Description rdf:about="http://transience.eu/ontologies/OM_Cost_Fixed_Electricity_Solar_PV">
    <rdf:type rdf:resource="http://www.w3.org/2002/07/owl#Class"/>
    <rdfs:subClassOf rdf:resource="http://transience.eu/ontologies/Variable"/>
    <rdfs:label>OM Cost|Fixed|Electricity|Solar|PV</rdfs:label>
    <rdfs:comment>Annual fixed operation &amp; maintainance cost of a new solar PV units. If more than one PV technology is modelled (e.g., centralized PV plant, distributed (rooftop) PV, crystalline SI PV, thin-film PV), modellers should report fixed O&amp;M costs  for each represented PV technology by adding variables OM Cost|Fixed|Electricity|Solar|PV|2, ... Capital|Cost|Electricity|Solar|PV|N (with N = number of represented PV technologies) (matching the assignment of plant types to technologies in the reporting of capital costs as documented in the comments sheet).</rdfs:comment>
    <ex:unit>US$2010/kW/yr</ex:unit>
  </rdf:Description>
  <rdf:Description rdf:about="http://transience.eu/ontologies/Carbon_Capture_Fossil_Energy_Demand_Industry">
    <rdf:type rdf:resource="http://www.w3.org/2002/07/owl#Class"/>
    <rdfs:subClassOf rdf:resource="http://transience.eu/ontologies/Variable"/>
    <rdfs:label>Carbon Capture|Fossil|Energy|Demand|Industry</rdfs:label>
    <rdfs:comment>total carbon dioxide emissions captured from fossil fuel use in industry (IPCC category 1A2), should be reported as positive numbers</rdfs:comment>
    <ex:unit>Mt CO2/yr</ex:unit>
  </rdf:Description>
  <rdf:Description rdf:about="http://transience.eu/ontologies/Secondary_Energy_Electricity_Geothermal">
    <rdf:type rdf:resource="http://www.w3.org/2002/07/owl#Class"/>
    <rdfs:subClassOf rdf:resource="http://transience.eu/ontologies/Variable"/>
    <rdfs:label>Secondary Energy|Electricity|Geothermal</rdfs:label>
    <rdfs:comment>net electricity production from all sources of geothermal energy (e.g., hydrothermal, enhanced geothermal systems)</rdfs:comment>
    <ex:unit>EJ/yr</ex:unit>
  </rdf:Description>
  <rdf:Description rdf:about="http://transience.eu/ontologies/Secondary_Energy_Electricity_Gas">
    <rdf:type rdf:resource="http://www.w3.org/2002/07/owl#Class"/>
    <rdfs:subClassOf rdf:resource="http://transience.eu/ontologies/Variable"/>
    <rdfs:label>Secondary Energy|Electricity|Gas</rdfs:label>
    <rdfs:comment>net electricity production from natural gas</rdfs:comment>
    <ex:unit>EJ/yr</ex:unit>
  </rdf:Description>
  <rdf:Description rdf:about="http://transience.eu/ontologies/Stock_materials_Buildings_buildings_types">
    <rdf:type rdf:resource="http://www.w3.org/2002/07/owl#Class"/>
    <rdfs:subClassOf rdf:resource="http://transience.eu/ontologies/Variable"/>
    <rdfs:label>Stock|[materials]|Buildings|[buildings types]</rdfs:label>
    <rdfs:comment>Material stock in buildingsÂ </rdfs:comment>
    <ex:unit>kg/yr</ex:unit>
  </rdf:Description>
  <rdf:Description rdf:about="http://transience.eu/ontologies/Capital_Cost_Hydrogen_Biomass_w_o_CCS">
    <rdf:type rdf:resource="http://www.w3.org/2002/07/owl#Class"/>
    <rdfs:subClassOf rdf:resource="http://transience.eu/ontologies/Variable"/>
    <rdfs:label>Capital Cost|Hydrogen|Biomass|w/o CCS</rdfs:label>
    <rdfs:comment>Capital cost of a new biomass to hydrogen plant w/o CCS. If more than one biomass to hydrogen technology is modelled, modellers should report capital costs for each represented biomass to hydrogen technology by adding variables Capital Cost|Hydrogen|Biomass|w/o CCS|2, ... Capital Cost|Hydrogen|Biomass|w/o CCS|N (with N = number of represented technologies). It is modeller's choice which biomass to hydrogen technologies to assign to type 1 (assigned to the variable without number suffix),2,...,N. The assignment should be documented in the comments sheet. </rdfs:comment>
    <ex:unit>US$2010/kW</ex:unit>
  </rdf:Description>
  <rdf:Description rdf:about="http://transience.eu/ontologies/Capacity_Electricity_Solar_CSP">
    <rdf:type rdf:resource="http://www.w3.org/2002/07/owl#Class"/>
    <rdfs:subClassOf rdf:resource="http://transience.eu/ontologies/Variable"/>
    <rdfs:label>Capacity|Electricity|Solar|CSP</rdfs:label>
    <rdfs:comment>Total installed (available) capacity of concentrating solar power (CSP). The installed (available) capacity of CSP by technology type for which capital costs are reported should be reported by adding variables Capacity|Electricity|Solar|CSP|1, ..., Capacity|Electricity|Solar|CSP|N (matching the assignment of plant types to technologies in the reporting of capital costs as documented in the comments sheet). </rdfs:comment>
    <ex:unit>GW</ex:unit>
  </rdf:Description>
  <rdf:Description rdf:about="http://transience.eu/ontologies/Export_Industry_Iron_and_Steel">
    <rdf:type rdf:resource="http://www.w3.org/2002/07/owl#Class"/>
    <rdfs:subClassOf rdf:resource="http://transience.eu/ontologies/Variable"/>
    <rdfs:label>Export|Industry|Iron and Steel</rdfs:label>
    <rdfs:comment>Export of iron &amp; steel measured in monetary units</rdfs:comment>
    <ex:unit>billion US$2010/yr</ex:unit>
  </rdf:Description>
  <rdf:Description rdf:about="http://transience.eu/ontologies/Efficiency_Gases_Biomass_w_o_CCS">
    <rdf:type rdf:resource="http://www.w3.org/2002/07/owl#Class"/>
    <rdfs:subClassOf rdf:resource="http://transience.eu/ontologies/Variable"/>
    <rdfs:label>Efficiency|Gases|Biomass|w/o CCS</rdfs:label>
    <rdfs:comment>Conversion efficiency (energy content of gases produced per unit of primary energy input) of a new coal to gas plant w/o CCS. The efficiency should refer to the plant type(s) for which capital costs have been reported. If capital cost for more than one plant type has been reported, modellers should report efficiency for the additional plant types by adding variables Efficiency|Gases|Coal|w/o CCS|2, ... Efficiency|Gases|Coal|w/o CCS|N (matching the assignment of plant types to technologies in the reporting of capital costs as documented in the comments sheet). </rdfs:comment>
    <ex:unit>%</ex:unit>
  </rdf:Description>
  <rdf:Description rdf:about="http://transience.eu/ontologies/Secondary_Energy_Liquids_Gas">
    <rdf:type rdf:resource="http://www.w3.org/2002/07/owl#Class"/>
    <rdfs:subClassOf rdf:resource="http://transience.eu/ontologies/Variable"/>
    <rdfs:label>Secondary Energy|Liquids|Gas</rdfs:label>
    <rdfs:comment>total production of fossil liquid synfuels from gas-to-liquids (GTL) technologies</rdfs:comment>
    <ex:unit>EJ/yr</ex:unit>
  </rdf:Description>
  <rdf:Description rdf:about="http://transience.eu/ontologies/ParameterInput">
    <rdf:type rdf:resource="http://www.w3.org/2002/07/owl#Class"/>
    <rdfs:subClassOf rdf:resource="http://transience.eu/ontologies/Parameter"/>
    <rdfs:comment>Parameter Input</rdfs:comment>
  </rdf:Description>
  <rdf:Description rdf:about="http://transience.eu/ontologies/Carbon_Capture_Biomass_Energy_Supply_Other">
    <rdf:type rdf:resource="http://www.w3.org/2002/07/owl#Class"/>
    <rdfs:subClassOf rdf:resource="http://transience.eu/ontologies/Variable"/>
    <rdfs:label>Carbon Capture|Biomass|Energy|Supply|Other</rdfs:label>
    <rdfs:comment>total carbon dioxide emissions captured from bioenergy use in other energy supply (part of IPCC category 1A), should be reported as positive numbers</rdfs:comment>
    <ex:unit>Mt CO2/yr</ex:unit>
  </rdf:Description>
  <rdf:Description rdf:about="http://transience.eu/ontologies/Investment_RnD_Energy_Supply">
    <rdf:type rdf:resource="http://www.w3.org/2002/07/owl#Class"/>
    <rdfs:subClassOf rdf:resource="http://transience.eu/ontologies/Variable"/>
    <rdfs:label>Investment|RnD|Energy Supply</rdfs:label>
    <rdfs:comment>Investments into research and development, energy supply sector</rdfs:comment>
    <ex:unit>billion US$2010/yr</ex:unit>
  </rdf:Description>
  <rdf:Description rdf:about="http://transience.eu/ontologies/Capital_Cost_Liquids_Oil">
    <rdf:type rdf:resource="http://www.w3.org/2002/07/owl#Class"/>
    <rdfs:subClassOf rdf:resource="http://transience.eu/ontologies/Variable"/>
    <rdfs:label>Capital Cost|Liquids|Oil</rdfs:label>
    <rdfs:comment>Capital cost of a new oil refining plant. If more than one refinery technology is modelled, modellers should report capital costs for each represented refinery technology by adding variables Capital Cost|Liquids|Oil|2, ... Capital Cost|Liquids|Oil|N (with N = number of represented technologies). It is modeller's choice which refinery technologies to assign to type 1 (assigned to the variable without number suffix),2,...,N. The assignment should be documented in the comments sheet. </rdfs:comment>
    <ex:unit>US$2010/kW</ex:unit>
  </rdf:Description>
  <rdf:Description rdf:about="http://transience.eu/ontologies/Production_Non-Ferrous_Metals_Aluminium_Primary_Volume">
    <rdf:type rdf:resource="http://www.w3.org/2002/07/owl#Class"/>
    <rdfs:subClassOf rdf:resource="http://transience.eu/ontologies/Variable"/>
    <rdfs:label>Production|Non-Ferrous Metals|Aluminium|Primary|Volume</rdfs:label>
    <rdfs:comment>production of primary aluminum </rdfs:comment>
    <ex:unit>Mt/yr</ex:unit>
  </rdf:Description>
  <rdf:Description rdf:about="http://transience.eu/ontologies/Energy_Service_Bunkers_Passenger_International_Shipping">
    <rdf:type rdf:resource="http://www.w3.org/2002/07/owl#Class"/>
    <rdfs:subClassOf rdf:resource="http://transience.eu/ontologies/Variable"/>
    <rdfs:label>Energy Service|Bunkers|Passenger|International Shipping</rdfs:label>
    <rdfs:comment>energy service demand for passenger transport operating on international shipping routes</rdfs:comment>
    <ex:unit>bn pkm/yr</ex:unit>
  </rdf:Description>
  <rdf:Description rdf:about="http://transience.eu/ontologies/Energy_Service_Transportation_Freight">
    <rdf:type rdf:resource="http://www.w3.org/2002/07/owl#Class"/>
    <rdfs:subClassOf rdf:resource="http://transience.eu/ontologies/Variable"/>
    <rdfs:label>Energy Service|Transportation|Freight</rdfs:label>
    <rdfs:comment>energy service demand for freight transport</rdfs:comment>
    <ex:unit>bn tkm/yr</ex:unit>
  </rdf:Description>
  <rdf:Description rdf:about="http://transience.eu/ontologies/Secondary_Energy_Heat_Coal">
    <rdf:type rdf:resource="http://www.w3.org/2002/07/owl#Class"/>
    <rdfs:subClassOf rdf:resource="http://transience.eu/ontologies/Variable"/>
    <rdfs:label>Secondary Energy|Heat|Coal</rdfs:label>
    <rdfs:comment>centralized heat generation from coal</rdfs:comment>
    <ex:unit>EJ/yr</ex:unit>
  </rdf:Description>
  <rdf:Description rdf:about="http://transience.eu/ontologies/Final_Energy_Residential_and_Commercial_Gases_Fossil">
    <rdf:type rdf:resource="http://www.w3.org/2002/07/owl#Class"/>
    <rdfs:subClassOf rdf:resource="http://transience.eu/ontologies/Variable"/>
    <rdfs:label>Final Energy|Residential and Commercial|Gases|Fossil</rdfs:label>
    <rdfs:comment>final energy consumption by the residential &amp; commercial sector of  synthetic or derived gases of fossil origin, excluding transmission/distribution losses</rdfs:comment>
    <ex:unit>EJ/yr</ex:unit>
  </rdf:Description>
  <rdf:Description rdf:about="http://transience.eu/ontologies/Final_Energy_Industry_Chemicals_Other">
    <rdf:type rdf:resource="http://www.w3.org/2002/07/owl#Class"/>
    <rdfs:subClassOf rdf:resource="http://transience.eu/ontologies/Variable"/>
    <rdfs:label>Final Energy|Industry|Chemicals|Other</rdfs:label>
    <rdfs:comment>Final energy consumption of other energy carriers by the chemicals sector (please provide a definition of the energy carriers in this category in the 'comments' tab)</rdfs:comment>
    <ex:unit>EJ/yr</ex:unit>
  </rdf:Description>
  <rdf:Description rdf:about="http://transience.eu/ontologies/Primary_Energy_Gas">
    <rdf:type rdf:resource="http://www.w3.org/2002/07/owl#Class"/>
    <rdfs:subClassOf rdf:resource="http://transience.eu/ontologies/Variable"/>
    <rdfs:label>Primary Energy|Gas</rdfs:label>
    <rdfs:comment>gas primary energy consumption</rdfs:comment>
    <ex:unit>EJ/yr</ex:unit>
  </rdf:Description>
  <rdf:Description rdf:about="http://transience.eu/ontologies/Final_Energy_Industry_Iron_and_Steel_Electricity">
    <rdf:type rdf:resource="http://www.w3.org/2002/07/owl#Class"/>
    <rdfs:subClassOf rdf:resource="http://transience.eu/ontologies/Variable"/>
    <rdfs:label>Final Energy|Industry|Iron and Steel|Electricity</rdfs:label>
    <rdfs:comment>Final energy consumption of electricity by the iron and steel sector</rdfs:comment>
    <ex:unit>EJ/yr</ex:unit>
  </rdf:Description>
  <rdf:Description rdf:about="http://transience.eu/ontologies/Price_Primary_Energy_Oil">
    <rdf:type rdf:resource="http://www.w3.org/2002/07/owl#Class"/>
    <rdfs:subClassOf rdf:resource="http://transience.eu/ontologies/Variable"/>
    <rdfs:label>Price|Primary Energy|Oil</rdfs:label>
    <rdfs:comment>crude oil price at the primary level (i.e. the spot price at the global or regional market)</rdfs:comment>
    <ex:unit>US$2010/GJ</ex:unit>
  </rdf:Description>
  <rdf:Description rdf:about="http://transience.eu/ontologies/Secondary_Energy_Electricity_Solar_PV_Residential">
    <rdf:type rdf:resource="http://www.w3.org/2002/07/owl#Class"/>
    <rdfs:subClassOf rdf:resource="http://transience.eu/ontologies/Variable"/>
    <rdfs:label>Secondary Energy|Electricity|Solar|PV|Residential</rdfs:label>
    <rdfs:comment>net electricity production from residential rooftop PV</rdfs:comment>
    <ex:unit>EJ/yr</ex:unit>
  </rdf:Description>
  <rdf:Description rdf:about="http://transience.eu/ontologies/Efficiency_Gases_Coal_w_o_CCS">
    <rdf:type rdf:resource="http://www.w3.org/2002/07/owl#Class"/>
    <rdfs:subClassOf rdf:resource="http://transience.eu/ontologies/Variable"/>
    <rdfs:label>Efficiency|Gases|Coal|w/o CCS</rdfs:label>
    <rdfs:comment>Conversion efficiency (energy content of gases produced per unit of primary energy input) of a new coal to gas plant w/o CCS. The efficiency should refer to the plant type(s) for which capital costs have been reported. If capital cost for more than one plant type has been reported, modellers should report efficiency for the additional plant types by adding variables Efficiency|Gases|Coal|w/o CCS|2, ... Efficiency|Gases|Coal|w/o CCS|N (matching the assignment of plant types to technologies in the reporting of capital costs as documented in the comments sheet). </rdfs:comment>
    <ex:unit>%</ex:unit>
  </rdf:Description>
  <rdf:Description rdf:about="http://transience.eu/ontologies/Materials_Demand_Non-Ferrous_Metals_Power_Sector">
    <rdf:type rdf:resource="http://www.w3.org/2002/07/owl#Class"/>
    <rdfs:subClassOf rdf:resource="http://transience.eu/ontologies/Variable"/>
    <rdfs:label>Materials Demand|Non-Ferrous Metals|Power Sector</rdfs:label>
    <rdfs:comment>Non-ferrous metals requirments from a certain end-use sector</rdfs:comment>
    <ex:unit>Mt/yr</ex:unit>
  </rdf:Description>
  <rdf:Description rdf:about="http://transience.eu/ontologies/Resource_use_Methanol_Industry_Petrochemicals">
    <rdf:type rdf:resource="http://www.w3.org/2002/07/owl#Class"/>
    <rdfs:subClassOf rdf:resource="http://transience.eu/ontologies/Variable"/>
    <rdfs:label>Resource use|Methanol|Industry|Petrochemicals</rdfs:label>
    <rdfs:comment>Use of methanol for non-energetic use including energetic use of by-products; C-content (only methanol supplied from outside, not including methanol produced within petrochemical system as intermediary product)</rdfs:comment>
    <ex:unit>Mt C_eq/yr</ex:unit>
  </rdf:Description>
  <rdf:Description rdf:about="http://transience.eu/ontologies/Emissions_CO2_Energy_Demand_Transportation_Gases">
    <rdf:type rdf:resource="http://www.w3.org/2002/07/owl#Class"/>
    <rdfs:subClassOf rdf:resource="http://transience.eu/ontologies/Variable"/>
    <rdfs:label>Emissions|CO2|Energy|Demand|Transportation|Gases</rdfs:label>
    <rdfs:comment>Fossil CO2 emissions from Gases use in the transportation sector (IPCC category 1A3)</rdfs:comment>
    <ex:unit>Mt CO2/yr</ex:unit>
  </rdf:Description>
  <rdf:Description rdf:about="http://transience.eu/ontologies/Stock_change_Steel_Other_demand_sectors_Product_categories">
    <rdf:type rdf:resource="http://www.w3.org/2002/07/owl#Class"/>
    <rdfs:subClassOf rdf:resource="http://transience.eu/ontologies/Variable"/>
    <rdfs:label>Stock change|Steel|Other|[demand sectors]|[Product categories]</rdfs:label>
    <rdfs:comment>Steel stock change in other sectorsÂ </rdfs:comment>
    <ex:unit>t/yr</ex:unit>
  </rdf:Description>
  <rdf:Description rdf:about="http://transience.eu/ontologies/Conversion_Input_Liquids_Electricity">
    <rdf:type rdf:resource="http://www.w3.org/2002/07/owl#Class"/>
    <rdfs:subClassOf rdf:resource="http://transience.eu/ontologies/Variable"/>
    <rdfs:label>Conversion Input|Liquids|Electricity</rdfs:label>
    <rdfs:comment>secondary energy consumption of efuels for the production of electricity</rdfs:comment>
    <ex:unit>EJ/yr</ex:unit>
  </rdf:Description>
  <rdf:Description rdf:about="http://transience.eu/ontologies/Final_Energy_Non-Energy_Use_Chemicals_Gases_Fossil">
    <rdf:type rdf:resource="http://www.w3.org/2002/07/owl#Class"/>
    <rdfs:subClassOf rdf:resource="http://transience.eu/ontologies/Variable"/>
    <rdfs:label>Final Energy|Non-Energy Use|Chemicals|Gases|Fossil</rdfs:label>
    <rdfs:comment>Final energy consumption of synthetic or derived gases of fossil origin by the chemical sector by the non-combustion processes</rdfs:comment>
    <ex:unit>EJ/yr</ex:unit>
  </rdf:Description>
  <rdf:Description rdf:about="http://transience.eu/ontologies/Inflow_Concrete_Other_demand_sectors_Product_categories">
    <rdf:type rdf:resource="http://www.w3.org/2002/07/owl#Class"/>
    <rdfs:subClassOf rdf:resource="http://transience.eu/ontologies/Variable"/>
    <rdfs:label>Inflow|Concrete|Other|[demand sectors]|[Product categories]</rdfs:label>
    <rdfs:comment>Concrete inflow for other sectorsÂ </rdfs:comment>
    <ex:unit>t/yr</ex:unit>
  </rdf:Description>
  <rdf:Description rdf:about="http://transience.eu/ontologies/Carbon_Capture_Fossil_Energy_Supply_Other">
    <rdf:type rdf:resource="http://www.w3.org/2002/07/owl#Class"/>
    <rdfs:subClassOf rdf:resource="http://transience.eu/ontologies/Variable"/>
    <rdfs:label>Carbon Capture|Fossil|Energy|Supply|Other</rdfs:label>
    <rdfs:comment>total carbon dioxide emissions captured from fossil fuel use in other energy supply (part of IPCC category 1A), should be reported as positive numbers</rdfs:comment>
    <ex:unit>Mt CO2/yr</ex:unit>
  </rdf:Description>
  <rdf:Description rdf:about="http://transience.eu/ontologies/Secondary_Energy_Electricity">
    <rdf:type rdf:resource="http://www.w3.org/2002/07/owl#Class"/>
    <rdfs:subClassOf rdf:resource="http://transience.eu/ontologies/Variable"/>
    <rdfs:label>Secondary Energy|Electricity</rdfs:label>
    <rdfs:comment>total net electricity production</rdfs:comment>
    <ex:unit>EJ/yr</ex:unit>
  </rdf:Description>
  <rdf:Description rdf:about="http://transience.eu/ontologies/Investment_Energy_Supply_Electricity_Electricity_Storage">
    <rdf:type rdf:resource="http://www.w3.org/2002/07/owl#Class"/>
    <rdfs:subClassOf rdf:resource="http://transience.eu/ontologies/Variable"/>
    <rdfs:label>Investment|Energy Supply|Electricity|Electricity Storage</rdfs:label>
    <rdfs:comment>investments in electricity storage technologies (e.g., batteries, compressed air storage reservoirs, etc.)</rdfs:comment>
    <ex:unit>billion US$2010/yr</ex:unit>
  </rdf:Description>
  <rdf:Description rdf:about="http://transience.eu/ontologies/Investment_Infrastructure_Residential_and_Commercial_Medium-Efficiency_Buildings">
    <rdf:type rdf:resource="http://www.w3.org/2002/07/owl#Class"/>
    <rdfs:subClassOf rdf:resource="http://transience.eu/ontologies/Variable"/>
    <rdfs:label>Investment|Infrastructure|Residential and Commercial|Medium-Efficiency Buildings</rdfs:label>
    <rdfs:comment>investment into residential and commercial buildings infrastructure (all types of new buildings that are relatively medium-range in their energy efficiency)</rdfs:comment>
    <ex:unit>billion US$2010/yr</ex:unit>
  </rdf:Description>
  <rdf:Description rdf:about="http://transience.eu/ontologies/Total_Scrap_Non-Ferrous_Metals_Other">
    <rdf:type rdf:resource="http://www.w3.org/2002/07/owl#Class"/>
    <rdfs:subClassOf rdf:resource="http://transience.eu/ontologies/Variable"/>
    <rdfs:label>Total Scrap|Non-Ferrous Metals|Other</rdfs:label>
    <rdfs:comment>Total potential of non-ferrous metals scrap material as a result of end of life products (before collection)</rdfs:comment>
    <ex:unit>Mt/yr</ex:unit>
  </rdf:Description>
  <rdf:Description rdf:about="http://transience.eu/ontologies/Energy_Service_Transportation_Passenger">
    <rdf:type rdf:resource="http://www.w3.org/2002/07/owl#Class"/>
    <rdfs:subClassOf rdf:resource="http://transience.eu/ontologies/Variable"/>
    <rdfs:label>Energy Service|Transportation|Passenger</rdfs:label>
    <rdfs:comment>energy service demand for passenger transport</rdfs:comment>
    <ex:unit>bn pkm/yr</ex:unit>
  </rdf:Description>
  <rdf:Description rdf:about="http://transience.eu/ontologies/Lifetime_Electricity_Wind_Onshore">
    <rdf:type rdf:resource="http://www.w3.org/2002/07/owl#Class"/>
    <rdfs:subClassOf rdf:resource="http://transience.eu/ontologies/Variable"/>
    <rdfs:label>Lifetime|Electricity|Wind|Onshore</rdfs:label>
    <rdfs:comment>Lifetime of a new onshore wind power plant. Lifetime should be calculated by summing all vintages of a  capacity unit (e.g. (1+1+0.9+0.7+0.5) * 10 years = 41 years) or by the e-folding time for exponential capacity depreciation.  The lifetime should refer to the plant type(s) for which capital costs have been reported. If capital cost for more than one plant type has been reported, modellers should report lifetime for the additional plant types by adding variables Lifetime|Electricity|Wind|Onshore|2, ... Lifetime|Electricity|Wind|Onshore|N (matching the assignment of plant types to technologies in the reporting of capital costs as documented in the comments sheet). </rdfs:comment>
    <ex:unit>years</ex:unit>
  </rdf:Description>
  <rdf:Description rdf:about="http://transience.eu/ontologies/Investment_Petrochemicals_Biomass_pyrolysis_and_gasification">
    <rdf:type rdf:resource="http://www.w3.org/2002/07/owl#Class"/>
    <rdfs:subClassOf rdf:resource="http://transience.eu/ontologies/Variable"/>
    <rdfs:label>Investment|Petrochemicals|Biomass pyrolysis and gasification</rdfs:label>
    <rdfs:comment>Investment in plants to produce syngas from biomass, including combined pyrolysis and gasification</rdfs:comment>
    <ex:unit>Mio â‚¬_2022/yr</ex:unit>
  </rdf:Description>
  <rdf:Description rdf:about="http://transience.eu/ontologies/Carbon_Sequestration_CCS_Total_Industry_Petrochemicals">
    <rdf:type rdf:resource="http://www.w3.org/2002/07/owl#Class"/>
    <rdfs:subClassOf rdf:resource="http://transience.eu/ontologies/Variable"/>
    <rdfs:label>Carbon Sequestration|CCS|Total|Industry|Petrochemicals</rdfs:label>
    <rdfs:comment>CO2 captured and stored, including both fossil and biogenic CO2</rdfs:comment>
    <ex:unit>Mt CO2/yr</ex:unit>
  </rdf:Description>
  <rdf:Description rdf:about="http://transience.eu/ontologies/Capacity_Electricity_Nuclear">
    <rdf:type rdf:resource="http://www.w3.org/2002/07/owl#Class"/>
    <rdfs:subClassOf rdf:resource="http://transience.eu/ontologies/Variable"/>
    <rdfs:label>Capacity|Electricity|Nuclear</rdfs:label>
    <rdfs:comment>Total installed (available) capacity of nuclear power plants. The installed (available) capacity of nuclear power plants by plant type for which capital costs are reported should be reported by adding variables Capacity|Electricity|Nuclear|1, ..., Capacity|Electricity|Nuclear|N (matching the assignment of plant types to technologies in the reporting of capital costs as documented in the comments sheet). </rdfs:comment>
    <ex:unit>GW</ex:unit>
  </rdf:Description>
  <rdf:Description rdf:about="http://transience.eu/ontologies/Production_Non-Ferrous_Metals_Bauxite_Volume">
    <rdf:type rdf:resource="http://www.w3.org/2002/07/owl#Class"/>
    <rdfs:subClassOf rdf:resource="http://transience.eu/ontologies/Variable"/>
    <rdfs:label>Production|Non-Ferrous Metals|Bauxite|Volume</rdfs:label>
    <rdfs:comment>production of bauxite (raw material used for the production of primary aluminum)</rdfs:comment>
    <ex:unit>Mt/yr</ex:unit>
  </rdf:Description>
  <rdf:Description rdf:about="http://transience.eu/ontologies/Final_Energy_Industry_Non-Ferrous_Metals_Liquids_Biomass">
    <rdf:type rdf:resource="http://www.w3.org/2002/07/owl#Class"/>
    <rdfs:subClassOf rdf:resource="http://transience.eu/ontologies/Variable"/>
    <rdfs:label>Final Energy|Industry|Non-Ferrous Metals|Liquids|Biomass</rdfs:label>
    <rdfs:comment>Final energy consumption of liquid biofuels by the non-ferrous metals sector</rdfs:comment>
    <ex:unit>EJ/yr</ex:unit>
  </rdf:Description>
  <rdf:Description rdf:about="http://transience.eu/ontologies/Final_Energy_Residential_and_Commercial_Solids_Fossil">
    <rdf:type rdf:resource="http://www.w3.org/2002/07/owl#Class"/>
    <rdfs:subClassOf rdf:resource="http://transience.eu/ontologies/Variable"/>
    <rdfs:label>Final Energy|Residential and Commercial|Solids|Fossil</rdfs:label>
    <rdfs:comment>final energy consumption of fossil solids by the residential &amp; commercial sector</rdfs:comment>
    <ex:unit>EJ/yr</ex:unit>
  </rdf:Description>
  <rdf:Description rdf:about="http://transience.eu/ontologies/Lifetime_Electricity_Wind">
    <rdf:type rdf:resource="http://www.w3.org/2002/07/owl#Class"/>
    <rdfs:subClassOf rdf:resource="http://transience.eu/ontologies/Variable"/>
    <rdfs:label>Lifetime|Electricity|Wind</rdfs:label>
    <rdfs:comment>Lifetime of a new wind power plant (report only if wind power is not separated in onshore and offshore). Lifetime should be calculated by summing all vintages of a  capacity unit (e.g. (1+1+0.9+0.7+0.5) * 10 years = 41 years) or by the e-folding time for exponential capacity depreciation.  The lifetime should refer to the plant type(s) for which capital costs have been reported. If capital cost for more than one plant type has been reported, modellers should report lifetime for the additional plant types by adding variables Lifetime|Electricity|Wind|2, ... Lifetime|Electricity|Wind|N (matching the assignment of plant types to technologies in the reporting of capital costs as documented in the comments sheet). </rdfs:comment>
    <ex:unit>years</ex:unit>
  </rdf:Description>
  <rdf:Description rdf:about="http://transience.eu/ontologies/Carbon_Capture_Fossil">
    <rdf:type rdf:resource="http://www.w3.org/2002/07/owl#Class"/>
    <rdfs:subClassOf rdf:resource="http://transience.eu/ontologies/Variable"/>
    <rdfs:label>Carbon Capture|Fossil</rdfs:label>
    <rdfs:comment>total carbon dioxide emissions captured from fossil fuel use, should be reported as positive numbers</rdfs:comment>
    <ex:unit>Mt CO2/yr</ex:unit>
  </rdf:Description>
  <rdf:Description rdf:about="http://transience.eu/ontologies/Secondary_Energy_Heat_Solar">
    <rdf:type rdf:resource="http://www.w3.org/2002/07/owl#Class"/>
    <rdfs:subClassOf rdf:resource="http://transience.eu/ontologies/Variable"/>
    <rdfs:label>Secondary Energy|Heat|Solar</rdfs:label>
    <rdfs:comment>centralized heat generation from solar energy</rdfs:comment>
    <ex:unit>EJ/yr</ex:unit>
  </rdf:Description>
  <rdf:Description rdf:about="http://transience.eu/ontologies/Emissions_CO2_AFOLU">
    <rdf:type rdf:resource="http://www.w3.org/2002/07/owl#Class"/>
    <rdfs:subClassOf rdf:resource="http://transience.eu/ontologies/Variable"/>
    <rdfs:label>Emissions|CO2|AFOLU</rdfs:label>
    <rdfs:comment>CO2 emissions from agriculture, forestry and other land use (IPCC category 3), exlcuding energy-related emissions from these sectors</rdfs:comment>
    <ex:unit>Mt CO2/yr</ex:unit>
  </rdf:Description>
  <rdf:Description rdf:about="http://transience.eu/ontologies/Energy_Use_Industry_Petrochemicals_Plastic_wastes">
    <rdf:type rdf:resource="http://www.w3.org/2002/07/owl#Class"/>
    <rdfs:subClassOf rdf:resource="http://transience.eu/ontologies/Variable"/>
    <rdfs:label>Energy Use|Industry|Petrochemicals|Plastic wastes</rdfs:label>
    <rdfs:comment>Use of plastic waste, including both, non-energetic use and energetic use of by-products of plastic waste processing</rdfs:comment>
    <ex:unit>Mt/yr</ex:unit>
  </rdf:Description>
  <rdf:Description rdf:about="http://transience.eu/ontologies/Export_Energy">
    <rdf:type rdf:resource="http://www.w3.org/2002/07/owl#Class"/>
    <rdfs:subClassOf rdf:resource="http://transience.eu/ontologies/Variable"/>
    <rdfs:label>Export|Energy</rdfs:label>
    <rdfs:comment>export of energy commodities measured in monetary units.</rdfs:comment>
    <ex:unit>billion US$2010/yr</ex:unit>
  </rdf:Description>
  <rdf:Description rdf:about="http://transience.eu/ontologies/Emissions_CO2_Industry_and_Industrial_Processes">
    <rdf:type rdf:resource="http://www.w3.org/2002/07/owl#Class"/>
    <rdfs:subClassOf rdf:resource="http://transience.eu/ontologies/Variable"/>
    <rdfs:label>Emissions|CO2|Industry and Industrial Processes</rdfs:label>
    <rdfs:comment>Fossil CO2 emissions from fuel combustion in industry (IPCC category 1A2) and from industrial processes (IPCC categories 2A, B, C, E), net of negative emissions from Bioenergy with CCS (BECCS)</rdfs:comment>
    <ex:unit>Mt CO2/yr</ex:unit>
  </rdf:Description>
  <rdf:Description rdf:about="http://transience.eu/ontologies/Secondary_Energy_Electricity_Fossil">
    <rdf:type rdf:resource="http://www.w3.org/2002/07/owl#Class"/>
    <rdfs:subClassOf rdf:resource="http://transience.eu/ontologies/Variable"/>
    <rdfs:label>Secondary Energy|Electricity|Fossil</rdfs:label>
    <rdfs:comment>net electricity production from coal, gas, conventional and unconventional oil</rdfs:comment>
    <ex:unit>EJ/yr</ex:unit>
  </rdf:Description>
  <rdf:Description rdf:about="http://transience.eu/ontologies/Secondary_Energy_Electricity_Hydrogen">
    <rdf:type rdf:resource="http://www.w3.org/2002/07/owl#Class"/>
    <rdfs:subClassOf rdf:resource="http://transience.eu/ontologies/Variable"/>
    <rdfs:label>Secondary Energy|Electricity|Hydrogen</rdfs:label>
    <rdfs:comment>net electricity production from hydrogen</rdfs:comment>
    <ex:unit>EJ/yr</ex:unit>
  </rdf:Description>
  <rdf:Description rdf:about="http://transience.eu/ontologies/Secondary_Energy_Solids_Biomass">
    <rdf:type rdf:resource="http://www.w3.org/2002/07/owl#Class"/>
    <rdfs:subClassOf rdf:resource="http://transience.eu/ontologies/Variable"/>
    <rdfs:label>Secondary Energy|Solids|Biomass</rdfs:label>
    <rdfs:comment>solid secondary energy carriers produced from biomass (e.g., commercial charcoal, wood chips, wood pellets). Tradional bioenergy use is excluded.  </rdfs:comment>
    <ex:unit>EJ/yr</ex:unit>
  </rdf:Description>
  <rdf:Description rdf:about="http://transience.eu/ontologies/Final_Energy_Industry_Pulp_and_Paper_Solids_Biomass">
    <rdf:type rdf:resource="http://www.w3.org/2002/07/owl#Class"/>
    <rdfs:subClassOf rdf:resource="http://transience.eu/ontologies/Variable"/>
    <rdfs:label>Final Energy|Industry|Pulp and Paper|Solids|Biomass</rdfs:label>
    <rdfs:comment>Final energy consumption of solid biomass (modern and traditional, including renewable waste) by the pulp and paper sector</rdfs:comment>
    <ex:unit>EJ/yr</ex:unit>
  </rdf:Description>
  <rdf:Description rdf:about="http://transience.eu/ontologies/Secondary_Energy_Hydrogen_Gas_w_o_CCS">
    <rdf:type rdf:resource="http://www.w3.org/2002/07/owl#Class"/>
    <rdfs:subClassOf rdf:resource="http://transience.eu/ontologies/Variable"/>
    <rdfs:label>Secondary Energy|Hydrogen|Gas|w/o CCS</rdfs:label>
    <rdfs:comment>hydrogen production from natural gas with freely vented CO2 emissions</rdfs:comment>
    <ex:unit>EJ/yr</ex:unit>
  </rdf:Description>
  <rdf:Description rdf:about="http://transience.eu/ontologies/Lifetime_Hydrogen_Coal_w_o_CCS">
    <rdf:type rdf:resource="http://www.w3.org/2002/07/owl#Class"/>
    <rdfs:subClassOf rdf:resource="http://transience.eu/ontologies/Variable"/>
    <rdfs:label>Lifetime|Hydrogen|Coal|w/o CCS</rdfs:label>
    <rdfs:comment>Lifetime of a new coal to hydrogen plant w/o CCS. Lifetime should be calculated by summing all vintages of a  capacity unit (e.g. (1+1+0.9+0.7+0.5) * 10 years = 41 years) or by the e-folding time for exponential capacity depreciation.  The lifetime should refer to the plant type(s) for which capital costs have been reported. If capital cost for more than one plant type has been reported, modellers should report lifetime for the additional plant types by adding variables Lifetime|Hydrogen|Coal|w/o CCS|2, ... Lifetime|Hydrogen|Coal|w/o CCS|N (matching the assignment of plant types to technologies in the reporting of capital costs as documented in the comments sheet). </rdfs:comment>
    <ex:unit>years</ex:unit>
  </rdf:Description>
  <rdf:Description rdf:about="http://transience.eu/ontologies/Secondary_Energy_Electricity_Other">
    <rdf:type rdf:resource="http://www.w3.org/2002/07/owl#Class"/>
    <rdfs:subClassOf rdf:resource="http://transience.eu/ontologies/Variable"/>
    <rdfs:label>Secondary Energy|Electricity|Other</rdfs:label>
    <rdfs:comment>net electricity production from sources that do not fit to any other category (please provide a definition of the sources in this category in the 'comments' tab)</rdfs:comment>
    <ex:unit>EJ/yr</ex:unit>
  </rdf:Description>
  <rdf:Description rdf:about="http://transience.eu/ontologies/Energy_Use_Industry_Petrochemicals_Naphtha">
    <rdf:type rdf:resource="http://www.w3.org/2002/07/owl#Class"/>
    <rdfs:subClassOf rdf:resource="http://transience.eu/ontologies/Variable"/>
    <rdfs:label>Energy Use|Industry|Petrochemicals|Naphtha</rdfs:label>
    <rdfs:comment>Use of naphtha, including both, non-energetic use and energetic use of by-products of naphtha processing</rdfs:comment>
    <ex:unit>Mt/yr</ex:unit>
  </rdf:Description>
  <rdf:Description rdf:about="http://transience.eu/ontologies/Inflow_Steel_Product_categories">
    <rdf:type rdf:resource="http://www.w3.org/2002/07/owl#Class"/>
    <rdfs:subClassOf rdf:resource="http://transience.eu/ontologies/Variable"/>
    <rdfs:label>Inflow|Steel|[Product categories]</rdfs:label>
    <rdfs:comment>Steel inflow</rdfs:comment>
    <ex:unit>t/yr</ex:unit>
  </rdf:Description>
  <rdf:Description rdf:about="http://transience.eu/ontologies/Investment_Energy_Supply_Electricity_Ocean">
    <rdf:type rdf:resource="http://www.w3.org/2002/07/owl#Class"/>
    <rdfs:subClassOf rdf:resource="http://transience.eu/ontologies/Variable"/>
    <rdfs:label>Investment|Energy Supply|Electricity|Ocean</rdfs:label>
    <rdfs:comment>investments in new power generation for the specified power plant category. If the model features several sub-categories, the total investments should be reported. For plants equipped with CCS, the investment in the capturing equipment should be included but not the one on transport and storage.</rdfs:comment>
    <ex:unit>billion US$2010/yr</ex:unit>
  </rdf:Description>
  <rdf:Description rdf:about="http://transience.eu/ontologies/Primary_Energy_Industry_Steel_Coking_coal">
    <rdf:type rdf:resource="http://www.w3.org/2002/07/owl#Class"/>
    <rdfs:subClassOf rdf:resource="http://transience.eu/ontologies/Variable"/>
    <rdfs:label>Primary Energy|Industry|Steel|Coking coal</rdfs:label>
    <rdfs:comment>Energy demand including own coke ovens and autoproduction of electricity</rdfs:comment>
    <ex:unit>PJ/yr</ex:unit>
  </rdf:Description>
  <rdf:Description rdf:about="http://transience.eu/ontologies/Final_Energy_Residential_and_Commercial_Solids_Biomass">
    <rdf:type rdf:resource="http://www.w3.org/2002/07/owl#Class"/>
    <rdfs:subClassOf rdf:resource="http://transience.eu/ontologies/Variable"/>
    <rdfs:label>Final Energy|Residential and Commercial|Solids|Biomass</rdfs:label>
    <rdfs:comment>final energy consumption by the residential &amp; commercial sector of solid biomass (modern and traditional), excluding final energy consumption of bioliquids which are reported in the liquids category</rdfs:comment>
    <ex:unit>EJ/yr</ex:unit>
  </rdf:Description>
  <rdf:Description rdf:about="http://transience.eu/ontologies/Final_Energy_Industry_Pulp_and_Paper_Heat">
    <rdf:type rdf:resource="http://www.w3.org/2002/07/owl#Class"/>
    <rdfs:subClassOf rdf:resource="http://transience.eu/ontologies/Variable"/>
    <rdfs:label>Final Energy|Industry|Pulp and Paper|Heat</rdfs:label>
    <rdfs:comment>Final energy consumption of centrally supplied heat by the pulp and paper sector</rdfs:comment>
    <ex:unit>EJ/yr</ex:unit>
  </rdf:Description>
  <rdf:Description rdf:about="http://transience.eu/ontologies/Primary_Energy_Biomass_1st_Generation">
    <rdf:type rdf:resource="http://www.w3.org/2002/07/owl#Class"/>
    <rdfs:subClassOf rdf:resource="http://transience.eu/ontologies/Variable"/>
    <rdfs:label>Primary Energy|Biomass|1st Generation</rdfs:label>
    <rdfs:comment>biomass primary energy from 1st generation biofuel crops (e.g., sugar cane, rapeseed oil, maize, sugar beet)</rdfs:comment>
    <ex:unit>EJ/yr</ex:unit>
  </rdf:Description>
  <rdf:Description rdf:about="http://transience.eu/ontologies/Investment_Energy_Supply_Liquids_Biomass">
    <rdf:type rdf:resource="http://www.w3.org/2002/07/owl#Class"/>
    <rdfs:subClassOf rdf:resource="http://transience.eu/ontologies/Variable"/>
    <rdfs:label>Investment|Energy Supply|Liquids|Biomass</rdfs:label>
    <rdfs:comment>investments for the production of biofuels. These should not include the costs of the feedstock. For plants equipped with CCS, the investment in the capturing equipment should be included but not the one on transport and storage.</rdfs:comment>
    <ex:unit>billion US$2010/yr</ex:unit>
  </rdf:Description>
  <rdf:Description rdf:about="http://transience.eu/ontologies/Final_Energy_Commercial_Gases_Fossil">
    <rdf:type rdf:resource="http://www.w3.org/2002/07/owl#Class"/>
    <rdfs:subClassOf rdf:resource="http://transience.eu/ontologies/Variable"/>
    <rdfs:label>Final Energy|Commercial|Gases|Fossil</rdfs:label>
    <rdfs:comment>final energy consumption by the commercial sector of  synthetic or derived gases of fossil origin, excluding transmission/distribution losses</rdfs:comment>
    <ex:unit>EJ/yr</ex:unit>
  </rdf:Description>
  <rdf:Description rdf:about="http://transience.eu/ontologies/Expenditure_household_Industry">
    <rdf:type rdf:resource="http://www.w3.org/2002/07/owl#Class"/>
    <rdfs:subClassOf rdf:resource="http://transience.eu/ontologies/Variable"/>
    <rdfs:label>Expenditure|household|Industry</rdfs:label>
    <rdfs:comment>expenditure of households for industrial goods.</rdfs:comment>
    <ex:unit>billion US$2010/yr</ex:unit>
  </rdf:Description>
  <rdf:Description rdf:about="http://transience.eu/ontologies/Investment_Energy_Supply_Electricity_Fossil">
    <rdf:type rdf:resource="http://www.w3.org/2002/07/owl#Class"/>
    <rdfs:subClassOf rdf:resource="http://transience.eu/ontologies/Variable"/>
    <rdfs:label>Investment|Energy Supply|Electricity|Fossil</rdfs:label>
    <rdfs:comment>investments in new power generation for the specified power plant category. If the model features several sub-categories, the total investments should be reported. For plants equipped with CCS, the investment in the capturing equipment should be included but not the one on transport and storage.</rdfs:comment>
    <ex:unit>billion US$2010/yr</ex:unit>
  </rdf:Description>
  <rdf:Description rdf:about="http://transience.eu/ontologies/Investment_Energy_Supply_Extraction_Bioenergy">
    <rdf:type rdf:resource="http://www.w3.org/2002/07/owl#Class"/>
    <rdfs:subClassOf rdf:resource="http://transience.eu/ontologies/Variable"/>
    <rdfs:label>Investment|Energy Supply|Extraction|Bioenergy</rdfs:label>
    <rdfs:comment>investments for extraction and production of bioenergy</rdfs:comment>
    <ex:unit>billion US$2010/yr</ex:unit>
  </rdf:Description>
  <rdf:Description rdf:about="http://transience.eu/ontologies/Capital_Cost_Electricity_Gas_w__CCS">
    <rdf:type rdf:resource="http://www.w3.org/2002/07/owl#Class"/>
    <rdfs:subClassOf rdf:resource="http://transience.eu/ontologies/Variable"/>
    <rdfs:label>Capital Cost|Electricity|Gas|w/ CCS</rdfs:label>
    <rdfs:comment>Capital cost of a new gas power plant with CCS. If more than one CCS gas power technology is modelled, modellers should report capital costs for each represented CCS gas power technology by adding variables Capital Cost|Electricity|Gas|w/ CCS|2, ... Capital Cost|Electricity|Gas|w/ CCS|N (with N = number of represented technologies). It is modeller's choice which CCS gas power technologies to assign to type 1 (assigned to the variable without number suffix),2,...,N. The assignment should be documented in the comments sheet. </rdfs:comment>
    <ex:unit>US$2010/kW</ex:unit>
  </rdf:Description>
  <rdf:Description rdf:about="http://transience.eu/ontologies/Gross_Emissions_CO2_Energy_Demand">
    <rdf:type rdf:resource="http://www.w3.org/2002/07/owl#Class"/>
    <rdfs:subClassOf rdf:resource="http://transience.eu/ontologies/Variable"/>
    <rdfs:label>Gross Emissions|CO2|Energy|Demand</rdfs:label>
    <rdfs:comment>Gross Fossil CO2 emissions from fuel combustion in industry (IPCC category 1A2), residential, commercial, institutional sectors and agriculture, forestry, fishing (AFOFI) (IPCC category 1A4a, 1A4b, 1A4c), and transportation sector (IPCC category 1A3), excluding pipeline emissions (IPCC category 1A3ei), not accounting for negative emissions from BECCS</rdfs:comment>
    <ex:unit>Mt CO2/yr</ex:unit>
  </rdf:Description>
  <rdf:Description rdf:about="http://transience.eu/ontologies/Capital_Cost_Gases_Biomass_w__CCS">
    <rdf:type rdf:resource="http://www.w3.org/2002/07/owl#Class"/>
    <rdfs:subClassOf rdf:resource="http://transience.eu/ontologies/Variable"/>
    <rdfs:label>Capital Cost|Gases|Biomass|w/ CCS</rdfs:label>
    <rdfs:comment>Capital cost of a new biomass to gas plant with CCS. If more than one CCS biomass to gas technology is modelled, modellers should report capital costs for each represented CCS biomass to  gas technology by adding variables Capital Cost|Gases|Biomass|w/ CCS|2, ... Capital Cost|Gases|Biomass|w/ CCS|N (with N = number of represented technologies). It is modeller's choice which CCS biomass to gas technologies to assign to type 1 (assigned to the variable without number suffix),2,...,N. The assignment should be documented in the comments sheet. </rdfs:comment>
    <ex:unit>US$2010/kW</ex:unit>
  </rdf:Description>
  <rdf:Description rdf:about="http://transience.eu/ontologies/Final_Energy_Non-Energy_Use_Liquids_Electricity">
    <rdf:type rdf:resource="http://www.w3.org/2002/07/owl#Class"/>
    <rdfs:subClassOf rdf:resource="http://transience.eu/ontologies/Variable"/>
    <rdfs:label>Final Energy|Non-Energy Use|Liquids|Electricity</rdfs:label>
    <rdfs:comment>Final energy consumption of synthetic liquids of fossil origin by the non-combustion processes</rdfs:comment>
    <ex:unit>EJ/yr</ex:unit>
  </rdf:Description>
  <rdf:Description rdf:about="http://transience.eu/ontologies/Final_Energy_Non-Energy_Use_Chemicals_Other">
    <rdf:type rdf:resource="http://www.w3.org/2002/07/owl#Class"/>
    <rdfs:subClassOf rdf:resource="http://transience.eu/ontologies/Variable"/>
    <rdfs:label>Final Energy|Non-Energy Use|Chemicals|Other</rdfs:label>
    <rdfs:comment>Final energy consumption of other feedstocks by the chemical sector by the non-combustion processes (please provide a definition of the feedstocks in this category in the 'comments' tab)</rdfs:comment>
    <ex:unit>EJ/yr</ex:unit>
  </rdf:Description>
  <rdf:Description rdf:about="http://transience.eu/ontologies/Consumption">
    <rdf:type rdf:resource="http://www.w3.org/2002/07/owl#Class"/>
    <rdfs:subClassOf rdf:resource="http://transience.eu/ontologies/Variable"/>
    <rdfs:label>Consumption</rdfs:label>
    <rdfs:comment>total consumption of all goods, by all consumers in a region</rdfs:comment>
    <ex:unit>billion US$2010/yr</ex:unit>
  </rdf:Description>
  <rdf:Description rdf:about="http://transience.eu/ontologies/Final_Energy_Transportation_Hydrogen_Biomass">
    <rdf:type rdf:resource="http://www.w3.org/2002/07/owl#Class"/>
    <rdfs:subClassOf rdf:resource="http://transience.eu/ontologies/Variable"/>
    <rdfs:label>Final Energy|Transportation|Hydrogen|Biomass</rdfs:label>
    <rdfs:comment>final energy consumption by the transportation sector of hydrogen from biomass</rdfs:comment>
    <ex:unit>EJ/yr</ex:unit>
  </rdf:Description>
  <rdf:Description rdf:about="http://transience.eu/ontologies/Final_Energy_Non-Energy_Use_Chemicals_Solids_Biomass">
    <rdf:type rdf:resource="http://www.w3.org/2002/07/owl#Class"/>
    <rdfs:subClassOf rdf:resource="http://transience.eu/ontologies/Variable"/>
    <rdfs:label>Final Energy|Non-Energy Use|Chemicals|Solids|Biomass</rdfs:label>
    <rdfs:comment>Final energy consumption of solid biomass (modern and traditional, including renewable waste) by the chemical sector by the non-combustion processes</rdfs:comment>
    <ex:unit>EJ/yr</ex:unit>
  </rdf:Description>
  <rdf:Description rdf:about="http://transience.eu/ontologies/Final_Energy_Transportation">
    <rdf:type rdf:resource="http://www.w3.org/2002/07/owl#Class"/>
    <rdfs:subClassOf rdf:resource="http://transience.eu/ontologies/Variable"/>
    <rdfs:label>Final Energy|Transportation</rdfs:label>
    <rdfs:comment>final energy consumed in the transportation sector, excluding bunker fuels, excluding pipelines</rdfs:comment>
    <ex:unit>EJ/yr</ex:unit>
  </rdf:Description>
  <rdf:Description rdf:about="http://transience.eu/ontologies/Primary_Energy_Biomass_Electricity_w__CCS">
    <rdf:type rdf:resource="http://www.w3.org/2002/07/owl#Class"/>
    <rdfs:subClassOf rdf:resource="http://transience.eu/ontologies/Variable"/>
    <rdfs:label>Primary Energy|Biomass|Electricity|w/ CCS</rdfs:label>
    <rdfs:comment>purpose-grown bioenergy crops, crop and forestry residue bioenergy, municipal solid waste bioenergy, traditional biomass primary energy input to electricity generation used in combination with CCS</rdfs:comment>
    <ex:unit>EJ/yr</ex:unit>
  </rdf:Description>
  <rdf:Description rdf:about="http://transience.eu/ontologies/Carbon_Sequestration_Plastic_products_Industry_Petrochemicals">
    <rdf:type rdf:resource="http://www.w3.org/2002/07/owl#Class"/>
    <rdfs:subClassOf rdf:resource="http://transience.eu/ontologies/Variable"/>
    <rdfs:label>Carbon Sequestration|Plastic products|Industry|Petrochemicals</rdfs:label>
    <rdfs:comment>Carbon (temporarily) stored in products, including both fossil and biogenic CO2 (including C stored in all products, independent of product life-time)</rdfs:comment>
    <ex:unit>Mt CO2_eq/yr</ex:unit>
  </rdf:Description>
  <rdf:Description rdf:about="http://transience.eu/ontologies/Lifetime_Liquids_Gas_w_o_CCS">
    <rdf:type rdf:resource="http://www.w3.org/2002/07/owl#Class"/>
    <rdfs:subClassOf rdf:resource="http://transience.eu/ontologies/Variable"/>
    <rdfs:label>Lifetime|Liquids|Gas|w/o CCS</rdfs:label>
    <rdfs:comment>Lifetime of a new gas to liquids plant w/o CCS. Lifetime should be calculated by summing all vintages of a  capacity unit (e.g. (1+1+0.9+0.7+0.5) * 10 years = 41 years) or by the e-folding time for exponential capacity depreciation.  The lifetime should refer to the plant type(s) for which capital costs have been reported. If capital cost for more than one plant type has been reported, modellers should report lifetime for the additional plant types by adding variables Lifetime|Liquids|Gas|w/o CCS|2, ... Lifetime|Liquids|Gas|w/o CCS|N (matching the assignment of plant types to technologies in the reporting of capital costs as documented in the comments sheet). </rdfs:comment>
    <ex:unit>years</ex:unit>
  </rdf:Description>
  <rdf:Description rdf:about="http://transience.eu/ontologies/Price_Final_Energy_Residential_Gases_Fossil">
    <rdf:type rdf:resource="http://www.w3.org/2002/07/owl#Class"/>
    <rdfs:subClassOf rdf:resource="http://transience.eu/ontologies/Variable"/>
    <rdfs:label>Price|Final Energy|Residential|Gases|Fossil</rdfs:label>
    <rdfs:comment>natural gas price at the final level in the residential sector. Prices should include the effect of carbon prices.</rdfs:comment>
    <ex:unit>US$2010/GJ</ex:unit>
  </rdf:Description>
  <rdf:Description rdf:about="http://transience.eu/ontologies/Investment_Energy_Supply_Extraction_Uranium">
    <rdf:type rdf:resource="http://www.w3.org/2002/07/owl#Class"/>
    <rdfs:subClassOf rdf:resource="http://transience.eu/ontologies/Variable"/>
    <rdfs:label>Investment|Energy Supply|Extraction|Uranium</rdfs:label>
    <rdfs:comment>investments for extraction and conversion of uranium. These should include mining, conversion and enrichment</rdfs:comment>
    <ex:unit>billion US$2010/yr</ex:unit>
  </rdf:Description>
  <rdf:Description rdf:about="http://transience.eu/ontologies/Final_Energy_Industry_Pulp_and_Paper_Gases_Biomass">
    <rdf:type rdf:resource="http://www.w3.org/2002/07/owl#Class"/>
    <rdfs:subClassOf rdf:resource="http://transience.eu/ontologies/Variable"/>
    <rdfs:label>Final Energy|Industry|Pulp and Paper|Gases|Biomass</rdfs:label>
    <rdfs:comment>Final energy consumption of biogas by the pulp and paper sector</rdfs:comment>
    <ex:unit>EJ/yr</ex:unit>
  </rdf:Description>
  <rdf:Description rdf:about="http://transience.eu/ontologies/Final_Energy_Industry_Iron_and_Steel_Solids_Coal">
    <rdf:type rdf:resource="http://www.w3.org/2002/07/owl#Class"/>
    <rdfs:subClassOf rdf:resource="http://transience.eu/ontologies/Variable"/>
    <rdfs:label>Final Energy|Industry|Iron and Steel|Solids|Coal</rdfs:label>
    <rdfs:comment>Final energy consumption of coal by the iron and steel sector</rdfs:comment>
    <ex:unit>EJ/yr</ex:unit>
  </rdf:Description>
  <rdf:Description rdf:about="http://transience.eu/ontologies/Secondary_Energy_Electricity_Solar_PV">
    <rdf:type rdf:resource="http://www.w3.org/2002/07/owl#Class"/>
    <rdfs:subClassOf rdf:resource="http://transience.eu/ontologies/Variable"/>
    <rdfs:label>Secondary Energy|Electricity|Solar|PV</rdfs:label>
    <rdfs:comment>net electricity production from solar photovoltaics (PV)</rdfs:comment>
    <ex:unit>EJ/yr</ex:unit>
  </rdf:Description>
  <rdf:Description rdf:about="http://transience.eu/ontologies/Final_Energy_Residential_and_Commercial_Liquids_Electricity">
    <rdf:type rdf:resource="http://www.w3.org/2002/07/owl#Class"/>
    <rdfs:subClassOf rdf:resource="http://transience.eu/ontologies/Variable"/>
    <rdfs:label>Final Energy|Residential and Commercial|Liquids|Electricity</rdfs:label>
    <rdfs:comment>final energy consumption by the residential &amp; commercial sector of liquid efuels ("power-to-liquid")</rdfs:comment>
    <ex:unit>EJ/yr</ex:unit>
  </rdf:Description>
  <rdf:Description rdf:about="http://transience.eu/ontologies/Final_Energy_Industry_Chemicals_Waste">
    <rdf:type rdf:resource="http://www.w3.org/2002/07/owl#Class"/>
    <rdfs:subClassOf rdf:resource="http://transience.eu/ontologies/Variable"/>
    <rdfs:label>Final Energy|Industry|Chemicals|Waste</rdfs:label>
    <rdfs:comment>Final energy consumption of non-renewable waste by the chemicals sector</rdfs:comment>
    <ex:unit>EJ/yr</ex:unit>
  </rdf:Description>
  <rdf:Description rdf:about="http://transience.eu/ontologies/Cost_Production_Steel_DRI_EAF_NG_CCS">
    <rdf:type rdf:resource="http://www.w3.org/2002/07/owl#Class"/>
    <rdfs:subClassOf rdf:resource="http://transience.eu/ontologies/Variable"/>
    <rdfs:label>Cost|Production|Steel|DRI_EAF_NG_CCS</rdfs:label>
    <rdfs:comment>Specific production cost of crude steel in DRI/EAF route when using natural gas as reducing gas and doing CCS; including CAPEX (annuity), fixed and variable OPEX, including CO2 transport and storage costs</rdfs:comment>
    <ex:unit>Mio â‚¬_2022 / t crude steel</ex:unit>
  </rdf:Description>
  <rdf:Description rdf:about="http://transience.eu/ontologies/Final_Energy_Industry_Petrochemicals_Steam">
    <rdf:type rdf:resource="http://www.w3.org/2002/07/owl#Class"/>
    <rdfs:subClassOf rdf:resource="http://transience.eu/ontologies/Variable"/>
    <rdfs:label>Final Energy|Industry|Petrochemicals|Steam</rdfs:label>
    <rdfs:comment>Final energy demand of steam (180-500Â°C) (to be supplied by CHP or boilers on-site or from external supply)</rdfs:comment>
    <ex:unit>PJ/yr</ex:unit>
  </rdf:Description>
  <rdf:Description rdf:about="http://transience.eu/ontologies/Final_Energy_Residential_Gases_Biomass">
    <rdf:type rdf:resource="http://www.w3.org/2002/07/owl#Class"/>
    <rdfs:subClassOf rdf:resource="http://transience.eu/ontologies/Variable"/>
    <rdfs:label>Final Energy|Residential|Gases|Biomass</rdfs:label>
    <rdfs:comment>final energy consumption by the residential sector of biogas, excluding transmission/distribution losses</rdfs:comment>
    <ex:unit>EJ/yr</ex:unit>
  </rdf:Description>
  <rdf:Description rdf:about="http://transience.eu/ontologies/Capital_Cost_Hydrogen_Electricity">
    <rdf:type rdf:resource="http://www.w3.org/2002/07/owl#Class"/>
    <rdfs:subClassOf rdf:resource="http://transience.eu/ontologies/Variable"/>
    <rdfs:label>Capital Cost|Hydrogen|Electricity</rdfs:label>
    <rdfs:comment>Capital cost of a new hydrogen-by-electrolysis plant. If more than hydrogen-by-electrolysis technology is modelled, modellers should report capital costs for each represented hydrogen-by-electrolysis technology by adding variables Capital Cost|Hydrogen|Electricity|2, ... Capital Cost|Hydrogen|Electricity|N (with N = number of represented technologies). It is modeller's choice which hydrogen-by-electrolysis technologies to assign to type 1 (assigned to the variable without number suffix),2,...,N. The assignment should be documented in the comments sheet. </rdfs:comment>
    <ex:unit>US$2010/kW</ex:unit>
  </rdf:Description>
  <rdf:Description rdf:about="http://transience.eu/ontologies/Final_Energy_Residential_Liquids_Fossil">
    <rdf:type rdf:resource="http://www.w3.org/2002/07/owl#Class"/>
    <rdfs:subClassOf rdf:resource="http://transience.eu/ontologies/Variable"/>
    <rdfs:label>Final Energy|Residential|Liquids|Fossil</rdfs:label>
    <rdfs:comment>final energy consumption by the residential sector of liquids from fossil origin (conventional &amp; unconventional petroleum, coal-to-liquids, gas-to-liquids)</rdfs:comment>
    <ex:unit>EJ/yr</ex:unit>
  </rdf:Description>
  <rdf:Description rdf:about="http://transience.eu/ontologies/Secondary_Energy_Liquids_Gas_w__CCS">
    <rdf:type rdf:resource="http://www.w3.org/2002/07/owl#Class"/>
    <rdfs:subClassOf rdf:resource="http://transience.eu/ontologies/Variable"/>
    <rdfs:label>Secondary Energy|Liquids|Gas|w/ CCS</rdfs:label>
    <rdfs:comment>total production of fossil liquid synfuels from gas-to-liquids (GTL) technologies with CCS</rdfs:comment>
    <ex:unit>EJ/yr</ex:unit>
  </rdf:Description>
  <rdf:Description rdf:about="http://transience.eu/ontologies/OM_Cost_Fixed_Hydrogen_Coal_w__CCS">
    <rdf:type rdf:resource="http://www.w3.org/2002/07/owl#Class"/>
    <rdfs:subClassOf rdf:resource="http://transience.eu/ontologies/Variable"/>
    <rdfs:label>OM Cost|Fixed|Hydrogen|Coal|w/ CCS</rdfs:label>
    <rdfs:comment>Annual fixed operation &amp; maintainance cost of a new coal to hydrogen plant with CCS. If more than one CCS coal to hydrogen technology is modelled, modellers should report fixed O&amp;M costs  for each represented CCS coal to hydrogen technology by adding variables OM Cost|Fixed|Hydrogen|Coal|w/ CCS|2, ... OM Cost|Fixed|Hydrogen|Coal|w/ CCS|N (with N = number of represented technologies) (matching the assignment of plant types to technologies in the reporting of capital costs as documented in the comments sheet).</rdfs:comment>
    <ex:unit>US$2010/kW/yr</ex:unit>
  </rdf:Description>
  <rdf:Description rdf:about="http://transience.eu/ontologies/Secondary_Energy_Electricity_Wind_Onshore">
    <rdf:type rdf:resource="http://www.w3.org/2002/07/owl#Class"/>
    <rdfs:subClassOf rdf:resource="http://transience.eu/ontologies/Variable"/>
    <rdfs:label>Secondary Energy|Electricity|Wind|Onshore</rdfs:label>
    <rdfs:comment>net electricity production from onshore wind energy</rdfs:comment>
    <ex:unit>EJ/yr</ex:unit>
  </rdf:Description>
  <rdf:Description rdf:about="http://transience.eu/ontologies/OM_Cost_Fixed_Hydrogen_Electricity">
    <rdf:type rdf:resource="http://www.w3.org/2002/07/owl#Class"/>
    <rdfs:subClassOf rdf:resource="http://transience.eu/ontologies/Variable"/>
    <rdfs:label>OM Cost|Fixed|Hydrogen|Electricity</rdfs:label>
    <rdfs:comment>Annual fixed operation &amp; maintainance cost of a new hydrogen-by-electrolysis plant. If more than hydrogen-by-electrolysis technology is modelled, modellers should report fixed O&amp;M costs  for each represented hydrogen-by-electrolysis technology by adding variables OM Cost|Fixed|Hydrogen|Electricity|2, ... OM Cost|Fixed|Hydrogen|Electricity|N (with N = number of represented technologies) (matching the assignment of plant types to technologies in the reporting of capital costs as documented in the comments sheet).</rdfs:comment>
    <ex:unit>US$2010/kW/yr</ex:unit>
  </rdf:Description>
  <rdf:Description rdf:about="http://transience.eu/ontologies/Emissions_CO2_Energy_Supply_Autoproduction">
    <rdf:type rdf:resource="http://www.w3.org/2002/07/owl#Class"/>
    <rdfs:subClassOf rdf:resource="http://transience.eu/ontologies/Variable"/>
    <rdfs:label>Emissions|CO2|Energy|Supply|Autoproduction</rdfs:label>
    <rdfs:comment>Fossil CO2 emissions from electricty/heat production for own use</rdfs:comment>
    <ex:unit>Mt CO2/yr</ex:unit>
  </rdf:Description>
  <rdf:Description rdf:about="http://transience.eu/ontologies/Inflow_Steel_Other_demand_sectors_Product_categories">
    <rdf:type rdf:resource="http://www.w3.org/2002/07/owl#Class"/>
    <rdfs:subClassOf rdf:resource="http://transience.eu/ontologies/Variable"/>
    <rdfs:label>Inflow|Steel|Other|[demand sectors]|[Product categories]</rdfs:label>
    <rdfs:comment>Steel inflow for other sectorsÂ </rdfs:comment>
    <ex:unit>t/yr</ex:unit>
  </rdf:Description>
  <rdf:Description rdf:about="http://transience.eu/ontologies/Energy_Service_Bunkers_Freight_International_Shipping">
    <rdf:type rdf:resource="http://www.w3.org/2002/07/owl#Class"/>
    <rdfs:subClassOf rdf:resource="http://transience.eu/ontologies/Variable"/>
    <rdfs:label>Energy Service|Bunkers|Freight|International Shipping</rdfs:label>
    <rdfs:comment>energy service demand for freight transport operating on international shipping routes</rdfs:comment>
    <ex:unit>bn tkm/yr</ex:unit>
  </rdf:Description>
  <rdf:Description rdf:about="http://transience.eu/ontologies/Stock_materials_Cars_car_types">
    <rdf:type rdf:resource="http://www.w3.org/2002/07/owl#Class"/>
    <rdfs:subClassOf rdf:resource="http://transience.eu/ontologies/Variable"/>
    <rdfs:label>Stock|[materials]|Cars|[car types]</rdfs:label>
    <rdfs:comment>Material stock in carsÂ </rdfs:comment>
    <ex:unit>t/yr</ex:unit>
  </rdf:Description>
  <rdf:Description rdf:about="http://transience.eu/ontologies/Primary_Energy_Industry_Steel_Hydrogen">
    <rdf:type rdf:resource="http://www.w3.org/2002/07/owl#Class"/>
    <rdfs:subClassOf rdf:resource="http://transience.eu/ontologies/Variable"/>
    <rdfs:label>Primary Energy|Industry|Steel|Hydrogen</rdfs:label>
    <rdfs:comment>Energy demand including own coke ovens and autoproduction of electricity</rdfs:comment>
    <ex:unit>PJ/yr</ex:unit>
  </rdf:Description>
  <rdf:Description rdf:about="http://transience.eu/ontologies/Investment_Energy_Supply_Electricity">
    <rdf:type rdf:resource="http://www.w3.org/2002/07/owl#Class"/>
    <rdfs:subClassOf rdf:resource="http://transience.eu/ontologies/Variable"/>
    <rdfs:label>Investment|Energy Supply|Electricity</rdfs:label>
    <rdfs:comment>Investments into electricity generation and supply (including electricity storage and transmission &amp; distribution)</rdfs:comment>
    <ex:unit>billion US$2010/yr</ex:unit>
  </rdf:Description>
  <rdf:Description rdf:about="http://transience.eu/ontologies/OM_Cost_Fixed_Electricity_Nuclear">
    <rdf:type rdf:resource="http://www.w3.org/2002/07/owl#Class"/>
    <rdfs:subClassOf rdf:resource="http://transience.eu/ontologies/Variable"/>
    <rdfs:label>OM Cost|Fixed|Electricity|Nuclear</rdfs:label>
    <rdfs:comment>Annual fixed operation &amp; maintainance cost of a new nuclear power plants. If more than one nuclear power plant technology is modelled (e.g., Gen II, III, IV; LWR, thermal reactors with other moderator materials, fast breeders), modellers should report fixed O&amp;M costs  for each represented nuclear power technology by adding variables OM Cost|Fixed|Electricity|Nuclear|2, ... Capital|Cost|Electricity|Nuclear|N (with N = number of represented nuclear power technologies) (matching the assignment of plant types to technologies in the reporting of capital costs as documented in the comments sheet).</rdfs:comment>
    <ex:unit>US$2010/kW/yr</ex:unit>
  </rdf:Description>
  <rdf:Description rdf:about="http://transience.eu/ontologies/Carbon_Capture_Storage_Other">
    <rdf:type rdf:resource="http://www.w3.org/2002/07/owl#Class"/>
    <rdfs:subClassOf rdf:resource="http://transience.eu/ontologies/Variable"/>
    <rdfs:label>Carbon Capture|Storage|Other</rdfs:label>
    <rdfs:comment>total carbon dioxide captured  and stored in geological deposits (e.g. in depleted oil and gas fields, unmined coal seams, saline aquifers) and the deep ocean, stored amounts should be reported as positive numbers through other techniques (please provide a definition of other sources in this category in the 'comments' tab)</rdfs:comment>
    <ex:unit>Mt CO2/yr</ex:unit>
  </rdf:Description>
  <rdf:Description rdf:about="http://transience.eu/ontologies/Export_Industry">
    <rdf:type rdf:resource="http://www.w3.org/2002/07/owl#Class"/>
    <rdfs:subClassOf rdf:resource="http://transience.eu/ontologies/Variable"/>
    <rdfs:label>Export|Industry</rdfs:label>
    <rdfs:comment>export of industrial (non-energy) commodities measured in monetary units.</rdfs:comment>
    <ex:unit>billion US$2010/yr</ex:unit>
  </rdf:Description>
  <rdf:Description rdf:about="http://transience.eu/ontologies/Primary_Energy_Industry_Steel_Hard_coal_">
    <rdf:type rdf:resource="http://www.w3.org/2002/07/owl#Class"/>
    <rdfs:subClassOf rdf:resource="http://transience.eu/ontologies/Variable"/>
    <rdfs:label>Primary Energy|Industry|Steel|Hard coal </rdfs:label>
    <rdfs:comment>Energy demand including own coke ovens and autoproduction of electricity</rdfs:comment>
    <ex:unit>PJ/yr</ex:unit>
  </rdf:Description>
  <rdf:Description rdf:about="http://transience.eu/ontologies/Total_Scrap_Iron_and_Steel_Power_Sector">
    <rdf:type rdf:resource="http://www.w3.org/2002/07/owl#Class"/>
    <rdfs:subClassOf rdf:resource="http://transience.eu/ontologies/Variable"/>
    <rdfs:label>Total Scrap|Iron and Steel|Power Sector</rdfs:label>
    <rdfs:comment>Total potential of iron &amp; steel scrap material as a result of end of life products (before collection)</rdfs:comment>
    <ex:unit>Mt/yr</ex:unit>
  </rdf:Description>
  <rdf:Description rdf:about="http://transience.eu/ontologies/GDP_MER">
    <rdf:type rdf:resource="http://www.w3.org/2002/07/owl#Class"/>
    <rdfs:subClassOf rdf:resource="http://transience.eu/ontologies/Variable"/>
    <rdfs:label>GDP|MER</rdfs:label>
    <rdfs:comment>GDP at market exchange rate</rdfs:comment>
    <ex:unit>billion US$2010/yr</ex:unit>
  </rdf:Description>
  <rdf:Description rdf:about="http://transience.eu/ontologies/Lifetime_Electricity_Geothermal">
    <rdf:type rdf:resource="http://www.w3.org/2002/07/owl#Class"/>
    <rdfs:subClassOf rdf:resource="http://transience.eu/ontologies/Variable"/>
    <rdfs:label>Lifetime|Electricity|Geothermal</rdfs:label>
    <rdfs:comment>Lifetime of a new geothermal power plant. Lifetime should be calculated by summing all vintages of a  capacity unit (e.g. (1+1+0.9+0.7+0.5) * 10 years = 41 years) or by the e-folding time for exponential capacity depreciation.  The lifetime should refer to the plant type(s) for which capital costs have been reported. If capital cost for more than one plant type has been reported, modellers should report lifetime for the additional plant types by adding variables Lifetime|Electricity|Geothermal|2, ... Lifetime|Electricity|Geothermal|N (matching the assignment of plant types to technologies in the reporting of capital costs as documented in the comments sheet). </rdfs:comment>
    <ex:unit>years</ex:unit>
  </rdf:Description>
  <rdf:Description rdf:about="http://transience.eu/ontologies/Investment_Infrastructure_Water_Other">
    <rdf:type rdf:resource="http://www.w3.org/2002/07/owl#Class"/>
    <rdfs:subClassOf rdf:resource="http://transience.eu/ontologies/Variable"/>
    <rdfs:label>Investment|Infrastructure|Water|Other</rdfs:label>
    <rdfs:comment>investment into water-related infrastructure (other than for thermal cooling and irrigation)</rdfs:comment>
    <ex:unit>billion US$2010/yr</ex:unit>
  </rdf:Description>
  <rdf:Description rdf:about="http://transience.eu/ontologies/Trade_Secondary_Energy_Liquids_Biomass_Volume">
    <rdf:type rdf:resource="http://www.w3.org/2002/07/owl#Class"/>
    <rdfs:subClassOf rdf:resource="http://transience.eu/ontologies/Variable"/>
    <rdfs:label>Trade|Secondary Energy|Liquids|Biomass|Volume</rdfs:label>
    <rdfs:comment>net exports of liquid biofuels, at the global level these should add up to the trade losses only (for those models that are able to split solid and liquid bioenergy)</rdfs:comment>
    <ex:unit>EJ/yr</ex:unit>
  </rdf:Description>
  <rdf:Description rdf:about="http://transience.eu/ontologies/Secondary_Energy_Electricity_Solar">
    <rdf:type rdf:resource="http://www.w3.org/2002/07/owl#Class"/>
    <rdfs:subClassOf rdf:resource="http://transience.eu/ontologies/Variable"/>
    <rdfs:label>Secondary Energy|Electricity|Solar</rdfs:label>
    <rdfs:comment>net electricity production from all sources of solar energy (e.g., PV and concentrating solar power)</rdfs:comment>
    <ex:unit>EJ/yr</ex:unit>
  </rdf:Description>
  <rdf:Description rdf:about="http://transience.eu/ontologies/Expenditure_RnD">
    <rdf:type rdf:resource="http://www.w3.org/2002/07/owl#Class"/>
    <rdfs:subClassOf rdf:resource="http://transience.eu/ontologies/Variable"/>
    <rdfs:label>Expenditure|RnD</rdfs:label>
    <rdfs:comment>expenditure on research and development</rdfs:comment>
    <ex:unit>billion US$2010/yr</ex:unit>
  </rdf:Description>
  <rdf:Description rdf:about="http://transience.eu/ontologies/Primary_Energy_Secondary_Energy_Trade">
    <rdf:type rdf:resource="http://www.w3.org/2002/07/owl#Class"/>
    <rdfs:subClassOf rdf:resource="http://transience.eu/ontologies/Variable"/>
    <rdfs:label>Primary Energy|Secondary Energy Trade</rdfs:label>
    <rdfs:comment>trade in secondary energy carriers that cannot be unambiguoulsy mapped to one of the existing primary energy categories (e.g. electricity, hydrogen, fossil synfuels, negative means net exports)</rdfs:comment>
    <ex:unit>EJ/yr</ex:unit>
  </rdf:Description>
  <rdf:Description rdf:about="http://transience.eu/ontologies/Total_Scrap_Non-Ferrous_Metals_Residential_and_Commercial">
    <rdf:type rdf:resource="http://www.w3.org/2002/07/owl#Class"/>
    <rdfs:subClassOf rdf:resource="http://transience.eu/ontologies/Variable"/>
    <rdfs:label>Total Scrap|Non-Ferrous Metals|Residential and Commercial</rdfs:label>
    <rdfs:comment>Total potential of non-ferrous metals scrap material as a result of end of life products (before collection)</rdfs:comment>
    <ex:unit>Mt/yr</ex:unit>
  </rdf:Description>
  <rdf:Description rdf:about="http://transience.eu/ontologies/Materials_Demand_Iron_and_Steel_Transportation">
    <rdf:type rdf:resource="http://www.w3.org/2002/07/owl#Class"/>
    <rdfs:subClassOf rdf:resource="http://transience.eu/ontologies/Variable"/>
    <rdfs:label>Materials Demand|Iron and Steel|Transportation</rdfs:label>
    <rdfs:comment>Iron and steel requirments from a certain end-use sector</rdfs:comment>
    <ex:unit>Mt/yr</ex:unit>
  </rdf:Description>
  <rdf:Description rdf:about="http://transience.eu/ontologies/Investment_Energy_Supply_Electricity_Biomass">
    <rdf:type rdf:resource="http://www.w3.org/2002/07/owl#Class"/>
    <rdfs:subClassOf rdf:resource="http://transience.eu/ontologies/Variable"/>
    <rdfs:label>Investment|Energy Supply|Electricity|Biomass</rdfs:label>
    <rdfs:comment>investments in new power generation for the specified power plant category. If the model features several sub-categories, the total investments should be reported. For plants equipped with CCS, the investment in the capturing equipment should be included but not the one on transport and storage.</rdfs:comment>
    <ex:unit>billion US$2010/yr</ex:unit>
  </rdf:Description>
  <rdf:Description rdf:about="http://transience.eu/ontologies/Expenditure_household_Services_health">
    <rdf:type rdf:resource="http://www.w3.org/2002/07/owl#Class"/>
    <rdfs:subClassOf rdf:resource="http://transience.eu/ontologies/Variable"/>
    <rdfs:label>Expenditure|household|Services|health</rdfs:label>
    <rdfs:comment>expenditure of households for health services.</rdfs:comment>
    <ex:unit>billion US$2010/yr</ex:unit>
  </rdf:Description>
  <rdf:Description rdf:about="http://transience.eu/ontologies/Final_Energy_Residential_Liquids_Electricity">
    <rdf:type rdf:resource="http://www.w3.org/2002/07/owl#Class"/>
    <rdfs:subClassOf rdf:resource="http://transience.eu/ontologies/Variable"/>
    <rdfs:label>Final Energy|Residential|Liquids|Electricity</rdfs:label>
    <rdfs:comment>final energy consumption by the residential sector of liquid efuels ("power-to-liquid")</rdfs:comment>
    <ex:unit>EJ/yr</ex:unit>
  </rdf:Description>
  <rdf:Description rdf:about="http://transience.eu/ontologies/Final_Energy_Residential_and_Commercial">
    <rdf:type rdf:resource="http://www.w3.org/2002/07/owl#Class"/>
    <rdfs:subClassOf rdf:resource="http://transience.eu/ontologies/Variable"/>
    <rdfs:label>Final Energy|Residential and Commercial</rdfs:label>
    <rdfs:comment>final energy consumed in the residential &amp; commercial sector</rdfs:comment>
    <ex:unit>EJ/yr</ex:unit>
  </rdf:Description>
  <rdf:Description rdf:about="http://transience.eu/ontologies/Efficiency_Liquids_Gas_w__CCS">
    <rdf:type rdf:resource="http://www.w3.org/2002/07/owl#Class"/>
    <rdfs:subClassOf rdf:resource="http://transience.eu/ontologies/Variable"/>
    <rdfs:label>Efficiency|Liquids|Gas|w/ CCS</rdfs:label>
    <rdfs:comment>Conversion efficiency (energy content of liquids produced per unit of primary energy input) of a new gas to liquids plant with CCS. The efficiency should refer to the plant type(s) for which capital costs have been reported. If capital cost for more than one plant type has been reported, modellers should report efficiency for the additional plant types by adding variables Efficiency|Liquids|Gas|w/ CCS|2, ... Efficiency|Liquids|Gas|w/ CCS|N (matching the assignment of plant types to technologies in the reporting of capital costs as documented in the comments sheet). </rdfs:comment>
    <ex:unit>%</ex:unit>
  </rdf:Description>
  <rdf:Description rdf:about="http://transience.eu/ontologies/Final_Energy_Industry_Chemicals_Solids_Biomass">
    <rdf:type rdf:resource="http://www.w3.org/2002/07/owl#Class"/>
    <rdfs:subClassOf rdf:resource="http://transience.eu/ontologies/Variable"/>
    <rdfs:label>Final Energy|Industry|Chemicals|Solids|Biomass</rdfs:label>
    <rdfs:comment>Final energy consumption of solid biomass (modern and traditional, including renewable waste) by the chemicals sector</rdfs:comment>
    <ex:unit>EJ/yr</ex:unit>
  </rdf:Description>
  <rdf:Description rdf:about="http://transience.eu/ontologies/Secondary_Energy_Gases">
    <rdf:type rdf:resource="http://www.w3.org/2002/07/owl#Class"/>
    <rdfs:subClassOf rdf:resource="http://transience.eu/ontologies/Variable"/>
    <rdfs:label>Secondary Energy|Gases</rdfs:label>
    <rdfs:comment>total production of gaseous fuels, including natural gas</rdfs:comment>
    <ex:unit>EJ/yr</ex:unit>
  </rdf:Description>
  <rdf:Description rdf:about="http://transience.eu/ontologies/Final_Energy_Residential_and_Commercial_Gases_Electricity">
    <rdf:type rdf:resource="http://www.w3.org/2002/07/owl#Class"/>
    <rdfs:subClassOf rdf:resource="http://transience.eu/ontologies/Variable"/>
    <rdfs:label>Final Energy|Residential and Commercial|Gases|Electricity</rdfs:label>
    <rdfs:comment>final energy consumption by the residential &amp; commercial sector of synthetic e-fuel gas ("power-to-gas"), excluding transmission/distribution losses</rdfs:comment>
    <ex:unit>EJ/yr</ex:unit>
  </rdf:Description>
  <rdf:Description rdf:about="http://transience.eu/ontologies/Investment">
    <rdf:type rdf:resource="http://www.w3.org/2002/07/owl#Class"/>
    <rdfs:subClassOf rdf:resource="http://transience.eu/ontologies/Variable"/>
    <rdfs:label>Investment</rdfs:label>
    <rdfs:comment>Total economy wide investments (macroecomic capital stock, energy system, R&amp;D, ...) </rdfs:comment>
    <ex:unit>billion US$2010/yr</ex:unit>
  </rdf:Description>
  <rdf:Description rdf:about="http://transience.eu/ontologies/Capital_Cost_Hydrogen_Biomass_w__CCS">
    <rdf:type rdf:resource="http://www.w3.org/2002/07/owl#Class"/>
    <rdfs:subClassOf rdf:resource="http://transience.eu/ontologies/Variable"/>
    <rdfs:label>Capital Cost|Hydrogen|Biomass|w/ CCS</rdfs:label>
    <rdfs:comment>Capital cost of a new biomass to hydrogen plant with CCS. If more than one CCS biomass to hydrogen technology is modelled, modellers should report capital costs for each represented CCS biomass to hydrogen technology by adding variables Capital Cost|Hydrogen|Biomass|w/ CCS|2, ... Capital Cost|Hydrogen|Biomass|w/ CCS|N (with N = number of represented technologies). It is modeller's choice which CCS biomass to hydrogen technologies to assign to type 1 (assigned to the variable without number suffix),2,...,N. The assignment should be documented in the comments sheet. </rdfs:comment>
    <ex:unit>US$2010/kW</ex:unit>
  </rdf:Description>
  <rdf:Description rdf:about="http://transience.eu/ontologies/Final_Energy_Industry_Other_Sector_Liquids_Fossil">
    <rdf:type rdf:resource="http://www.w3.org/2002/07/owl#Class"/>
    <rdfs:subClassOf rdf:resource="http://transience.eu/ontologies/Variable"/>
    <rdfs:label>Final Energy|Industry|Other Sector|Liquids|Fossil</rdfs:label>
    <rdfs:comment>Final energy consumption of liquids of fossil origin by other industry sectors</rdfs:comment>
    <ex:unit>EJ/yr</ex:unit>
  </rdf:Description>
  <rdf:Description rdf:about="http://transience.eu/ontologies/Primary_Energy_Gas_Electricity_w__CCS">
    <rdf:type rdf:resource="http://www.w3.org/2002/07/owl#Class"/>
    <rdfs:subClassOf rdf:resource="http://transience.eu/ontologies/Variable"/>
    <rdfs:label>Primary Energy|Gas|Electricity|w/ CCS</rdfs:label>
    <rdfs:comment>gas primary energy input to electricity generation used in combination with CCS</rdfs:comment>
    <ex:unit>EJ/yr</ex:unit>
  </rdf:Description>
  <rdf:Description rdf:about="http://transience.eu/ontologies/Price_Final_Energy_Residential_Gases_Biomass">
    <rdf:type rdf:resource="http://www.w3.org/2002/07/owl#Class"/>
    <rdfs:subClassOf rdf:resource="http://transience.eu/ontologies/Variable"/>
    <rdfs:label>Price|Final Energy|Residential|Gases|Biomass</rdfs:label>
    <rdfs:comment>biogas price at the final level in the residential sector. Prices should include the effect of carbon prices.</rdfs:comment>
    <ex:unit>US$2010/GJ</ex:unit>
  </rdf:Description>
  <rdf:Description rdf:about="http://transience.eu/ontologies/Total_Scrap_Non-Ferrous_Metals_Transportation">
    <rdf:type rdf:resource="http://www.w3.org/2002/07/owl#Class"/>
    <rdfs:subClassOf rdf:resource="http://transience.eu/ontologies/Variable"/>
    <rdfs:label>Total Scrap|Non-Ferrous Metals|Transportation</rdfs:label>
    <rdfs:comment>Total potential of non-ferrous metals scrap material as a result of end of life products (before collection)</rdfs:comment>
    <ex:unit>Mt/yr</ex:unit>
  </rdf:Description>
  <rdf:Description rdf:about="http://transience.eu/ontologies/Secondary_Energy_Gases_Coal">
    <rdf:type rdf:resource="http://www.w3.org/2002/07/owl#Class"/>
    <rdfs:subClassOf rdf:resource="http://transience.eu/ontologies/Variable"/>
    <rdfs:label>Secondary Energy|Gases|Coal</rdfs:label>
    <rdfs:comment>total production of coal gas from coal gasification</rdfs:comment>
    <ex:unit>EJ/yr</ex:unit>
  </rdf:Description>
  <rdf:Description rdf:about="http://transience.eu/ontologies/Consumption_change_demand_sectors">
    <rdf:type rdf:resource="http://www.w3.org/2002/07/owl#Class"/>
    <rdfs:subClassOf rdf:resource="http://transience.eu/ontologies/ParameterInput"/>
    <rdfs:label>Consumption change|[demand sectors]</rdfs:label>
    <rdfs:comment>Consumption changeÂ </rdfs:comment>
    <ex:unit>%</ex:unit>
  </rdf:Description>
  <rdf:Description rdf:about="http://transience.eu/ontologies/Secondary_Energy_Hydrogen_Gas">
    <rdf:type rdf:resource="http://www.w3.org/2002/07/owl#Class"/>
    <rdfs:subClassOf rdf:resource="http://transience.eu/ontologies/Variable"/>
    <rdfs:label>Secondary Energy|Hydrogen|Gas</rdfs:label>
    <rdfs:comment>hydrogen production from gas</rdfs:comment>
    <ex:unit>EJ/yr</ex:unit>
  </rdf:Description>
  <rdf:Description rdf:about="http://transience.eu/ontologies/Final_Energy_Commercial_Solids_Biomass_Traditional">
    <rdf:type rdf:resource="http://www.w3.org/2002/07/owl#Class"/>
    <rdfs:subClassOf rdf:resource="http://transience.eu/ontologies/Variable"/>
    <rdfs:label>Final Energy|Commercial|Solids|Biomass|Traditional</rdfs:label>
    <rdfs:comment>final energy traditional biomass consumption by the commercial sector</rdfs:comment>
    <ex:unit>EJ/yr</ex:unit>
  </rdf:Description>
  <rdf:Description rdf:about="http://transience.eu/ontologies/Trade_Secondary_Energy_Liquids_Oil_Value">
    <rdf:type rdf:resource="http://www.w3.org/2002/07/owl#Class"/>
    <rdfs:subClassOf rdf:resource="http://transience.eu/ontologies/Variable"/>
    <rdfs:label>Trade|Secondary Energy|Liquids|Oil|Value</rdfs:label>
    <rdfs:comment>value of net exports of liquid fuels from petroleum including both conventional and unconventional sources, at the global level these should add up to the trade losses only</rdfs:comment>
    <ex:unit>EJ/yr</ex:unit>
  </rdf:Description>
  <rdf:Description rdf:about="http://transience.eu/ontologies/Final_Energy_Industry_Steel_Hydrogen">
    <rdf:type rdf:resource="http://www.w3.org/2002/07/owl#Class"/>
    <rdfs:subClassOf rdf:resource="http://transience.eu/ontologies/Variable"/>
    <rdfs:label>Final Energy|Industry|Steel|Hydrogen</rdfs:label>
    <rdfs:comment>Final energy. System boundaries in line with energy accounting</rdfs:comment>
    <ex:unit>PJ/yr</ex:unit>
  </rdf:Description>
  <rdf:Description rdf:about="http://transience.eu/ontologies/Final_Energy_Industry_Non-Ferrous_Metals_Solids_Coal">
    <rdf:type rdf:resource="http://www.w3.org/2002/07/owl#Class"/>
    <rdfs:subClassOf rdf:resource="http://transience.eu/ontologies/Variable"/>
    <rdfs:label>Final Energy|Industry|Non-Ferrous Metals|Solids|Coal</rdfs:label>
    <rdfs:comment>Final energy consumption of coal by the non-ferrous metals sector</rdfs:comment>
    <ex:unit>EJ/yr</ex:unit>
  </rdf:Description>
  <rdf:Description rdf:about="http://transience.eu/ontologies/Final_Energy_Non-Energy_Use_Chemicals_Solids_Coal">
    <rdf:type rdf:resource="http://www.w3.org/2002/07/owl#Class"/>
    <rdfs:subClassOf rdf:resource="http://transience.eu/ontologies/Variable"/>
    <rdfs:label>Final Energy|Non-Energy Use|Chemicals|Solids|Coal</rdfs:label>
    <rdfs:comment>Final energy consumption of coal by the chemical sector by the non-combustion processes</rdfs:comment>
    <ex:unit>EJ/yr</ex:unit>
  </rdf:Description>
  <rdf:Description rdf:about="http://transience.eu/ontologies/Carbon_Capture_Biomass">
    <rdf:type rdf:resource="http://www.w3.org/2002/07/owl#Class"/>
    <rdfs:subClassOf rdf:resource="http://transience.eu/ontologies/Variable"/>
    <rdfs:label>Carbon Capture|Biomass</rdfs:label>
    <rdfs:comment>total carbon dioxide emissions captured  from bioenergy use, should be reported as positive numbers</rdfs:comment>
    <ex:unit>Mt CO2/yr</ex:unit>
  </rdf:Description>
  <rdf:Description rdf:about="http://transience.eu/ontologies/Emissions_CO2">
    <rdf:type rdf:resource="http://www.w3.org/2002/07/owl#Class"/>
    <rdfs:subClassOf rdf:resource="http://transience.eu/ontologies/Variable"/>
    <rdfs:label>Emissions|CO2</rdfs:label>
    <rdfs:comment>total CO2 emissions</rdfs:comment>
    <ex:unit>Mt CO2/yr</ex:unit>
  </rdf:Description>
  <rdf:Description rdf:about="http://transience.eu/ontologies/Capital_Cost_Electricity_Wind_Onshore">
    <rdf:type rdf:resource="http://www.w3.org/2002/07/owl#Class"/>
    <rdfs:subClassOf rdf:resource="http://transience.eu/ontologies/Variable"/>
    <rdfs:label>Capital Cost|Electricity|Wind|Onshore</rdfs:label>
    <rdfs:comment>Capital cost of a new onshore wind power plants. This variable should only be filled, if wind power is separated into onshore and offshore. If more than one onshore wind power technology is modelled (e.g., wind power units with different hub height and capacity), modellers should report capital costs for each represented wind power technology by adding variables Capital Cost|Electricity|Wind|Onshore|2, ... Capital|Cost|Electricity|Wind|Onshore|N (with N = number of represented onshore wind power technologies). It is modeller's choice which onshore wind power technologies to assign to type 1 (assigned to the variable without number suffix),2,...,N. The assignment should be documented in the comments sheet. </rdfs:comment>
    <ex:unit>US$2010/kW</ex:unit>
  </rdf:Description>
  <rdf:Description rdf:about="http://transience.eu/ontologies/Secondary_Energy_Heat_Other">
    <rdf:type rdf:resource="http://www.w3.org/2002/07/owl#Class"/>
    <rdfs:subClassOf rdf:resource="http://transience.eu/ontologies/Variable"/>
    <rdfs:label>Secondary Energy|Heat|Other</rdfs:label>
    <rdfs:comment>centralized heat generation from sources that do not fit any other category (please provide a definition of the sources in this category in the 'comments' tab)</rdfs:comment>
    <ex:unit>EJ/yr</ex:unit>
  </rdf:Description>
  <rdf:Description rdf:about="http://transience.eu/ontologies/Trade_Emissions_Allowances_Volume">
    <rdf:type rdf:resource="http://www.w3.org/2002/07/owl#Class"/>
    <rdfs:subClassOf rdf:resource="http://transience.eu/ontologies/Variable"/>
    <rdfs:label>Trade|Emissions Allowances|Volume</rdfs:label>
    <rdfs:comment>physical trade volume in GHG emission allowances</rdfs:comment>
    <ex:unit>Mt CO2-equiv/yr</ex:unit>
  </rdf:Description>
  <rdf:Description rdf:about="http://transience.eu/ontologies/Final_Energy_Transportation_Other">
    <rdf:type rdf:resource="http://www.w3.org/2002/07/owl#Class"/>
    <rdfs:subClassOf rdf:resource="http://transience.eu/ontologies/Variable"/>
    <rdfs:label>Final Energy|Transportation|Other</rdfs:label>
    <rdfs:comment>final energy consumption by the transportation sector of other sources that do not fit to any other category (please provide a definition of the sources in this category in the 'comments' tab)</rdfs:comment>
    <ex:unit>EJ/yr</ex:unit>
  </rdf:Description>
  <rdf:Description rdf:about="http://transience.eu/ontologies/Final_Energy_Industry_Chemicals_Gases_Electricity">
    <rdf:type rdf:resource="http://www.w3.org/2002/07/owl#Class"/>
    <rdfs:subClassOf rdf:resource="http://transience.eu/ontologies/Variable"/>
    <rdfs:label>Final Energy|Industry|Chemicals|Gases|Electricity</rdfs:label>
    <rdfs:comment>Final energy consumption of synthetic e-fuel gas ("power-to-gas") by the chemicals sector</rdfs:comment>
    <ex:unit>EJ/yr</ex:unit>
  </rdf:Description>
  <rdf:Description rdf:about="http://transience.eu/ontologies/Primary_Energy_Hydro">
    <rdf:type rdf:resource="http://www.w3.org/2002/07/owl#Class"/>
    <rdfs:subClassOf rdf:resource="http://transience.eu/ontologies/Variable"/>
    <rdfs:label>Primary Energy|Hydro</rdfs:label>
    <rdfs:comment>total hydro primary energy consumption</rdfs:comment>
    <ex:unit>EJ/yr</ex:unit>
  </rdf:Description>
  <rdf:Description rdf:about="http://transience.eu/ontologies/Export_Industry_Non-Ferrous_Metals_Volume">
    <rdf:type rdf:resource="http://www.w3.org/2002/07/owl#Class"/>
    <rdfs:subClassOf rdf:resource="http://transience.eu/ontologies/Variable"/>
    <rdfs:label>Export|Industry|Non-Ferrous Metals|Volume</rdfs:label>
    <rdfs:comment>Export of non-ferrous metals</rdfs:comment>
    <ex:unit>Mt/yr</ex:unit>
  </rdf:Description>
  <rdf:Description rdf:about="http://transience.eu/ontologies/Energy_Service_Transportation_Freight_Road">
    <rdf:type rdf:resource="http://www.w3.org/2002/07/owl#Class"/>
    <rdfs:subClassOf rdf:resource="http://transience.eu/ontologies/Variable"/>
    <rdfs:label>Energy Service|Transportation|Freight|Road</rdfs:label>
    <rdfs:comment>energy service demand for freight transport on roads</rdfs:comment>
    <ex:unit>bn tkm/yr</ex:unit>
  </rdf:Description>
  <rdf:Description rdf:about="http://transience.eu/ontologies/Secondary_Energy_Hydrogen_Gas_w__CCS">
    <rdf:type rdf:resource="http://www.w3.org/2002/07/owl#Class"/>
    <rdfs:subClassOf rdf:resource="http://transience.eu/ontologies/Variable"/>
    <rdfs:label>Secondary Energy|Hydrogen|Gas|w/ CCS</rdfs:label>
    <rdfs:comment>hydrogen production from natural gas with a CO2 capture component</rdfs:comment>
    <ex:unit>EJ/yr</ex:unit>
  </rdf:Description>
  <rdf:Description rdf:about="http://transience.eu/ontologies/Production_Iron_and_Steel_Secondary_Steel_Volume">
    <rdf:type rdf:resource="http://www.w3.org/2002/07/owl#Class"/>
    <rdfs:subClassOf rdf:resource="http://transience.eu/ontologies/Variable"/>
    <rdfs:label>Production|Iron and Steel|Secondary Steel|Volume</rdfs:label>
    <rdfs:comment>Production of secondary steel from recycling of scrap</rdfs:comment>
    <ex:unit>Mt/yr</ex:unit>
  </rdf:Description>
  <rdf:Description rdf:about="http://transience.eu/ontologies/Outflow_Cars_car_types">
    <rdf:type rdf:resource="http://www.w3.org/2002/07/owl#Class"/>
    <rdfs:subClassOf rdf:resource="http://transience.eu/ontologies/Variable"/>
    <rdfs:label>Outflow|Cars|[car types]</rdfs:label>
    <rdfs:comment>Car outflow</rdfs:comment>
    <ex:unit>cars/yr</ex:unit>
  </rdf:Description>
  <rdf:Description rdf:about="http://transience.eu/ontologies/Export">
    <rdf:type rdf:resource="http://www.w3.org/2002/07/owl#Class"/>
    <rdfs:subClassOf rdf:resource="http://transience.eu/ontologies/Variable"/>
    <rdfs:label>Export</rdfs:label>
    <rdfs:comment>total exports measured in monetary quantities.</rdfs:comment>
    <ex:unit>billion US$2010/yr</ex:unit>
  </rdf:Description>
  <rdf:Description rdf:about="http://transience.eu/ontologies/Resource_use_Plastic_Waste_Industry_Petrochemicals">
    <rdf:type rdf:resource="http://www.w3.org/2002/07/owl#Class"/>
    <rdfs:subClassOf rdf:resource="http://transience.eu/ontologies/Variable"/>
    <rdfs:label>Resource use|Plastic Waste|Industry|Petrochemicals</rdfs:label>
    <rdfs:comment>Use of plastic waste for non-energetic use including energetic use of by-products; C-content</rdfs:comment>
    <ex:unit>Mt C_eq/yr</ex:unit>
  </rdf:Description>
  <rdf:Description rdf:about="http://transience.eu/ontologies/Collected_Scrap_Non-Ferrous_Metals_Other">
    <rdf:type rdf:resource="http://www.w3.org/2002/07/owl#Class"/>
    <rdfs:subClassOf rdf:resource="http://transience.eu/ontologies/Variable"/>
    <rdfs:label>Collected Scrap|Non-Ferrous Metals|Other</rdfs:label>
    <rdfs:comment>Collected non-ferrous metals scrap coming from other sectors (available to be used in recycling)</rdfs:comment>
    <ex:unit>Mt/yr</ex:unit>
  </rdf:Description>
  <rdf:Description rdf:about="http://transience.eu/ontologies/Lifetime_Liquids_Gas_w__CCS">
    <rdf:type rdf:resource="http://www.w3.org/2002/07/owl#Class"/>
    <rdfs:subClassOf rdf:resource="http://transience.eu/ontologies/Variable"/>
    <rdfs:label>Lifetime|Liquids|Gas|w/ CCS</rdfs:label>
    <rdfs:comment>Lifetime of a new gas to liquids plant with CCS. Lifetime should be calculated by summing all vintages of a  capacity unit (e.g. (1+1+0.9+0.7+0.5) * 10 years = 41 years) or by the e-folding time for exponential capacity depreciation.  The lifetime should refer to the plant type(s) for which capital costs have been reported. If capital cost for more than one plant type has been reported, modellers should report lifetime for the additional plant types by adding variables Lifetime|Liquids|Gas|w/ CCS|2, ... Lifetime|Liquids|Gas|w/ CCS|N (matching the assignment of plant types to technologies in the reporting of capital costs as documented in the comments sheet). </rdfs:comment>
    <ex:unit>years</ex:unit>
  </rdf:Description>
  <rdf:Description rdf:about="http://transience.eu/ontologies/Final_Energy_Transportation_Liquids_Fossil">
    <rdf:type rdf:resource="http://www.w3.org/2002/07/owl#Class"/>
    <rdfs:subClassOf rdf:resource="http://transience.eu/ontologies/Variable"/>
    <rdfs:label>Final Energy|Transportation|Liquids|Fossil</rdfs:label>
    <rdfs:comment>final energy consumption by the transportation sector of fossil based liquids (from conventional &amp; unconventional oil, coal-to-liquids, gas-to-liquids)</rdfs:comment>
    <ex:unit>EJ/yr</ex:unit>
  </rdf:Description>
  <rdf:Description rdf:about="http://transience.eu/ontologies/Carbon_Capture_Usage_Other">
    <rdf:type rdf:resource="http://www.w3.org/2002/07/owl#Class"/>
    <rdfs:subClassOf rdf:resource="http://transience.eu/ontologies/Variable"/>
    <rdfs:label>Carbon Capture|Usage|Other</rdfs:label>
    <rdfs:comment>total carbon dioxide captured and used in other short-lived products</rdfs:comment>
    <ex:unit>Mt CO2/yr</ex:unit>
  </rdf:Description>
  <rdf:Description rdf:about="http://transience.eu/ontologies/Investment_Energy_Supply_Electricity_Transmission_and_Distribution">
    <rdf:type rdf:resource="http://www.w3.org/2002/07/owl#Class"/>
    <rdfs:subClassOf rdf:resource="http://transience.eu/ontologies/Variable"/>
    <rdfs:label>Investment|Energy Supply|Electricity|Transmission and Distribution</rdfs:label>
    <rdfs:comment>investments in transmission and distribution of power generation</rdfs:comment>
    <ex:unit>billion US$2010/yr</ex:unit>
  </rdf:Description>
  <rdf:Description rdf:about="http://transience.eu/ontologies/Carbon_Capture_Direct_Air_Capture">
    <rdf:type rdf:resource="http://www.w3.org/2002/07/owl#Class"/>
    <rdfs:subClassOf rdf:resource="http://transience.eu/ontologies/Variable"/>
    <rdfs:label>Carbon Capture|Direct Air Capture</rdfs:label>
    <rdfs:comment>total carbon dioxide captured through direct air capture</rdfs:comment>
    <ex:unit>Mt CO2/yr</ex:unit>
  </rdf:Description>
  <rdf:Description rdf:about="http://transience.eu/ontologies/Primary_Energy_Coal">
    <rdf:type rdf:resource="http://www.w3.org/2002/07/owl#Class"/>
    <rdfs:subClassOf rdf:resource="http://transience.eu/ontologies/Variable"/>
    <rdfs:label>Primary Energy|Coal</rdfs:label>
    <rdfs:comment>coal primary energy consumption</rdfs:comment>
    <ex:unit>EJ/yr</ex:unit>
  </rdf:Description>
  <rdf:Description rdf:about="http://transience.eu/ontologies/Production_Non-Metallic_Minerals_Clinker_Volume">
    <rdf:type rdf:resource="http://www.w3.org/2002/07/owl#Class"/>
    <rdfs:subClassOf rdf:resource="http://transience.eu/ontologies/Variable"/>
    <rdfs:label>Production|Non-Metallic Minerals|Clinker|Volume</rdfs:label>
    <rdfs:comment>production of clinker (intermediate material for the production of cement)</rdfs:comment>
    <ex:unit>Mt/yr</ex:unit>
  </rdf:Description>
  <rdf:Description rdf:about="http://transience.eu/ontologies/Import_Industry_Iron_and_Steel_Secondary_Steel">
    <rdf:type rdf:resource="http://www.w3.org/2002/07/owl#Class"/>
    <rdfs:subClassOf rdf:resource="http://transience.eu/ontologies/Variable"/>
    <rdfs:label>Import|Industry|Iron and Steel|Secondary Steel</rdfs:label>
    <rdfs:comment>Import of secondary steel measured in monetary units</rdfs:comment>
    <ex:unit>billion US$2010/yr</ex:unit>
  </rdf:Description>
  <rdf:Description rdf:about="http://transience.eu/ontologies/Collected_Scrap_Iron_and_Steel">
    <rdf:type rdf:resource="http://www.w3.org/2002/07/owl#Class"/>
    <rdfs:subClassOf rdf:resource="http://transience.eu/ontologies/Variable"/>
    <rdfs:label>Collected Scrap|Iron and Steel</rdfs:label>
    <rdfs:comment>Collected iron and steel scrap</rdfs:comment>
    <ex:unit>Mt/yr</ex:unit>
  </rdf:Description>
  <rdf:Description rdf:about="http://transience.eu/ontologies/Secondary_Energy_Electricity_Coal">
    <rdf:type rdf:resource="http://www.w3.org/2002/07/owl#Class"/>
    <rdfs:subClassOf rdf:resource="http://transience.eu/ontologies/Variable"/>
    <rdfs:label>Secondary Energy|Electricity|Coal</rdfs:label>
    <rdfs:comment>net electricity production from coal</rdfs:comment>
    <ex:unit>EJ/yr</ex:unit>
  </rdf:Description>
  <rdf:Description rdf:about="http://transience.eu/ontologies/Secondary_Energy_Gases_Fossil">
    <rdf:type rdf:resource="http://www.w3.org/2002/07/owl#Class"/>
    <rdfs:subClassOf rdf:resource="http://transience.eu/ontologies/Variable"/>
    <rdfs:label>Secondary Energy|Gases|Fossil</rdfs:label>
    <rdfs:comment>total production of gas from fossils</rdfs:comment>
    <ex:unit>EJ/yr</ex:unit>
  </rdf:Description>
  <rdf:Description rdf:about="http://transience.eu/ontologies/Production_Petrochemicals_Methanol">
    <rdf:type rdf:resource="http://www.w3.org/2002/07/owl#Class"/>
    <rdfs:subClassOf rdf:resource="http://transience.eu/ontologies/Variable"/>
    <rdfs:label>Production|Petrochemicals|Methanol</rdfs:label>
    <rdfs:comment>Production of methanol (intermediary production for HVC)</rdfs:comment>
    <ex:unit>Mt/yr</ex:unit>
  </rdf:Description>
  <rdf:Description rdf:about="http://transience.eu/ontologies/Final_Energy_Industry_Pulp_and_Paper_Liquids_Fossil">
    <rdf:type rdf:resource="http://www.w3.org/2002/07/owl#Class"/>
    <rdfs:subClassOf rdf:resource="http://transience.eu/ontologies/Variable"/>
    <rdfs:label>Final Energy|Industry|Pulp and Paper|Liquids|Fossil</rdfs:label>
    <rdfs:comment>Final energy consumption of liquids of fossil origin by the pulp and paper sector</rdfs:comment>
    <ex:unit>EJ/yr</ex:unit>
  </rdf:Description>
  <rdf:Description rdf:about="http://transience.eu/ontologies/Final_Energy_Industry_Iron_and_Steel_Gases_Biomass">
    <rdf:type rdf:resource="http://www.w3.org/2002/07/owl#Class"/>
    <rdfs:subClassOf rdf:resource="http://transience.eu/ontologies/Variable"/>
    <rdfs:label>Final Energy|Industry|Iron and Steel|Gases|Biomass</rdfs:label>
    <rdfs:comment>Final energy consumption of biogas by the iron and steel sector</rdfs:comment>
    <ex:unit>EJ/yr</ex:unit>
  </rdf:Description>
  <rdf:Description rdf:about="http://transience.eu/ontologies/Production_Non-Metallic_Minerals_Volume">
    <rdf:type rdf:resource="http://www.w3.org/2002/07/owl#Class"/>
    <rdfs:subClassOf rdf:resource="http://transience.eu/ontologies/Variable"/>
    <rdfs:label>Production|Non-Metallic Minerals|Volume</rdfs:label>
    <rdfs:comment>production of non-metallic minerals, which include cement, ceramic, glass, lime</rdfs:comment>
    <ex:unit>Mt/yr</ex:unit>
  </rdf:Description>
  <rdf:Description rdf:about="http://transience.eu/ontologies/Trade_Secondary_Energy_Liquids_Gas_Value">
    <rdf:type rdf:resource="http://www.w3.org/2002/07/owl#Class"/>
    <rdfs:subClassOf rdf:resource="http://transience.eu/ontologies/Variable"/>
    <rdfs:label>Trade|Secondary Energy|Liquids|Gas|Value</rdfs:label>
    <rdfs:comment>value of net exports of fossil liquid synfuels from gas-to-liquids (GTL) technologies, at the global level these should add up to the trade losses only</rdfs:comment>
    <ex:unit>EJ/yr</ex:unit>
  </rdf:Description>
  <rdf:Description rdf:about="http://transience.eu/ontologies/Carbon_Capture_Usage_Liquids">
    <rdf:type rdf:resource="http://www.w3.org/2002/07/owl#Class"/>
    <rdfs:subClassOf rdf:resource="http://transience.eu/ontologies/Variable"/>
    <rdfs:label>Carbon Capture|Usage|Liquids</rdfs:label>
    <rdfs:comment>total carbon dioxide captured and used in synthetic liquids (e.g. as feedstock in industry or for synthetic fuels)</rdfs:comment>
    <ex:unit>Mt CO2/yr</ex:unit>
  </rdf:Description>
  <rdf:Description rdf:about="http://transience.eu/ontologies/Import_Industry_Chemicals_High_Value_Chemicals">
    <rdf:type rdf:resource="http://www.w3.org/2002/07/owl#Class"/>
    <rdfs:subClassOf rdf:resource="http://transience.eu/ontologies/Variable"/>
    <rdfs:label>Import|Industry|Chemicals|High Value Chemicals</rdfs:label>
    <rdfs:comment>Import of high value chemicals measured in monetary units</rdfs:comment>
    <ex:unit>billion US$2010/yr</ex:unit>
  </rdf:Description>
  <rdf:Description rdf:about="http://transience.eu/ontologies/Energy_Use_Industry_Petrochemicals_Biomass">
    <rdf:type rdf:resource="http://www.w3.org/2002/07/owl#Class"/>
    <rdfs:subClassOf rdf:resource="http://transience.eu/ontologies/Variable"/>
    <rdfs:label>Energy Use|Industry|Petrochemicals|Biomass</rdfs:label>
    <rdfs:comment>Use of biomass, including both, non-energetic use and energetic use of by-products of biomass processing</rdfs:comment>
    <ex:unit>Mt/yr</ex:unit>
  </rdf:Description>
  <rdf:Description rdf:about="http://transience.eu/ontologies/Investment_Energy_Supply_Electricity_Solar">
    <rdf:type rdf:resource="http://www.w3.org/2002/07/owl#Class"/>
    <rdfs:subClassOf rdf:resource="http://transience.eu/ontologies/Variable"/>
    <rdfs:label>Investment|Energy Supply|Electricity|Solar</rdfs:label>
    <rdfs:comment>investments in new power generation for the specified power plant category. If the model features several sub-categories, the total investments should be reported. For plants equipped with CCS, the investment in the capturing equipment should be included but not the one on transport and storage.</rdfs:comment>
    <ex:unit>billion US$2010/yr</ex:unit>
  </rdf:Description>
  <rdf:Description rdf:about="http://transience.eu/ontologies/Final_Energy_Non-Energy_Use">
    <rdf:type rdf:resource="http://www.w3.org/2002/07/owl#Class"/>
    <rdfs:subClassOf rdf:resource="http://transience.eu/ontologies/Variable"/>
    <rdfs:label>Final Energy|Non-Energy Use</rdfs:label>
    <rdfs:comment>final energy consumption by the non-combustion processes</rdfs:comment>
    <ex:unit>EJ/yr</ex:unit>
  </rdf:Description>
  <rdf:Description rdf:about="http://transience.eu/ontologies/Lifetime_Liquids_Biomass_w__CCS">
    <rdf:type rdf:resource="http://www.w3.org/2002/07/owl#Class"/>
    <rdfs:subClassOf rdf:resource="http://transience.eu/ontologies/Variable"/>
    <rdfs:label>Lifetime|Liquids|Biomass|w/ CCS</rdfs:label>
    <rdfs:comment>Lifetime of a new biomass to liquids plant with CCS. Lifetime should be calculated by summing all vintages of a  capacity unit (e.g. (1+1+0.9+0.7+0.5) * 10 years = 41 years) or by the e-folding time for exponential capacity depreciation.  The lifetime should refer to the plant type(s) for which capital costs have been reported. If capital cost for more than one plant type has been reported, modellers should report lifetime for the additional plant types by adding variables Lifetime|Liquids|Biomass|w/ CCS|2, ... Lifetime|Liquids|Biomass|w/ CCS|N (matching the assignment of plant types to technologies in the reporting of capital costs as documented in the comments sheet). </rdfs:comment>
    <ex:unit>years</ex:unit>
  </rdf:Description>
  <rdf:Description rdf:about="http://transience.eu/ontologies/Price_Final_Energy_Industry_Electricity">
    <rdf:type rdf:resource="http://www.w3.org/2002/07/owl#Class"/>
    <rdfs:subClassOf rdf:resource="http://transience.eu/ontologies/Variable"/>
    <rdfs:label>Price|Final Energy|Industry|Electricity</rdfs:label>
    <rdfs:comment>electricity price at the final level in the industry sector. Prices should include the effect of carbon prices.</rdfs:comment>
    <ex:unit>US$2010/GJ</ex:unit>
  </rdf:Description>
  <rdf:Description rdf:about="http://transience.eu/ontologies/Final_Energy_Residential_Heat">
    <rdf:type rdf:resource="http://www.w3.org/2002/07/owl#Class"/>
    <rdfs:subClassOf rdf:resource="http://transience.eu/ontologies/Variable"/>
    <rdfs:label>Final Energy|Residential|Heat</rdfs:label>
    <rdfs:comment>final energy consumption by the residential sector of heat (e.g., district heat, process heat, solar heating and warm water), excluding transmission/distribution losses</rdfs:comment>
    <ex:unit>EJ/yr</ex:unit>
  </rdf:Description>
  <rdf:Description rdf:about="http://transience.eu/ontologies/Expenditure_Household">
    <rdf:type rdf:resource="http://www.w3.org/2002/07/owl#Class"/>
    <rdfs:subClassOf rdf:resource="http://transience.eu/ontologies/Variable"/>
    <rdfs:label>Expenditure|Household</rdfs:label>
    <rdfs:comment>Total household expenditure</rdfs:comment>
    <ex:unit>billion US$2010/yr</ex:unit>
  </rdf:Description>
  <rdf:Description rdf:about="http://transience.eu/ontologies/Carbon_Capture_Industrial_Processes">
    <rdf:type rdf:resource="http://www.w3.org/2002/07/owl#Class"/>
    <rdfs:subClassOf rdf:resource="http://transience.eu/ontologies/Variable"/>
    <rdfs:label>Carbon Capture|Industrial Processes</rdfs:label>
    <rdfs:comment>total carbon dioxide emissions captured from industrial processes (e.g., cement production, but not from fossil fuel burning) use, should be reported as positive numbers</rdfs:comment>
    <ex:unit>Mt CO2/yr</ex:unit>
  </rdf:Description>
  <rdf:Description rdf:about="http://transience.eu/ontologies/Capital_Cost_Liquids_Biomass_w__CCS">
    <rdf:type rdf:resource="http://www.w3.org/2002/07/owl#Class"/>
    <rdfs:subClassOf rdf:resource="http://transience.eu/ontologies/Variable"/>
    <rdfs:label>Capital Cost|Liquids|Biomass|w/ CCS</rdfs:label>
    <rdfs:comment>Capital cost of a new biomass to liquids plant with CCS. If more than one CCS BTL technology is modelled, modellers should report capital costs for each represented CCS BTL technology by adding variables Capital Cost|Liquids|Biomass|w/ CCS|2, ... Capital Cost|Liquids|Biomass|w/ CCS|N (with N = number of represented technologies). It is modeller's choice which CCS BTL technologies to assign to type 1 (assigned to the variable without number suffix),2,...,N. The assignment should be documented in the comments sheet. </rdfs:comment>
    <ex:unit>US$2010/kW</ex:unit>
  </rdf:Description>
  <rdf:Description rdf:about="http://transience.eu/ontologies/Primary_Energy_Oil">
    <rdf:type rdf:resource="http://www.w3.org/2002/07/owl#Class"/>
    <rdfs:subClassOf rdf:resource="http://transience.eu/ontologies/Variable"/>
    <rdfs:label>Primary Energy|Oil</rdfs:label>
    <rdfs:comment>conventional &amp; unconventional oil primary energy consumption</rdfs:comment>
    <ex:unit>EJ/yr</ex:unit>
  </rdf:Description>
  <rdf:Description rdf:about="http://transience.eu/ontologies/Capital_Cost_Gases_Biomass_w_o_CCS">
    <rdf:type rdf:resource="http://www.w3.org/2002/07/owl#Class"/>
    <rdfs:subClassOf rdf:resource="http://transience.eu/ontologies/Variable"/>
    <rdfs:label>Capital Cost|Gases|Biomass|w/o CCS</rdfs:label>
    <rdfs:comment>Capital cost of a new biomass to gas plant w/o CCS. If more than one biomass to gas technology is modelled, modellers should report capital costs for each represented biomass to gas technology by adding variables Capital Cost|Gases|Biomass|w/o CCS|2, ... Capital Cost|Gases|Biomass|w/o CCS|N (with N = number of represented technologies). It is modeller's choice which biomass to gas technologies to assign to type 1 (assigned to the variable without number suffix),2,...,N. The assignment should be documented in the comments sheet. </rdfs:comment>
    <ex:unit>US$2010/kW</ex:unit>
  </rdf:Description>
  <rdf:Description rdf:about="http://transience.eu/ontologies/Final_Energy_Industry_Chemicals_Liquids_Biomass">
    <rdf:type rdf:resource="http://www.w3.org/2002/07/owl#Class"/>
    <rdfs:subClassOf rdf:resource="http://transience.eu/ontologies/Variable"/>
    <rdfs:label>Final Energy|Industry|Chemicals|Liquids|Biomass</rdfs:label>
    <rdfs:comment>Final energy consumption of liquid biofuels by the chemicals sector</rdfs:comment>
    <ex:unit>EJ/yr</ex:unit>
  </rdf:Description>
  <rdf:Description rdf:about="http://transience.eu/ontologies/Investment_Energy_Supply_Extraction_Gas">
    <rdf:type rdf:resource="http://www.w3.org/2002/07/owl#Class"/>
    <rdfs:subClassOf rdf:resource="http://transience.eu/ontologies/Variable"/>
    <rdfs:label>Investment|Energy Supply|Extraction|Gas</rdfs:label>
    <rdfs:comment>investments for extraction and conversion of natural gas. These should include upstream, LNG chain and transmission and distribution</rdfs:comment>
    <ex:unit>billion US$2010/yr</ex:unit>
  </rdf:Description>
  <rdf:Description rdf:about="http://transience.eu/ontologies/Secondary_Energy_Electricity_Oil_w_o_CCS">
    <rdf:type rdf:resource="http://www.w3.org/2002/07/owl#Class"/>
    <rdfs:subClassOf rdf:resource="http://transience.eu/ontologies/Variable"/>
    <rdfs:label>Secondary Energy|Electricity|Oil|w/o CCS</rdfs:label>
    <rdfs:comment>net electricity production from refined liquids with freely vented CO2 emissions</rdfs:comment>
    <ex:unit>EJ/yr</ex:unit>
  </rdf:Description>
  <rdf:Description rdf:about="http://transience.eu/ontologies/Energy_Service_Bunkers_Passenger_International_Aviation">
    <rdf:type rdf:resource="http://www.w3.org/2002/07/owl#Class"/>
    <rdfs:subClassOf rdf:resource="http://transience.eu/ontologies/Variable"/>
    <rdfs:label>Energy Service|Bunkers|Passenger|International Aviation</rdfs:label>
    <rdfs:comment>energy service demand for passenger transport operating on international aviation routes</rdfs:comment>
    <ex:unit>bn pkm/yr</ex:unit>
  </rdf:Description>
  <rdf:Description rdf:about="http://transience.eu/ontologies/Secondary_Energy_Hydrogen_Biomass_w__CCS">
    <rdf:type rdf:resource="http://www.w3.org/2002/07/owl#Class"/>
    <rdfs:subClassOf rdf:resource="http://transience.eu/ontologies/Variable"/>
    <rdfs:label>Secondary Energy|Hydrogen|Biomass|w/ CCS</rdfs:label>
    <rdfs:comment>hydrogen production from biomass with a CO2 capture component</rdfs:comment>
    <ex:unit>EJ/yr</ex:unit>
  </rdf:Description>
  <rdf:Description rdf:about="http://transience.eu/ontologies/Production_Plastics_Product_categories">
    <rdf:type rdf:resource="http://www.w3.org/2002/07/owl#Class"/>
    <rdfs:subClassOf rdf:resource="http://transience.eu/ontologies/ParameterOutput"/>
    <rdfs:label>Production|Plastics|[Product categories]</rdfs:label>
    <rdfs:comment>Plastics productionÂ </rdfs:comment>
    <ex:unit>t/yr</ex:unit>
  </rdf:Description>
  <rdf:Description rdf:about="http://transience.eu/ontologies/Employment_Industry_Energy_Intensive">
    <rdf:type rdf:resource="http://www.w3.org/2002/07/owl#Class"/>
    <rdfs:subClassOf rdf:resource="http://transience.eu/ontologies/Variable"/>
    <rdfs:label>Employment|Industry|Energy Intensive</rdfs:label>
    <rdfs:comment>Number of employed inhabitants (payrolls) in energy-intensive industry (based on ILO classification)</rdfs:comment>
    <ex:unit>million</ex:unit>
  </rdf:Description>
  <rdf:Description rdf:about="http://transience.eu/ontologies/Import_Industry_Iron_and_Steel">
    <rdf:type rdf:resource="http://www.w3.org/2002/07/owl#Class"/>
    <rdfs:subClassOf rdf:resource="http://transience.eu/ontologies/Variable"/>
    <rdfs:label>Import|Industry|Iron and Steel</rdfs:label>
    <rdfs:comment>Import of iron &amp; steel measured in monetary units</rdfs:comment>
    <ex:unit>billion US$2010/yr</ex:unit>
  </rdf:Description>
  <rdf:Description rdf:about="http://transience.eu/ontologies/Final_Energy_Commercial_Other">
    <rdf:type rdf:resource="http://www.w3.org/2002/07/owl#Class"/>
    <rdfs:subClassOf rdf:resource="http://transience.eu/ontologies/Variable"/>
    <rdfs:label>Final Energy|Commercial|Other</rdfs:label>
    <rdfs:comment>final energy consumption by the commercial sector of other sources that do not fit to any other category (please provide a definition of the sources in this category in the 'comments' tab)</rdfs:comment>
    <ex:unit>EJ/yr</ex:unit>
  </rdf:Description>
  <rdf:Description rdf:about="http://transience.eu/ontologies/Final_Energy_Industry_Pulp_and_Paper_Liquids">
    <rdf:type rdf:resource="http://www.w3.org/2002/07/owl#Class"/>
    <rdfs:subClassOf rdf:resource="http://transience.eu/ontologies/Variable"/>
    <rdfs:label>Final Energy|Industry|Pulp and Paper|Liquids</rdfs:label>
    <rdfs:comment>Final energy consumption of refined liquids of the pulp and paper sector (conventional &amp; unconventional oil, biofuels, coal-to-liquids, gas-to-liquids, efuels)</rdfs:comment>
    <ex:unit>EJ/yr</ex:unit>
  </rdf:Description>
  <rdf:Description rdf:about="http://transience.eu/ontologies/Capital_Cost_Liquids_Gas_w_o_CCS">
    <rdf:type rdf:resource="http://www.w3.org/2002/07/owl#Class"/>
    <rdfs:subClassOf rdf:resource="http://transience.eu/ontologies/Variable"/>
    <rdfs:label>Capital Cost|Liquids|Gas|w/o CCS</rdfs:label>
    <rdfs:comment>Capital cost of a new gas to liquids plant w/o CCS. If more than one GTL technology is modelled, modellers should report capital costs for each represented GTL technology by adding variables Capital Cost|Liquids|Gas|w/o CCS|2, ... Capital Cost|Liquids|Gas|w/o CCS|N (with N = number of represented technologies). It is modeller's choice which GTL technologies to assign to type 1 (assigned to the variable without number suffix),2,...,N. The assignment should be documented in the comments sheet. </rdfs:comment>
    <ex:unit>US$2010/kW</ex:unit>
  </rdf:Description>
  <rdf:Description rdf:about="http://transience.eu/ontologies/Lifetime_Hydrogen_Electricity">
    <rdf:type rdf:resource="http://www.w3.org/2002/07/owl#Class"/>
    <rdfs:subClassOf rdf:resource="http://transience.eu/ontologies/Variable"/>
    <rdfs:label>Lifetime|Hydrogen|Electricity</rdfs:label>
    <rdfs:comment>Lifetime of a new hydrogen-by-electrolysis plant. Lifetime should be calculated by summing all vintages of a  capacity unit (e.g. (1+1+0.9+0.7+0.5) * 10 years = 41 years) or by the e-folding time for exponential capacity depreciation.  The lifetime should refer to the plant type(s) for which capital costs have been reported. If capital cost for more than one plant type has been reported, modellers should report lifetime for the additional plant types by adding variables Lifetime|Hydrogen|Electricity|w/ CCS|2, ... Lifetime|Hydrogen|Electricity|w/ CCS|N (matching the assignment of plant types to technologies in the reporting of capital costs as documented in the comments sheet). </rdfs:comment>
    <ex:unit>years</ex:unit>
  </rdf:Description>
  <rdf:Description rdf:about="http://transience.eu/ontologies/Secondary_Energy_Electricity_Ocean">
    <rdf:type rdf:resource="http://www.w3.org/2002/07/owl#Class"/>
    <rdfs:subClassOf rdf:resource="http://transience.eu/ontologies/Variable"/>
    <rdfs:label>Secondary Energy|Electricity|Ocean</rdfs:label>
    <rdfs:comment>net electricity production from all sources of ocean energy (e.g., tidal, wave, ocean thermal electricity generation)</rdfs:comment>
    <ex:unit>EJ/yr</ex:unit>
  </rdf:Description>
  <rdf:Description rdf:about="http://transience.eu/ontologies/Final_Energy_Carbon_Removal">
    <rdf:type rdf:resource="http://www.w3.org/2002/07/owl#Class"/>
    <rdfs:subClassOf rdf:resource="http://transience.eu/ontologies/Variable"/>
    <rdfs:label>Final Energy|Carbon Removal</rdfs:label>
    <rdfs:comment>Final energy consumption by carbon dioxide removal processes</rdfs:comment>
    <ex:unit>EJ/yr</ex:unit>
  </rdf:Description>
  <rdf:Description rdf:about="http://transience.eu/ontologies/Capital_Cost_Electricity_Geothermal">
    <rdf:type rdf:resource="http://www.w3.org/2002/07/owl#Class"/>
    <rdfs:subClassOf rdf:resource="http://transience.eu/ontologies/Variable"/>
    <rdfs:label>Capital Cost|Electricity|Geothermal</rdfs:label>
    <rdfs:comment>Capital cost of a new geothermal power plant. If more than one geothermal power technology is modelled, modellers should report capital costs for each represented geothermal power technology by adding variables Capital Cost|Electricity|Geothermal|2, ... Capital Cost|Electricity|Geothermal|N (with N = number of represented technologies). It is modeller's choice which hydropower technologies to assign to type 1 (assigned to the variable without number suffix),2,...,N. The assignment should be documented in the comments sheet. </rdfs:comment>
    <ex:unit>US$2010/kW</ex:unit>
  </rdf:Description>
  <rdf:Description rdf:about="http://transience.eu/ontologies/Inflow_Concrete_Product_categories">
    <rdf:type rdf:resource="http://www.w3.org/2002/07/owl#Class"/>
    <rdfs:subClassOf rdf:resource="http://transience.eu/ontologies/Variable"/>
    <rdfs:label>Inflow|Concrete|[Product categories]</rdfs:label>
    <rdfs:comment>Concrete inflowÂ </rdfs:comment>
    <ex:unit>t/yr</ex:unit>
  </rdf:Description>
  <rdf:Description rdf:about="http://transience.eu/ontologies/Final_Energy_Industry_Other_Sector">
    <rdf:type rdf:resource="http://www.w3.org/2002/07/owl#Class"/>
    <rdfs:subClassOf rdf:resource="http://transience.eu/ontologies/Variable"/>
    <rdfs:label>Final Energy|Industry|Other Sector</rdfs:label>
    <rdfs:comment>Final energy consumed by other industry sectors, excluding feedstocks (please provide a definition of the industries in this category in the 'comments' tab)</rdfs:comment>
    <ex:unit>EJ/yr</ex:unit>
  </rdf:Description>
  <rdf:Description rdf:about="http://transience.eu/ontologies/Investment_Energy_Supply_Electricity_Other">
    <rdf:type rdf:resource="http://www.w3.org/2002/07/owl#Class"/>
    <rdfs:subClassOf rdf:resource="http://transience.eu/ontologies/Variable"/>
    <rdfs:label>Investment|Energy Supply|Electricity|Other</rdfs:label>
    <rdfs:comment>investments in new power generation for the specified power plant category. If the model features several sub-categories, the total investments should be reported. For plants equipped with CCS, the investment in the capturing equipment should be included but not the one on transport and storage.</rdfs:comment>
    <ex:unit>billion US$2010/yr</ex:unit>
  </rdf:Description>
  <rdf:Description rdf:about="http://transience.eu/ontologies/GDP_PPP">
    <rdf:type rdf:resource="http://www.w3.org/2002/07/owl#Class"/>
    <rdfs:subClassOf rdf:resource="http://transience.eu/ontologies/Variable"/>
    <rdfs:label>GDP|PPP</rdfs:label>
    <rdfs:comment>GDP converted to International $ using purchasing power parity (PPP)</rdfs:comment>
    <ex:unit>billion US$2010/yr</ex:unit>
  </rdf:Description>
  <rdf:Description rdf:about="http://transience.eu/ontologies/Emissions_CO2_Energy_Demand_Industry_Other_Sector">
    <rdf:type rdf:resource="http://www.w3.org/2002/07/owl#Class"/>
    <rdfs:subClassOf rdf:resource="http://transience.eu/ontologies/Variable"/>
    <rdfs:label>Emissions|CO2|Energy|Demand|Industry|Other Sector</rdfs:label>
    <rdfs:comment>Fossil CO2 emissions from fuel combustion in industry in other sectors (please provide a definition of thesesectors in this category in the 'comments' tab)</rdfs:comment>
    <ex:unit>Mt CO2/yr</ex:unit>
  </rdf:Description>
  <rdf:Description rdf:about="http://transience.eu/ontologies/Capacity_Electricity_Biomass_w__CCS">
    <rdf:type rdf:resource="http://www.w3.org/2002/07/owl#Class"/>
    <rdfs:subClassOf rdf:resource="http://transience.eu/ontologies/Variable"/>
    <rdfs:label>Capacity|Electricity|Biomass|w/ CCS</rdfs:label>
    <rdfs:comment>Total installed (available) capacity of biomass power plants with CCS, including plants held in an operating reserve. The installed (available) capacity of CCS biomass power plants by plant type for which capital costs are reported should be reported by adding variables Capacity|Electricity|Biomass|w/ CCS|1, ..., Capacity|Electricity|Biomass|w/ CCS|N (matching the assignment of plant types to technologies in the reporting of capital costs as documented in the comments sheet). </rdfs:comment>
    <ex:unit>GW</ex:unit>
  </rdf:Description>
  <rdf:Description rdf:about="http://transience.eu/ontologies/Carbon_Capture_Biomass_Energy_Supply_Electricity">
    <rdf:type rdf:resource="http://www.w3.org/2002/07/owl#Class"/>
    <rdfs:subClassOf rdf:resource="http://transience.eu/ontologies/Variable"/>
    <rdfs:label>Carbon Capture|Biomass|Energy|Supply|Electricity</rdfs:label>
    <rdfs:comment>total carbon dioxide emissions captured from bioenergy use in electricity production (part of IPCC category 1A1a), should be reported as positive numbers</rdfs:comment>
    <ex:unit>Mt CO2/yr</ex:unit>
  </rdf:Description>
  <rdf:Description rdf:about="http://transience.eu/ontologies/Secondary_Energy_Liquids_Biomass">
    <rdf:type rdf:resource="http://www.w3.org/2002/07/owl#Class"/>
    <rdfs:subClassOf rdf:resource="http://transience.eu/ontologies/Variable"/>
    <rdfs:label>Secondary Energy|Liquids|Biomass</rdfs:label>
    <rdfs:comment>total liquid biofuels production</rdfs:comment>
    <ex:unit>EJ/yr</ex:unit>
  </rdf:Description>
  <rdf:Description rdf:about="http://transience.eu/ontologies/Import_Industry_Other_Sector">
    <rdf:type rdf:resource="http://www.w3.org/2002/07/owl#Class"/>
    <rdfs:subClassOf rdf:resource="http://transience.eu/ontologies/Variable"/>
    <rdfs:label>Import|Industry|Other Sector</rdfs:label>
    <rdfs:comment>Import of other industry products measured in monetary units</rdfs:comment>
    <ex:unit>billion US$2010/yr</ex:unit>
  </rdf:Description>
  <rdf:Description rdf:about="http://transience.eu/ontologies/Efficiency_Liquids_Gas_w_o_CCS">
    <rdf:type rdf:resource="http://www.w3.org/2002/07/owl#Class"/>
    <rdfs:subClassOf rdf:resource="http://transience.eu/ontologies/Variable"/>
    <rdfs:label>Efficiency|Liquids|Gas|w/o CCS</rdfs:label>
    <rdfs:comment>Conversion efficiency (energy content of liquids produced per unit of primary energy input) of a new gas to liquids plant w/o CCS. The efficiency should refer to the plant type(s) for which capital costs have been reported. If capital cost for more than one plant type has been reported, modellers should report efficiency for the additional plant types by adding variables Efficiency|Liquids|Gas|w/o CCS|2, ... Efficiency|Liquids|Gas|w/o CCS|N (matching the assignment of plant types to technologies in the reporting of capital costs as documented in the comments sheet). </rdfs:comment>
    <ex:unit>%</ex:unit>
  </rdf:Description>
  <rdf:Description rdf:about="http://transience.eu/ontologies/Outflow_Steel_Other_demand_sectors_Product_categories">
    <rdf:type rdf:resource="http://www.w3.org/2002/07/owl#Class"/>
    <rdfs:subClassOf rdf:resource="http://transience.eu/ontologies/Variable"/>
    <rdfs:label>Outflow|Steel|Other|[demand sectors]|[Product categories]</rdfs:label>
    <rdfs:comment>Steel outflow from other sectorsÂ </rdfs:comment>
    <ex:unit>t/yr</ex:unit>
  </rdf:Description>
  <rdf:Description rdf:about="http://transience.eu/ontologies/Export_Industry_Chemicals">
    <rdf:type rdf:resource="http://www.w3.org/2002/07/owl#Class"/>
    <rdfs:subClassOf rdf:resource="http://transience.eu/ontologies/Variable"/>
    <rdfs:label>Export|Industry|Chemicals</rdfs:label>
    <rdfs:comment>Export of chemicals measured in monetary units</rdfs:comment>
    <ex:unit>billion US$2010/yr</ex:unit>
  </rdf:Description>
  <rdf:Description rdf:about="http://transience.eu/ontologies/Investment_Energy_Supply_Electricity_Non-fossil">
    <rdf:type rdf:resource="http://www.w3.org/2002/07/owl#Class"/>
    <rdfs:subClassOf rdf:resource="http://transience.eu/ontologies/Variable"/>
    <rdfs:label>Investment|Energy Supply|Electricity|Non-fossil</rdfs:label>
    <rdfs:comment>investments in new power generation for the specified power plant category. If the model features several sub-categories, the total investments should be reported. For plants equipped with CCS, the investment in the capturing equipment should be included but not the one on transport and storage.</rdfs:comment>
    <ex:unit>billion US$2010/yr</ex:unit>
  </rdf:Description>
  <rdf:Description rdf:about="http://transience.eu/ontologies/Final_Energy_Residential_and_Commercial_Heat">
    <rdf:type rdf:resource="http://www.w3.org/2002/07/owl#Class"/>
    <rdfs:subClassOf rdf:resource="http://transience.eu/ontologies/Variable"/>
    <rdfs:label>Final Energy|Residential and Commercial|Heat</rdfs:label>
    <rdfs:comment>final energy consumption by the residential &amp; commercial sector of heat (e.g., district heat, process heat, solar heating and warm water), excluding transmission/distribution losses</rdfs:comment>
    <ex:unit>EJ/yr</ex:unit>
  </rdf:Description>
  <rdf:Description rdf:about="http://transience.eu/ontologies/Final_Energy_Non-Energy_Use_Solids_Coal">
    <rdf:type rdf:resource="http://www.w3.org/2002/07/owl#Class"/>
    <rdfs:subClassOf rdf:resource="http://transience.eu/ontologies/Variable"/>
    <rdfs:label>Final Energy|Non-Energy Use|Solids|Coal</rdfs:label>
    <rdfs:comment>Final energy coal consumption by the non-combustion processes</rdfs:comment>
    <ex:unit>EJ/yr</ex:unit>
  </rdf:Description>
  <rdf:Description rdf:about="http://transience.eu/ontologies/Final_Energy_Industry_Chemicals_Solids">
    <rdf:type rdf:resource="http://www.w3.org/2002/07/owl#Class"/>
    <rdfs:subClassOf rdf:resource="http://transience.eu/ontologies/Variable"/>
    <rdfs:label>Final Energy|Industry|Chemicals|Solids</rdfs:label>
    <rdfs:comment>Final energy solid fuel consumption by the chemicals sector (including coal and solid biomass)</rdfs:comment>
    <ex:unit>EJ/yr</ex:unit>
  </rdf:Description>
  <rdf:Description rdf:about="http://transience.eu/ontologies/Price_Final_Energy_Industry_Hydrogen">
    <rdf:type rdf:resource="http://www.w3.org/2002/07/owl#Class"/>
    <rdfs:subClassOf rdf:resource="http://transience.eu/ontologies/Variable"/>
    <rdfs:label>Price|Final Energy|Industry|Hydrogen</rdfs:label>
    <rdfs:comment>Hydrogen price at the final level in the industrial sector. Prices should include the effect of carbon prices and all other taxes.</rdfs:comment>
    <ex:unit>US$2010/GJ</ex:unit>
  </rdf:Description>
  <rdf:Description rdf:about="http://transience.eu/ontologies/Final_Energy_Non-Energy_Use_Gases_Biomass">
    <rdf:type rdf:resource="http://www.w3.org/2002/07/owl#Class"/>
    <rdfs:subClassOf rdf:resource="http://transience.eu/ontologies/Variable"/>
    <rdfs:label>Final Energy|Non-Energy Use|Gases|Biomass</rdfs:label>
    <rdfs:comment>Final energy consumption of biogas by the non-combustion processes</rdfs:comment>
    <ex:unit>EJ/yr</ex:unit>
  </rdf:Description>
  <rdf:Description rdf:about="http://transience.eu/ontologies/Secondary_Energy_Electricity_Non-Biomass_Renewables">
    <rdf:type rdf:resource="http://www.w3.org/2002/07/owl#Class"/>
    <rdfs:subClassOf rdf:resource="http://transience.eu/ontologies/Variable"/>
    <rdfs:label>Secondary Energy|Electricity|Non-Biomass Renewables</rdfs:label>
    <rdfs:comment>net electricity production from hydro, wind, solar, geothermal, ocean, and other renewable sources (excluding bioenergy). This is a summary category for all the non-biomass renewables.</rdfs:comment>
    <ex:unit>EJ/yr</ex:unit>
  </rdf:Description>
  <rdf:Description rdf:about="http://transience.eu/ontologies/Secondary_Energy_Liquids_Electricity">
    <rdf:type rdf:resource="http://www.w3.org/2002/07/owl#Class"/>
    <rdfs:subClassOf rdf:resource="http://transience.eu/ontologies/Variable"/>
    <rdfs:label>Secondary Energy|Liquids|Electricity</rdfs:label>
    <rdfs:comment>total production of liquid fuels from electricity (efuels)</rdfs:comment>
    <ex:unit>EJ/yr</ex:unit>
  </rdf:Description>
  <rdf:Description rdf:about="http://transience.eu/ontologies/Production_Steel_Crude_steel_Volume">
    <rdf:type rdf:resource="http://www.w3.org/2002/07/owl#Class"/>
    <rdfs:subClassOf rdf:resource="http://transience.eu/ontologies/Variable"/>
    <rdfs:label>Production|Steel|Crude steel|Volume</rdfs:label>
    <rdfs:comment>Production of crude steel</rdfs:comment>
    <ex:unit>Mt/yr</ex:unit>
  </rdf:Description>
  <rdf:Description rdf:about="http://transience.eu/ontologies/Final_Energy_Industry_Other_Sector_Hydrogen">
    <rdf:type rdf:resource="http://www.w3.org/2002/07/owl#Class"/>
    <rdfs:subClassOf rdf:resource="http://transience.eu/ontologies/Variable"/>
    <rdfs:label>Final Energy|Industry|Other Sector|Hydrogen</rdfs:label>
    <rdfs:comment>Final energy consumption of hydrogen by other industry sectors</rdfs:comment>
    <ex:unit>EJ/yr</ex:unit>
  </rdf:Description>
  <rdf:Description rdf:about="http://transience.eu/ontologies/Final_Energy_Industry_Pulp_and_Paper_Waste">
    <rdf:type rdf:resource="http://www.w3.org/2002/07/owl#Class"/>
    <rdfs:subClassOf rdf:resource="http://transience.eu/ontologies/Variable"/>
    <rdfs:label>Final Energy|Industry|Pulp and Paper|Waste</rdfs:label>
    <rdfs:comment>Final energy consumption of non-renewable waste by the pulp and paper sector</rdfs:comment>
    <ex:unit>EJ/yr</ex:unit>
  </rdf:Description>
  <rdf:Description rdf:about="http://transience.eu/ontologies/Final_Energy_Industry_Non-Ferrous_Metals_Solids_Biomass">
    <rdf:type rdf:resource="http://www.w3.org/2002/07/owl#Class"/>
    <rdfs:subClassOf rdf:resource="http://transience.eu/ontologies/Variable"/>
    <rdfs:label>Final Energy|Industry|Non-Ferrous Metals|Solids|Biomass</rdfs:label>
    <rdfs:comment>Final energy consumption of solid biomass (modern and traditional, including renewable waste) by the non-ferrous metals sector</rdfs:comment>
    <ex:unit>EJ/yr</ex:unit>
  </rdf:Description>
  <rdf:Description rdf:about="http://transience.eu/ontologies/Primary_Energy_Other">
    <rdf:type rdf:resource="http://www.w3.org/2002/07/owl#Class"/>
    <rdfs:subClassOf rdf:resource="http://transience.eu/ontologies/Variable"/>
    <rdfs:label>Primary Energy|Other</rdfs:label>
    <rdfs:comment>primary energy consumption from sources that do not fit to any other category (direct equivalent, please provide a definition of the sources in this category in the 'comments' tab)</rdfs:comment>
    <ex:unit>EJ/yr</ex:unit>
  </rdf:Description>
  <rdf:Description rdf:about="http://transience.eu/ontologies/Final_Energy_Carbon_Removal_Other">
    <rdf:type rdf:resource="http://www.w3.org/2002/07/owl#Class"/>
    <rdfs:subClassOf rdf:resource="http://transience.eu/ontologies/Variable"/>
    <rdfs:label>Final Energy|Carbon Removal|Other</rdfs:label>
    <rdfs:comment>Final energy consumption of other sources that do not fit to any other category by carbon dioxide removal processes</rdfs:comment>
    <ex:unit>EJ/yr</ex:unit>
  </rdf:Description>
  <rdf:Description rdf:about="http://transience.eu/ontologies/Conversion_Input_Hydrogen_Liquids_Autoproduction">
    <rdf:type rdf:resource="http://www.w3.org/2002/07/owl#Class"/>
    <rdfs:subClassOf rdf:resource="http://transience.eu/ontologies/Variable"/>
    <rdfs:label>Conversion Input|Hydrogen|Liquids|Autoproduction</rdfs:label>
    <rdfs:comment>secondary energy consumption of hydrogen for the autoproduction of liquids, incl. hydrocarbon inputs for olefine production</rdfs:comment>
    <ex:unit>EJ/yr</ex:unit>
  </rdf:Description>
  <rdf:Description rdf:about="http://transience.eu/ontologies/Primary_Energy_Coal_Electricity">
    <rdf:type rdf:resource="http://www.w3.org/2002/07/owl#Class"/>
    <rdfs:subClassOf rdf:resource="http://transience.eu/ontologies/Variable"/>
    <rdfs:label>Primary Energy|Coal|Electricity</rdfs:label>
    <rdfs:comment>coal primary energy input to electricity generation </rdfs:comment>
    <ex:unit>EJ/yr</ex:unit>
  </rdf:Description>
  <rdf:Description rdf:about="http://transience.eu/ontologies/Production_Other_Sector_Value">
    <rdf:type rdf:resource="http://www.w3.org/2002/07/owl#Class"/>
    <rdfs:subClassOf rdf:resource="http://transience.eu/ontologies/Variable"/>
    <rdfs:label>Production|Other Sector|Value</rdfs:label>
    <rdfs:comment>production of other industry products</rdfs:comment>
    <ex:unit>billion US$2010/yr</ex:unit>
  </rdf:Description>
  <rdf:Description rdf:about="http://transience.eu/ontologies/Emissions_CO2_Other">
    <rdf:type rdf:resource="http://www.w3.org/2002/07/owl#Class"/>
    <rdfs:subClassOf rdf:resource="http://transience.eu/ontologies/Variable"/>
    <rdfs:label>Emissions|CO2|Other</rdfs:label>
    <rdfs:comment>CO2 emissions from other sources (please provide a definition of other sources in this category in the 'comments' tab)</rdfs:comment>
    <ex:unit>Mt CO2/yr</ex:unit>
  </rdf:Description>
  <rdf:Description rdf:about="http://transience.eu/ontologies/Energy_Service_Transportation_Passenger_Road_LDV">
    <rdf:type rdf:resource="http://www.w3.org/2002/07/owl#Class"/>
    <rdfs:subClassOf rdf:resource="http://transience.eu/ontologies/Variable"/>
    <rdfs:label>Energy Service|Transportation|Passenger|Road|LDV</rdfs:label>
    <rdfs:comment>energy service demand for passenger transport on roads (light-duty vehicles: passenger cars and light trucks/SUVs/vans)</rdfs:comment>
    <ex:unit>bn pkm/yr</ex:unit>
  </rdf:Description>
  <rdf:Description rdf:about="http://transience.eu/ontologies/Materials_Demand_Non-metallic_minerals_Cement_Infrastructures">
    <rdf:type rdf:resource="http://www.w3.org/2002/07/owl#Class"/>
    <rdfs:subClassOf rdf:resource="http://transience.eu/ontologies/Variable"/>
    <rdfs:label>Materials Demand|Non-metallic minerals|Cement|Infrastructures</rdfs:label>
    <rdfs:comment>Cement requirments from a certain end-use sector</rdfs:comment>
    <ex:unit>Mt/yr</ex:unit>
  </rdf:Description>
  <rdf:Description rdf:about="http://transience.eu/ontologies/Primary_Energy_Gas_w_o_CCS">
    <rdf:type rdf:resource="http://www.w3.org/2002/07/owl#Class"/>
    <rdfs:subClassOf rdf:resource="http://transience.eu/ontologies/Variable"/>
    <rdfs:label>Primary Energy|Gas|w/o CCS</rdfs:label>
    <rdfs:comment>gas primary energy consumption without CCS</rdfs:comment>
    <ex:unit>EJ/yr</ex:unit>
  </rdf:Description>
  <rdf:Description rdf:about="http://transience.eu/ontologies/Secondary_Energy_Hydrogen_Nuclear">
    <rdf:type rdf:resource="http://www.w3.org/2002/07/owl#Class"/>
    <rdfs:subClassOf rdf:resource="http://transience.eu/ontologies/Variable"/>
    <rdfs:label>Secondary Energy|Hydrogen|Nuclear</rdfs:label>
    <rdfs:comment>total hydrogen production from nuclear energy (e.g. thermochemical water splitting with nucelar heat)</rdfs:comment>
    <ex:unit>EJ/yr</ex:unit>
  </rdf:Description>
  <rdf:Description rdf:about="http://transience.eu/ontologies/Emissions_CO2_Industrial_Processes_Other_Sector">
    <rdf:type rdf:resource="http://www.w3.org/2002/07/owl#Class"/>
    <rdfs:subClassOf rdf:resource="http://transience.eu/ontologies/Variable"/>
    <rdfs:label>Emissions|CO2|Industrial Processes|Other Sector</rdfs:label>
    <rdfs:comment>CO2 emissions from industrial processes from chemicals</rdfs:comment>
    <ex:unit>Mt CO2/yr</ex:unit>
  </rdf:Description>
  <rdf:Description rdf:about="http://transience.eu/ontologies/Final_Energy_Industry_Other_Sector_Liquids_Biomass">
    <rdf:type rdf:resource="http://www.w3.org/2002/07/owl#Class"/>
    <rdfs:subClassOf rdf:resource="http://transience.eu/ontologies/Variable"/>
    <rdfs:label>Final Energy|Industry|Other Sector|Liquids|Biomass</rdfs:label>
    <rdfs:comment>Final energy consumption of liquid biofuels by other industry sectors</rdfs:comment>
    <ex:unit>EJ/yr</ex:unit>
  </rdf:Description>
  <rdf:Description rdf:about="http://transience.eu/ontologies/Investment_Energy_Supply_CO2_Transport_and_Storage">
    <rdf:type rdf:resource="http://www.w3.org/2002/07/owl#Class"/>
    <rdfs:subClassOf rdf:resource="http://transience.eu/ontologies/Variable"/>
    <rdfs:label>Investment|Energy Supply|CO2 Transport and Storage</rdfs:label>
    <rdfs:comment>investment in CO2 transport and storage (note that investment in the capturing equipment should be included along with the power plant technology)</rdfs:comment>
    <ex:unit>billion US$2010/yr</ex:unit>
  </rdf:Description>
  <rdf:Description rdf:about="http://transience.eu/ontologies/Secondary_Energy_Electricity_Nuclear">
    <rdf:type rdf:resource="http://www.w3.org/2002/07/owl#Class"/>
    <rdfs:subClassOf rdf:resource="http://transience.eu/ontologies/Variable"/>
    <rdfs:label>Secondary Energy|Electricity|Nuclear</rdfs:label>
    <rdfs:comment>net electricity production from nuclear energy</rdfs:comment>
    <ex:unit>EJ/yr</ex:unit>
  </rdf:Description>
  <rdf:Description rdf:about="http://transience.eu/ontologies/Final_Energy_Industry_Chemicals_Electricity">
    <rdf:type rdf:resource="http://www.w3.org/2002/07/owl#Class"/>
    <rdfs:subClassOf rdf:resource="http://transience.eu/ontologies/Variable"/>
    <rdfs:label>Final Energy|Industry|Chemicals|Electricity</rdfs:label>
    <rdfs:comment>Final energy consumption of electricity by the chemical sector</rdfs:comment>
    <ex:unit>EJ/yr</ex:unit>
  </rdf:Description>
  <rdf:Description rdf:about="http://transience.eu/ontologies/Primary_Energy_Coal_w_o_CCS">
    <rdf:type rdf:resource="http://www.w3.org/2002/07/owl#Class"/>
    <rdfs:subClassOf rdf:resource="http://transience.eu/ontologies/Variable"/>
    <rdfs:label>Primary Energy|Coal|w/o CCS</rdfs:label>
    <rdfs:comment>coal primary energy consumption without CCS</rdfs:comment>
    <ex:unit>EJ/yr</ex:unit>
  </rdf:Description>
  <rdf:Description rdf:about="http://transience.eu/ontologies/Trade_Primary_Energy_Gas_Volume">
    <rdf:type rdf:resource="http://www.w3.org/2002/07/owl#Class"/>
    <rdfs:subClassOf rdf:resource="http://transience.eu/ontologies/Variable"/>
    <rdfs:label>Trade|Primary Energy|Gas|Volume</rdfs:label>
    <rdfs:comment>net exports of natural gas, at the global level these should add up to the trade losses only</rdfs:comment>
    <ex:unit>EJ/yr</ex:unit>
  </rdf:Description>
  <rdf:Description rdf:about="http://transience.eu/ontologies/Emissions_CO2_AFOLU_Land_Wetlands">
    <rdf:type rdf:resource="http://www.w3.org/2002/07/owl#Class"/>
    <rdfs:subClassOf rdf:resource="http://transience.eu/ontologies/Variable"/>
    <rdfs:label>Emissions|CO2|AFOLU|Land|Wetlands</rdfs:label>
    <rdfs:comment>CO2 emissions from managed peatlands (drained and rewetted)</rdfs:comment>
    <ex:unit>Mt CO2/yr</ex:unit>
  </rdf:Description>
  <rdf:Description rdf:about="http://transience.eu/ontologies/Final_Energy_Industry_Other_Sector_Liquids">
    <rdf:type rdf:resource="http://www.w3.org/2002/07/owl#Class"/>
    <rdfs:subClassOf rdf:resource="http://transience.eu/ontologies/Variable"/>
    <rdfs:label>Final Energy|Industry|Other Sector|Liquids</rdfs:label>
    <rdfs:comment>Final energy consumption of refined liquids by other industry sectors (conventional &amp; unconventional oil, biofuels, coal-to-liquids, gas-to-liquids, efuels)</rdfs:comment>
    <ex:unit>EJ/yr</ex:unit>
  </rdf:Description>
  <rdf:Description rdf:about="http://transience.eu/ontologies/OM_Cost_Fixed_Electricity_Gas_w_o_CCS">
    <rdf:type rdf:resource="http://www.w3.org/2002/07/owl#Class"/>
    <rdfs:subClassOf rdf:resource="http://transience.eu/ontologies/Variable"/>
    <rdfs:label>OM Cost|Fixed|Electricity|Gas|w/o CCS</rdfs:label>
    <rdfs:comment>Annual fixed operation &amp; maintainance cost of a new gas power plant w/o CCS. If more than one gas power technology is modelled, modellers should report fixed O&amp;M costs  for each represented gas power technology by adding variables OM Cost|Fixed|Electricity|Gas|w/o CCS|2, ... OM Cost|Fixed|Electricity|Gas|w/o CCS|N (with N = number of represented technologies) (matching the assignment of plant types to technologies in the reporting of capital costs as documented in the comments sheet).</rdfs:comment>
    <ex:unit>US$2010/kW/yr</ex:unit>
  </rdf:Description>
  <rdf:Description rdf:about="http://transience.eu/ontologies/Price_Primary_Energy_Coal">
    <rdf:type rdf:resource="http://www.w3.org/2002/07/owl#Class"/>
    <rdfs:subClassOf rdf:resource="http://transience.eu/ontologies/Variable"/>
    <rdfs:label>Price|Primary Energy|Coal</rdfs:label>
    <rdfs:comment>coal price at the primary level (i.e. the spot price at the global or regional market)</rdfs:comment>
    <ex:unit>US$2010/GJ</ex:unit>
  </rdf:Description>
  <rdf:Description rdf:about="http://transience.eu/ontologies/Final_Energy_Industry_Chemicals_Liquids">
    <rdf:type rdf:resource="http://www.w3.org/2002/07/owl#Class"/>
    <rdfs:subClassOf rdf:resource="http://transience.eu/ontologies/Variable"/>
    <rdfs:label>Final Energy|Industry|Chemicals|Liquids</rdfs:label>
    <rdfs:comment>Final energy consumption of refined liquids by the chemicals sector (conventional &amp; unconventional oil, biofuels, coal-to-liquids, gas-to-liquids, efuels)</rdfs:comment>
    <ex:unit>EJ/yr</ex:unit>
  </rdf:Description>
  <rdf:Description rdf:about="http://transience.eu/ontologies/Import_Industry_Non-Metallic_Minerals">
    <rdf:type rdf:resource="http://www.w3.org/2002/07/owl#Class"/>
    <rdfs:subClassOf rdf:resource="http://transience.eu/ontologies/Variable"/>
    <rdfs:label>Import|Industry|Non-Metallic Minerals</rdfs:label>
    <rdfs:comment>Import of non-metallic minerals measured in monetary units</rdfs:comment>
    <ex:unit>billion US$2010/yr</ex:unit>
  </rdf:Description>
  <rdf:Description rdf:about="http://transience.eu/ontologies/Final_Energy_Commercial_Liquids_Fossil">
    <rdf:type rdf:resource="http://www.w3.org/2002/07/owl#Class"/>
    <rdfs:subClassOf rdf:resource="http://transience.eu/ontologies/Variable"/>
    <rdfs:label>Final Energy|Commercial|Liquids|Fossil</rdfs:label>
    <rdfs:comment>final energy consumption by the commercial sector of liquids from fossil origin (conventional &amp; unconventional petroleum, coal-to-liquids, gas-to-liquids)</rdfs:comment>
    <ex:unit>EJ/yr</ex:unit>
  </rdf:Description>
  <rdf:Description rdf:about="http://transience.eu/ontologies/Emissions_CO2_Energy_Demand_Transportation">
    <rdf:type rdf:resource="http://www.w3.org/2002/07/owl#Class"/>
    <rdfs:subClassOf rdf:resource="http://transience.eu/ontologies/Variable"/>
    <rdfs:label>Emissions|CO2|Energy|Demand|Transportation</rdfs:label>
    <rdfs:comment>Fossil CO2 emissions from fuel combustion in transportation sector (IPCC category 1A3), excluding pipeline emissions (IPCC category 1A3ei), excluding emissions from international bunkers (IPCC category 1A3ai and 1A3di) </rdfs:comment>
    <ex:unit>Mt CO2/yr</ex:unit>
  </rdf:Description>
  <rdf:Description rdf:about="http://transience.eu/ontologies/Final_Energy_Industry_Iron_and_Steel_Liquids_Biomass">
    <rdf:type rdf:resource="http://www.w3.org/2002/07/owl#Class"/>
    <rdfs:subClassOf rdf:resource="http://transience.eu/ontologies/Variable"/>
    <rdfs:label>Final Energy|Industry|Iron and Steel|Liquids|Biomass</rdfs:label>
    <rdfs:comment>Final energy consumption of liquid biofuels by the iron and steel sector</rdfs:comment>
    <ex:unit>EJ/yr</ex:unit>
  </rdf:Description>
  <rdf:Description rdf:about="http://transience.eu/ontologies/Final_Energy_Industry_Iron_and_Steel_Heat">
    <rdf:type rdf:resource="http://www.w3.org/2002/07/owl#Class"/>
    <rdfs:subClassOf rdf:resource="http://transience.eu/ontologies/Variable"/>
    <rdfs:label>Final Energy|Industry|Iron and Steel|Heat</rdfs:label>
    <rdfs:comment>Final energy consumption of centrally supplied heat by the iron and steel sector</rdfs:comment>
    <ex:unit>EJ/yr</ex:unit>
  </rdf:Description>
  <rdf:Description rdf:about="http://transience.eu/ontologies/Emissions_CO2_Waste_Biomass">
    <rdf:type rdf:resource="http://www.w3.org/2002/07/owl#Class"/>
    <rdfs:subClassOf rdf:resource="http://transience.eu/ontologies/Variable"/>
    <rdfs:label>Emissions|CO2|Waste|Biomass</rdfs:label>
    <rdfs:comment>CO2 emissions from waste of biogenic origin, e.g. bioplastics</rdfs:comment>
    <ex:unit>Mt CO2/yr</ex:unit>
  </rdf:Description>
  <rdf:Description rdf:about="http://transience.eu/ontologies/Investment_Energy_Supply_Extraction_Oil">
    <rdf:type rdf:resource="http://www.w3.org/2002/07/owl#Class"/>
    <rdfs:subClassOf rdf:resource="http://transience.eu/ontologies/Variable"/>
    <rdfs:label>Investment|Energy Supply|Extraction|Oil</rdfs:label>
    <rdfs:comment>investments for extraction and conversion of oil. These should include upstream, transport and refining</rdfs:comment>
    <ex:unit>billion US$2010/yr</ex:unit>
  </rdf:Description>
  <rdf:Description rdf:about="http://transience.eu/ontologies/Final_Energy_Industry_Steel_Biomass">
    <rdf:type rdf:resource="http://www.w3.org/2002/07/owl#Class"/>
    <rdfs:subClassOf rdf:resource="http://transience.eu/ontologies/Variable"/>
    <rdfs:label>Final Energy|Industry|Steel|Biomass</rdfs:label>
    <rdfs:comment>Final energy. System boundaries in line with energy accounting</rdfs:comment>
    <ex:unit>PJ/yr</ex:unit>
  </rdf:Description>
  <rdf:Description rdf:about="http://transience.eu/ontologies/Secondary_Energy_Hydrogen_Fossil_w_o_CCS">
    <rdf:type rdf:resource="http://www.w3.org/2002/07/owl#Class"/>
    <rdfs:subClassOf rdf:resource="http://transience.eu/ontologies/Variable"/>
    <rdfs:label>Secondary Energy|Hydrogen|Fossil|w/o CCS</rdfs:label>
    <rdfs:comment>hydrogen production from fossil fuels with freely vented CO2 emissions</rdfs:comment>
    <ex:unit>EJ/yr</ex:unit>
  </rdf:Description>
  <rdf:Description rdf:about="http://transience.eu/ontologies/Carbon_Capture_Storage_Fossil_Energy_Supply_Hydrogen">
    <rdf:type rdf:resource="http://www.w3.org/2002/07/owl#Class"/>
    <rdfs:subClassOf rdf:resource="http://transience.eu/ontologies/Variable"/>
    <rdfs:label>Carbon Capture|Storage|Fossil|Energy|Supply|Hydrogen</rdfs:label>
    <rdfs:comment>total carbon dioxide emissions captured from fossil fuel use in hydrogen production (part of IPCC category 1A) and stored in geological deposits (e.g. in depleted oil and gas fields, unmined coal seams, saline aquifers) and the deep ocean, stored amounts should be reported as positive numbers</rdfs:comment>
    <ex:unit>Mt CO2/yr</ex:unit>
  </rdf:Description>
  <rdf:Description rdf:about="http://transience.eu/ontologies/Final_Energy_Industry_Other_Sector_Electricity">
    <rdf:type rdf:resource="http://www.w3.org/2002/07/owl#Class"/>
    <rdfs:subClassOf rdf:resource="http://transience.eu/ontologies/Variable"/>
    <rdfs:label>Final Energy|Industry|Other Sector|Electricity</rdfs:label>
    <rdfs:comment>Final energy consumption of electricity by other industry sectors</rdfs:comment>
    <ex:unit>EJ/yr</ex:unit>
  </rdf:Description>
  <rdf:Description rdf:about="http://transience.eu/ontologies/Final_Energy_Residential_and_Commercial_Electricity">
    <rdf:type rdf:resource="http://www.w3.org/2002/07/owl#Class"/>
    <rdfs:subClassOf rdf:resource="http://transience.eu/ontologies/Variable"/>
    <rdfs:label>Final Energy|Residential and Commercial|Electricity</rdfs:label>
    <rdfs:comment>final energy consumption by the residential &amp; commercial sector of electricity (including on-site solar PV), excluding transmission/distribution losses</rdfs:comment>
    <ex:unit>EJ/yr</ex:unit>
  </rdf:Description>
  <rdf:Description rdf:about="http://transience.eu/ontologies/Carbon_Capture_Storage_Electricity">
    <rdf:type rdf:resource="http://www.w3.org/2002/07/owl#Class"/>
    <rdfs:subClassOf rdf:resource="http://transience.eu/ontologies/Variable"/>
    <rdfs:label>Carbon Capture|Storage|Electricity</rdfs:label>
    <rdfs:comment>total carbon dioxide emissions captured from hydrogen or synthetic fuel use and stored in geological deposits (e.g. in depleted oil and gas fields, unmined coal seams, saline aquifers) and the deep ocean, stored amounts should be reported as positive numbers</rdfs:comment>
    <ex:unit>Mt CO2/yr</ex:unit>
  </rdf:Description>
  <rdf:Description rdf:about="http://transience.eu/ontologies/Investment_Energy_Supply_Electricity_Oil_w_o_CCS">
    <rdf:type rdf:resource="http://www.w3.org/2002/07/owl#Class"/>
    <rdfs:subClassOf rdf:resource="http://transience.eu/ontologies/Variable"/>
    <rdfs:label>Investment|Energy Supply|Electricity|Oil|w/o CCS</rdfs:label>
    <rdfs:comment>investments in new power generation for the specified power plant category. If the model features several sub-categories, the total investments should be reported. For plants equipped with CCS, the investment in the capturing equipment should be included but not the one on transport and storage.</rdfs:comment>
    <ex:unit>billion US$2010/yr</ex:unit>
  </rdf:Description>
  <rdf:Description rdf:about="http://transience.eu/ontologies/Final_Energy_Industry_Non-Ferrous_Metals_Liquids_Electricity">
    <rdf:type rdf:resource="http://www.w3.org/2002/07/owl#Class"/>
    <rdfs:subClassOf rdf:resource="http://transience.eu/ontologies/Variable"/>
    <rdfs:label>Final Energy|Industry|Non-Ferrous Metals|Liquids|Electricity</rdfs:label>
    <rdfs:comment>Final energy consumption of synthetic liquid efuels ("power-to-liquid") by the non-ferrous metals sector</rdfs:comment>
    <ex:unit>EJ/yr</ex:unit>
  </rdf:Description>
  <rdf:Description rdf:about="http://transience.eu/ontologies/Trade_Secondary_Energy_Liquids_Oil_Volume">
    <rdf:type rdf:resource="http://www.w3.org/2002/07/owl#Class"/>
    <rdfs:subClassOf rdf:resource="http://transience.eu/ontologies/Variable"/>
    <rdfs:label>Trade|Secondary Energy|Liquids|Oil|Volume</rdfs:label>
    <rdfs:comment>net exports of liquid fuels from petroleum including both conventional and unconventional sources, at the global level these should add up to the trade losses only</rdfs:comment>
    <ex:unit>EJ/yr</ex:unit>
  </rdf:Description>
  <rdf:Description rdf:about="http://transience.eu/ontologies/Material_intensity_material_building_type_age_cohort">
    <rdf:type rdf:resource="http://www.w3.org/2002/07/owl#Class"/>
    <rdfs:subClassOf rdf:resource="http://transience.eu/ontologies/ParameterInput"/>
    <rdfs:label>Material intensity|[material]|[building type]|[age cohort]</rdfs:label>
    <rdfs:comment>Material intensity buildingsÂ </rdfs:comment>
    <ex:unit>kg/m2</ex:unit>
  </rdf:Description>
  <rdf:Description rdf:about="http://transience.eu/ontologies/Production_Steel_Product_categories">
    <rdf:type rdf:resource="http://www.w3.org/2002/07/owl#Class"/>
    <rdfs:subClassOf rdf:resource="http://transience.eu/ontologies/ParameterOutput"/>
    <rdfs:label>Production|Steel|[Product categories]</rdfs:label>
    <rdfs:comment>Steel productionÂ </rdfs:comment>
    <ex:unit>t/yr</ex:unit>
  </rdf:Description>
  <rdf:Description rdf:about="http://transience.eu/ontologies/Secondary_Energy_Hydrogen_Biomass_w_o_CCS">
    <rdf:type rdf:resource="http://www.w3.org/2002/07/owl#Class"/>
    <rdfs:subClassOf rdf:resource="http://transience.eu/ontologies/Variable"/>
    <rdfs:label>Secondary Energy|Hydrogen|Biomass|w/o CCS</rdfs:label>
    <rdfs:comment>hydrogen production from biomass with freely vented CO2 emissions</rdfs:comment>
    <ex:unit>EJ/yr</ex:unit>
  </rdf:Description>
  <rdf:Description rdf:about="http://transience.eu/ontologies/Final_Energy_Industry_Steel_Off-gases">
    <rdf:type rdf:resource="http://www.w3.org/2002/07/owl#Class"/>
    <rdfs:subClassOf rdf:resource="http://transience.eu/ontologies/Variable"/>
    <rdfs:label>Final Energy|Industry|Steel|Off-gases</rdfs:label>
    <rdfs:comment>Final energy. System boundaries in line with energy accounting</rdfs:comment>
    <ex:unit>PJ/yr</ex:unit>
  </rdf:Description>
  <rdf:Description rdf:about="http://transience.eu/ontologies/Final_Energy_Industry_Iron_and_Steel_Gases">
    <rdf:type rdf:resource="http://www.w3.org/2002/07/owl#Class"/>
    <rdfs:subClassOf rdf:resource="http://transience.eu/ontologies/Variable"/>
    <rdfs:label>Final Energy|Industry|Iron and Steel|Gases</rdfs:label>
    <rdfs:comment>Final energy consumption of gases by the iron and steel sector (natural gas, biogas, coal-gas), excluding transmission/distribution losses</rdfs:comment>
    <ex:unit>EJ/yr</ex:unit>
  </rdf:Description>
  <rdf:Description rdf:about="http://transience.eu/ontologies/OM_Cost_Fixed_Hydrogen_Biomass_w_o_CCS">
    <rdf:type rdf:resource="http://www.w3.org/2002/07/owl#Class"/>
    <rdfs:subClassOf rdf:resource="http://transience.eu/ontologies/Variable"/>
    <rdfs:label>OM Cost|Fixed|Hydrogen|Biomass|w/o CCS</rdfs:label>
    <rdfs:comment>Annual fixed operation &amp; maintainance cost of a new biomass to hydrogen plant w/o CCS. If more than one biomass to hydrogen technology is modelled, modellers should report fixed O&amp;M costs  for each represented biomass to hydrogen technology by adding variables OM Cost|Fixed|Hydrogen|Biomass|w/o CCS|2, ... OM Cost|Fixed|Hydrogen|Biomass|w/o CCS|N (with N = number of represented technologies) (matching the assignment of plant types to technologies in the reporting of capital costs as documented in the comments sheet).</rdfs:comment>
    <ex:unit>US$2010/kW/yr</ex:unit>
  </rdf:Description>
  <rdf:Description rdf:about="http://transience.eu/ontologies/Primary_Energy_Biomass_Electricity_w_o_CCS">
    <rdf:type rdf:resource="http://www.w3.org/2002/07/owl#Class"/>
    <rdfs:subClassOf rdf:resource="http://transience.eu/ontologies/Variable"/>
    <rdfs:label>Primary Energy|Biomass|Electricity|w/o CCS</rdfs:label>
    <rdfs:comment>purpose-grown bioenergy crops, crop and forestry residue bioenergy, municipal solid waste bioenergy, traditional biomass primary energy input to electricity generation without CCS</rdfs:comment>
    <ex:unit>EJ/yr</ex:unit>
  </rdf:Description>
  <rdf:Description rdf:about="http://transience.eu/ontologies/Final_Energy_Commercial_Liquids">
    <rdf:type rdf:resource="http://www.w3.org/2002/07/owl#Class"/>
    <rdfs:subClassOf rdf:resource="http://transience.eu/ontologies/Variable"/>
    <rdfs:label>Final Energy|Commercial|Liquids</rdfs:label>
    <rdfs:comment>final energy consumption by the commercial sector of refined liquids (conventional &amp; unconventional oil, biofuels, coal-to-liquids, gas-to-liquids)</rdfs:comment>
    <ex:unit>EJ/yr</ex:unit>
  </rdf:Description>
  <rdf:Description rdf:about="http://transience.eu/ontologies/Price_Carbon_Net_Industry">
    <rdf:type rdf:resource="http://www.w3.org/2002/07/owl#Class"/>
    <rdfs:subClassOf rdf:resource="http://transience.eu/ontologies/Variable"/>
    <rdfs:label>Price|Carbon|Net|Industry</rdfs:label>
    <rdfs:comment>Net price of carbon applicable at national level for industry sector (= sum of all overlapping regulations)</rdfs:comment>
    <ex:unit>US$2010/t CO2</ex:unit>
  </rdf:Description>
  <rdf:Description rdf:about="http://transience.eu/ontologies/Final_Energy_Industry_Non-Ferrous_Metals_Solar">
    <rdf:type rdf:resource="http://www.w3.org/2002/07/owl#Class"/>
    <rdfs:subClassOf rdf:resource="http://transience.eu/ontologies/Variable"/>
    <rdfs:label>Final Energy|Industry|Non-Ferrous Metals|Solar</rdfs:label>
    <rdfs:comment>Final energy consumption of solar thermal heat by the non-ferrous metals sector</rdfs:comment>
    <ex:unit>EJ/yr</ex:unit>
  </rdf:Description>
  <rdf:Description rdf:about="http://transience.eu/ontologies/Emissions_CO2_Waste">
    <rdf:type rdf:resource="http://www.w3.org/2002/07/owl#Class"/>
    <rdfs:subClassOf rdf:resource="http://transience.eu/ontologies/Variable"/>
    <rdfs:label>Emissions|CO2|Waste</rdfs:label>
    <rdfs:comment>CO2 emissions from waste (IPCC categories 6C), not including the burning of waste for electricity or heat supply (these emissions should be reported under the respective categories of CO2|Energy)</rdfs:comment>
    <ex:unit>Mt CO2/yr</ex:unit>
  </rdf:Description>
  <rdf:Description rdf:about="http://transience.eu/ontologies/Import_Industry_Pulp_and_Paper">
    <rdf:type rdf:resource="http://www.w3.org/2002/07/owl#Class"/>
    <rdfs:subClassOf rdf:resource="http://transience.eu/ontologies/Variable"/>
    <rdfs:label>Import|Industry|Pulp and Paper</rdfs:label>
    <rdfs:comment>Import of pulp and paper measured in monetary units</rdfs:comment>
    <ex:unit>billion US$2010/yr</ex:unit>
  </rdf:Description>
  <rdf:Description rdf:about="http://transience.eu/ontologies/Secondary_Energy_Electricity_Wind_Offshore">
    <rdf:type rdf:resource="http://www.w3.org/2002/07/owl#Class"/>
    <rdfs:subClassOf rdf:resource="http://transience.eu/ontologies/Variable"/>
    <rdfs:label>Secondary Energy|Electricity|Wind|Offshore</rdfs:label>
    <rdfs:comment>net electricity production from offshore wind energy</rdfs:comment>
    <ex:unit>EJ/yr</ex:unit>
  </rdf:Description>
  <rdf:Description rdf:about="http://transience.eu/ontologies/Secondary_Energy_Heat_Oil">
    <rdf:type rdf:resource="http://www.w3.org/2002/07/owl#Class"/>
    <rdfs:subClassOf rdf:resource="http://transience.eu/ontologies/Variable"/>
    <rdfs:label>Secondary Energy|Heat|Oil</rdfs:label>
    <rdfs:comment>centralized heat generation from oil products </rdfs:comment>
    <ex:unit>EJ/yr</ex:unit>
  </rdf:Description>
  <rdf:Description rdf:about="http://transience.eu/ontologies/Export_Industry_Chemicals_High_Value_Chemicals_Volume">
    <rdf:type rdf:resource="http://www.w3.org/2002/07/owl#Class"/>
    <rdfs:subClassOf rdf:resource="http://transience.eu/ontologies/Variable"/>
    <rdfs:label>Export|Industry|Chemicals|High Value Chemicals|Volume</rdfs:label>
    <rdfs:comment>Export of high value chemicals</rdfs:comment>
    <ex:unit>Mt/yr</ex:unit>
  </rdf:Description>
  <rdf:Description rdf:about="http://transience.eu/ontologies/Capital_Cost_Electricity_Hydro">
    <rdf:type rdf:resource="http://www.w3.org/2002/07/owl#Class"/>
    <rdfs:subClassOf rdf:resource="http://transience.eu/ontologies/Variable"/>
    <rdfs:label>Capital Cost|Electricity|Hydro</rdfs:label>
    <rdfs:comment>Capital cost of a new hydropower plant. If more than one hydropower technology is modelled, modellers should report capital costs for each represented hydropower technology by adding variables Capital Cost|Electricity|Hydro|2, ... Capital Cost|Electricity|Hydro|N (with N = number of represented technologies). It is modeller's choice which hydropower technologies to assign to type 1 (assigned to the variable without number suffix),2,...,N. The assignment should be documented in the comments sheet. </rdfs:comment>
    <ex:unit>US$2010/kW</ex:unit>
  </rdf:Description>
  <rdf:Description rdf:about="http://transience.eu/ontologies/Cost_Production_Steel_BF_BOF">
    <rdf:type rdf:resource="http://www.w3.org/2002/07/owl#Class"/>
    <rdfs:subClassOf rdf:resource="http://transience.eu/ontologies/Variable"/>
    <rdfs:label>Cost|Production|Steel|BF/BOF</rdfs:label>
    <rdfs:comment>Specific production cost of crude steel in BF/BOF route, including CAPEX (annuity), fixed and variable OPEX</rdfs:comment>
    <ex:unit>Mio â‚¬_2022 / t crude steel</ex:unit>
  </rdf:Description>
  <rdf:Description rdf:about="http://transience.eu/ontologies/Interest_Rate_Real">
    <rdf:type rdf:resource="http://www.w3.org/2002/07/owl#Class"/>
    <rdfs:subClassOf rdf:resource="http://transience.eu/ontologies/Variable"/>
    <rdfs:label>Interest Rate|Real</rdfs:label>
    <rdfs:comment>Real interest rate or return on capital that is relevant for energy system investments</rdfs:comment>
    <ex:unit>%</ex:unit>
  </rdf:Description>
  <rdf:Description rdf:about="http://transience.eu/ontologies/Secondary_Energy_Electricity_Curtailment">
    <rdf:type rdf:resource="http://www.w3.org/2002/07/owl#Class"/>
    <rdfs:subClassOf rdf:resource="http://transience.eu/ontologies/Variable"/>
    <rdfs:label>Secondary Energy|Electricity|Curtailment</rdfs:label>
    <rdfs:comment>curtailment of electricity production due to oversupply from variable renewable sources (typically from wind and solar)</rdfs:comment>
    <ex:unit>EJ/yr</ex:unit>
  </rdf:Description>
  <rdf:Description rdf:about="http://transience.eu/ontologies/Final_Energy_Non-Energy_Use_Chemicals_Liquids_Fossil">
    <rdf:type rdf:resource="http://www.w3.org/2002/07/owl#Class"/>
    <rdfs:subClassOf rdf:resource="http://transience.eu/ontologies/Variable"/>
    <rdfs:label>Final Energy|Non-Energy Use|Chemicals|Liquids|Fossil</rdfs:label>
    <rdfs:comment>Final energy consumption of liquids of fossil origin (conventional &amp; unconventional petroleum, coal-to-liquids, gas-to-liquids)by the chemical sector by the non-combustion processes</rdfs:comment>
    <ex:unit>EJ/yr</ex:unit>
  </rdf:Description>
  <rdf:Description rdf:about="http://transience.eu/ontologies/Secondary_Energy_Liquids">
    <rdf:type rdf:resource="http://www.w3.org/2002/07/owl#Class"/>
    <rdfs:subClassOf rdf:resource="http://transience.eu/ontologies/Variable"/>
    <rdfs:label>Secondary Energy|Liquids</rdfs:label>
    <rdfs:comment>total production of refined liquid fuels from all energy sources (incl. oil products, synthetic fossil fuels from gas and coal, biofuels)</rdfs:comment>
    <ex:unit>EJ/yr</ex:unit>
  </rdf:Description>
  <rdf:Description rdf:about="http://transience.eu/ontologies/Final_Energy_Industry_Chemicals_Gases_Fossil">
    <rdf:type rdf:resource="http://www.w3.org/2002/07/owl#Class"/>
    <rdfs:subClassOf rdf:resource="http://transience.eu/ontologies/Variable"/>
    <rdfs:label>Final Energy|Industry|Chemicals|Gases|Fossil</rdfs:label>
    <rdfs:comment>Final energy consumption of synthetic or derived gases of fossil origin by the chemicals sector</rdfs:comment>
    <ex:unit>EJ/yr</ex:unit>
  </rdf:Description>
  <rdf:Description rdf:about="http://transience.eu/ontologies/Final_Energy_Non-Energy_Use_Chemicals_Liquids">
    <rdf:type rdf:resource="http://www.w3.org/2002/07/owl#Class"/>
    <rdfs:subClassOf rdf:resource="http://transience.eu/ontologies/Variable"/>
    <rdfs:label>Final Energy|Non-Energy Use|Chemicals|Liquids</rdfs:label>
    <rdfs:comment>Final energy consumption of liquids by the chemical sector by the non-combustion processes</rdfs:comment>
    <ex:unit>EJ/yr</ex:unit>
  </rdf:Description>
  <rdf:Description rdf:about="http://transience.eu/ontologies/Production_Steel_Primary_crude_steel_DRI_natural_gas_route">
    <rdf:type rdf:resource="http://www.w3.org/2002/07/owl#Class"/>
    <rdfs:subClassOf rdf:resource="http://transience.eu/ontologies/Variable"/>
    <rdfs:label>Production|Steel|Primary crude steel|DRI natural gas route</rdfs:label>
    <rdfs:comment>Production of primary crude steel in DRI route with natural gas as reducing gas (including both: processing of DRI into steel in EAF and in Smelter/BOF)</rdfs:comment>
    <ex:unit>Mt/yr</ex:unit>
  </rdf:Description>
  <rdf:Description rdf:about="http://transience.eu/ontologies/Final_Energy_Commercial_Gases_Biomass">
    <rdf:type rdf:resource="http://www.w3.org/2002/07/owl#Class"/>
    <rdfs:subClassOf rdf:resource="http://transience.eu/ontologies/Variable"/>
    <rdfs:label>Final Energy|Commercial|Gases|Biomass</rdfs:label>
    <rdfs:comment>final energy consumption by the commercial sector of biogas, excluding transmission/distribution losses</rdfs:comment>
    <ex:unit>EJ/yr</ex:unit>
  </rdf:Description>
  <rdf:Description rdf:about="http://transience.eu/ontologies/Resource_use_Biomass_Industry_Petrochemicals">
    <rdf:type rdf:resource="http://www.w3.org/2002/07/owl#Class"/>
    <rdfs:subClassOf rdf:resource="http://transience.eu/ontologies/Variable"/>
    <rdfs:label>Resource use|Biomass|Industry|Petrochemicals</rdfs:label>
    <rdfs:comment>Use of biomass for non-energetic use including energetic use of by-products; C-content</rdfs:comment>
    <ex:unit>Mt C_eq/yr</ex:unit>
  </rdf:Description>
  <rdf:Description rdf:about="http://transience.eu/ontologies/Emissions_CO2_(w_o_bunkers)">
    <rdf:type rdf:resource="http://www.w3.org/2002/07/owl#Class"/>
    <rdfs:subClassOf rdf:resource="http://transience.eu/ontologies/Variable"/>
    <rdfs:label>Emissions|CO2 (w/o bunkers)</rdfs:label>
    <rdfs:comment>total CO2 emissions excluding emissions from international bunkers (IPCC category 1A3ai and 1A3di) </rdfs:comment>
    <ex:unit>Mt CO2/yr</ex:unit>
  </rdf:Description>
  <rdf:Description rdf:about="http://transience.eu/ontologies/Final_Energy_Residential_Solids_Biomass">
    <rdf:type rdf:resource="http://www.w3.org/2002/07/owl#Class"/>
    <rdfs:subClassOf rdf:resource="http://transience.eu/ontologies/Variable"/>
    <rdfs:label>Final Energy|Residential|Solids|Biomass</rdfs:label>
    <rdfs:comment>final energy solid biomass consumption by the residential sector</rdfs:comment>
    <ex:unit>EJ/yr</ex:unit>
  </rdf:Description>
  <rdf:Description rdf:about="http://transience.eu/ontologies/Investment_Infrastructure_Residential_and_Commercial_High-Efficiency_Buildings">
    <rdf:type rdf:resource="http://www.w3.org/2002/07/owl#Class"/>
    <rdfs:subClassOf rdf:resource="http://transience.eu/ontologies/Variable"/>
    <rdfs:label>Investment|Infrastructure|Residential and Commercial|High-Efficiency Buildings</rdfs:label>
    <rdfs:comment>investment into residential and commercial buildings infrastructure (all types of new buildings that are relatively high in their energy efficiency)</rdfs:comment>
    <ex:unit>billion US$2010/yr</ex:unit>
  </rdf:Description>
  <rdf:Description rdf:about="http://transience.eu/ontologies/Investment_Energy_Supply_Hydrogen_Renewable">
    <rdf:type rdf:resource="http://www.w3.org/2002/07/owl#Class"/>
    <rdfs:subClassOf rdf:resource="http://transience.eu/ontologies/Variable"/>
    <rdfs:label>Investment|Energy Supply|Hydrogen|Renewable</rdfs:label>
    <rdfs:comment>investments for the production of hydrogen from the specified source. For plants equipped with CCS, the investment in the capturing equipment should be included but not the one on transport and storage.</rdfs:comment>
    <ex:unit>billion US$2010/yr</ex:unit>
  </rdf:Description>
  <rdf:Description rdf:about="http://transience.eu/ontologies/Lifetime_Hydrogen_Gas_w__CCS">
    <rdf:type rdf:resource="http://www.w3.org/2002/07/owl#Class"/>
    <rdfs:subClassOf rdf:resource="http://transience.eu/ontologies/Variable"/>
    <rdfs:label>Lifetime|Hydrogen|Gas|w/ CCS</rdfs:label>
    <rdfs:comment>Lifetime of a new gas to hydrogen plant with CCS. Lifetime should be calculated by summing all vintages of a  capacity unit (e.g. (1+1+0.9+0.7+0.5) * 10 years = 41 years) or by the e-folding time for exponential capacity depreciation.  The lifetime should refer to the plant type(s) for which capital costs have been reported. If capital cost for more than one plant type has been reported, modellers should report lifetime for the additional plant types by adding variables Lifetime|Hydrogen|Gas|w/ CCS|2, ... Lifetime|Hydrogen|Gas|w/ CCS|N (matching the assignment of plant types to technologies in the reporting of capital costs as documented in the comments sheet). </rdfs:comment>
    <ex:unit>years</ex:unit>
  </rdf:Description>
  <rdf:Description rdf:about="http://transience.eu/ontologies/Material_intensity_material_car_type">
    <rdf:type rdf:resource="http://www.w3.org/2002/07/owl#Class"/>
    <rdfs:subClassOf rdf:resource="http://transience.eu/ontologies/ParameterInput"/>
    <rdfs:label>Material intensity|[material]|[car type]</rdfs:label>
    <rdfs:comment>Material intensity passenger carsÂ </rdfs:comment>
    <ex:unit>kg/car</ex:unit>
  </rdf:Description>
  <rdf:Description rdf:about="http://transience.eu/ontologies/Emissions_CO2_Energy_Demand_Industry_Non-Ferrous_Metals">
    <rdf:type rdf:resource="http://www.w3.org/2002/07/owl#Class"/>
    <rdfs:subClassOf rdf:resource="http://transience.eu/ontologies/Variable"/>
    <rdfs:label>Emissions|CO2|Energy|Demand|Industry|Non-Ferrous Metals</rdfs:label>
    <rdfs:comment>Fossil CO2 emissions from fuel combustion in industry in the non-ferrous metals sector</rdfs:comment>
    <ex:unit>Mt CO2/yr</ex:unit>
  </rdf:Description>
  <rdf:Description rdf:about="http://transience.eu/ontologies/Unemployment_Rate">
    <rdf:type rdf:resource="http://www.w3.org/2002/07/owl#Class"/>
    <rdfs:subClassOf rdf:resource="http://transience.eu/ontologies/Variable"/>
    <rdfs:label>Unemployment|Rate</rdfs:label>
    <rdfs:comment>Fraction of unemployed inhabitants (based on ILO classification)</rdfs:comment>
    <ex:unit>%</ex:unit>
  </rdf:Description>
  <rdf:Description rdf:about="http://transience.eu/ontologies/Final_Energy_Non-Energy_Use_Liquids_Fossil">
    <rdf:type rdf:resource="http://www.w3.org/2002/07/owl#Class"/>
    <rdfs:subClassOf rdf:resource="http://transience.eu/ontologies/Variable"/>
    <rdfs:label>Final Energy|Non-Energy Use|Liquids|Fossil</rdfs:label>
    <rdfs:comment>Final energy consumption of liquids of fossil origin (conventional &amp; unconventional petroleum, coal-to-liquids, gas-to-liquids)by the non-combustion processes</rdfs:comment>
    <ex:unit>EJ/yr</ex:unit>
  </rdf:Description>
  <rdf:Description rdf:about="http://transience.eu/ontologies/Stock_change_Plastics_Other_demand_sectors_Product_categories">
    <rdf:type rdf:resource="http://www.w3.org/2002/07/owl#Class"/>
    <rdfs:subClassOf rdf:resource="http://transience.eu/ontologies/Variable"/>
    <rdfs:label>Stock change|Plastics|Other|[demand sectors]|[Product categories]</rdfs:label>
    <rdfs:comment>Plastics stock change in other sectorsÂ </rdfs:comment>
    <ex:unit>t/yr</ex:unit>
  </rdf:Description>
  <rdf:Description rdf:about="http://transience.eu/ontologies/Energy_Use_Industry_Petrochemicals_Other_Feedstock">
    <rdf:type rdf:resource="http://www.w3.org/2002/07/owl#Class"/>
    <rdfs:subClassOf rdf:resource="http://transience.eu/ontologies/Variable"/>
    <rdfs:label>Energy Use|Industry|Petrochemicals|Other Feedstock</rdfs:label>
    <rdfs:comment>Use of other feedstock, including both, non-energetic use and energetic use of by-products from feedstock processing</rdfs:comment>
    <ex:unit>Mt/yr</ex:unit>
  </rdf:Description>
  <rdf:Description rdf:about="http://transience.eu/ontologies/Efficiency_Hydrogen_Coal_w__CCS">
    <rdf:type rdf:resource="http://www.w3.org/2002/07/owl#Class"/>
    <rdfs:subClassOf rdf:resource="http://transience.eu/ontologies/Variable"/>
    <rdfs:label>Efficiency|Hydrogen|Coal|w/ CCS</rdfs:label>
    <rdfs:comment>Conversion efficiency (energy content of hydrogen produced per unit of primary energy input) of a new coal to hydrogen plant with CCS. The efficiency should refer to the plant type(s) for which capital costs have been reported. If capital cost for more than one plant type has been reported, modellers should report efficiency for the additional plant types by adding variables Efficiency|Hydrogen|Coal|w/ CCS|2, ... Efficiency|Hydrogen|Coal|w/ CCS|N (matching the assignment of plant types to technologies in the reporting of capital costs as documented in the comments sheet). </rdfs:comment>
    <ex:unit>%</ex:unit>
  </rdf:Description>
  <rdf:Description rdf:about="http://transience.eu/ontologies/Stock_Cars_car_types">
    <rdf:type rdf:resource="http://www.w3.org/2002/07/owl#Class"/>
    <rdfs:subClassOf rdf:resource="http://transience.eu/ontologies/Variable"/>
    <rdfs:subClassOf rdf:resource="http://transience.eu/ontologies/ParameterInput"/>
    <rdfs:label>Stock|Cars|[car types]</rdfs:label>
    <rdfs:comment>Car stock</rdfs:comment>
    <rdfs:comment>Passenger car inflow</rdfs:comment>
    <ex:unit>cars/yr</ex:unit>
    <ex:unit>car</ex:unit>
  </rdf:Description>
  <rdf:Description rdf:about="http://transience.eu/ontologies/Secondary_Energy_Liquids_Gas_w_o_CCS">
    <rdf:type rdf:resource="http://www.w3.org/2002/07/owl#Class"/>
    <rdfs:subClassOf rdf:resource="http://transience.eu/ontologies/Variable"/>
    <rdfs:label>Secondary Energy|Liquids|Gas|w/o CCS</rdfs:label>
    <rdfs:comment>total production of fossil liquid synfuels from gas-to-liquids (GTL) technologies without CCS</rdfs:comment>
    <ex:unit>EJ/yr</ex:unit>
  </rdf:Description>
  <rdf:Description rdf:about="http://transience.eu/ontologies/Efficiency_Hydrogen_Coal_w_o_CCS">
    <rdf:type rdf:resource="http://www.w3.org/2002/07/owl#Class"/>
    <rdfs:subClassOf rdf:resource="http://transience.eu/ontologies/Variable"/>
    <rdfs:label>Efficiency|Hydrogen|Coal|w/o CCS</rdfs:label>
    <rdfs:comment>Conversion efficiency (energy content of hydrogen produced per unit of primary energy input) of a new coal to hydrogen plant w/o CCS. The efficiency should refer to the plant type(s) for which capital costs have been reported. If capital cost for more than one plant type has been reported, modellers should report efficiency for the additional plant types by adding variables Efficiency|Hydrogen|Coal|w/o CCS|2, ... Efficiency|Hydrogen|Coal|w/o CCS|N (matching the assignment of plant types to technologies in the reporting of capital costs as documented in the comments sheet). </rdfs:comment>
    <ex:unit>%</ex:unit>
  </rdf:Description>
  <rdf:Description rdf:about="http://transience.eu/ontologies/Policy_Cost_Equivalent_Variation">
    <rdf:type rdf:resource="http://www.w3.org/2002/07/owl#Class"/>
    <rdfs:subClassOf rdf:resource="http://transience.eu/ontologies/Variable"/>
    <rdfs:label>Policy Cost|Equivalent Variation</rdfs:label>
    <rdfs:comment>equivalent variation associated with the given policy</rdfs:comment>
    <ex:unit>billion US$2010/yr</ex:unit>
  </rdf:Description>
  <rdf:Description rdf:about="http://transience.eu/ontologies/Carbon_Capture_Usage_Gases">
    <rdf:type rdf:resource="http://www.w3.org/2002/07/owl#Class"/>
    <rdfs:subClassOf rdf:resource="http://transience.eu/ontologies/Variable"/>
    <rdfs:label>Carbon Capture|Usage|Gases</rdfs:label>
    <rdfs:comment>total carbon dioxide captured and used in synthetic gases (e.g. as feedstock in industry or for synthetic fuels)</rdfs:comment>
    <ex:unit>Mt CO2/yr</ex:unit>
  </rdf:Description>
  <rdf:Description rdf:about="http://transience.eu/ontologies/Lifetime_Gases_Coal_w__CCS">
    <rdf:type rdf:resource="http://www.w3.org/2002/07/owl#Class"/>
    <rdfs:subClassOf rdf:resource="http://transience.eu/ontologies/Variable"/>
    <rdfs:label>Lifetime|Gases|Coal|w/ CCS</rdfs:label>
    <rdfs:comment>Lifetime of a new coal to gas plant with CCS. Lifetime should be calculated by summing all vintages of a  capacity unit (e.g. (1+1+0.9+0.7+0.5) * 10 years = 41 years) or by the e-folding time for exponential capacity depreciation.  The lifetime should refer to the plant type(s) for which capital costs have been reported. If capital cost for more than one plant type has been reported, modellers should report lifetime for the additional plant types by adding variables Lifetime|Gases|Coal|w/ CCS|2, ... Lifetime|Gases|Coal|w/ CCS|N (matching the assignment of plant types to technologies in the reporting of capital costs as documented in the comments sheet). </rdfs:comment>
    <ex:unit>years</ex:unit>
  </rdf:Description>
  <rdf:Description rdf:about="http://transience.eu/ontologies/Final_Energy_Industry_Other_Sector_Solids_Biomass">
    <rdf:type rdf:resource="http://www.w3.org/2002/07/owl#Class"/>
    <rdfs:subClassOf rdf:resource="http://transience.eu/ontologies/Variable"/>
    <rdfs:label>Final Energy|Industry|Other Sector|Solids|Biomass</rdfs:label>
    <rdfs:comment>Final energy consumption of solid biomass (modern and traditional, including renewable waste) by other industry sectors</rdfs:comment>
    <ex:unit>EJ/yr</ex:unit>
  </rdf:Description>
  <rdf:Description rdf:about="http://transience.eu/ontologies/Expenditure_Government">
    <rdf:type rdf:resource="http://www.w3.org/2002/07/owl#Class"/>
    <rdfs:subClassOf rdf:resource="http://transience.eu/ontologies/Variable"/>
    <rdfs:label>Expenditure|Government</rdfs:label>
    <rdfs:comment>total government expenditure</rdfs:comment>
    <ex:unit>billion US$2010/yr</ex:unit>
  </rdf:Description>
  <rdf:Description rdf:about="http://transience.eu/ontologies/Production_Non-Metallic_Minerals_Cement_Volume">
    <rdf:type rdf:resource="http://www.w3.org/2002/07/owl#Class"/>
    <rdfs:subClassOf rdf:resource="http://transience.eu/ontologies/Variable"/>
    <rdfs:label>Production|Non-Metallic Minerals|Cement|Volume</rdfs:label>
    <rdfs:comment>production of cement</rdfs:comment>
    <ex:unit>Mt/yr</ex:unit>
  </rdf:Description>
  <rdf:Description rdf:about="http://transience.eu/ontologies/Final_Energy_Residential_and_Commercial_Liquids">
    <rdf:type rdf:resource="http://www.w3.org/2002/07/owl#Class"/>
    <rdfs:subClassOf rdf:resource="http://transience.eu/ontologies/Variable"/>
    <rdfs:label>Final Energy|Residential and Commercial|Liquids</rdfs:label>
    <rdfs:comment>final energy consumption by the residential &amp; commercial sector of refined liquids (conventional &amp; unconventional oil, biofuels, coal-to-liquids, gas-to-liquids)</rdfs:comment>
    <ex:unit>EJ/yr</ex:unit>
  </rdf:Description>
  <rdf:Description rdf:about="http://transience.eu/ontologies/Secondary_Energy_Hydrogen_Fossil_w__CCS">
    <rdf:type rdf:resource="http://www.w3.org/2002/07/owl#Class"/>
    <rdfs:subClassOf rdf:resource="http://transience.eu/ontologies/Variable"/>
    <rdfs:label>Secondary Energy|Hydrogen|Fossil|w/ CCS</rdfs:label>
    <rdfs:comment>hydrogen production from fossil fuels with a CO2 capture component</rdfs:comment>
    <ex:unit>EJ/yr</ex:unit>
  </rdf:Description>
  <rdf:Description rdf:about="http://transience.eu/ontologies/Investment_Energy_Supply_Electricity_Gas_w__CCS">
    <rdf:type rdf:resource="http://www.w3.org/2002/07/owl#Class"/>
    <rdfs:subClassOf rdf:resource="http://transience.eu/ontologies/Variable"/>
    <rdfs:label>Investment|Energy Supply|Electricity|Gas|w/ CCS</rdfs:label>
    <rdfs:comment>investments in new power generation for the specified power plant category. If the model features several sub-categories, the total investments should be reported. For plants equipped with CCS, the investment in the capturing equipment should be included but not the one on transport and storage.</rdfs:comment>
    <ex:unit>billion US$2010/yr</ex:unit>
  </rdf:Description>
  <rdf:Description rdf:about="http://transience.eu/ontologies/Energy_Service_Transportation_Freight_Other">
    <rdf:type rdf:resource="http://www.w3.org/2002/07/owl#Class"/>
    <rdfs:subClassOf rdf:resource="http://transience.eu/ontologies/Variable"/>
    <rdfs:label>Energy Service|Transportation|Freight|Other</rdfs:label>
    <rdfs:comment>energy service demand for freight transport using other modes (please provide a definition of the modes in this category in the 'comments' tab)</rdfs:comment>
    <ex:unit>bn tkm/yr</ex:unit>
  </rdf:Description>
  <rdf:Description rdf:about="http://transience.eu/ontologies/Price_Final_Energy_Residential_Solids_Biomass">
    <rdf:type rdf:resource="http://www.w3.org/2002/07/owl#Class"/>
    <rdfs:subClassOf rdf:resource="http://transience.eu/ontologies/Variable"/>
    <rdfs:label>Price|Final Energy|Residential|Solids|Biomass</rdfs:label>
    <rdfs:comment>price for solids from biomass at the final level in the residential sector. Prices should include the effect of carbon prices.</rdfs:comment>
    <ex:unit>US$2010/GJ</ex:unit>
  </rdf:Description>
  <rdf:Description rdf:about="http://transience.eu/ontologies/Secondary_Energy_Liquids_Coal_w_o_CCS">
    <rdf:type rdf:resource="http://www.w3.org/2002/07/owl#Class"/>
    <rdfs:subClassOf rdf:resource="http://transience.eu/ontologies/Variable"/>
    <rdfs:label>Secondary Energy|Liquids|Coal|w/o CCS</rdfs:label>
    <rdfs:comment>total production of fossil liquid synfuels from coal-to-liquids (CTL) technologies without CCS</rdfs:comment>
    <ex:unit>EJ/yr</ex:unit>
  </rdf:Description>
  <rdf:Description rdf:about="http://transience.eu/ontologies/Production_Chemicals_Volume">
    <rdf:type rdf:resource="http://www.w3.org/2002/07/owl#Class"/>
    <rdfs:subClassOf rdf:resource="http://transience.eu/ontologies/Variable"/>
    <rdfs:label>Production|Chemicals|Volume</rdfs:label>
    <rdfs:comment>production of chemicals (e.g. sulfuric acid)</rdfs:comment>
    <ex:unit>Mt/yr</ex:unit>
  </rdf:Description>
  <rdf:Description rdf:about="http://transience.eu/ontologies/Import_Energy">
    <rdf:type rdf:resource="http://www.w3.org/2002/07/owl#Class"/>
    <rdfs:subClassOf rdf:resource="http://transience.eu/ontologies/Variable"/>
    <rdfs:label>Import|Energy</rdfs:label>
    <rdfs:comment>import of energy commodities measured in monetary units.</rdfs:comment>
    <ex:unit>billion US$2010/yr</ex:unit>
  </rdf:Description>
  <rdf:Description rdf:about="http://transience.eu/ontologies/Final_Energy_Non-Energy_Use_Liquids">
    <rdf:type rdf:resource="http://www.w3.org/2002/07/owl#Class"/>
    <rdfs:subClassOf rdf:resource="http://transience.eu/ontologies/Variable"/>
    <rdfs:label>Final Energy|Non-Energy Use|Liquids</rdfs:label>
    <rdfs:comment>final energy consumption of liquids (conventional &amp; unconventional oil, biofuels, coal-to-liquids, gas-to-liquids) by the non-combustion processes</rdfs:comment>
    <ex:unit>EJ/yr</ex:unit>
  </rdf:Description>
  <rdf:Description rdf:about="http://transience.eu/ontologies/Lifetime_Gases_Coal_w_o_CCS">
    <rdf:type rdf:resource="http://www.w3.org/2002/07/owl#Class"/>
    <rdfs:subClassOf rdf:resource="http://transience.eu/ontologies/Variable"/>
    <rdfs:label>Lifetime|Gases|Coal|w/o CCS</rdfs:label>
    <rdfs:comment>Lifetime of a new coal to gas plant w/o CCS. Lifetime should be calculated by summing all vintages of a  capacity unit (e.g. (1+1+0.9+0.7+0.5) * 10 years = 41 years) or by the e-folding time for exponential capacity depreciation.  The lifetime should refer to the plant type(s) for which capital costs have been reported. If capital cost for more than one plant type has been reported, modellers should report lifetime for the additional plant types by adding variables Lifetime|Gases|Coal|w/o CCS|2, ... Lifetime|Gases|Coal|w/o CCS|N (matching the assignment of plant types to technologies in the reporting of capital costs as documented in the comments sheet). </rdfs:comment>
    <ex:unit>years</ex:unit>
  </rdf:Description>
  <rdf:Description rdf:about="http://transience.eu/ontologies/Final_Energy_Non-Energy_Use_Hydrogen">
    <rdf:type rdf:resource="http://www.w3.org/2002/07/owl#Class"/>
    <rdfs:subClassOf rdf:resource="http://transience.eu/ontologies/Variable"/>
    <rdfs:label>Final Energy|Non-Energy Use|Hydrogen</rdfs:label>
    <rdfs:comment>final energy consumption of hydrogen by the non-combustion processes</rdfs:comment>
    <ex:unit>EJ/yr</ex:unit>
  </rdf:Description>
  <rdf:Description rdf:about="http://transience.eu/ontologies/Carbon_Capture_Usage">
    <rdf:type rdf:resource="http://www.w3.org/2002/07/owl#Class"/>
    <rdfs:subClassOf rdf:resource="http://transience.eu/ontologies/Variable"/>
    <rdfs:label>Carbon Capture|Usage</rdfs:label>
    <rdfs:comment>total carbon dioxide captured and used</rdfs:comment>
    <ex:unit>Mt CO2/yr</ex:unit>
  </rdf:Description>
  <rdf:Description rdf:about="http://transience.eu/ontologies/Subsidies_Food">
    <rdf:type rdf:resource="http://www.w3.org/2002/07/owl#Class"/>
    <rdfs:subClassOf rdf:resource="http://transience.eu/ontologies/Variable"/>
    <rdfs:label>Subsidies|Food</rdfs:label>
    <rdfs:comment>Food subsidies (both to producers and consumers)</rdfs:comment>
    <ex:unit>billion US$2010/yr</ex:unit>
  </rdf:Description>
  <rdf:Description rdf:about="http://transience.eu/ontologies/Expenditure_Energy_Fossil">
    <rdf:type rdf:resource="http://www.w3.org/2002/07/owl#Class"/>
    <rdfs:subClassOf rdf:resource="http://transience.eu/ontologies/Variable"/>
    <rdfs:label>Expenditure|Energy|Fossil</rdfs:label>
    <rdfs:comment>Fossil fuel expenditure</rdfs:comment>
    <ex:unit>billion US$2010/yr</ex:unit>
  </rdf:Description>
  <rdf:Description rdf:about="http://transience.eu/ontologies/Final_Energy_Industry_Chemicals_Solids_Coal">
    <rdf:type rdf:resource="http://www.w3.org/2002/07/owl#Class"/>
    <rdfs:subClassOf rdf:resource="http://transience.eu/ontologies/Variable"/>
    <rdfs:label>Final Energy|Industry|Chemicals|Solids|Coal</rdfs:label>
    <rdfs:comment>Final energy consumption of coal by the chemicals sector</rdfs:comment>
    <ex:unit>EJ/yr</ex:unit>
  </rdf:Description>
  <rdf:Description rdf:about="http://transience.eu/ontologies/Gross_Emissions_CO2_Energy_and_Industrial_Processes">
    <rdf:type rdf:resource="http://www.w3.org/2002/07/owl#Class"/>
    <rdfs:subClassOf rdf:resource="http://transience.eu/ontologies/Variable"/>
    <rdfs:label>Gross Emissions|CO2|Energy and Industrial Processes</rdfs:label>
    <rdfs:comment>Gross Fossil CO2 emissions from energy use on supply and demand side (IPCC category 1A, 1B) and from industrial processes (IPCC categories 2A, B, C, E), including emissions from international bunkers, not accounting for negative emissions from BECCS</rdfs:comment>
    <ex:unit>Mt CO2/yr</ex:unit>
  </rdf:Description>
  <rdf:Description rdf:about="http://transience.eu/ontologies/Lifetime_Electricity_Solar_CSP">
    <rdf:type rdf:resource="http://www.w3.org/2002/07/owl#Class"/>
    <rdfs:subClassOf rdf:resource="http://transience.eu/ontologies/Variable"/>
    <rdfs:label>Lifetime|Electricity|Solar|CSP</rdfs:label>
    <rdfs:comment>Lifetime of a new concentrated solar power plant. Lifetime should be calculated by summing all vintages of a  capacity unit (e.g. (1+1+0.9+0.7+0.5) * 10 years = 41 years) or by the e-folding time for exponential capacity depreciation.  The lifetime should refer to the plant type(s) for which capital costs have been reported. If capital cost for more than one plant type has been reported, modellers should report lifetime for the additional plant types by adding variables Lifetime|Electricity|Solar|CSP|2, ... Lifetime|Electricity|Solar|CSP|N (matching the assignment of plant types to technologies in the reporting of capital costs as documented in the comments sheet). </rdfs:comment>
    <ex:unit>years</ex:unit>
  </rdf:Description>
  <rdf:Description rdf:about="http://transience.eu/ontologies/Primary_Energy_Oil_Electricity_w_o_CCS">
    <rdf:type rdf:resource="http://www.w3.org/2002/07/owl#Class"/>
    <rdfs:subClassOf rdf:resource="http://transience.eu/ontologies/Variable"/>
    <rdfs:label>Primary Energy|Oil|Electricity|w/o CCS</rdfs:label>
    <rdfs:comment>conventional &amp; unconventional oil primary energy input to electricity generation without CCS</rdfs:comment>
    <ex:unit>EJ/yr</ex:unit>
  </rdf:Description>
  <rdf:Description rdf:about="http://transience.eu/ontologies/Emissions_CO2_Energy_Demand_Industry_Chemicals">
    <rdf:type rdf:resource="http://www.w3.org/2002/07/owl#Class"/>
    <rdfs:subClassOf rdf:resource="http://transience.eu/ontologies/Variable"/>
    <rdfs:label>Emissions|CO2|Energy|Demand|Industry|Chemicals</rdfs:label>
    <rdfs:comment>Fossil CO2 emissions from fuel combustion in industry in the chemicals sector</rdfs:comment>
    <ex:unit>Mt CO2/yr</ex:unit>
  </rdf:Description>
  <rdf:Description rdf:about="http://transience.eu/ontologies/Carbon_Capture_Biomass_Energy_Supply_Gases">
    <rdf:type rdf:resource="http://www.w3.org/2002/07/owl#Class"/>
    <rdfs:subClassOf rdf:resource="http://transience.eu/ontologies/Variable"/>
    <rdfs:label>Carbon Capture|Biomass|Energy|Supply|Gases</rdfs:label>
    <rdfs:comment>total carbon dioxide emissions captured from bioenergy use in gaseous fuel production, excl. hydrogen (part of IPCC category 1A), should be reported as positive numbers</rdfs:comment>
    <ex:unit>Mt CO2/yr</ex:unit>
  </rdf:Description>
  <rdf:Description rdf:about="http://transience.eu/ontologies/Final_Energy_Industry_Steel_Electricity">
    <rdf:type rdf:resource="http://www.w3.org/2002/07/owl#Class"/>
    <rdfs:subClassOf rdf:resource="http://transience.eu/ontologies/Variable"/>
    <rdfs:label>Final Energy|Industry|Steel|Electricity</rdfs:label>
    <rdfs:comment>Final energy. System boundaries in line with energy accounting</rdfs:comment>
    <ex:unit>PJ/yr</ex:unit>
  </rdf:Description>
  <rdf:Description rdf:about="http://transience.eu/ontologies/Investment_Energy_Demand_Transportation_Passenger_Road_LDV_EV">
    <rdf:type rdf:resource="http://www.w3.org/2002/07/owl#Class"/>
    <rdfs:subClassOf rdf:resource="http://transience.eu/ontologies/Variable"/>
    <rdfs:label>Investment|Energy Demand|Transportation|Passenger|Road|LDV|EV</rdfs:label>
    <rdfs:comment>investments into new vehicle technologies in the transport sector (light-duty cars and trucks: electric vehicle technologies, including all-electrics and plug-in hybrids)</rdfs:comment>
    <ex:unit>billion US$2010/yr</ex:unit>
  </rdf:Description>
  <rdf:Description rdf:about="http://transience.eu/ontologies/Capital_Cost_Liquids_Biomass_w_o_CCS">
    <rdf:type rdf:resource="http://www.w3.org/2002/07/owl#Class"/>
    <rdfs:subClassOf rdf:resource="http://transience.eu/ontologies/Variable"/>
    <rdfs:label>Capital Cost|Liquids|Biomass|w/o CCS</rdfs:label>
    <rdfs:comment>Capital cost of a new biomass to liquids plant w/o CCS. If more than one BTL technology is modelled, modellers should report capital costs for each represented BTL technology by adding variables Capital Cost|Liquids|Biomass|w/o CCS|2, ... Capital Cost|Liquids|Biomass|w/o CCS|N (with N = number of represented technologies). It is modeller's choice which BTL technologies to assign to type 1 (assigned to the variable without number suffix),2,...,N. The assignment should be documented in the comments sheet. </rdfs:comment>
    <ex:unit>US$2010/kW</ex:unit>
  </rdf:Description>
  <rdf:Description rdf:about="http://transience.eu/ontologies/Final_Energy_Non-Energy_Use_Chemicals_Waste">
    <rdf:type rdf:resource="http://www.w3.org/2002/07/owl#Class"/>
    <rdfs:subClassOf rdf:resource="http://transience.eu/ontologies/Variable"/>
    <rdfs:label>Final Energy|Non-Energy Use|Chemicals|Waste</rdfs:label>
    <rdfs:comment>Final energy consumption of non-renewable waste by the chemical sector by the non-combustion processes</rdfs:comment>
    <ex:unit>EJ/yr</ex:unit>
  </rdf:Description>
  <rdf:Description rdf:about="http://transience.eu/ontologies/Import_Industry_Iron_and_Steel_Primary_Steel">
    <rdf:type rdf:resource="http://www.w3.org/2002/07/owl#Class"/>
    <rdfs:subClassOf rdf:resource="http://transience.eu/ontologies/Variable"/>
    <rdfs:label>Import|Industry|Iron and Steel|Primary Steel</rdfs:label>
    <rdfs:comment>Import of primary steel measured in monetary units</rdfs:comment>
    <ex:unit>billion US$2010/yr</ex:unit>
  </rdf:Description>
  <rdf:Description rdf:about="http://transience.eu/ontologies/Emissions_CO2_AFOLU_Land_Positive">
    <rdf:type rdf:resource="http://www.w3.org/2002/07/owl#Class"/>
    <rdfs:subClassOf rdf:resource="http://transience.eu/ontologies/Variable"/>
    <rdfs:label>Emissions|CO2|AFOLU|Land|Positive</rdfs:label>
    <rdfs:comment>positive CO2 emissions from Land Use, Land-Use Change and Forestry (LULUCF), e.g. from deforestation</rdfs:comment>
    <ex:unit>Mt CO2/yr</ex:unit>
  </rdf:Description>
  <rdf:Description rdf:about="http://transience.eu/ontologies/Import_Industry">
    <rdf:type rdf:resource="http://www.w3.org/2002/07/owl#Class"/>
    <rdfs:subClassOf rdf:resource="http://transience.eu/ontologies/Variable"/>
    <rdfs:label>Import|Industry</rdfs:label>
    <rdfs:comment>import of industrial (non-energy) commodities measured in monetary units.</rdfs:comment>
    <ex:unit>billion US$2010/yr</ex:unit>
  </rdf:Description>
  <rdf:Description rdf:about="http://transience.eu/ontologies/Capacity_Petrochemicals_MtO">
    <rdf:type rdf:resource="http://www.w3.org/2002/07/owl#Class"/>
    <rdfs:subClassOf rdf:resource="http://transience.eu/ontologies/Variable"/>
    <rdfs:label>Capacity|Petrochemicals|MtO</rdfs:label>
    <rdfs:comment>Capacity for olefin production in the Methanol-to-olefins routes; the value refers to the amount of methanol input that can be processed per year</rdfs:comment>
    <ex:unit>Mt methanol input / yr</ex:unit>
  </rdf:Description>
  <rdf:Description rdf:about="http://transience.eu/ontologies/Investment_Energy_Supply_Hydrogen">
    <rdf:type rdf:resource="http://www.w3.org/2002/07/owl#Class"/>
    <rdfs:subClassOf rdf:resource="http://transience.eu/ontologies/Variable"/>
    <rdfs:label>Investment|Energy Supply|Hydrogen</rdfs:label>
    <rdfs:comment>investments for the production of hydrogen from all energy sources (fossil, biomass, electrolysis). For plants equipped with CCS, the investment in the capturing equipment should be included but not the one on transport and storage.</rdfs:comment>
    <ex:unit>billion US$2010/yr</ex:unit>
  </rdf:Description>
  <rdf:Description rdf:about="http://transience.eu/ontologies/Final_Energy_Carbon_Removal_Hydrogen">
    <rdf:type rdf:resource="http://www.w3.org/2002/07/owl#Class"/>
    <rdfs:subClassOf rdf:resource="http://transience.eu/ontologies/Variable"/>
    <rdfs:label>Final Energy|Carbon Removal|Hydrogen</rdfs:label>
    <rdfs:comment>Final energy consumption of hydrogen by carbon dioxide removal processes</rdfs:comment>
    <ex:unit>EJ/yr</ex:unit>
  </rdf:Description>
  <rdf:Description rdf:about="http://transience.eu/ontologies/Collected_Scrap_Iron_and_Steel_Other">
    <rdf:type rdf:resource="http://www.w3.org/2002/07/owl#Class"/>
    <rdfs:subClassOf rdf:resource="http://transience.eu/ontologies/Variable"/>
    <rdfs:label>Collected Scrap|Iron and Steel|Other</rdfs:label>
    <rdfs:comment>Collected iron &amp; steel scrap coming from other sectors (available to be used in recycling)</rdfs:comment>
    <ex:unit>Mt/yr</ex:unit>
  </rdf:Description>
  <rdf:Description rdf:about="http://transience.eu/ontologies/Capacity_Electricity_Coal_w__CCS">
    <rdf:type rdf:resource="http://www.w3.org/2002/07/owl#Class"/>
    <rdfs:subClassOf rdf:resource="http://transience.eu/ontologies/Variable"/>
    <rdfs:label>Capacity|Electricity|Coal|w/ CCS</rdfs:label>
    <rdfs:comment>Total installed (available) capacity of coal power plants with CCS, including plants held in an operating reserve. The installed (available) capacity of CCS coal power plants by plant type for which capital costs are reported should be reported by adding variables Capacity|Electricity|Coal|w/ CCS|1, ..., Capacity|Electricity|Coal|w/ CCS|N (matching the assignment of plant types to technologies in the reporting of capital costs as documented in the comments sheet). </rdfs:comment>
    <ex:unit>GW</ex:unit>
  </rdf:Description>
  <rdf:Description rdf:about="http://transience.eu/ontologies/Emissions_CO2_Energy_Supply">
    <rdf:type rdf:resource="http://www.w3.org/2002/07/owl#Class"/>
    <rdfs:subClassOf rdf:resource="http://transience.eu/ontologies/Variable"/>
    <rdfs:label>Emissions|CO2|Energy|Supply</rdfs:label>
    <rdfs:comment>Fossil CO2 emissions from fuel combustion and fugitive emissions from fuels: electricity and heat production and distribution (IPCC category 1A1a), other energy conversion (e.g. refineries, synfuel production, solid fuel processing, IPCC category 1Ab, 1Ac), incl. pipeline transportation (IPCC category 1A3ei), fugitive emissions from fuels (IPCC category 1B) and emissions from carbon dioxide transport and storage (IPCC category 1C), net of negative emissions from Bioenergy with CCS (BECCS), incl. industrial autoproduction</rdfs:comment>
    <ex:unit>Mt CO2/yr</ex:unit>
  </rdf:Description>
  <rdf:Description rdf:about="http://transience.eu/ontologies/Final_Energy_Residential_Hydrogen">
    <rdf:type rdf:resource="http://www.w3.org/2002/07/owl#Class"/>
    <rdfs:subClassOf rdf:resource="http://transience.eu/ontologies/Variable"/>
    <rdfs:label>Final Energy|Residential|Hydrogen</rdfs:label>
    <rdfs:comment>final energy consumption by the residential sector of hydrogen</rdfs:comment>
    <ex:unit>EJ/yr</ex:unit>
  </rdf:Description>
  <rdf:Description rdf:about="http://transience.eu/ontologies/Secondary_Energy_Electricity_Biomass">
    <rdf:type rdf:resource="http://www.w3.org/2002/07/owl#Class"/>
    <rdfs:subClassOf rdf:resource="http://transience.eu/ontologies/Variable"/>
    <rdfs:label>Secondary Energy|Electricity|Biomass</rdfs:label>
    <rdfs:comment>net electricity production from municipal solid waste, purpose-grown biomass, crop residues, forest industry waste, biogas</rdfs:comment>
    <ex:unit>EJ/yr</ex:unit>
  </rdf:Description>
  <rdf:Description rdf:about="http://transience.eu/ontologies/Capital_Cost_Gases_Coal_w_o_CCS">
    <rdf:type rdf:resource="http://www.w3.org/2002/07/owl#Class"/>
    <rdfs:subClassOf rdf:resource="http://transience.eu/ontologies/Variable"/>
    <rdfs:label>Capital Cost|Gases|Coal|w/o CCS</rdfs:label>
    <rdfs:comment>Capital cost of a new coal to gas plant w/o CCS. If more than one coal to gas technology is modelled, modellers should report capital costs for each represented coal to gas technology by adding variables Capital Cost|Gases|Coal|w/o CCS|2, ... Capital Cost|Gases|Coal|w/o CCS|N (with N = number of represented technologies). It is modeller's choice which coal to gas technologies to assign to type 1 (assigned to the variable without number suffix),2,...,N. The assignment should be documented in the comments sheet. </rdfs:comment>
    <ex:unit>US$2010/kW</ex:unit>
  </rdf:Description>
  <rdf:Description rdf:about="http://transience.eu/ontologies/Primary_Energy_Industry_Steel_Coke">
    <rdf:type rdf:resource="http://www.w3.org/2002/07/owl#Class"/>
    <rdfs:subClassOf rdf:resource="http://transience.eu/ontologies/Variable"/>
    <rdfs:label>Primary Energy|Industry|Steel|Coke</rdfs:label>
    <rdfs:comment>Energy demand including own coke ovens and autoproduction of electricity. Imported coke only</rdfs:comment>
    <ex:unit>PJ/yr</ex:unit>
  </rdf:Description>
  <rdf:Description rdf:about="http://transience.eu/ontologies/Expenditure_household_Food">
    <rdf:type rdf:resource="http://www.w3.org/2002/07/owl#Class"/>
    <rdfs:subClassOf rdf:resource="http://transience.eu/ontologies/Variable"/>
    <rdfs:label>Expenditure|household|Food</rdfs:label>
    <rdfs:comment>expenditure of households for food.</rdfs:comment>
    <ex:unit>billion US$2010/yr</ex:unit>
  </rdf:Description>
  <rdf:Description rdf:about="http://transience.eu/ontologies/Carbon_Capture_Biomass_Energy_Supply_Liquids">
    <rdf:type rdf:resource="http://www.w3.org/2002/07/owl#Class"/>
    <rdfs:subClassOf rdf:resource="http://transience.eu/ontologies/Variable"/>
    <rdfs:label>Carbon Capture|Biomass|Energy|Supply|Liquids</rdfs:label>
    <rdfs:comment>total carbon dioxide emissions captured from bioenergy use in liquid fuel production (part of IPCC category 1A), should be reported as positive numbers</rdfs:comment>
    <ex:unit>Mt CO2/yr</ex:unit>
  </rdf:Description>
  <rdf:Description rdf:about="http://transience.eu/ontologies/Production_Cement">
    <rdf:type rdf:resource="http://www.w3.org/2002/07/owl#Class"/>
    <rdfs:subClassOf rdf:resource="http://transience.eu/ontologies/ParameterOutput"/>
    <rdfs:label>Production|Cement</rdfs:label>
    <rdfs:comment>Cement productionÂ </rdfs:comment>
    <ex:unit>t/yr</ex:unit>
  </rdf:Description>
  <rdf:Description rdf:about="http://transience.eu/ontologies/Efficiency_Liquids_Oil">
    <rdf:type rdf:resource="http://www.w3.org/2002/07/owl#Class"/>
    <rdfs:subClassOf rdf:resource="http://transience.eu/ontologies/Variable"/>
    <rdfs:label>Efficiency|Liquids|Oil</rdfs:label>
    <rdfs:comment>Conversion efficiency (energy content of liquids produced per unit of primary energy input) of a new oil refining plant. The efficiency should refer to the plant type(s) for which capital costs have been reported. If capital cost for more than one plant type has been reported, modellers should report efficiency for the additional plant types by adding variables Efficiency|Liquids|Oil|2, ... Efficiency|Electricity|Oil|w/o CCS|N (matching the assignment of plant types to technologies in the reporting of capital costs as documented in the comments sheet). </rdfs:comment>
    <ex:unit>%</ex:unit>
  </rdf:Description>
  <rdf:Description rdf:about="http://transience.eu/ontologies/Carbon_Capture_Industry_Fossil">
    <rdf:type rdf:resource="http://www.w3.org/2002/07/owl#Class"/>
    <rdfs:subClassOf rdf:resource="http://transience.eu/ontologies/Variable"/>
    <rdfs:label>Carbon Capture|Industry|Fossil</rdfs:label>
    <rdfs:comment>total carbon dioxide emissions from fossil fuel use captured in industry sector</rdfs:comment>
    <ex:unit>Mt CO2/yr</ex:unit>
  </rdf:Description>
  <rdf:Description rdf:about="http://transience.eu/ontologies/Final_Energy_Industry_Petrochemicals_High_temperature_heat">
    <rdf:type rdf:resource="http://www.w3.org/2002/07/owl#Class"/>
    <rdfs:subClassOf rdf:resource="http://transience.eu/ontologies/Variable"/>
    <rdfs:label>Final Energy|Industry|Petrochemicals|High temperature heat</rdfs:label>
    <rdfs:comment>Final energy demand of heat &gt; 500 Â°C (to be supplied by heat provision technologies on-site, which are not specified by the model)</rdfs:comment>
    <ex:unit>PJ/yr</ex:unit>
  </rdf:Description>
  <rdf:Description rdf:about="http://transience.eu/ontologies/Outflow_materials_Cars_car_types">
    <rdf:type rdf:resource="http://www.w3.org/2002/07/owl#Class"/>
    <rdfs:subClassOf rdf:resource="http://transience.eu/ontologies/Variable"/>
    <rdfs:label>Outflow|[materials]|Cars|[car types]</rdfs:label>
    <rdfs:comment>Material outflows from carsÂ </rdfs:comment>
    <ex:unit>t/yr</ex:unit>
  </rdf:Description>
  <rdf:Description rdf:about="http://transience.eu/ontologies/Carbon_Capture_Fossil_Energy_Supply_Hydrogen">
    <rdf:type rdf:resource="http://www.w3.org/2002/07/owl#Class"/>
    <rdfs:subClassOf rdf:resource="http://transience.eu/ontologies/Variable"/>
    <rdfs:label>Carbon Capture|Fossil|Energy|Supply|Hydrogen</rdfs:label>
    <rdfs:comment>total carbon dioxide emissions captured from fossil fuel use in hydrogen production (part of IPCC category 1A), should be reported as positive numbers</rdfs:comment>
    <ex:unit>Mt CO2/yr</ex:unit>
  </rdf:Description>
  <rdf:Description rdf:about="http://transience.eu/ontologies/Production_Non-Metallic_Minerals_Cement_Value">
    <rdf:type rdf:resource="http://www.w3.org/2002/07/owl#Class"/>
    <rdfs:subClassOf rdf:resource="http://transience.eu/ontologies/Variable"/>
    <rdfs:label>Production|Non-Metallic Minerals|Cement|Value</rdfs:label>
    <rdfs:comment>Production of cement</rdfs:comment>
    <ex:unit>billion US$2010/yr</ex:unit>
  </rdf:Description>
  <rdf:Description rdf:about="http://transience.eu/ontologies/Efficiency_Gases_Biomass_w__CCS">
    <rdf:type rdf:resource="http://www.w3.org/2002/07/owl#Class"/>
    <rdfs:subClassOf rdf:resource="http://transience.eu/ontologies/Variable"/>
    <rdfs:label>Efficiency|Gases|Biomass|w/ CCS</rdfs:label>
    <rdfs:comment>Conversion efficiency (energy content of gases produced per unit of primary energy input) of a new biomass to gas plant with CCS. The efficiency should refer to the plant type(s) for which capital costs have been reported. If capital cost for more than one plant type has been reported, modellers should report efficiency for the additional plant types by adding variables Efficiency|Gases|Biomass|w/ CCS|2, ... Efficiency|Gases|Biomass|w/ CCS|N (matching the assignment of plant types to technologies in the reporting of capital costs as documented in the comments sheet). </rdfs:comment>
    <ex:unit>%</ex:unit>
  </rdf:Description>
  <rdf:Description rdf:about="http://transience.eu/ontologies/Export_Industry_Chemicals_Plastics">
    <rdf:type rdf:resource="http://www.w3.org/2002/07/owl#Class"/>
    <rdfs:subClassOf rdf:resource="http://transience.eu/ontologies/Variable"/>
    <rdfs:label>Export|Industry|Chemicals|Plastics</rdfs:label>
    <rdfs:comment>Export of plastics measured in monetary units</rdfs:comment>
    <ex:unit>billion US$2010/yr</ex:unit>
  </rdf:Description>
  <rdf:Description rdf:about="http://transience.eu/ontologies/Production_Iron_and_Steel_Iron_Ore_Volume">
    <rdf:type rdf:resource="http://www.w3.org/2002/07/owl#Class"/>
    <rdfs:subClassOf rdf:resource="http://transience.eu/ontologies/Variable"/>
    <rdfs:label>Production|Iron and Steel|Iron Ore|Volume</rdfs:label>
    <rdfs:comment>production of iron ore (raw material used for the production of primary steel and iron)</rdfs:comment>
    <ex:unit>Mt/yr</ex:unit>
  </rdf:Description>
  <rdf:Description rdf:about="http://transience.eu/ontologies/Lifetime_Hydrogen_Coal_w__CCS">
    <rdf:type rdf:resource="http://www.w3.org/2002/07/owl#Class"/>
    <rdfs:subClassOf rdf:resource="http://transience.eu/ontologies/Variable"/>
    <rdfs:label>Lifetime|Hydrogen|Coal|w/ CCS</rdfs:label>
    <rdfs:comment>Lifetime of a new coal to hydrogen plant with CCS. Lifetime should be calculated by summing all vintages of a  capacity unit (e.g. (1+1+0.9+0.7+0.5) * 10 years = 41 years) or by the e-folding time for exponential capacity depreciation.  The lifetime should refer to the plant type(s) for which capital costs have been reported. If capital cost for more than one plant type has been reported, modellers should report lifetime for the additional plant types by adding variables Lifetime|Hydrogen|Coal|w/ CCS|2, ... Lifetime|Hydrogen|Coal|w/ CCS|N (matching the assignment of plant types to technologies in the reporting of capital costs as documented in the comments sheet). </rdfs:comment>
    <ex:unit>years</ex:unit>
  </rdf:Description>
  <rdf:Description rdf:about="http://transience.eu/ontologies/Lifetime_Electricity_Nuclear">
    <rdf:type rdf:resource="http://www.w3.org/2002/07/owl#Class"/>
    <rdfs:subClassOf rdf:resource="http://transience.eu/ontologies/Variable"/>
    <rdfs:label>Lifetime|Electricity|Nuclear</rdfs:label>
    <rdfs:comment>Lifetime of a new nuclear power plant. Lifetime should be calculated by summing all vintages of a  capacity unit (e.g. (1+1+0.9+0.7+0.5) * 10 years = 41 years) or by the e-folding time for exponential capacity depreciation.  The lifetime should refer to the plant type(s) for which capital costs have been reported. If capital cost for more than one plant type has been reported, modellers should report lifetime for the additional plant types by adding variables Lifetime|Electricity|Nuclear|2, ... Lifetime|Electricity|Nuclear|N (matching the assignment of plant types to technologies in the reporting of capital costs as documented in the comments sheet). </rdfs:comment>
    <ex:unit>years</ex:unit>
  </rdf:Description>
  <rdf:Description rdf:about="http://transience.eu/ontologies/Production_Pulp_and_Paper_Volume">
    <rdf:type rdf:resource="http://www.w3.org/2002/07/owl#Class"/>
    <rdfs:subClassOf rdf:resource="http://transience.eu/ontologies/Variable"/>
    <rdfs:label>Production|Pulp and Paper|Volume</rdfs:label>
    <rdfs:comment>production of pulp and paper</rdfs:comment>
    <ex:unit>Mt/yr</ex:unit>
  </rdf:Description>
  <rdf:Description rdf:about="http://transience.eu/ontologies/Final_Energy_Industry_Non-Ferrous_Metals_Gases">
    <rdf:type rdf:resource="http://www.w3.org/2002/07/owl#Class"/>
    <rdfs:subClassOf rdf:resource="http://transience.eu/ontologies/Variable"/>
    <rdfs:label>Final Energy|Industry|Non-Ferrous Metals|Gases</rdfs:label>
    <rdfs:comment>Final energy consumption of gases of the non-ferrous metals sector (natural gas, biogas, coal-gas), excluding transmission/distribution losses</rdfs:comment>
    <ex:unit>EJ/yr</ex:unit>
  </rdf:Description>
  <rdf:Description rdf:about="http://transience.eu/ontologies/Conversion_Input_Electricity_Hydrogen_Autoproduction">
    <rdf:type rdf:resource="http://www.w3.org/2002/07/owl#Class"/>
    <rdfs:subClassOf rdf:resource="http://transience.eu/ontologies/Variable"/>
    <rdfs:label>Conversion Input|Electricity|Hydrogen|Autoproduction</rdfs:label>
    <rdfs:comment>secondary energy consumption of electricity for the autoproduction of hydrogen</rdfs:comment>
    <ex:unit>EJ/yr</ex:unit>
  </rdf:Description>
  <rdf:Description rdf:about="http://transience.eu/ontologies/Inflow_Plastics_Other_demand_sectors_Product_categories">
    <rdf:type rdf:resource="http://www.w3.org/2002/07/owl#Class"/>
    <rdfs:subClassOf rdf:resource="http://transience.eu/ontologies/Variable"/>
    <rdfs:label>Inflow|Plastics|Other|[demand sectors]|[Product categories]</rdfs:label>
    <rdfs:comment>Plastics inflow for other sectorsÂ </rdfs:comment>
    <ex:unit>t/yr</ex:unit>
  </rdf:Description>
  <rdf:Description rdf:about="http://transience.eu/ontologies/Carbon_Capture_Storage_Biomass_Energy_Demand_Industry">
    <rdf:type rdf:resource="http://www.w3.org/2002/07/owl#Class"/>
    <rdfs:subClassOf rdf:resource="http://transience.eu/ontologies/Variable"/>
    <rdfs:label>Carbon Capture|Storage|Biomass|Energy|Demand|Industry</rdfs:label>
    <rdfs:comment>total carbon dioxide emissions captured from bioenergy use in industry (IPCC category 1A2) and stored in geological deposits (e.g. in depleted oil and gas fields, unmined coal seams, saline aquifers) and the deep ocean, stored amounts should be reported as positive numbers</rdfs:comment>
    <ex:unit>Mt CO2/yr</ex:unit>
  </rdf:Description>
  <rdf:Description rdf:about="http://transience.eu/ontologies/Trade_Primary_Energy_Coal_Volume">
    <rdf:type rdf:resource="http://www.w3.org/2002/07/owl#Class"/>
    <rdfs:subClassOf rdf:resource="http://transience.eu/ontologies/Variable"/>
    <rdfs:label>Trade|Primary Energy|Coal|Volume</rdfs:label>
    <rdfs:comment>net exports of coal, at the global level these should add up to the trade losses only</rdfs:comment>
    <ex:unit>EJ/yr</ex:unit>
  </rdf:Description>
  <rdf:Description rdf:about="http://transience.eu/ontologies/Capacity_Electricity_Wind">
    <rdf:type rdf:resource="http://www.w3.org/2002/07/owl#Class"/>
    <rdfs:subClassOf rdf:resource="http://transience.eu/ontologies/Variable"/>
    <rdfs:label>Capacity|Electricity|Wind</rdfs:label>
    <rdfs:comment>Total installed (available) capacity of wind power plants (onshore + offshore). The installed (available) capacity of wind power plants by plant type for which capital costs are reported should be reported by adding variables Capacity|Electricity|Wind|1, ..., Capacity|Electricity|Wind|N (matching the assignment of plant types to technologies in the reporting of capital costs as documented in the comments sheet). </rdfs:comment>
    <ex:unit>GW</ex:unit>
  </rdf:Description>
  <rdf:Description rdf:about="http://transience.eu/ontologies/Tariffs_Average_Imports">
    <rdf:type rdf:resource="http://www.w3.org/2002/07/owl#Class"/>
    <rdfs:subClassOf rdf:resource="http://transience.eu/ontologies/Variable"/>
    <rdfs:label>Tariffs|Average|Imports</rdfs:label>
    <rdfs:comment>Average tariffs for imports (most relevant for developed countries)</rdfs:comment>
    <ex:unit>%</ex:unit>
  </rdf:Description>
  <rdf:Description rdf:about="http://transience.eu/ontologies/Lifetime_Electricity_Hydro">
    <rdf:type rdf:resource="http://www.w3.org/2002/07/owl#Class"/>
    <rdfs:subClassOf rdf:resource="http://transience.eu/ontologies/Variable"/>
    <rdfs:label>Lifetime|Electricity|Hydro</rdfs:label>
    <rdfs:comment>Lifetime of a new hydropower plant. Lifetime should be calculated by summing all vintages of a  capacity unit (e.g. (1+1+0.9+0.7+0.5) * 10 years = 41 years) or by the e-folding time for exponential capacity depreciation.  The lifetime should refer to the plant type(s) for which capital costs have been reported. If capital cost for more than one plant type has been reported, modellers should report lifetime for the additional plant types by adding variables Lifetime|Electricity|Hydro|2, ... Lifetime|Electricity|Hydro|N (matching the assignment of plant types to technologies in the reporting of capital costs as documented in the comments sheet). </rdfs:comment>
    <ex:unit>years</ex:unit>
  </rdf:Description>
  <rdf:Description rdf:about="http://transience.eu/ontologies/Capacity_Electricity_Gas_w_o_CCS">
    <rdf:type rdf:resource="http://www.w3.org/2002/07/owl#Class"/>
    <rdfs:subClassOf rdf:resource="http://transience.eu/ontologies/Variable"/>
    <rdfs:label>Capacity|Electricity|Gas|w/o CCS</rdfs:label>
    <rdfs:comment>Total installed (available) capacity of gas power plants without CCS, including plants held in an operating reserve. The installed (available) capacity of gas power plants by plant type for which capital costs are reported should be reported by adding variables Capacity|Electricity|Gas|w/o CCS|1, ..., Capacity|Electricity|Gas|w/o CCS|N (matching the assignment of plant types to technologies in the reporting of capital costs as documented in the comments sheet). </rdfs:comment>
    <ex:unit>GW</ex:unit>
  </rdf:Description>
  <rdf:Description rdf:about="http://transience.eu/ontologies/OM_Cost_Fixed_Electricity_Wind_Offshore">
    <rdf:type rdf:resource="http://www.w3.org/2002/07/owl#Class"/>
    <rdfs:subClassOf rdf:resource="http://transience.eu/ontologies/Variable"/>
    <rdfs:label>OM Cost|Fixed|Electricity|Wind|Offshore</rdfs:label>
    <rdfs:comment>Annual fixed operation &amp; maintainance cost of a new offshore wind power plants. This variable should only be filled, if wind power is separated into onshore and offshore. If more than one offshore wind power technology is modelled (e.g., wind power units with different hub height and capacity), modellers should report fixed O&amp;M costs  for each represented wind power technology by adding variables OM Cost|Fixed|Electricity|Wind|Offshore|2, ... Capital|Cost|Electricity|Wind|Offshore|N (with N = number of represented offshore wind power technologies) (matching the assignment of plant types to technologies in the reporting of capital costs as documented in the comments sheet).</rdfs:comment>
    <ex:unit>US$2010/kW/yr</ex:unit>
  </rdf:Description>
  <rdf:Description rdf:about="http://transience.eu/ontologies/Final_Energy_Industry_Petrochemicals_Electricity">
    <rdf:type rdf:resource="http://www.w3.org/2002/07/owl#Class"/>
    <rdfs:subClassOf rdf:resource="http://transience.eu/ontologies/Variable"/>
    <rdfs:label>Final Energy|Industry|Petrochemicals|Electricity</rdfs:label>
    <rdfs:comment>Final energy demand. To be supplied by autoproduction in CHP or by external supply </rdfs:comment>
    <ex:unit>PJ/yr</ex:unit>
  </rdf:Description>
  <rdf:Description rdf:about="http://transience.eu/ontologies/Import_Industry_Iron_and_Steel_Volume">
    <rdf:type rdf:resource="http://www.w3.org/2002/07/owl#Class"/>
    <rdfs:subClassOf rdf:resource="http://transience.eu/ontologies/Variable"/>
    <rdfs:label>Import|Industry|Iron and Steel|Volume</rdfs:label>
    <rdfs:comment>Import of iron &amp; steel</rdfs:comment>
    <ex:unit>Mt/yr</ex:unit>
  </rdf:Description>
  <rdf:Description rdf:about="http://transience.eu/ontologies/Production_Iron_and_Steel_Value">
    <rdf:type rdf:resource="http://www.w3.org/2002/07/owl#Class"/>
    <rdfs:subClassOf rdf:resource="http://transience.eu/ontologies/Variable"/>
    <rdfs:label>Production|Iron and Steel|Value</rdfs:label>
    <rdfs:comment>production of steel</rdfs:comment>
    <ex:unit>billion US$2010/yr</ex:unit>
  </rdf:Description>
  <rdf:Description rdf:about="http://transience.eu/ontologies/Efficiency_Hydrogen_Electricity">
    <rdf:type rdf:resource="http://www.w3.org/2002/07/owl#Class"/>
    <rdfs:subClassOf rdf:resource="http://transience.eu/ontologies/Variable"/>
    <rdfs:label>Efficiency|Hydrogen|Electricity</rdfs:label>
    <rdfs:comment>Conversion efficiency (energy content of hydrogen produced per unit of electricity input) of a new hydrogen-by-electrolysis plant. The efficiency should refer to the plant type(s) for which capital costs have been reported. If capital cost for more than one plant type has been reported, modellers should report efficiency for the additional plant types by adding variables Efficiency|Hydrogen|Electricity|2, ... Efficiency|Hydrogen|Electricity|w/ CCS|N (matching the assignment of plant types to technologies in the reporting of capital costs as documented in the comments sheet). </rdfs:comment>
    <ex:unit>%</ex:unit>
  </rdf:Description>
  <rdf:Description rdf:about="http://transience.eu/ontologies/Final_Energy_Industry_Other_Sector_Gases">
    <rdf:type rdf:resource="http://www.w3.org/2002/07/owl#Class"/>
    <rdfs:subClassOf rdf:resource="http://transience.eu/ontologies/Variable"/>
    <rdfs:label>Final Energy|Industry|Other Sector|Gases</rdfs:label>
    <rdfs:comment>Final energy consumption of gases by other industry sectors (natural gas, biogas, coal-gas), excluding transmission/distribution losses</rdfs:comment>
    <ex:unit>EJ/yr</ex:unit>
  </rdf:Description>
  <rdf:Description rdf:about="http://transience.eu/ontologies/Final_Energy_Industry_Other_Sector_Gases_Fossil">
    <rdf:type rdf:resource="http://www.w3.org/2002/07/owl#Class"/>
    <rdfs:subClassOf rdf:resource="http://transience.eu/ontologies/Variable"/>
    <rdfs:label>Final Energy|Industry|Other Sector|Gases|Fossil</rdfs:label>
    <rdfs:comment>Final energy consumption of gases of fossil origin by other industry sectors</rdfs:comment>
    <ex:unit>EJ/yr</ex:unit>
  </rdf:Description>
  <rdf:Description rdf:about="http://transience.eu/ontologies/Production_Iron_and_Steel_Volume">
    <rdf:type rdf:resource="http://www.w3.org/2002/07/owl#Class"/>
    <rdfs:subClassOf rdf:resource="http://transience.eu/ontologies/Variable"/>
    <rdfs:label>Production|Iron and Steel|Volume</rdfs:label>
    <rdfs:comment>production of steel</rdfs:comment>
    <ex:unit>Mt/yr</ex:unit>
  </rdf:Description>
  <rdf:Description rdf:about="http://transience.eu/ontologies/Primary_Energy_Solar">
    <rdf:type rdf:resource="http://www.w3.org/2002/07/owl#Class"/>
    <rdfs:subClassOf rdf:resource="http://transience.eu/ontologies/Variable"/>
    <rdfs:label>Primary Energy|Solar</rdfs:label>
    <rdfs:comment>total solar primary energy consumption</rdfs:comment>
    <ex:unit>EJ/yr</ex:unit>
  </rdf:Description>
  <rdf:Description rdf:about="http://transience.eu/ontologies/Capital_Cost_Gases_Coal_w__CCS">
    <rdf:type rdf:resource="http://www.w3.org/2002/07/owl#Class"/>
    <rdfs:subClassOf rdf:resource="http://transience.eu/ontologies/Variable"/>
    <rdfs:label>Capital Cost|Gases|Coal|w/ CCS</rdfs:label>
    <rdfs:comment>Capital cost of a new coal to gas plant with CCS. If more than one CCS coal to gas technology is modelled, modellers should report capital costs for each represented CCS coal to  gas technology by adding variables Capital Cost|Gases|Coal|w/ CCS|2, ... Capital Cost|Gases|Coal|w/ CCS|N (with N = number of represented technologies). It is modeller's choice which CCS coal to gas technologies to assign to type 1 (assigned to the variable without number suffix),2,...,N. The assignment should be documented in the comments sheet. </rdfs:comment>
    <ex:unit>US$2010/kW</ex:unit>
  </rdf:Description>
  <rdf:Description rdf:about="http://transience.eu/ontologies/Policy_Cost_Other">
    <rdf:type rdf:resource="http://www.w3.org/2002/07/owl#Class"/>
    <rdfs:subClassOf rdf:resource="http://transience.eu/ontologies/Variable"/>
    <rdfs:label>Policy Cost|Other</rdfs:label>
    <rdfs:comment>any other indicator of policy cost (e.g., compensated variation). (please indicate what type of policy cost is measured on the 'comments' tab)</rdfs:comment>
    <ex:unit>billion US$2010/yr</ex:unit>
  </rdf:Description>
  <rdf:Description rdf:about="http://transience.eu/ontologies/Decoupling_demand_sectors">
    <rdf:type rdf:resource="http://www.w3.org/2002/07/owl#Class"/>
    <rdfs:subClassOf rdf:resource="http://transience.eu/ontologies/ParameterInput"/>
    <rdfs:label>Decoupling|[demand sectors]</rdfs:label>
    <rdfs:comment>DecouplingÂ </rdfs:comment>
    <ex:unit>none</ex:unit>
  </rdf:Description>
  <rdf:Description rdf:about="http://transience.eu/ontologies/Capital_Cost_Hydrogen_Gas_w_o_CCS">
    <rdf:type rdf:resource="http://www.w3.org/2002/07/owl#Class"/>
    <rdfs:subClassOf rdf:resource="http://transience.eu/ontologies/Variable"/>
    <rdfs:label>Capital Cost|Hydrogen|Gas|w/o CCS</rdfs:label>
    <rdfs:comment>Capital cost of a new gas to hydrogen plant w/o CCS. If more than one gas to hydrogen technology is modelled, modellers should report capital costs for each represented gas to hydrogen technology by adding variables Capital Cost|Hydrogen|Gas|w/o CCS|2, ... Capital Cost|Hydrogen|Gas|w/o CCS|N (with N = number of represented technologies). It is modeller's choice which gas to hydrogen technologies to assign to type 1 (assigned to the variable without number suffix),2,...,N. The assignment should be documented in the comments sheet. </rdfs:comment>
    <ex:unit>US$2010/kW</ex:unit>
  </rdf:Description>
  <rdf:Description rdf:about="http://transience.eu/ontologies/Capital_Cost_Liquids_Coal_w_o_CCS">
    <rdf:type rdf:resource="http://www.w3.org/2002/07/owl#Class"/>
    <rdfs:subClassOf rdf:resource="http://transience.eu/ontologies/Variable"/>
    <rdfs:label>Capital Cost|Liquids|Coal|w/o CCS</rdfs:label>
    <rdfs:comment>Capital cost of a new coal to liquids plant w/o CCS. If more than one CTL technology is modelled, modellers should report capital costs for each represented CTL technology by adding variables Capital Cost|Liquids|Coal|w/o CCS|2, ... Capital Cost|Liquids|Coal|w/o CCS|N (with N = number of represented technologies). It is modeller's choice which CTL technologies to assign to type 1 (assigned to the variable without number suffix),2,...,N. The assignment should be documented in the comments sheet. </rdfs:comment>
    <ex:unit>US$2010/kW</ex:unit>
  </rdf:Description>
  <rdf:Description rdf:about="http://transience.eu/ontologies/Cost_Production_Steel_DRI_SAF_BOF_NG">
    <rdf:type rdf:resource="http://www.w3.org/2002/07/owl#Class"/>
    <rdfs:subClassOf rdf:resource="http://transience.eu/ontologies/Variable"/>
    <rdfs:label>Cost|Production|Steel|DRI_SAF_BOF_NG</rdfs:label>
    <rdfs:comment>Specific production cost of crude steel in DRI/Smelter/BOF route when using natural gas as reducing gas; including CAPEX (annuity), fixed and variable OPEX</rdfs:comment>
    <ex:unit>Mio â‚¬_2022 / t crude steel</ex:unit>
  </rdf:Description>
  <rdf:Description rdf:about="http://transience.eu/ontologies/Price_Final_Energy_Residential_Solids_Fossil">
    <rdf:type rdf:resource="http://www.w3.org/2002/07/owl#Class"/>
    <rdfs:subClassOf rdf:resource="http://transience.eu/ontologies/Variable"/>
    <rdfs:label>Price|Final Energy|Residential|Solids|Fossil</rdfs:label>
    <rdfs:comment>price for solids from fossils at the final level in the residential sector. Prices should include the effect of carbon prices.</rdfs:comment>
    <ex:unit>US$2010/GJ</ex:unit>
  </rdf:Description>
  <rdf:Description rdf:about="http://transience.eu/ontologies/Final_Energy_Industry_Non-Ferrous_Metals_Gases_Fossil">
    <rdf:type rdf:resource="http://www.w3.org/2002/07/owl#Class"/>
    <rdfs:subClassOf rdf:resource="http://transience.eu/ontologies/Variable"/>
    <rdfs:label>Final Energy|Industry|Non-Ferrous Metals|Gases|Fossil</rdfs:label>
    <rdfs:comment>Final energy consumption of synthetic or derived gases of fossil origin by the non-ferrous metals sector</rdfs:comment>
    <ex:unit>EJ/yr</ex:unit>
  </rdf:Description>
  <rdf:Description rdf:about="http://transience.eu/ontologies/Capital_Cost_Electricity_Biomass_w__CCS">
    <rdf:type rdf:resource="http://www.w3.org/2002/07/owl#Class"/>
    <rdfs:subClassOf rdf:resource="http://transience.eu/ontologies/Variable"/>
    <rdfs:label>Capital Cost|Electricity|Biomass|w/ CCS</rdfs:label>
    <rdfs:comment>Capital cost of a new biomass power plant with CCS. If more than one CCS biomass power technology is modelled, modellers should report capital costs for each represented CCS biomass power technology by adding variables Capital Cost|Electricity|Biomass|w/ CCS|2, ... Capital Cost|Electricity|Biomass|w/ CCS|N (with N = number of represented technologies). It is modeller's choice which CCS biomass power technologies to assign to type 1 (assigned to the variable without number suffix),2,...,N. The assignment should be documented in the comments sheet. </rdfs:comment>
    <ex:unit>US$2010/kW</ex:unit>
  </rdf:Description>
  <rdf:Description rdf:about="http://transience.eu/ontologies/Final_Energy_Non-Energy_Use_Waste">
    <rdf:type rdf:resource="http://www.w3.org/2002/07/owl#Class"/>
    <rdfs:subClassOf rdf:resource="http://transience.eu/ontologies/Variable"/>
    <rdfs:label>Final Energy|Non-Energy Use|Waste</rdfs:label>
    <rdfs:comment>Final energy consumption of non-renewable waste by the non-combustion processes</rdfs:comment>
    <ex:unit>EJ/yr</ex:unit>
  </rdf:Description>
  <rdf:Description rdf:about="http://transience.eu/ontologies/Import_Industry_Non-Ferrous_Metals_Aluminum_Volume">
    <rdf:type rdf:resource="http://www.w3.org/2002/07/owl#Class"/>
    <rdfs:subClassOf rdf:resource="http://transience.eu/ontologies/Variable"/>
    <rdfs:label>Import|Industry|Non-Ferrous Metals|Aluminum|Volume</rdfs:label>
    <rdfs:comment>Import of aluminium</rdfs:comment>
    <ex:unit>Mt/yr</ex:unit>
  </rdf:Description>
  <rdf:Description rdf:about="http://transience.eu/ontologies/Secondary_Energy_Liquids_Coal">
    <rdf:type rdf:resource="http://www.w3.org/2002/07/owl#Class"/>
    <rdfs:subClassOf rdf:resource="http://transience.eu/ontologies/Variable"/>
    <rdfs:label>Secondary Energy|Liquids|Coal</rdfs:label>
    <rdfs:comment>total production of fossil liquid synfuels from coal-to-liquids (CTL) technologies</rdfs:comment>
    <ex:unit>EJ/yr</ex:unit>
  </rdf:Description>
  <rdf:Description rdf:about="http://transience.eu/ontologies/Final_Energy_Carbon_Removal_Gases">
    <rdf:type rdf:resource="http://www.w3.org/2002/07/owl#Class"/>
    <rdfs:subClassOf rdf:resource="http://transience.eu/ontologies/Variable"/>
    <rdfs:label>Final Energy|Carbon Removal|Gases</rdfs:label>
    <rdfs:comment>Final energy consumption of gases by carbon dioxide removal processes</rdfs:comment>
    <ex:unit>EJ/yr</ex:unit>
  </rdf:Description>
  <rdf:Description rdf:about="http://transience.eu/ontologies/Trade_Secondary_Energy_Electricity_Volume">
    <rdf:type rdf:resource="http://www.w3.org/2002/07/owl#Class"/>
    <rdfs:subClassOf rdf:resource="http://transience.eu/ontologies/Variable"/>
    <rdfs:label>Trade|Secondary Energy|Electricity|Volume</rdfs:label>
    <rdfs:comment>net exports of electricity, at the global level these should add up to the trade losses only</rdfs:comment>
    <ex:unit>EJ/yr</ex:unit>
  </rdf:Description>
  <rdf:Description rdf:about="http://transience.eu/ontologies/Primary_Energy_Oil_Electricity_w__CCS">
    <rdf:type rdf:resource="http://www.w3.org/2002/07/owl#Class"/>
    <rdfs:subClassOf rdf:resource="http://transience.eu/ontologies/Variable"/>
    <rdfs:label>Primary Energy|Oil|Electricity|w/ CCS</rdfs:label>
    <rdfs:comment>conventional &amp; unconventional oil primary energy input to electricity generation used in combination with CCS</rdfs:comment>
    <ex:unit>EJ/yr</ex:unit>
  </rdf:Description>
  <rdf:Description rdf:about="http://transience.eu/ontologies/OM_Cost_Fixed_Hydrogen_Gas_w__CCS">
    <rdf:type rdf:resource="http://www.w3.org/2002/07/owl#Class"/>
    <rdfs:subClassOf rdf:resource="http://transience.eu/ontologies/Variable"/>
    <rdfs:label>OM Cost|Fixed|Hydrogen|Gas|w/ CCS</rdfs:label>
    <rdfs:comment>Annual fixed operation &amp; maintainance cost of a new gas to hydrogen plant with CCS. If more than one CCS gas to hydrogen technology is modelled, modellers should report fixed O&amp;M costs  for each represented CCS gas to hydrogen technology by adding variables OM Cost|Fixed|Hydrogen|Gas|w/ CCS|2, ... OM Cost|Fixed|Hydrogen|Gas|w/ CCS|N (with N = number of represented technologies) (matching the assignment of plant types to technologies in the reporting of capital costs as documented in the comments sheet).</rdfs:comment>
    <ex:unit>US$2010/kW/yr</ex:unit>
  </rdf:Description>
  <rdf:Description rdf:about="http://transience.eu/ontologies/Trade_Primary_Energy_Oil_Value">
    <rdf:type rdf:resource="http://www.w3.org/2002/07/owl#Class"/>
    <rdfs:subClassOf rdf:resource="http://transience.eu/ontologies/Variable"/>
    <rdfs:label>Trade|Primary Energy|Oil|Value</rdfs:label>
    <rdfs:comment>value of net exports of crude oil, at the global level these should add up to the trade losses only</rdfs:comment>
    <ex:unit>billion US$2010/yr</ex:unit>
  </rdf:Description>
  <rdf:Description rdf:about="http://transience.eu/ontologies/Investment_Energy_Supply_Heat">
    <rdf:type rdf:resource="http://www.w3.org/2002/07/owl#Class"/>
    <rdfs:subClassOf rdf:resource="http://transience.eu/ontologies/Variable"/>
    <rdfs:label>Investment|Energy Supply|Heat</rdfs:label>
    <rdfs:comment>investments in heat generation facilities</rdfs:comment>
    <ex:unit>billion US$2010/yr</ex:unit>
  </rdf:Description>
  <rdf:Description rdf:about="http://transience.eu/ontologies/Energy_Service_Transportation_Passenger_Road">
    <rdf:type rdf:resource="http://www.w3.org/2002/07/owl#Class"/>
    <rdfs:subClassOf rdf:resource="http://transience.eu/ontologies/Variable"/>
    <rdfs:label>Energy Service|Transportation|Passenger|Road</rdfs:label>
    <rdfs:comment>energy service demand for passenger transport on roads</rdfs:comment>
    <ex:unit>bn pkm/yr</ex:unit>
  </rdf:Description>
  <rdf:Description rdf:about="http://transience.eu/ontologies/Investment_Energy_Supply_Electricity_Oil">
    <rdf:type rdf:resource="http://www.w3.org/2002/07/owl#Class"/>
    <rdfs:subClassOf rdf:resource="http://transience.eu/ontologies/Variable"/>
    <rdfs:label>Investment|Energy Supply|Electricity|Oil</rdfs:label>
    <rdfs:comment>investments in new power generation for the specified power plant category. If the model features several sub-categories, the total investments should be reported. For plants equipped with CCS, the investment in the capturing equipment should be included but not the one on transport and storage.</rdfs:comment>
    <ex:unit>billion US$2010/yr</ex:unit>
  </rdf:Description>
  <rdf:Description rdf:about="http://transience.eu/ontologies/">
    <rdf:type rdf:resource="http://www.w3.org/2002/07/owl#Ontology"/>
  </rdf:Description>
  <rdf:Description rdf:about="http://transience.eu/ontologies/Variable">
    <rdf:type rdf:resource="http://www.w3.org/2002/07/owl#Class"/>
    <rdfs:comment>Base class for all Variables</rdfs:comment>
  </rdf:Description>
  <rdf:Description rdf:about="http://transience.eu/ontologies/Secondary_Energy_Electricity_Biomass_w__CCS">
    <rdf:type rdf:resource="http://www.w3.org/2002/07/owl#Class"/>
    <rdfs:subClassOf rdf:resource="http://transience.eu/ontologies/Variable"/>
    <rdfs:label>Secondary Energy|Electricity|Biomass|w/ CCS</rdfs:label>
    <rdfs:comment>net electricity production from municipal solid waste, purpose-grown biomass, crop residues, forest industry waste with a CO2 capture component</rdfs:comment>
    <ex:unit>EJ/yr</ex:unit>
  </rdf:Description>
  <rdf:Description rdf:about="http://transience.eu/ontologies/Secondary_Energy_Solids">
    <rdf:type rdf:resource="http://www.w3.org/2002/07/owl#Class"/>
    <rdfs:subClassOf rdf:resource="http://transience.eu/ontologies/Variable"/>
    <rdfs:label>Secondary Energy|Solids</rdfs:label>
    <rdfs:comment>solid secondary energy carriers (e.g., briquettes, coke, wood chips, wood pellets)</rdfs:comment>
    <ex:unit>EJ/yr</ex:unit>
  </rdf:Description>
  <rdf:Description rdf:about="http://transience.eu/ontologies/Investment_Energy_Supply_Electricity_Coal">
    <rdf:type rdf:resource="http://www.w3.org/2002/07/owl#Class"/>
    <rdfs:subClassOf rdf:resource="http://transience.eu/ontologies/Variable"/>
    <rdfs:label>Investment|Energy Supply|Electricity|Coal</rdfs:label>
    <rdfs:comment>investments in new power generation for the specified power plant category. If the model features several sub-categories, the total investments should be reported. For plants equipped with CCS, the investment in the capturing equipment should be included but not the one on transport and storage.</rdfs:comment>
    <ex:unit>billion US$2010/yr</ex:unit>
  </rdf:Description>
  <rdf:Description rdf:about="http://transience.eu/ontologies/Final_Energy_Industry_Non-Ferrous_Metals_Heat">
    <rdf:type rdf:resource="http://www.w3.org/2002/07/owl#Class"/>
    <rdfs:subClassOf rdf:resource="http://transience.eu/ontologies/Variable"/>
    <rdfs:label>Final Energy|Industry|Non-Ferrous Metals|Heat</rdfs:label>
    <rdfs:comment>Final energy consumption of centrally supplied heat by the non-ferrous metals sector</rdfs:comment>
    <ex:unit>EJ/yr</ex:unit>
  </rdf:Description>
  <rdf:Description rdf:about="http://transience.eu/ontologies/Primary_Energy_Biomass_w_o_CCS">
    <rdf:type rdf:resource="http://www.w3.org/2002/07/owl#Class"/>
    <rdfs:subClassOf rdf:resource="http://transience.eu/ontologies/Variable"/>
    <rdfs:label>Primary Energy|Biomass|w/o CCS</rdfs:label>
    <rdfs:comment>purpose-grown bioenergy crops, crop and forestry residue bioenergy, municipal solid waste bioenergy, traditional biomass primary energy consumption without CCS</rdfs:comment>
    <ex:unit>EJ/yr</ex:unit>
  </rdf:Description>
  <rdf:Description rdf:about="http://transience.eu/ontologies/Secondary_Energy_Liquids_Biomass_1st_Generation">
    <rdf:type rdf:resource="http://www.w3.org/2002/07/owl#Class"/>
    <rdfs:subClassOf rdf:resource="http://transience.eu/ontologies/Variable"/>
    <rdfs:label>Secondary Energy|Liquids|Biomass|1st Generation</rdfs:label>
    <rdfs:comment>liquid biofuels production from 1st generation technologies, relying on e.g. corn, sugar, oil </rdfs:comment>
    <ex:unit>EJ/yr</ex:unit>
  </rdf:Description>
  <rdf:Description rdf:about="http://transience.eu/ontologies/Secondary_Energy_Liquids_Coal_w__CCS">
    <rdf:type rdf:resource="http://www.w3.org/2002/07/owl#Class"/>
    <rdfs:subClassOf rdf:resource="http://transience.eu/ontologies/Variable"/>
    <rdfs:label>Secondary Energy|Liquids|Coal|w/ CCS</rdfs:label>
    <rdfs:comment>total production of fossil liquid synfuels from coal-to-liquids (CTL) technologies with CCS</rdfs:comment>
    <ex:unit>EJ/yr</ex:unit>
  </rdf:Description>
  <rdf:Description rdf:about="http://transience.eu/ontologies/Production_Steel_DRI_Volume">
    <rdf:type rdf:resource="http://www.w3.org/2002/07/owl#Class"/>
    <rdfs:subClassOf rdf:resource="http://transience.eu/ontologies/Variable"/>
    <rdfs:label>Production|Steel|DRI|Volume</rdfs:label>
    <rdfs:comment>Production of DRI (including DRI which is processed into steel)</rdfs:comment>
    <ex:unit>Mt/yr</ex:unit>
  </rdf:Description>
  <rdf:Description rdf:about="http://transience.eu/ontologies/Stock_Steel_Other_demand_sectors_Product_categories">
    <rdf:type rdf:resource="http://www.w3.org/2002/07/owl#Class"/>
    <rdfs:subClassOf rdf:resource="http://transience.eu/ontologies/Variable"/>
    <rdfs:label>Stock|Steel|Other|[demand sectors]|[Product categories]</rdfs:label>
    <rdfs:comment>Steel stock in other sectorsÂ </rdfs:comment>
    <ex:unit>t/yr</ex:unit>
  </rdf:Description>
  <rdf:Description rdf:about="http://transience.eu/ontologies/Investment_Energy_Supply_Hydrogen_Fossil">
    <rdf:type rdf:resource="http://www.w3.org/2002/07/owl#Class"/>
    <rdfs:subClassOf rdf:resource="http://transience.eu/ontologies/Variable"/>
    <rdfs:label>Investment|Energy Supply|Hydrogen|Fossil</rdfs:label>
    <rdfs:comment>investments for the production of hydrogen from the specified source. For plants equipped with CCS, the investment in the capturing equipment should be included but not the one on transport and storage.</rdfs:comment>
    <ex:unit>billion US$2010/yr</ex:unit>
  </rdf:Description>
  <rdf:Description rdf:about="http://transience.eu/ontologies/Gross_Emissions_CO2_Energy">
    <rdf:type rdf:resource="http://www.w3.org/2002/07/owl#Class"/>
    <rdfs:subClassOf rdf:resource="http://transience.eu/ontologies/Variable"/>
    <rdfs:label>Gross Emissions|CO2|Energy</rdfs:label>
    <rdfs:comment>Gross Fossil CO2 emissions from energy use on supply and demand side (IPCC category 1A, 1B), not accounting for negative emissions from BECCS</rdfs:comment>
    <ex:unit>Mt CO2/yr</ex:unit>
  </rdf:Description>
  <rdf:Description rdf:about="http://transience.eu/ontologies/Price_Final_Energy_Residential_Liquids_Fossil">
    <rdf:type rdf:resource="http://www.w3.org/2002/07/owl#Class"/>
    <rdfs:subClassOf rdf:resource="http://transience.eu/ontologies/Variable"/>
    <rdfs:label>Price|Final Energy|Residential|Liquids|Fossil</rdfs:label>
    <rdfs:comment>fossil liquid fuel (including oil, coal-to-liquids, gas-to-liquids) price at the final level in the residential sector. Prices should include the effect of carbon prices.</rdfs:comment>
    <ex:unit>US$2010/GJ</ex:unit>
  </rdf:Description>
  <rdf:Description rdf:about="http://transience.eu/ontologies/Collected_Scrap_Iron_and_Steel_Power_Sector">
    <rdf:type rdf:resource="http://www.w3.org/2002/07/owl#Class"/>
    <rdfs:subClassOf rdf:resource="http://transience.eu/ontologies/Variable"/>
    <rdfs:label>Collected Scrap|Iron and Steel|Power Sector</rdfs:label>
    <rdfs:comment>Collected iron &amp; steel scrap coming from power sector (available to be used in recycling)</rdfs:comment>
    <ex:unit>Mt/yr</ex:unit>
  </rdf:Description>
  <rdf:Description rdf:about="http://transience.eu/ontologies/Inflow_materials_Cars_car_types">
    <rdf:type rdf:resource="http://www.w3.org/2002/07/owl#Class"/>
    <rdfs:subClassOf rdf:resource="http://transience.eu/ontologies/Variable"/>
    <rdfs:label>Inflow|[materials]|Cars|[car types]</rdfs:label>
    <rdfs:comment>Material inflows for carsÂ </rdfs:comment>
    <ex:unit>t/yr</ex:unit>
  </rdf:Description>
  <rdf:Description rdf:about="http://transience.eu/ontologies/Cost_Production_Steel_DRI_EAF_H2">
    <rdf:type rdf:resource="http://www.w3.org/2002/07/owl#Class"/>
    <rdfs:subClassOf rdf:resource="http://transience.eu/ontologies/Variable"/>
    <rdfs:label>Cost|Production|Steel|DRI_EAF_H2</rdfs:label>
    <rdfs:comment>Specific production cost of crude steel in DRI/EAF route when using hydrogen as reducing gas; including CAPEX (annuity), fixed and variable OPEX</rdfs:comment>
    <ex:unit>Mio â‚¬_2022 / t crude steel</ex:unit>
  </rdf:Description>
  <rdf:Description rdf:about="http://transience.eu/ontologies/Investment_Energy_Supply_Electricity_Non-Biomass_Renewables">
    <rdf:type rdf:resource="http://www.w3.org/2002/07/owl#Class"/>
    <rdfs:subClassOf rdf:resource="http://transience.eu/ontologies/Variable"/>
    <rdfs:label>Investment|Energy Supply|Electricity|Non-Biomass Renewables</rdfs:label>
    <rdfs:comment>investments in new power generation for the specified power plant category. If the model features several sub-categories, the total investments should be reported. For plants equipped with CCS, the investment in the capturing equipment should be included but not the one on transport and storage.</rdfs:comment>
    <ex:unit>billion US$2010/yr</ex:unit>
  </rdf:Description>
  <rdf:Description rdf:about="http://transience.eu/ontologies/Policy_Cost_Additional_Total_Energy_System_Cost">
    <rdf:type rdf:resource="http://www.w3.org/2002/07/owl#Class"/>
    <rdfs:subClassOf rdf:resource="http://transience.eu/ontologies/Variable"/>
    <rdfs:label>Policy Cost|Additional Total Energy System Cost</rdfs:label>
    <rdfs:comment>additional energy system cost associated with the policy</rdfs:comment>
    <ex:unit>billion US$2010/yr</ex:unit>
  </rdf:Description>
  <rdf:Description rdf:about="http://transience.eu/ontologies/Outflow_Steel_Scrap_Types">
    <rdf:type rdf:resource="http://www.w3.org/2002/07/owl#Class"/>
    <rdfs:subClassOf rdf:resource="http://transience.eu/ontologies/ParameterOutput"/>
    <rdfs:label>Outflow|Steel|Scrap|[Types]</rdfs:label>
    <rdfs:comment>Steel scrapÂ </rdfs:comment>
    <ex:unit>t/yr</ex:unit>
  </rdf:Description>
  <rdf:Description rdf:about="http://transience.eu/ontologies/Production_Chemicals_Naphtha_Volume">
    <rdf:type rdf:resource="http://www.w3.org/2002/07/owl#Class"/>
    <rdfs:subClassOf rdf:resource="http://transience.eu/ontologies/Variable"/>
    <rdfs:label>Production|Chemicals|Naphtha|Volume</rdfs:label>
    <rdfs:comment>production of naphtha (raw material for the production of high value chemicals, e.g. olefins)</rdfs:comment>
    <ex:unit>Mt/yr</ex:unit>
  </rdf:Description>
  <rdf:Description rdf:about="http://transience.eu/ontologies/Final_Energy_Industry_Other_Sector_Waste">
    <rdf:type rdf:resource="http://www.w3.org/2002/07/owl#Class"/>
    <rdfs:subClassOf rdf:resource="http://transience.eu/ontologies/Variable"/>
    <rdfs:label>Final Energy|Industry|Other Sector|Waste</rdfs:label>
    <rdfs:comment>Final energy consumption of non-renewable waste by other industry sectors</rdfs:comment>
    <ex:unit>EJ/yr</ex:unit>
  </rdf:Description>
  <rdf:Description rdf:about="http://transience.eu/ontologies/Energy_Service_Transportation_Passenger_Cycling">
    <rdf:type rdf:resource="http://www.w3.org/2002/07/owl#Class"/>
    <rdfs:subClassOf rdf:resource="http://transience.eu/ontologies/Variable"/>
    <rdfs:label>Energy Service|Transportation|Passenger|Cycling</rdfs:label>
    <rdfs:comment>energy service demand for passenger transport on bicycles</rdfs:comment>
    <ex:unit>bn pkm/yr</ex:unit>
  </rdf:Description>
  <rdf:Description rdf:about="http://transience.eu/ontologies/OM_Cost_Fixed_Gases_Coal_w__CCS">
    <rdf:type rdf:resource="http://www.w3.org/2002/07/owl#Class"/>
    <rdfs:subClassOf rdf:resource="http://transience.eu/ontologies/Variable"/>
    <rdfs:label>OM Cost|Fixed|Gases|Coal|w/ CCS</rdfs:label>
    <rdfs:comment>Annual fixed operation &amp; maintainance cost of a new coal to gas plant with CCS. If more than one CCS coal to gas technology is modelled, modellers should report fixed O&amp;M costs  for each represented CCS coal to  gas technology by adding variables OM Cost|Fixed|Gases|Coal|w/ CCS|2, ... OM Cost|Fixed|Gases|Coal|w/ CCS|N (with N = number of represented technologies) (matching the assignment of plant types to technologies in the reporting of capital costs as documented in the comments sheet).</rdfs:comment>
    <ex:unit>US$2010/kW/yr</ex:unit>
  </rdf:Description>
  <rdf:Description rdf:about="http://transience.eu/ontologies/Emissions_GHG_Allowance_Allocation">
    <rdf:type rdf:resource="http://www.w3.org/2002/07/owl#Class"/>
    <rdfs:subClassOf rdf:resource="http://transience.eu/ontologies/Variable"/>
    <rdfs:label>Emissions|GHG|Allowance Allocation</rdfs:label>
    <rdfs:comment>allocation of GHG emission allowances to a region</rdfs:comment>
    <ex:unit>Mt CO2-equiv/yr</ex:unit>
  </rdf:Description>
  <rdf:Description rdf:about="http://transience.eu/ontologies/Export_Industry_Non-Metallic_Minerals_Cement">
    <rdf:type rdf:resource="http://www.w3.org/2002/07/owl#Class"/>
    <rdfs:subClassOf rdf:resource="http://transience.eu/ontologies/Variable"/>
    <rdfs:label>Export|Industry|Non-Metallic Minerals|Cement</rdfs:label>
    <rdfs:comment>Export of cement measured in monetary units</rdfs:comment>
    <ex:unit>billion US$2010/yr</ex:unit>
  </rdf:Description>
  <rdf:Description rdf:about="http://transience.eu/ontologies/Emissions_CO2_AFOLU_Land">
    <rdf:type rdf:resource="http://www.w3.org/2002/07/owl#Class"/>
    <rdfs:subClassOf rdf:resource="http://transience.eu/ontologies/Variable"/>
    <rdfs:label>Emissions|CO2|AFOLU|Land</rdfs:label>
    <rdfs:comment>net CO2 emissions from Land Use, Land-Use Change and Forestry (LULUCF)</rdfs:comment>
    <ex:unit>Mt CO2/yr</ex:unit>
  </rdf:Description>
  <rdf:Description rdf:about="http://transience.eu/ontologies/Final_Energy_Commercial_Solids_Fossil">
    <rdf:type rdf:resource="http://www.w3.org/2002/07/owl#Class"/>
    <rdfs:subClassOf rdf:resource="http://transience.eu/ontologies/Variable"/>
    <rdfs:label>Final Energy|Commercial|Solids|Fossil</rdfs:label>
    <rdfs:comment>final energy consumption of fossil solids by the commercial sector</rdfs:comment>
    <ex:unit>EJ/yr</ex:unit>
  </rdf:Description>
  <rdf:Description rdf:about="http://transience.eu/ontologies/Secondary_Energy_Solids_Fossil">
    <rdf:type rdf:resource="http://www.w3.org/2002/07/owl#Class"/>
    <rdfs:subClassOf rdf:resource="http://transience.eu/ontologies/Variable"/>
    <rdfs:label>Secondary Energy|Solids|Fossil</rdfs:label>
    <rdfs:comment>solid secondary energy carriers produced from fossils (e.g., briquettes, coke)</rdfs:comment>
    <ex:unit>EJ/yr</ex:unit>
  </rdf:Description>
  <rdf:Description rdf:about="http://transience.eu/ontologies/Production_Non-Ferrous_Metals_Alumina_Volume">
    <rdf:type rdf:resource="http://www.w3.org/2002/07/owl#Class"/>
    <rdfs:subClassOf rdf:resource="http://transience.eu/ontologies/Variable"/>
    <rdfs:label>Production|Non-Ferrous Metals|Alumina|Volume</rdfs:label>
    <rdfs:comment>production of alumina (intermediate product for the production of primary aluminum)</rdfs:comment>
    <ex:unit>Mt/yr</ex:unit>
  </rdf:Description>
  <rdf:Description rdf:about="http://transience.eu/ontologies/Trade_Uranium_Mass">
    <rdf:type rdf:resource="http://www.w3.org/2002/07/owl#Class"/>
    <rdfs:subClassOf rdf:resource="http://transience.eu/ontologies/Variable"/>
    <rdfs:label>Trade|Uranium|Mass</rdfs:label>
    <rdfs:comment>net exports of Uranium, at the global level these should add up to the trade losses only</rdfs:comment>
    <ex:unit>kt U/yr</ex:unit>
  </rdf:Description>
  <rdf:Description rdf:about="http://transience.eu/ontologies/Final_Energy_Non-Energy_Use_Other">
    <rdf:type rdf:resource="http://www.w3.org/2002/07/owl#Class"/>
    <rdfs:subClassOf rdf:resource="http://transience.eu/ontologies/Variable"/>
    <rdfs:label>Final Energy|Non-Energy Use|Other</rdfs:label>
    <rdfs:comment>Final energy consumption of other feedstocks by the non-combustion processes (please provide a definition of the feedstocks in this category in the 'comments' tab)</rdfs:comment>
    <ex:unit>EJ/yr</ex:unit>
  </rdf:Description>
  <rdf:Description rdf:about="http://transience.eu/ontologies/Final_Energy_Industry_Iron_and_Steel_Liquids">
    <rdf:type rdf:resource="http://www.w3.org/2002/07/owl#Class"/>
    <rdfs:subClassOf rdf:resource="http://transience.eu/ontologies/Variable"/>
    <rdfs:label>Final Energy|Industry|Iron and Steel|Liquids</rdfs:label>
    <rdfs:comment>Final energy consumption of refined liquids by the iron and steel sector (conventional &amp; unconventional oil, biofuels, coal-to-liquids, gas-to-liquids, efuels)</rdfs:comment>
    <ex:unit>EJ/yr</ex:unit>
  </rdf:Description>
  <rdf:Description rdf:about="http://transience.eu/ontologies/Secondary_Energy_Liquids_Biomass_w__CCS">
    <rdf:type rdf:resource="http://www.w3.org/2002/07/owl#Class"/>
    <rdfs:subClassOf rdf:resource="http://transience.eu/ontologies/Variable"/>
    <rdfs:label>Secondary Energy|Liquids|Biomass|w/ CCS</rdfs:label>
    <rdfs:comment>total production of liquid biofuels from facilities with CCS</rdfs:comment>
    <ex:unit>EJ/yr</ex:unit>
  </rdf:Description>
  <rdf:Description rdf:about="http://transience.eu/ontologies/Final_Energy_Transportation_(w__bunkers)">
    <rdf:type rdf:resource="http://www.w3.org/2002/07/owl#Class"/>
    <rdfs:subClassOf rdf:resource="http://transience.eu/ontologies/Variable"/>
    <rdfs:label>Final Energy|Transportation (w/ bunkers)</rdfs:label>
    <rdfs:comment>final energy consumed in the transportation sector, including bunker fuels, excluding pipelines</rdfs:comment>
    <ex:unit>EJ/yr</ex:unit>
  </rdf:Description>
  <rdf:Description rdf:about="http://transience.eu/ontologies/Stock_change_Concrete_Other_demand_sectors_Product_categories">
    <rdf:type rdf:resource="http://www.w3.org/2002/07/owl#Class"/>
    <rdfs:subClassOf rdf:resource="http://transience.eu/ontologies/Variable"/>
    <rdfs:label>Stock change|Concrete|Other|[demand sectors]|[Product categories]</rdfs:label>
    <rdfs:comment>Concrete stock change in other sectorsÂ </rdfs:comment>
    <ex:unit>t/yr</ex:unit>
  </rdf:Description>
  <rdf:Description rdf:about="http://transience.eu/ontologies/Final_Energy_Residential_and_Commercial_Hydrogen">
    <rdf:type rdf:resource="http://www.w3.org/2002/07/owl#Class"/>
    <rdfs:subClassOf rdf:resource="http://transience.eu/ontologies/Variable"/>
    <rdfs:label>Final Energy|Residential and Commercial|Hydrogen</rdfs:label>
    <rdfs:comment>final energy consumption by the residential &amp; commercial sector of hydrogen</rdfs:comment>
    <ex:unit>EJ/yr</ex:unit>
  </rdf:Description>
  <rdf:Description rdf:about="http://transience.eu/ontologies/Capital_Cost_Electricity_Wind_Offshore">
    <rdf:type rdf:resource="http://www.w3.org/2002/07/owl#Class"/>
    <rdfs:subClassOf rdf:resource="http://transience.eu/ontologies/Variable"/>
    <rdfs:label>Capital Cost|Electricity|Wind|Offshore</rdfs:label>
    <rdfs:comment>Capital cost of a new offshore wind power plants. This variable should only be filled, if wind power is separated into onshore and offshore. If more than one offshore wind power technology is modelled (e.g., wind power units with different hub height and capacity), modellers should report capital costs for each represented wind power technology by adding variables Capital Cost|Electricity|Wind|Offshore|2, ... Capital|Cost|Electricity|Wind|Offshore|N (with N = number of represented offshore wind power technologies). It is modeller's choice which offshore wind power technologies to assign to type 1 (assigned to the variable without number suffix),2,...,N. The assignment should be documented in the comments sheet. </rdfs:comment>
    <ex:unit>US$2010/kW</ex:unit>
  </rdf:Description>
  <rdf:Description rdf:about="http://transience.eu/ontologies/Final_Energy_Residential_Electricity">
    <rdf:type rdf:resource="http://www.w3.org/2002/07/owl#Class"/>
    <rdfs:subClassOf rdf:resource="http://transience.eu/ontologies/Variable"/>
    <rdfs:label>Final Energy|Residential|Electricity</rdfs:label>
    <rdfs:comment>final energy consumption by the residential sector of electricity (including on-site solar PV), excluding transmission/distribution losses</rdfs:comment>
    <ex:unit>EJ/yr</ex:unit>
  </rdf:Description>
  <rdf:Description rdf:about="http://transience.eu/ontologies/Lifetime_Electricity_Coal_w_o_CCS">
    <rdf:type rdf:resource="http://www.w3.org/2002/07/owl#Class"/>
    <rdfs:subClassOf rdf:resource="http://transience.eu/ontologies/Variable"/>
    <rdfs:label>Lifetime|Electricity|Coal|w/o CCS</rdfs:label>
    <rdfs:comment>Lifetime of a new coal power plant w/o CCS. Lifetime should be calculated by summing all vintages of a  capacity unit (e.g. (1+1+0.9+0.7+0.5) * 10 years = 41 years) or by the e-folding time for exponential capacity depreciation.  The lifetime should refer to the plant type(s) for which capital costs have been reported. If capital cost for more than one plant type has been reported, modellers should report lifetime for the additional plant types by adding variables Lifetime|Electricity|Coal|w/o CCS|2, ... Lifetime|Electricity|Coal|w/o CCS|N (matching the assignment of plant types to technologies in the reporting of capital costs as documented in the comments sheet). </rdfs:comment>
    <ex:unit>years</ex:unit>
  </rdf:Description>
  <rdf:Description rdf:about="http://transience.eu/ontologies/Final_Energy_Transportation_Gases">
    <rdf:type rdf:resource="http://www.w3.org/2002/07/owl#Class"/>
    <rdfs:subClassOf rdf:resource="http://transience.eu/ontologies/Variable"/>
    <rdfs:label>Final Energy|Transportation|Gases</rdfs:label>
    <rdfs:comment>final energy consumption by the transportation sector of gases (natural gas, biogas, coal-gas), excluding transmission/distribution losses</rdfs:comment>
    <ex:unit>EJ/yr</ex:unit>
  </rdf:Description>
  <rdf:Description rdf:about="http://transience.eu/ontologies/Final_Energy_Industry_Iron_and_Steel_Gases_Electricity">
    <rdf:type rdf:resource="http://www.w3.org/2002/07/owl#Class"/>
    <rdfs:subClassOf rdf:resource="http://transience.eu/ontologies/Variable"/>
    <rdfs:label>Final Energy|Industry|Iron and Steel|Gases|Electricity</rdfs:label>
    <rdfs:comment>Final energy consumption of synthetic e-fuel gas ("power-to-gas") by the iron and steel sector</rdfs:comment>
    <ex:unit>EJ/yr</ex:unit>
  </rdf:Description>
  <rdf:Description rdf:about="http://transience.eu/ontologies/Carbon_Capture_Storage_Fossil_Energy_Supply_Other">
    <rdf:type rdf:resource="http://www.w3.org/2002/07/owl#Class"/>
    <rdfs:subClassOf rdf:resource="http://transience.eu/ontologies/Variable"/>
    <rdfs:label>Carbon Capture|Storage|Fossil|Energy|Supply|Other</rdfs:label>
    <rdfs:comment>total carbon dioxide emissions captured from fossil fuel use in other energy supply (part of IPCC category 1A) and stored in geological deposits (e.g. in depleted oil and gas fields, unmined coal seams, saline aquifers) and the deep ocean, stored amounts should be reported as positive numbers</rdfs:comment>
    <ex:unit>Mt CO2/yr</ex:unit>
  </rdf:Description>
  <rdf:Description rdf:about="http://transience.eu/ontologies/Emissions_CO2_Industrial_Processes_Pulp_and_Paper">
    <rdf:type rdf:resource="http://www.w3.org/2002/07/owl#Class"/>
    <rdfs:subClassOf rdf:resource="http://transience.eu/ontologies/Variable"/>
    <rdfs:label>Emissions|CO2|Industrial Processes|Pulp and Paper</rdfs:label>
    <rdfs:comment>CO2 emissions from industrial processes from chemicals</rdfs:comment>
    <ex:unit>Mt CO2/yr</ex:unit>
  </rdf:Description>
  <rdf:Description rdf:about="http://transience.eu/ontologies/Investment_Infrastructure_Water_Cooling">
    <rdf:type rdf:resource="http://www.w3.org/2002/07/owl#Class"/>
    <rdfs:subClassOf rdf:resource="http://transience.eu/ontologies/Variable"/>
    <rdfs:label>Investment|Infrastructure|Water|Cooling</rdfs:label>
    <rdfs:comment>investment into water-related infrastructure (thermal cooling at energy and industrial facilities)</rdfs:comment>
    <ex:unit>billion US$2010/yr</ex:unit>
  </rdf:Description>
  <rdf:Description rdf:about="http://transience.eu/ontologies/Final_Energy_Non-Energy_Use_Solids_Biomass">
    <rdf:type rdf:resource="http://www.w3.org/2002/07/owl#Class"/>
    <rdfs:subClassOf rdf:resource="http://transience.eu/ontologies/Variable"/>
    <rdfs:label>Final Energy|Non-Energy Use|Solids|Biomass</rdfs:label>
    <rdfs:comment>Final energy consumption of solid biomass (modern and traditional, including renewable waste) by the non-combustion processes</rdfs:comment>
    <ex:unit>EJ/yr</ex:unit>
  </rdf:Description>
  <rdf:Description rdf:about="http://transience.eu/ontologies/Energy_Service_Bunkers_Freight_International_Aviation">
    <rdf:type rdf:resource="http://www.w3.org/2002/07/owl#Class"/>
    <rdfs:subClassOf rdf:resource="http://transience.eu/ontologies/Variable"/>
    <rdfs:label>Energy Service|Bunkers|Freight|International Aviation</rdfs:label>
    <rdfs:comment>energy service demand for freight transport operating on international aviation routes</rdfs:comment>
    <ex:unit>bn tkm/yr</ex:unit>
  </rdf:Description>
  <rdf:Description rdf:about="http://transience.eu/ontologies/Materials_Demand_Iron_and_Steel_Pre-consumer_Scrap">
    <rdf:type rdf:resource="http://www.w3.org/2002/07/owl#Class"/>
    <rdfs:subClassOf rdf:resource="http://transience.eu/ontologies/Variable"/>
    <rdfs:label>Materials Demand|Iron and Steel|Pre-consumer Scrap</rdfs:label>
    <rdfs:comment>Iron and steel requirments from a certain end-use sector</rdfs:comment>
    <ex:unit>Mt/yr</ex:unit>
  </rdf:Description>
  <rdf:Description rdf:about="http://transience.eu/ontologies/Conversion_Input_Electricity_Heat">
    <rdf:type rdf:resource="http://www.w3.org/2002/07/owl#Class"/>
    <rdfs:subClassOf rdf:resource="http://transience.eu/ontologies/Variable"/>
    <rdfs:label>Conversion Input|Electricity|Heat</rdfs:label>
    <rdfs:comment>secondary energy consumption of electricity for the production of heat (large-scale heat pumps)</rdfs:comment>
    <ex:unit>EJ/yr</ex:unit>
  </rdf:Description>
  <rdf:Description rdf:about="http://transience.eu/ontologies/Investment_Infrastructure_Industry_Non-Green">
    <rdf:type rdf:resource="http://www.w3.org/2002/07/owl#Class"/>
    <rdfs:subClassOf rdf:resource="http://transience.eu/ontologies/Variable"/>
    <rdfs:label>Investment|Infrastructure|Industry|Non-Green</rdfs:label>
    <rdfs:comment>investment into industrial infrastructure (all types of new factories, plants, manufacturing facilities, etc. that are not overly efficient and do not utilize clean energy, as well as retrofits of non-green infrastructure that are neither efficient nor use clean energy)</rdfs:comment>
    <ex:unit>billion US$2010/yr</ex:unit>
  </rdf:Description>
  <rdf:Description rdf:about="http://transience.eu/ontologies/Investment_Infrastructure_Industry_Green">
    <rdf:type rdf:resource="http://www.w3.org/2002/07/owl#Class"/>
    <rdfs:subClassOf rdf:resource="http://transience.eu/ontologies/Variable"/>
    <rdfs:label>Investment|Infrastructure|Industry|Green</rdfs:label>
    <rdfs:comment>investment into industrial infrastructure (all types of new factories, plants, manufacturing facilities, etc. that are more efficient and utilize clean energy, as well as retrofits of non-green infrastructure to be more efficient and use clean energy)</rdfs:comment>
    <ex:unit>billion US$2010/yr</ex:unit>
  </rdf:Description>
  <rdf:Description rdf:about="http://transience.eu/ontologies/Employment">
    <rdf:type rdf:resource="http://www.w3.org/2002/07/owl#Class"/>
    <rdfs:subClassOf rdf:resource="http://transience.eu/ontologies/Variable"/>
    <rdfs:label>Employment</rdfs:label>
    <rdfs:comment>Number of employed inhabitants (based on ILO classification)</rdfs:comment>
    <ex:unit>million</ex:unit>
  </rdf:Description>
  <rdf:Description rdf:about="http://transience.eu/ontologies/OM_Cost_Fixed_Hydrogen_Biomass_w__CCS">
    <rdf:type rdf:resource="http://www.w3.org/2002/07/owl#Class"/>
    <rdfs:subClassOf rdf:resource="http://transience.eu/ontologies/Variable"/>
    <rdfs:label>OM Cost|Fixed|Hydrogen|Biomass|w/ CCS</rdfs:label>
    <rdfs:comment>Annual fixed operation &amp; maintainance cost of a new biomass to hydrogen plant with CCS. If more than one CCS biomass to hydrogen technology is modelled, modellers should report fixed O&amp;M costs  for each represented CCS biomass to hydrogen technology by adding variables OM Cost|Fixed|Hydrogen|Biomass|w/ CCS|2, ... OM Cost|Fixed|Hydrogen|Biomass|w/ CCS|N (with N = number of represented technologies) (matching the assignment of plant types to technologies in the reporting of capital costs as documented in the comments sheet).</rdfs:comment>
    <ex:unit>US$2010/kW/yr</ex:unit>
  </rdf:Description>
  <rdf:Description rdf:about="http://transience.eu/ontologies/Carbon_Capture_Biomass_Energy_Supply_Hydrogen">
    <rdf:type rdf:resource="http://www.w3.org/2002/07/owl#Class"/>
    <rdfs:subClassOf rdf:resource="http://transience.eu/ontologies/Variable"/>
    <rdfs:label>Carbon Capture|Biomass|Energy|Supply|Hydrogen</rdfs:label>
    <rdfs:comment>total carbon dioxide emissions captured from bioenergy use in hydrogen production (part of IPCC category 1A), should be reported as positive numbers</rdfs:comment>
    <ex:unit>Mt CO2/yr</ex:unit>
  </rdf:Description>
  <rdf:Description rdf:about="http://transience.eu/ontologies/Final_Energy_Industry_Pulp_and_Paper_Gases_Fossil">
    <rdf:type rdf:resource="http://www.w3.org/2002/07/owl#Class"/>
    <rdfs:subClassOf rdf:resource="http://transience.eu/ontologies/Variable"/>
    <rdfs:label>Final Energy|Industry|Pulp and Paper|Gases|Fossil</rdfs:label>
    <rdfs:comment>Final energy consumption of synthetic or derived gases of fossil origin by the pulp and paper sector</rdfs:comment>
    <ex:unit>EJ/yr</ex:unit>
  </rdf:Description>
  <rdf:Description rdf:about="http://transience.eu/ontologies/Price_Carbon">
    <rdf:type rdf:resource="http://www.w3.org/2002/07/owl#Class"/>
    <rdfs:subClassOf rdf:resource="http://transience.eu/ontologies/Variable"/>
    <rdfs:label>Price|Carbon</rdfs:label>
    <rdfs:comment>price of carbon (for regional aggregrates the weighted price of carbon by subregion should be used)</rdfs:comment>
    <ex:unit>US$2010/t CO2</ex:unit>
  </rdf:Description>
  <rdf:Description rdf:about="http://transience.eu/ontologies/Efficiency_Electricity_Biomass_w_o_CCS">
    <rdf:type rdf:resource="http://www.w3.org/2002/07/owl#Class"/>
    <rdfs:subClassOf rdf:resource="http://transience.eu/ontologies/Variable"/>
    <rdfs:label>Efficiency|Electricity|Biomass|w/o CCS</rdfs:label>
    <rdfs:comment>Conversion efficiency (electricity produced per unit of primary energy input) of a new biomass power plant w/o CCS. The efficiency should refer to the plant type(s) for which capital costs have been reported. If capital cost for more than one plant type has been reported, modellers should report efficiency for the additional plant types by adding variables Efficiency|Electricity|Biomass|w/o CCS|2, ... Efficiency|Electricity|Biomass|w/o CCS|N (matching the assignment of plant types to technologies in the reporting of capital costs as documented in the comments sheet). </rdfs:comment>
    <ex:unit>%</ex:unit>
  </rdf:Description>
  <rdf:Description rdf:about="http://transience.eu/ontologies/Collected_Scrap_Non-Ferrous_Metals_Transportation">
    <rdf:type rdf:resource="http://www.w3.org/2002/07/owl#Class"/>
    <rdfs:subClassOf rdf:resource="http://transience.eu/ontologies/Variable"/>
    <rdfs:label>Collected Scrap|Non-Ferrous Metals|Transportation</rdfs:label>
    <rdfs:comment>Collected non-ferrous metals scrap coming from transport sector (available to be used in recycling)</rdfs:comment>
    <ex:unit>Mt/yr</ex:unit>
  </rdf:Description>
  <rdf:Description rdf:about="http://transience.eu/ontologies/Import_Industry_Non-Metallic_Minerals_Cement_Volume">
    <rdf:type rdf:resource="http://www.w3.org/2002/07/owl#Class"/>
    <rdfs:subClassOf rdf:resource="http://transience.eu/ontologies/Variable"/>
    <rdfs:label>Import|Industry|Non-Metallic Minerals|Cement|Volume</rdfs:label>
    <rdfs:comment>Import of cement</rdfs:comment>
    <ex:unit>Mt/yr</ex:unit>
  </rdf:Description>
  <rdf:Description rdf:about="http://transience.eu/ontologies/Revenue_government">
    <rdf:type rdf:resource="http://www.w3.org/2002/07/owl#Class"/>
    <rdfs:subClassOf rdf:resource="http://transience.eu/ontologies/Variable"/>
    <rdfs:label>Revenue|government</rdfs:label>
    <rdfs:comment>government revenue</rdfs:comment>
    <ex:unit>billion US$2010/yr</ex:unit>
  </rdf:Description>
  <rdf:Description rdf:about="http://transience.eu/ontologies/Primary_Energy_Coal_Electricity_w_o_CCS">
    <rdf:type rdf:resource="http://www.w3.org/2002/07/owl#Class"/>
    <rdfs:subClassOf rdf:resource="http://transience.eu/ontologies/Variable"/>
    <rdfs:label>Primary Energy|Coal|Electricity|w/o CCS</rdfs:label>
    <rdfs:comment>coal primary energy input to electricity generation  without CCS</rdfs:comment>
    <ex:unit>EJ/yr</ex:unit>
  </rdf:Description>
  <rdf:Description rdf:about="http://transience.eu/ontologies/Cost_Production_Steel_DRI_SAF_BOF_BECCS">
    <rdf:type rdf:resource="http://www.w3.org/2002/07/owl#Class"/>
    <rdfs:subClassOf rdf:resource="http://transience.eu/ontologies/Variable"/>
    <rdfs:label>Cost|Production|Steel|DRI_SAF_BOF_BECCS</rdfs:label>
    <rdfs:comment>Specific production cost of crude steel in DRI/Smelter/BOF route when using biogenic syngas as reducing gas and doing CCS; including CAPEX (annuity), fixed and variable OPEX</rdfs:comment>
    <ex:unit>Mio â‚¬_2022 / t crude steel</ex:unit>
  </rdf:Description>
  <rdf:Description rdf:about="http://transience.eu/ontologies/Final_Energy_Industry_Non-Ferrous_Metals_Gases_Biomass">
    <rdf:type rdf:resource="http://www.w3.org/2002/07/owl#Class"/>
    <rdfs:subClassOf rdf:resource="http://transience.eu/ontologies/Variable"/>
    <rdfs:label>Final Energy|Industry|Non-Ferrous Metals|Gases|Biomass</rdfs:label>
    <rdfs:comment>Final energy consumption of biogas by the non-ferrous metals sector</rdfs:comment>
    <ex:unit>EJ/yr</ex:unit>
  </rdf:Description>
  <rdf:Description rdf:about="http://transience.eu/ontologies/Secondary_Energy_Electricity_Oil_w__CCS">
    <rdf:type rdf:resource="http://www.w3.org/2002/07/owl#Class"/>
    <rdfs:subClassOf rdf:resource="http://transience.eu/ontologies/Variable"/>
    <rdfs:label>Secondary Energy|Electricity|Oil|w/ CCS</rdfs:label>
    <rdfs:comment>net electricity production from refined liquids with a CO2 capture component</rdfs:comment>
    <ex:unit>EJ/yr</ex:unit>
  </rdf:Description>
  <rdf:Description rdf:about="http://transience.eu/ontologies/ParameterOutput">
    <rdf:type rdf:resource="http://www.w3.org/2002/07/owl#Class"/>
    <rdfs:subClassOf rdf:resource="http://transience.eu/ontologies/Parameter"/>
    <rdfs:comment>Parameter Output</rdfs:comment>
  </rdf:Description>
  <rdf:Description rdf:about="http://transience.eu/ontologies/Investment_Energy_Demand_Transportation_Freight_Road_HDT_EV">
    <rdf:type rdf:resource="http://www.w3.org/2002/07/owl#Class"/>
    <rdfs:subClassOf rdf:resource="http://transience.eu/ontologies/Variable"/>
    <rdfs:label>Investment|Energy Demand|Transportation|Freight|Road|HDT|EV</rdfs:label>
    <rdfs:comment>investments into new vehicle technologies in the transport sector (heavy-duty freight trucks: electric vehicle technologies, including all-electrics and plug-in hybrids)</rdfs:comment>
    <ex:unit>billion US$2010/yr</ex:unit>
  </rdf:Description>
  <rdf:Description rdf:about="http://transience.eu/ontologies/Capital_Cost_Hydrogen_Coal_w__CCS">
    <rdf:type rdf:resource="http://www.w3.org/2002/07/owl#Class"/>
    <rdfs:subClassOf rdf:resource="http://transience.eu/ontologies/Variable"/>
    <rdfs:label>Capital Cost|Hydrogen|Coal|w/ CCS</rdfs:label>
    <rdfs:comment>Capital cost of a new coal to hydrogen plant with CCS. If more than one CCS coal to hydrogen technology is modelled, modellers should report capital costs for each represented CCS coal to hydrogen technology by adding variables Capital Cost|Hydrogen|Coal|w/ CCS|2, ... Capital Cost|Hydrogen|Coal|w/ CCS|N (with N = number of represented technologies). It is modeller's choice which CCS coal to hydrogen technologies to assign to type 1 (assigned to the variable without number suffix),2,...,N. The assignment should be documented in the comments sheet. </rdfs:comment>
    <ex:unit>US$2010/kW</ex:unit>
  </rdf:Description>
  <rdf:Description rdf:about="http://transience.eu/ontologies/Emissions_CO2_Industry_Steel">
    <rdf:type rdf:resource="http://www.w3.org/2002/07/owl#Class"/>
    <rdfs:subClassOf rdf:resource="http://transience.eu/ontologies/Variable"/>
    <rdfs:label>Emissions|CO2|Industry|Steel</rdfs:label>
    <rdfs:comment>Net CO2 emissions, including both, energy related and process related emissions</rdfs:comment>
    <ex:unit>Mt CO2/yr</ex:unit>
  </rdf:Description>
  <rdf:Description rdf:about="http://transience.eu/ontologies/Population">
    <rdf:type rdf:resource="http://www.w3.org/2002/07/owl#Class"/>
    <rdfs:subClassOf rdf:resource="http://transience.eu/ontologies/Variable"/>
    <rdfs:label>Population</rdfs:label>
    <rdfs:comment>Total population</rdfs:comment>
    <ex:unit>million</ex:unit>
  </rdf:Description>
  <rdf:Description rdf:about="http://transience.eu/ontologies/Final_Energy_Industry_Non-Ferrous_Metals_Solids">
    <rdf:type rdf:resource="http://www.w3.org/2002/07/owl#Class"/>
    <rdfs:subClassOf rdf:resource="http://transience.eu/ontologies/Variable"/>
    <rdfs:label>Final Energy|Industry|Non-Ferrous Metals|Solids</rdfs:label>
    <rdfs:comment>Final energy consumption of solid fuels of the non-ferrous metals sector (including coal and solid biomass)</rdfs:comment>
    <ex:unit>EJ/yr</ex:unit>
  </rdf:Description>
  <rdf:Description rdf:about="http://transience.eu/ontologies/Final_Energy_Non-Energy_Use_Gases">
    <rdf:type rdf:resource="http://www.w3.org/2002/07/owl#Class"/>
    <rdfs:subClassOf rdf:resource="http://transience.eu/ontologies/Variable"/>
    <rdfs:label>Final Energy|Non-Energy Use|Gases</rdfs:label>
    <rdfs:comment>final energy consumption of gases (natural gas, biogas, coal-gas) by the non-combustion processes</rdfs:comment>
    <ex:unit>EJ/yr</ex:unit>
  </rdf:Description>
  <rdf:Description rdf:about="http://transience.eu/ontologies/Materials_Demand_Non-Ferrous_Metals_Residential_and_Commercial">
    <rdf:type rdf:resource="http://www.w3.org/2002/07/owl#Class"/>
    <rdfs:subClassOf rdf:resource="http://transience.eu/ontologies/Variable"/>
    <rdfs:label>Materials Demand|Non-Ferrous Metals|Residential and Commercial</rdfs:label>
    <rdfs:comment>Non-ferrous metals requirments from a certain end-use sector</rdfs:comment>
    <ex:unit>Mt/yr</ex:unit>
  </rdf:Description>
  <rdf:Description rdf:about="http://transience.eu/ontologies/Final_Energy_Industry_Non-Ferrous_Metals_Hydrogen">
    <rdf:type rdf:resource="http://www.w3.org/2002/07/owl#Class"/>
    <rdfs:subClassOf rdf:resource="http://transience.eu/ontologies/Variable"/>
    <rdfs:label>Final Energy|Industry|Non-Ferrous Metals|Hydrogen</rdfs:label>
    <rdfs:comment>Final energy consumption of hydrogen of the non-ferrous metals sector</rdfs:comment>
    <ex:unit>EJ/yr</ex:unit>
  </rdf:Description>
  <rdf:Description rdf:about="http://transience.eu/ontologies/Final_Energy_Residential_Solids">
    <rdf:type rdf:resource="http://www.w3.org/2002/07/owl#Class"/>
    <rdfs:subClassOf rdf:resource="http://transience.eu/ontologies/Variable"/>
    <rdfs:label>Final Energy|Residential|Solids</rdfs:label>
    <rdfs:comment>final energy solid fuel consumption by the residential sector (including coal and solid biomass)</rdfs:comment>
    <ex:unit>EJ/yr</ex:unit>
  </rdf:Description>
  <rdf:Description rdf:about="http://transience.eu/ontologies/Import_Industry_Iron_and_Steel_Secondary_Steel_Volume">
    <rdf:type rdf:resource="http://www.w3.org/2002/07/owl#Class"/>
    <rdfs:subClassOf rdf:resource="http://transience.eu/ontologies/Variable"/>
    <rdfs:label>Import|Industry|Iron and Steel|Secondary Steel|Volume</rdfs:label>
    <rdfs:comment>Import of secondary steel</rdfs:comment>
    <ex:unit>Mt/yr</ex:unit>
  </rdf:Description>
  <rdf:Description rdf:about="http://transience.eu/ontologies/Primary_Energy_Ocean">
    <rdf:type rdf:resource="http://www.w3.org/2002/07/owl#Class"/>
    <rdfs:subClassOf rdf:resource="http://transience.eu/ontologies/Variable"/>
    <rdfs:label>Primary Energy|Ocean</rdfs:label>
    <rdfs:comment>total ocean primary energy consumption</rdfs:comment>
    <ex:unit>EJ/yr</ex:unit>
  </rdf:Description>
  <rdf:Description rdf:about="http://transience.eu/ontologies/Inflow_materials_Buildings_building_types">
    <rdf:type rdf:resource="http://www.w3.org/2002/07/owl#Class"/>
    <rdfs:subClassOf rdf:resource="http://transience.eu/ontologies/Variable"/>
    <rdfs:label>Inflow|[materials]|Buildings|[building types]</rdfs:label>
    <rdfs:comment>Material inflows for buildingsÂ </rdfs:comment>
    <ex:unit>kg/yr</ex:unit>
  </rdf:Description>
  <rdf:Description rdf:about="http://transience.eu/ontologies/Final_Energy_Industry_Steel_Coke">
    <rdf:type rdf:resource="http://www.w3.org/2002/07/owl#Class"/>
    <rdfs:subClassOf rdf:resource="http://transience.eu/ontologies/Variable"/>
    <rdfs:label>Final Energy|Industry|Steel|Coke</rdfs:label>
    <rdfs:comment>Final energy. System boundaries in line with energy accounting</rdfs:comment>
    <ex:unit>PJ/yr</ex:unit>
  </rdf:Description>
  <rdf:Description rdf:about="http://transience.eu/ontologies/Final_Energy_Industry_Pulp_and_Paper">
    <rdf:type rdf:resource="http://www.w3.org/2002/07/owl#Class"/>
    <rdfs:subClassOf rdf:resource="http://transience.eu/ontologies/Variable"/>
    <rdfs:label>Final Energy|Industry|Pulp and Paper</rdfs:label>
    <rdfs:comment>Final energy consumption of the pulp and paper sector</rdfs:comment>
    <ex:unit>EJ/yr</ex:unit>
  </rdf:Description>
  <rdf:Description rdf:about="http://transience.eu/ontologies/Carbon_Sequestration_CCS_Fossil_Industry_Steel">
    <rdf:type rdf:resource="http://www.w3.org/2002/07/owl#Class"/>
    <rdfs:subClassOf rdf:resource="http://transience.eu/ontologies/Variable"/>
    <rdfs:label>Carbon Sequestration|CCS|Fossil|Industry|Steel</rdfs:label>
    <rdfs:comment>Fossil CO2 captured and stored</rdfs:comment>
    <ex:unit>Mt CO2/yr</ex:unit>
  </rdf:Description>
  <rdf:Description rdf:about="http://transience.eu/ontologies/Final_Energy_Residential_Liquids">
    <rdf:type rdf:resource="http://www.w3.org/2002/07/owl#Class"/>
    <rdfs:subClassOf rdf:resource="http://transience.eu/ontologies/Variable"/>
    <rdfs:label>Final Energy|Residential|Liquids</rdfs:label>
    <rdfs:comment>final energy consumption by the residential sector of refined liquids (conventional &amp; unconventional oil, biofuels, coal-to-liquids, gas-to-liquids)</rdfs:comment>
    <ex:unit>EJ/yr</ex:unit>
  </rdf:Description>
  <rdf:Description rdf:about="http://transience.eu/ontologies/Final_Energy_Industry_Non-Ferrous_Metals_Other">
    <rdf:type rdf:resource="http://www.w3.org/2002/07/owl#Class"/>
    <rdfs:subClassOf rdf:resource="http://transience.eu/ontologies/Variable"/>
    <rdfs:label>Final Energy|Industry|Non-Ferrous Metals|Other</rdfs:label>
    <rdfs:comment>Final energy consumption of other energy carriers by the non-ferrous metals sector (please provide a definition of the energy carriers in this category in the 'comments' tab)</rdfs:comment>
    <ex:unit>EJ/yr</ex:unit>
  </rdf:Description>
  <rdf:Description rdf:about="http://transience.eu/ontologies/Carbon_Capture_Other">
    <rdf:type rdf:resource="http://www.w3.org/2002/07/owl#Class"/>
    <rdfs:subClassOf rdf:resource="http://transience.eu/ontologies/Variable"/>
    <rdfs:label>Carbon Capture|Other</rdfs:label>
    <rdfs:comment>total carbon dioxide captured through other techniques  (please provide a definition of other sources in this category in the 'comments' tab)</rdfs:comment>
    <ex:unit>Mt CO2/yr</ex:unit>
  </rdf:Description>
  <rdf:Description rdf:about="http://transience.eu/ontologies/Energy_Use_Industry_Petrochemicals_Hydrogen">
    <rdf:type rdf:resource="http://www.w3.org/2002/07/owl#Class"/>
    <rdfs:subClassOf rdf:resource="http://transience.eu/ontologies/Variable"/>
    <rdfs:label>Energy Use|Industry|Petrochemicals|Hydrogen</rdfs:label>
    <rdfs:comment>Use of hydrogen, including both, non-energetic use and energetic use of by-products of hydrogen processing</rdfs:comment>
    <ex:unit>Mt/yr</ex:unit>
  </rdf:Description>
  <rdf:Description rdf:about="http://transience.eu/ontologies/Unemployment">
    <rdf:type rdf:resource="http://www.w3.org/2002/07/owl#Class"/>
    <rdfs:subClassOf rdf:resource="http://transience.eu/ontologies/Variable"/>
    <rdfs:label>Unemployment</rdfs:label>
    <rdfs:comment>Number of unemployed inhabitants (based on ILO classification)</rdfs:comment>
    <ex:unit>million</ex:unit>
  </rdf:Description>
  <rdf:Description rdf:about="http://transience.eu/ontologies/Secondary_Energy_Liquids_Oil">
    <rdf:type rdf:resource="http://www.w3.org/2002/07/owl#Class"/>
    <rdfs:subClassOf rdf:resource="http://transience.eu/ontologies/Variable"/>
    <rdfs:label>Secondary Energy|Liquids|Oil</rdfs:label>
    <rdfs:comment>total production of liquid fuels from petroleum, including both conventional and unconventional sources</rdfs:comment>
    <ex:unit>EJ/yr</ex:unit>
  </rdf:Description>
  <rdf:Description rdf:about="http://transience.eu/ontologies/OM_Cost_Fixed_Electricity_Hydro">
    <rdf:type rdf:resource="http://www.w3.org/2002/07/owl#Class"/>
    <rdfs:subClassOf rdf:resource="http://transience.eu/ontologies/Variable"/>
    <rdfs:label>OM Cost|Fixed|Electricity|Hydro</rdfs:label>
    <rdfs:comment>Annual fixed operation &amp; maintainance cost of a new hydropower plant. If more than one hydropower technology is modelled, modellers should report fixed O&amp;M costs  for each represented hydropower technology by adding variables OM Cost|Fixed|Electricity|Hydro|2, ... OM Cost|Fixed|Electricity|Hydro|N (with N = number of represented technologies) (matching the assignment of plant types to technologies in the reporting of capital costs as documented in the comments sheet).</rdfs:comment>
    <ex:unit>US$2010/kW/yr</ex:unit>
  </rdf:Description>
  <rdf:Description rdf:about="http://transience.eu/ontologies/Carbon_Capture_Storage">
    <rdf:type rdf:resource="http://www.w3.org/2002/07/owl#Class"/>
    <rdfs:subClassOf rdf:resource="http://transience.eu/ontologies/Variable"/>
    <rdfs:label>Carbon Capture|Storage</rdfs:label>
    <rdfs:comment>total carbon dioxide emissions captured and stored in geological deposits (e.g. in depleted oil and gas fields, unmined coal seams, saline aquifers) and the deep ocean, stored amounts should be reported as positive numbers</rdfs:comment>
    <ex:unit>Mt CO2/yr</ex:unit>
  </rdf:Description>
  <rdf:Description rdf:about="http://transience.eu/ontologies/Carbon_Capture_Fossil_Energy_Supply_Gases">
    <rdf:type rdf:resource="http://www.w3.org/2002/07/owl#Class"/>
    <rdfs:subClassOf rdf:resource="http://transience.eu/ontologies/Variable"/>
    <rdfs:label>Carbon Capture|Fossil|Energy|Supply|Gases</rdfs:label>
    <rdfs:comment>total carbon dioxide emissions captured from fossil fuel use in gaseous fuel production, excl. hydrogen (part of IPCC category 1A), should be reported as positive numbers</rdfs:comment>
    <ex:unit>Mt CO2/yr</ex:unit>
  </rdf:Description>
  <rdf:Description rdf:about="http://transience.eu/ontologies/Investment_Energy_Demand_Transportation_Passenger_Road_LDV_FCV">
    <rdf:type rdf:resource="http://www.w3.org/2002/07/owl#Class"/>
    <rdfs:subClassOf rdf:resource="http://transience.eu/ontologies/Variable"/>
    <rdfs:label>Investment|Energy Demand|Transportation|Passenger|Road|LDV|FCV</rdfs:label>
    <rdfs:comment>investments into new vehicle technologies in the transport sector (light-duty cars and trucks: fuel cell technologies running on hydrogen or another type of fuel)</rdfs:comment>
    <ex:unit>billion US$2010/yr</ex:unit>
  </rdf:Description>
  <rdf:Description rdf:about="http://transience.eu/ontologies/Conversion_Input_Hydrogen_Electricity">
    <rdf:type rdf:resource="http://www.w3.org/2002/07/owl#Class"/>
    <rdfs:subClassOf rdf:resource="http://transience.eu/ontologies/Variable"/>
    <rdfs:label>Conversion Input|Hydrogen|Electricity</rdfs:label>
    <rdfs:comment>secondary energy consumption of hydrogen for the production of electricity</rdfs:comment>
    <ex:unit>EJ/yr</ex:unit>
  </rdf:Description>
  <rdf:Description rdf:about="http://transience.eu/ontologies/Final_Energy_Residential">
    <rdf:type rdf:resource="http://www.w3.org/2002/07/owl#Class"/>
    <rdfs:subClassOf rdf:resource="http://transience.eu/ontologies/Variable"/>
    <rdfs:label>Final Energy|Residential</rdfs:label>
    <rdfs:comment>final energy consumed in the residential sector</rdfs:comment>
    <ex:unit>EJ/yr</ex:unit>
  </rdf:Description>
  <rdf:Description rdf:about="http://transience.eu/ontologies/Efficiency_Electricity_Gas_w__CCS">
    <rdf:type rdf:resource="http://www.w3.org/2002/07/owl#Class"/>
    <rdfs:subClassOf rdf:resource="http://transience.eu/ontologies/Variable"/>
    <rdfs:label>Efficiency|Electricity|Gas|w/ CCS</rdfs:label>
    <rdfs:comment>Conversion efficiency (electricity produced per unit of primary energy input) of a new gas power plant with CCS. The efficiency should refer to the plant type(s) for which capital costs have been reported. If capital cost for more than one plant type has been reported, modellers should report efficiency for the additional plant types by adding variables Efficiency|Electricity|Gas|w/ CCS|2, ... Efficiency|Electricity|Gas|w/ CCS|N (matching the assignment of plant types to technologies in the reporting of capital costs as documented in the comments sheet). </rdfs:comment>
    <ex:unit>%</ex:unit>
  </rdf:Description>
  <rdf:Description rdf:about="http://transience.eu/ontologies/Trade_Secondary_Energy_Liquids_Biomass_Value">
    <rdf:type rdf:resource="http://www.w3.org/2002/07/owl#Class"/>
    <rdfs:subClassOf rdf:resource="http://transience.eu/ontologies/Variable"/>
    <rdfs:label>Trade|Secondary Energy|Liquids|Biomass|Value</rdfs:label>
    <rdfs:comment>value of net exports of liquid biofuels, at the global level these should add up to the trade losses only (for those models that are able to split solid and liquid bioenergy)</rdfs:comment>
    <ex:unit>EJ/yr</ex:unit>
  </rdf:Description>
  <rdf:Description rdf:about="http://transience.eu/ontologies/Primary_Energy_Biomass_w__CCS">
    <rdf:type rdf:resource="http://www.w3.org/2002/07/owl#Class"/>
    <rdfs:subClassOf rdf:resource="http://transience.eu/ontologies/Variable"/>
    <rdfs:label>Primary Energy|Biomass|w/ CCS</rdfs:label>
    <rdfs:comment>purpose-grown bioenergy crops, crop and forestry residue bioenergy, municipal solid waste bioenergy, traditional biomass primary energy consumption used in combination with CCS</rdfs:comment>
    <ex:unit>EJ/yr</ex:unit>
  </rdf:Description>
  <rdf:Description rdf:about="http://transience.eu/ontologies/Secondary_Energy_Electricity_Fossil_w_o_CCS">
    <rdf:type rdf:resource="http://www.w3.org/2002/07/owl#Class"/>
    <rdfs:subClassOf rdf:resource="http://transience.eu/ontologies/Variable"/>
    <rdfs:label>Secondary Energy|Electricity|Fossil|w/o CCS</rdfs:label>
    <rdfs:comment>net electricity production from coal, gas, conventional and unconventional oil without CCS</rdfs:comment>
    <ex:unit>EJ/yr</ex:unit>
  </rdf:Description>
  <rdf:Description rdf:about="http://transience.eu/ontologies/Capacity_Steel_blast_furnace">
    <rdf:type rdf:resource="http://www.w3.org/2002/07/owl#Class"/>
    <rdfs:subClassOf rdf:resource="http://transience.eu/ontologies/Variable"/>
    <rdfs:label>Capacity|Steel|blast furnace</rdfs:label>
    <rdfs:comment>Capacity of blast furnace for iron production in Mt iron / year</rdfs:comment>
    <ex:unit>Mt/yr</ex:unit>
  </rdf:Description>
  <rdf:Description rdf:about="http://transience.eu/ontologies/Primary_Energy_Wind">
    <rdf:type rdf:resource="http://www.w3.org/2002/07/owl#Class"/>
    <rdfs:subClassOf rdf:resource="http://transience.eu/ontologies/Variable"/>
    <rdfs:label>Primary Energy|Wind</rdfs:label>
    <rdfs:comment>total wind primary energy consumption</rdfs:comment>
    <ex:unit>EJ/yr</ex:unit>
  </rdf:Description>
  <rdf:Description rdf:about="http://transience.eu/ontologies/Emissions_CO2_Industrial_Processes_Chemicals">
    <rdf:type rdf:resource="http://www.w3.org/2002/07/owl#Class"/>
    <rdfs:subClassOf rdf:resource="http://transience.eu/ontologies/Variable"/>
    <rdfs:label>Emissions|CO2|Industrial Processes|Chemicals</rdfs:label>
    <rdfs:comment>CO2 emissions from industrial processes from chemicals</rdfs:comment>
    <ex:unit>Mt CO2/yr</ex:unit>
  </rdf:Description>
  <rdf:Description rdf:about="http://transience.eu/ontologies/Final_Energy_Carbon_Removal_Direct_Air_Capture">
    <rdf:type rdf:resource="http://www.w3.org/2002/07/owl#Class"/>
    <rdfs:subClassOf rdf:resource="http://transience.eu/ontologies/Variable"/>
    <rdfs:label>Final Energy|Carbon Removal|Direct Air Capture</rdfs:label>
    <rdfs:comment>Final energy consumption by direct air capture</rdfs:comment>
    <ex:unit>EJ/yr</ex:unit>
  </rdf:Description>
  <rdf:Description rdf:about="http://transience.eu/ontologies/Employment_Industry">
    <rdf:type rdf:resource="http://www.w3.org/2002/07/owl#Class"/>
    <rdfs:subClassOf rdf:resource="http://transience.eu/ontologies/Variable"/>
    <rdfs:label>Employment|Industry</rdfs:label>
    <rdfs:comment>Number of employed inhabitants (payrolls) in industry (based on ILO classification)</rdfs:comment>
    <ex:unit>million</ex:unit>
  </rdf:Description>
  <rdf:Description rdf:about="http://transience.eu/ontologies/Export_Industry_Non-Metallic_Minerals_Volume">
    <rdf:type rdf:resource="http://www.w3.org/2002/07/owl#Class"/>
    <rdfs:subClassOf rdf:resource="http://transience.eu/ontologies/Variable"/>
    <rdfs:label>Export|Industry|Non-Metallic Minerals|Volume</rdfs:label>
    <rdfs:comment>Export of non-metallic minerals</rdfs:comment>
    <ex:unit>Mt/yr</ex:unit>
  </rdf:Description>
  <rdf:Description rdf:about="http://transience.eu/ontologies/Final_Energy_Carbon_Removal_Heat">
    <rdf:type rdf:resource="http://www.w3.org/2002/07/owl#Class"/>
    <rdfs:subClassOf rdf:resource="http://transience.eu/ontologies/Variable"/>
    <rdfs:label>Final Energy|Carbon Removal|Heat</rdfs:label>
    <rdfs:comment>Final energy consumption of heat by carbon dioxide removal processes</rdfs:comment>
    <ex:unit>EJ/yr</ex:unit>
  </rdf:Description>
  <rdf:Description rdf:about="http://transience.eu/ontologies/Outflow_Concrete_Product_categories">
    <rdf:type rdf:resource="http://www.w3.org/2002/07/owl#Class"/>
    <rdfs:subClassOf rdf:resource="http://transience.eu/ontologies/Variable"/>
    <rdfs:label>Outflow|Concrete|[Product categories]</rdfs:label>
    <rdfs:comment>Concrete outflowÂ </rdfs:comment>
    <ex:unit>t/yr</ex:unit>
  </rdf:Description>
  <rdf:Description rdf:about="http://transience.eu/ontologies/Carbon_Capture_Fossil_Energy_Supply_Electricity">
    <rdf:type rdf:resource="http://www.w3.org/2002/07/owl#Class"/>
    <rdfs:subClassOf rdf:resource="http://transience.eu/ontologies/Variable"/>
    <rdfs:label>Carbon Capture|Fossil|Energy|Supply|Electricity</rdfs:label>
    <rdfs:comment>total carbon dioxide emissions captured from fossil fuel use in electricity production (part of IPCC category 1A1a), should be reported as positive numbers</rdfs:comment>
    <ex:unit>Mt CO2/yr</ex:unit>
  </rdf:Description>
  <rdf:Description rdf:about="http://transience.eu/ontologies/Final_Energy_Non-Energy_Use_Gases_Fossil">
    <rdf:type rdf:resource="http://www.w3.org/2002/07/owl#Class"/>
    <rdfs:subClassOf rdf:resource="http://transience.eu/ontologies/Variable"/>
    <rdfs:label>Final Energy|Non-Energy Use|Gases|Fossil</rdfs:label>
    <rdfs:comment>Final energy consumption of synthetic or derived gases of fossil origin by the non-combustion processes</rdfs:comment>
    <ex:unit>EJ/yr</ex:unit>
  </rdf:Description>
  <rdf:Description rdf:about="http://transience.eu/ontologies/Secondary_Energy_Electricity_Oil">
    <rdf:type rdf:resource="http://www.w3.org/2002/07/owl#Class"/>
    <rdfs:subClassOf rdf:resource="http://transience.eu/ontologies/Variable"/>
    <rdfs:label>Secondary Energy|Electricity|Oil</rdfs:label>
    <rdfs:comment>net electricity production from refined liquid oil products</rdfs:comment>
    <ex:unit>EJ/yr</ex:unit>
  </rdf:Description>
  <rdf:Description rdf:about="http://transience.eu/ontologies/Final_Energy_Commercial_Solids_Biomass">
    <rdf:type rdf:resource="http://www.w3.org/2002/07/owl#Class"/>
    <rdfs:subClassOf rdf:resource="http://transience.eu/ontologies/Variable"/>
    <rdfs:label>Final Energy|Commercial|Solids|Biomass</rdfs:label>
    <rdfs:comment>final energy solid biomass consumption by the commercial sector</rdfs:comment>
    <ex:unit>EJ/yr</ex:unit>
  </rdf:Description>
  <rdf:Description rdf:about="http://transience.eu/ontologies/Investment_Energy_Supply_Electricity_Wind">
    <rdf:type rdf:resource="http://www.w3.org/2002/07/owl#Class"/>
    <rdfs:subClassOf rdf:resource="http://transience.eu/ontologies/Variable"/>
    <rdfs:label>Investment|Energy Supply|Electricity|Wind</rdfs:label>
    <rdfs:comment>investments in new power generation for the specified power plant category. If the model features several sub-categories, the total investments should be reported. For plants equipped with CCS, the investment in the capturing equipment should be included but not the one on transport and storage.</rdfs:comment>
    <ex:unit>billion US$2010/yr</ex:unit>
  </rdf:Description>
  <rdf:Description rdf:about="http://transience.eu/ontologies/Secondary_Energy_Electricity_Coal_w__CCS">
    <rdf:type rdf:resource="http://www.w3.org/2002/07/owl#Class"/>
    <rdfs:subClassOf rdf:resource="http://transience.eu/ontologies/Variable"/>
    <rdfs:label>Secondary Energy|Electricity|Coal|w/ CCS</rdfs:label>
    <rdfs:comment>net electricity production from coal with a CO2 capture component</rdfs:comment>
    <ex:unit>EJ/yr</ex:unit>
  </rdf:Description>
  <rdf:Description rdf:about="http://transience.eu/ontologies/Final_Energy_Commercial_Gases_Electricity">
    <rdf:type rdf:resource="http://www.w3.org/2002/07/owl#Class"/>
    <rdfs:subClassOf rdf:resource="http://transience.eu/ontologies/Variable"/>
    <rdfs:label>Final Energy|Commercial|Gases|Electricity</rdfs:label>
    <rdfs:comment>final energy consumption by the commercial sector of synthetic e-fuel gas ("power-to-gas"), excluding transmission/distribution losses</rdfs:comment>
    <ex:unit>EJ/yr</ex:unit>
  </rdf:Description>
  <rdf:Description rdf:about="http://transience.eu/ontologies/Carbon_Capture_Storage_Biomass_Energy_Supply_Liquids">
    <rdf:type rdf:resource="http://www.w3.org/2002/07/owl#Class"/>
    <rdfs:subClassOf rdf:resource="http://transience.eu/ontologies/Variable"/>
    <rdfs:label>Carbon Capture|Storage|Biomass|Energy|Supply|Liquids</rdfs:label>
    <rdfs:comment>total carbon dioxide emissions captured from bioenergy use in liquid fuel production (part of IPCC category 1A) and stored in geological deposits (e.g. in depleted oil and gas fields, unmined coal seams, saline aquifers) and the deep ocean, stored amounts should be reported as positive numbers</rdfs:comment>
    <ex:unit>Mt CO2/yr</ex:unit>
  </rdf:Description>
  <rdf:Description rdf:about="http://transience.eu/ontologies/Lifetime_Electricity_Wind_Offshore">
    <rdf:type rdf:resource="http://www.w3.org/2002/07/owl#Class"/>
    <rdfs:subClassOf rdf:resource="http://transience.eu/ontologies/Variable"/>
    <rdfs:label>Lifetime|Electricity|Wind|Offshore</rdfs:label>
    <rdfs:comment>Lifetime of a new offshore wind power plant. Lifetime should be calculated by summing all vintages of a  capacity unit (e.g. (1+1+0.9+0.7+0.5) * 10 years = 41 years) or by the e-folding time for exponential capacity depreciation.  The lifetime should refer to the plant type(s) for which capital costs have been reported. If capital cost for more than one plant type has been reported, modellers should report lifetime for the additional plant types by adding variables Lifetime|Electricity|Wind|Offshore|2, ... Lifetime|Electricity|Wind|Offshore|N (matching the assignment of plant types to technologies in the reporting of capital costs as documented in the comments sheet). </rdfs:comment>
    <ex:unit>years</ex:unit>
  </rdf:Description>
  <rdf:Description rdf:about="http://transience.eu/ontologies/OM_Cost_Fixed_Electricity_Coal_w__CCS">
    <rdf:type rdf:resource="http://www.w3.org/2002/07/owl#Class"/>
    <rdfs:subClassOf rdf:resource="http://transience.eu/ontologies/Variable"/>
    <rdfs:label>OM Cost|Fixed|Electricity|Coal|w/ CCS</rdfs:label>
    <rdfs:comment>Annual fixed operation &amp; maintainance cost of a new coal power plant with CCS. If more than one CCS coal power technology is modelled (e.g. subcritical PC with post-combustion capture, supercritical PC with post-combustion capture, supercritical PC with oxyfuel combustion and capture, IGCC with pre-combustion capture), modellers should report fixed O&amp;M costs  for each represented CCS coal power technology by adding variables OM Cost|Fixed|Electricity|Coal|w/ CCS|2, ... OM Cost|Fixed|Electricity|Coal|w/ CCS|N (with N = number of represented technologies) (matching the assignment of plant types to technologies in the reporting of capital costs as documented in the comments sheet).</rdfs:comment>
    <ex:unit>US$2010/kW/yr</ex:unit>
  </rdf:Description>
  <rdf:Description rdf:about="http://transience.eu/ontologies/Total_Scrap_Non-Ferrous_Metals">
    <rdf:type rdf:resource="http://www.w3.org/2002/07/owl#Class"/>
    <rdfs:subClassOf rdf:resource="http://transience.eu/ontologies/Variable"/>
    <rdfs:label>Total Scrap|Non-Ferrous Metals</rdfs:label>
    <rdfs:comment>Total potential of non-ferrous metals scrap material as a result of end of life products (before collection)</rdfs:comment>
    <ex:unit>Mt/yr</ex:unit>
  </rdf:Description>
  <rdf:Description rdf:about="http://transience.eu/ontologies/Production_Steel_Primary_crude_steel_Volume">
    <rdf:type rdf:resource="http://www.w3.org/2002/07/owl#Class"/>
    <rdfs:subClassOf rdf:resource="http://transience.eu/ontologies/Variable"/>
    <rdfs:label>Production|Steel|Primary crude steel|Volume</rdfs:label>
    <rdfs:comment>Production of primary crude steel</rdfs:comment>
    <ex:unit>Mt/yr</ex:unit>
  </rdf:Description>
  <rdf:Description rdf:about="http://transience.eu/ontologies/Investment_Energy_Demand_Transportation_Passenger_Road_LDV_ICE">
    <rdf:type rdf:resource="http://www.w3.org/2002/07/owl#Class"/>
    <rdfs:subClassOf rdf:resource="http://transience.eu/ontologies/Variable"/>
    <rdfs:label>Investment|Energy Demand|Transportation|Passenger|Road|LDV|ICE</rdfs:label>
    <rdfs:comment>investments into new vehicle technologies in the transport sector (light-duty cars and trucks: internal combustion engine technologies running on any type of liquid or gaseous fuel)</rdfs:comment>
    <ex:unit>billion US$2010/yr</ex:unit>
  </rdf:Description>
  <rdf:Description rdf:about="http://transience.eu/ontologies/Carbon_Capture">
    <rdf:type rdf:resource="http://www.w3.org/2002/07/owl#Class"/>
    <rdfs:subClassOf rdf:resource="http://transience.eu/ontologies/Variable"/>
    <rdfs:label>Carbon Capture</rdfs:label>
    <rdfs:comment>total carbon dioxide emissions captured, i.e. captured CO2 stream from bioenergy use, fossil fuel use, industrial processes, and direct air capture; should be reported as positive numbers</rdfs:comment>
    <ex:unit>Mt CO2/yr</ex:unit>
  </rdf:Description>
  <rdf:Description rdf:about="http://transience.eu/ontologies/Capacity_Electricity_Oil_w_o_CCS">
    <rdf:type rdf:resource="http://www.w3.org/2002/07/owl#Class"/>
    <rdfs:subClassOf rdf:resource="http://transience.eu/ontologies/Variable"/>
    <rdfs:label>Capacity|Electricity|Oil|w/o CCS</rdfs:label>
    <rdfs:comment>Total installed (available) capacity of oil power plants without CCS, including plants held in an operating reserve. The installed (available) capacity of oil power plants by plant type for which capital costs are reported should be reported by adding variables Capacity|Electricity|Oil|w/o CCS|1, ..., Capacity|Electricity|Oil|w/o CCS|N (matching the assignment of plant types to technologies in the reporting of capital costs as documented in the comments sheet). </rdfs:comment>
    <ex:unit>GW</ex:unit>
  </rdf:Description>
  <rdf:Description rdf:about="http://transience.eu/ontologies/Import">
    <rdf:type rdf:resource="http://www.w3.org/2002/07/owl#Class"/>
    <rdfs:subClassOf rdf:resource="http://transience.eu/ontologies/Variable"/>
    <rdfs:label>Import</rdfs:label>
    <rdfs:comment>total imports measured in monetary quantities.</rdfs:comment>
    <ex:unit>billion US$2010/yr</ex:unit>
  </rdf:Description>
  <rdf:Description rdf:about="http://transience.eu/ontologies/Export_Industry_Chemicals_Plastics_Volume">
    <rdf:type rdf:resource="http://www.w3.org/2002/07/owl#Class"/>
    <rdfs:subClassOf rdf:resource="http://transience.eu/ontologies/Variable"/>
    <rdfs:label>Export|Industry|Chemicals|Plastics|Volume</rdfs:label>
    <rdfs:comment>Export of plastics</rdfs:comment>
    <ex:unit>Mt/yr</ex:unit>
  </rdf:Description>
  <rdf:Description rdf:about="http://transience.eu/ontologies/Primary_Energy_Coal_Electricity_w__CCS">
    <rdf:type rdf:resource="http://www.w3.org/2002/07/owl#Class"/>
    <rdfs:subClassOf rdf:resource="http://transience.eu/ontologies/Variable"/>
    <rdfs:label>Primary Energy|Coal|Electricity|w/ CCS</rdfs:label>
    <rdfs:comment>coal primary energy input to electricity generation  used in combination with CCS</rdfs:comment>
    <ex:unit>EJ/yr</ex:unit>
  </rdf:Description>
  <rdf:Description rdf:about="http://transience.eu/ontologies/Production_Iron_and_Steel_Primary_Steel_Value">
    <rdf:type rdf:resource="http://www.w3.org/2002/07/owl#Class"/>
    <rdfs:subClassOf rdf:resource="http://transience.eu/ontologies/Variable"/>
    <rdfs:label>Production|Iron and Steel|Primary Steel|Value</rdfs:label>
    <rdfs:comment>Production of primary / virgin steel</rdfs:comment>
    <ex:unit>billion US$2010/yr</ex:unit>
  </rdf:Description>
  <rdf:Description rdf:about="http://transience.eu/ontologies/Primary_Energy_Non-Biomass_Renewables">
    <rdf:type rdf:resource="http://www.w3.org/2002/07/owl#Class"/>
    <rdfs:subClassOf rdf:resource="http://transience.eu/ontologies/Variable"/>
    <rdfs:label>Primary Energy|Non-Biomass Renewables</rdfs:label>
    <rdfs:comment>non-biomass renewable primary energy consumption (direct equivalent, includes hydro electricity, wind electricity, geothermal electricity and heat, solar electricity and heat and hydrogen, ocean energy)</rdfs:comment>
    <ex:unit>EJ/yr</ex:unit>
  </rdf:Description>
  <rdf:Description rdf:about="http://transience.eu/ontologies/Final_Energy_Industry_Iron_and_Steel_Other">
    <rdf:type rdf:resource="http://www.w3.org/2002/07/owl#Class"/>
    <rdfs:subClassOf rdf:resource="http://transience.eu/ontologies/Variable"/>
    <rdfs:label>Final Energy|Industry|Iron and Steel|Other</rdfs:label>
    <rdfs:comment>Final energy consumption of other energy carriers by the iron and steel sector (please provide a definition of the energy carriers in this category in the 'comments' tab)</rdfs:comment>
    <ex:unit>EJ/yr</ex:unit>
  </rdf:Description>
  <rdf:Description rdf:about="http://transience.eu/ontologies/Capacity_Petrochemicals_Biomass_pyrolysis_and_gasification">
    <rdf:type rdf:resource="http://www.w3.org/2002/07/owl#Class"/>
    <rdfs:subClassOf rdf:resource="http://transience.eu/ontologies/Variable"/>
    <rdfs:label>Capacity|Petrochemicals|Biomass pyrolysis and gasification</rdfs:label>
    <rdfs:comment>Capacity for production of biogenic syngas from biomass via combined pyrolysis and gasification; the value refers to the amount of dry biomass input that can be processed per year</rdfs:comment>
    <ex:unit>Mt biomass input / yr</ex:unit>
  </rdf:Description>
  <rdf:Description rdf:about="http://transience.eu/ontologies/Lifetime_Gases_Biomass_w_o_CCS">
    <rdf:type rdf:resource="http://www.w3.org/2002/07/owl#Class"/>
    <rdfs:subClassOf rdf:resource="http://transience.eu/ontologies/Variable"/>
    <rdfs:label>Lifetime|Gases|Biomass|w/o CCS</rdfs:label>
    <rdfs:comment>Lifetime of a new biomass to gas plant w/o CCS. Lifetime should be calculated by summing all vintages of a  capacity unit (e.g. (1+1+0.9+0.7+0.5) * 10 years = 41 years) or by the e-folding time for exponential capacity depreciation.  The lifetime should refer to the plant type(s) for which capital costs have been reported. If capital cost for more than one plant type has been reported, modellers should report lifetime for the additional plant types by adding variables Lifetime|Gases|Biomass|w/o CCS|2, ... Lifetime|Gases|Biomass|w/o CCS|N (matching the assignment of plant types to technologies in the reporting of capital costs as documented in the comments sheet). </rdfs:comment>
    <ex:unit>years</ex:unit>
  </rdf:Description>
  <rdf:Description rdf:about="http://transience.eu/ontologies/Final_Energy_Industry_Iron_and_Steel_Solids_Biomass">
    <rdf:type rdf:resource="http://www.w3.org/2002/07/owl#Class"/>
    <rdfs:subClassOf rdf:resource="http://transience.eu/ontologies/Variable"/>
    <rdfs:label>Final Energy|Industry|Iron and Steel|Solids|Biomass</rdfs:label>
    <rdfs:comment>Final energy consumption of solid biomass (modern and traditional, including renewable waste) by the iron and steel sector</rdfs:comment>
    <ex:unit>EJ/yr</ex:unit>
  </rdf:Description>
  <rdf:Description rdf:about="http://transience.eu/ontologies/Energy_Use_Industry_Petrochemicals_Methanol">
    <rdf:type rdf:resource="http://www.w3.org/2002/07/owl#Class"/>
    <rdfs:subClassOf rdf:resource="http://transience.eu/ontologies/Variable"/>
    <rdfs:label>Energy Use|Industry|Petrochemicals|Methanol</rdfs:label>
    <rdfs:comment>Use of externally supplied methanol, including both, non-energetic use and energetic use of by-products from methanol processing  (only supply from outside, not including methanol produced inside the petrochemical system from other feedstock)</rdfs:comment>
    <ex:unit>Mt/yr</ex:unit>
  </rdf:Description>
  <rdf:Description rdf:about="http://transience.eu/ontologies/Final_Energy_Non-Energy_Use_Chemicals_Liquids_Biomass">
    <rdf:type rdf:resource="http://www.w3.org/2002/07/owl#Class"/>
    <rdfs:subClassOf rdf:resource="http://transience.eu/ontologies/Variable"/>
    <rdfs:label>Final Energy|Non-Energy Use|Chemicals|Liquids|Biomass</rdfs:label>
    <rdfs:comment>Final energy consumption of liquid biofuels by the chemical sector by the non-combustion processes</rdfs:comment>
    <ex:unit>EJ/yr</ex:unit>
  </rdf:Description>
  <rdf:Description rdf:about="http://transience.eu/ontologies/Carbon_Capture_Biomass_Energy_Demand_Industry">
    <rdf:type rdf:resource="http://www.w3.org/2002/07/owl#Class"/>
    <rdfs:subClassOf rdf:resource="http://transience.eu/ontologies/Variable"/>
    <rdfs:label>Carbon Capture|Biomass|Energy|Demand|Industry</rdfs:label>
    <rdfs:comment>total carbon dioxide emissions captured from bioenergy use in industry (IPCC category 1A2), should be reported as positive numbers</rdfs:comment>
    <ex:unit>Mt CO2/yr</ex:unit>
  </rdf:Description>
  <rdf:Description rdf:about="http://transience.eu/ontologies/Final_Energy_Transportation_Electricity">
    <rdf:type rdf:resource="http://www.w3.org/2002/07/owl#Class"/>
    <rdfs:subClassOf rdf:resource="http://transience.eu/ontologies/Variable"/>
    <rdfs:label>Final Energy|Transportation|Electricity</rdfs:label>
    <rdfs:comment>final energy consumption by the transportation sector of electricity (including on-site solar PV), excluding transmission/distribution losses</rdfs:comment>
    <ex:unit>EJ/yr</ex:unit>
  </rdf:Description>
  <rdf:Description rdf:about="http://transience.eu/ontologies/Energy_Service_Transportation_Passenger_Railways">
    <rdf:type rdf:resource="http://www.w3.org/2002/07/owl#Class"/>
    <rdfs:subClassOf rdf:resource="http://transience.eu/ontologies/Variable"/>
    <rdfs:label>Energy Service|Transportation|Passenger|Railways</rdfs:label>
    <rdfs:comment>energy service demand for passenger transport on railways</rdfs:comment>
    <ex:unit>bn pkm/yr</ex:unit>
  </rdf:Description>
  <rdf:Description rdf:about="http://transience.eu/ontologies/Investment_Energy_Supply_Extraction_Fossil">
    <rdf:type rdf:resource="http://www.w3.org/2002/07/owl#Class"/>
    <rdfs:subClassOf rdf:resource="http://transience.eu/ontologies/Variable"/>
    <rdfs:label>Investment|Energy Supply|Extraction|Fossil</rdfs:label>
    <rdfs:comment>investments for all types of fossil extraction</rdfs:comment>
    <ex:unit>billion US$2010/yr</ex:unit>
  </rdf:Description>
  <rdf:Description rdf:about="http://transience.eu/ontologies/Carbon_Capture_Storage_Biomass_Energy_Supply_Electricity">
    <rdf:type rdf:resource="http://www.w3.org/2002/07/owl#Class"/>
    <rdfs:subClassOf rdf:resource="http://transience.eu/ontologies/Variable"/>
    <rdfs:label>Carbon Capture|Storage|Biomass|Energy|Supply|Electricity</rdfs:label>
    <rdfs:comment>total carbon dioxide emissions captured from bioenergy use in electricity production (part of IPCC category 1A1a) and stored in geological deposits (e.g. in depleted oil and gas fields, unmined coal seams, saline aquifers) and the deep ocean, stored amounts should be reported as positive numbers</rdfs:comment>
    <ex:unit>Mt CO2/yr</ex:unit>
  </rdf:Description>
  <rdf:Description rdf:about="http://transience.eu/ontologies/Primary_Energy_Oil_Electricity">
    <rdf:type rdf:resource="http://www.w3.org/2002/07/owl#Class"/>
    <rdfs:subClassOf rdf:resource="http://transience.eu/ontologies/Variable"/>
    <rdfs:label>Primary Energy|Oil|Electricity</rdfs:label>
    <rdfs:comment>conventional &amp; unconventional oil primary energy input to electricity generation</rdfs:comment>
    <ex:unit>EJ/yr</ex:unit>
  </rdf:Description>
  <rdf:Description rdf:about="http://transience.eu/ontologies/Carbon_Capture_Storage_Fossil_Energy_Demand_Industry">
    <rdf:type rdf:resource="http://www.w3.org/2002/07/owl#Class"/>
    <rdfs:subClassOf rdf:resource="http://transience.eu/ontologies/Variable"/>
    <rdfs:label>Carbon Capture|Storage|Fossil|Energy|Demand|Industry</rdfs:label>
    <rdfs:comment>total carbon dioxide emissions captured from fossil fuel use in industry (IPCC category 1A2) and stored in geological deposits (e.g. in depleted oil and gas fields, unmined coal seams, saline aquifers) and the deep ocean, stored amounts should be reported as positive numbers</rdfs:comment>
    <ex:unit>Mt CO2/yr</ex:unit>
  </rdf:Description>
  <rdf:Description rdf:about="http://transience.eu/ontologies/Materials_Demand_Iron_and_Steel_Residential_and_Commercial">
    <rdf:type rdf:resource="http://www.w3.org/2002/07/owl#Class"/>
    <rdfs:subClassOf rdf:resource="http://transience.eu/ontologies/Variable"/>
    <rdfs:label>Materials Demand|Iron and Steel|Residential and Commercial</rdfs:label>
    <rdfs:comment>Iron and steel requirments from a certain end-use sector</rdfs:comment>
    <ex:unit>Mt/yr</ex:unit>
  </rdf:Description>
  <rdf:Description rdf:about="http://transience.eu/ontologies/Production_Non-Ferrous_Metals_Aluminium_Volume">
    <rdf:type rdf:resource="http://www.w3.org/2002/07/owl#Class"/>
    <rdfs:subClassOf rdf:resource="http://transience.eu/ontologies/Variable"/>
    <rdfs:label>Production|Non-Ferrous Metals|Aluminium|Volume</rdfs:label>
    <rdfs:comment>production of aluminum (inlcudes primary and secondary aluminium)</rdfs:comment>
    <ex:unit>Mt/yr</ex:unit>
  </rdf:Description>
  <rdf:Description rdf:about="http://transience.eu/ontologies/OM_Cost_Fixed_Electricity_Wind_Onshore">
    <rdf:type rdf:resource="http://www.w3.org/2002/07/owl#Class"/>
    <rdfs:subClassOf rdf:resource="http://transience.eu/ontologies/Variable"/>
    <rdfs:label>OM Cost|Fixed|Electricity|Wind|Onshore</rdfs:label>
    <rdfs:comment>Annual fixed operation &amp; maintainance cost of a new onshore wind power plants. This variable should only be filled, if wind power is separated into onshore and offshore. If more than one onshore wind power technology is modelled (e.g., wind power units with different hub height and capacity), modellers should report fixed O&amp;M costs  for each represented wind power technology by adding variables OM Cost|Fixed|Electricity|Wind|Onshore|2, ... Capital|Cost|Electricity|Wind|Onshore|N (with N = number of represented onshore wind power technologies) (matching the assignment of plant types to technologies in the reporting of capital costs as documented in the comments sheet).</rdfs:comment>
    <ex:unit>US$2010/kW/yr</ex:unit>
  </rdf:Description>
  <rdf:Description rdf:about="http://transience.eu/ontologies/Secondary_Energy_Liquids_Fossil_w_o_CCS">
    <rdf:type rdf:resource="http://www.w3.org/2002/07/owl#Class"/>
    <rdfs:subClassOf rdf:resource="http://transience.eu/ontologies/Variable"/>
    <rdfs:label>Secondary Energy|Liquids|Fossil|w/o CCS</rdfs:label>
    <rdfs:comment>total production of fossil liquid synfuels from facilities without CCS</rdfs:comment>
    <ex:unit>EJ/yr</ex:unit>
  </rdf:Description>
  <rdf:Description rdf:about="http://transience.eu/ontologies/Investment_Energy_Supply_Liquids_Oil">
    <rdf:type rdf:resource="http://www.w3.org/2002/07/owl#Class"/>
    <rdfs:subClassOf rdf:resource="http://transience.eu/ontologies/Variable"/>
    <rdfs:label>Investment|Energy Supply|Liquids|Oil</rdfs:label>
    <rdfs:comment>investments for the production of fossil fuels from oil refineries For plants equipped with CCS, the investment in the capturing equipment should be included but not the one on transport and storage.</rdfs:comment>
    <ex:unit>billion US$2010/yr</ex:unit>
  </rdf:Description>
  <rdf:Description rdf:about="http://transience.eu/ontologies/Capacity_Steel_BOF">
    <rdf:type rdf:resource="http://www.w3.org/2002/07/owl#Class"/>
    <rdfs:subClassOf rdf:resource="http://transience.eu/ontologies/Variable"/>
    <rdfs:label>Capacity|Steel|BOF</rdfs:label>
    <rdfs:comment>Capacity of electric arc furnaces for crude steel production in Mt crude steel / year</rdfs:comment>
    <ex:unit>Mt/yr</ex:unit>
  </rdf:Description>
  <rdf:Description rdf:about="http://transience.eu/ontologies/Final_Energy_Residential_and_Commercial_Gases_Biomass">
    <rdf:type rdf:resource="http://www.w3.org/2002/07/owl#Class"/>
    <rdfs:subClassOf rdf:resource="http://transience.eu/ontologies/Variable"/>
    <rdfs:label>Final Energy|Residential and Commercial|Gases|Biomass</rdfs:label>
    <rdfs:comment>final energy consumption by the residential &amp; commercial sector of biogas, excluding transmission/distribution losses</rdfs:comment>
    <ex:unit>EJ/yr</ex:unit>
  </rdf:Description>
  <rdf:Description rdf:about="http://transience.eu/ontologies/Energy_Service_Transportation_Passenger_Other">
    <rdf:type rdf:resource="http://www.w3.org/2002/07/owl#Class"/>
    <rdfs:subClassOf rdf:resource="http://transience.eu/ontologies/Variable"/>
    <rdfs:label>Energy Service|Transportation|Passenger|Other</rdfs:label>
    <rdfs:comment>energy service demand for passenger transport using other modes (please provide a definition of the modes in this category in the 'comments' tab)</rdfs:comment>
    <ex:unit>bn pkm/yr</ex:unit>
  </rdf:Description>
  <rdf:Description rdf:about="http://transience.eu/ontologies/Secondary_Energy_Electricity_Wind">
    <rdf:type rdf:resource="http://www.w3.org/2002/07/owl#Class"/>
    <rdfs:subClassOf rdf:resource="http://transience.eu/ontologies/Variable"/>
    <rdfs:label>Secondary Energy|Electricity|Wind</rdfs:label>
    <rdfs:comment>net electricity production from wind energy (on- and offshore)</rdfs:comment>
    <ex:unit>EJ/yr</ex:unit>
  </rdf:Description>
  <rdf:Description rdf:about="http://transience.eu/ontologies/Secondary_Energy_Liquids_Biomass_Residues">
    <rdf:type rdf:resource="http://www.w3.org/2002/07/owl#Class"/>
    <rdfs:subClassOf rdf:resource="http://transience.eu/ontologies/Variable"/>
    <rdfs:label>Secondary Energy|Liquids|Biomass|Residues</rdfs:label>
    <rdfs:comment>liquid biofuels production from residues (forest and agriculture)</rdfs:comment>
    <ex:unit>EJ/yr</ex:unit>
  </rdf:Description>
  <rdf:Description rdf:about="http://transience.eu/ontologies/Investment_Energy_Supply_Electricity_Oil_w__CCS">
    <rdf:type rdf:resource="http://www.w3.org/2002/07/owl#Class"/>
    <rdfs:subClassOf rdf:resource="http://transience.eu/ontologies/Variable"/>
    <rdfs:label>Investment|Energy Supply|Electricity|Oil|w/ CCS</rdfs:label>
    <rdfs:comment>investments in new power generation for the specified power plant category. If the model features several sub-categories, the total investments should be reported. For plants equipped with CCS, the investment in the capturing equipment should be included but not the one on transport and storage.</rdfs:comment>
    <ex:unit>billion US$2010/yr</ex:unit>
  </rdf:Description>
  <rdf:Description rdf:about="http://transience.eu/ontologies/Secondary_Energy_Liquids_Other">
    <rdf:type rdf:resource="http://www.w3.org/2002/07/owl#Class"/>
    <rdfs:subClassOf rdf:resource="http://transience.eu/ontologies/Variable"/>
    <rdfs:label>Secondary Energy|Liquids|Other</rdfs:label>
    <rdfs:comment>total production of liquids from sources that do not fit any other category</rdfs:comment>
    <ex:unit>EJ/yr</ex:unit>
  </rdf:Description>
  <rdf:Description rdf:about="http://transience.eu/ontologies/OM_Cost_Fixed_Electricity_Geothermal">
    <rdf:type rdf:resource="http://www.w3.org/2002/07/owl#Class"/>
    <rdfs:subClassOf rdf:resource="http://transience.eu/ontologies/Variable"/>
    <rdfs:label>OM Cost|Fixed|Electricity|Geothermal</rdfs:label>
    <rdfs:comment>Annual fixed operation &amp; maintainance cost of a new geothermal power plants. If more than one geothermal power plant technology is modelled (e.g., hydrothermal, hard dry rock), modellers should report fixed O&amp;M costs  for each represented geothermal power technology by adding variables OM Cost|Fixed|Electricity|Geothermal|2, ... Capital|Cost|Electricity|Geothermal|N (with N = number of represented geothermal power technologies) (matching the assignment of plant types to technologies in the reporting of capital costs as documented in the comments sheet).</rdfs:comment>
    <ex:unit>US$2010/kW/yr</ex:unit>
  </rdf:Description>
  <rdf:Description rdf:about="http://transience.eu/ontologies/Gross_Emissions_CO2_Energy_Demand_Industry">
    <rdf:type rdf:resource="http://www.w3.org/2002/07/owl#Class"/>
    <rdfs:subClassOf rdf:resource="http://transience.eu/ontologies/Variable"/>
    <rdfs:label>Gross Emissions|CO2|Energy|Demand|Industry</rdfs:label>
    <rdfs:comment>Gross Fossil CO2 emissions from fuel combustion in industry (IPCC category 1A2), not accounting for negative emissions from BECCS, excluding emissions related to feedstocks</rdfs:comment>
    <ex:unit>Mt CO2/yr</ex:unit>
  </rdf:Description>
  <rdf:Description rdf:about="http://transience.eu/ontologies/Final_Energy_Industry_Iron_and_Steel_Hydrogen">
    <rdf:type rdf:resource="http://www.w3.org/2002/07/owl#Class"/>
    <rdfs:subClassOf rdf:resource="http://transience.eu/ontologies/Variable"/>
    <rdfs:label>Final Energy|Industry|Iron and Steel|Hydrogen</rdfs:label>
    <rdfs:comment>Final energy consumption of hydrogen by the iron and steel sector</rdfs:comment>
    <ex:unit>EJ/yr</ex:unit>
  </rdf:Description>
  <rdf:Description rdf:about="http://transience.eu/ontologies/Final_Energy_Industry_Other_Sector_Gases_Biomass">
    <rdf:type rdf:resource="http://www.w3.org/2002/07/owl#Class"/>
    <rdfs:subClassOf rdf:resource="http://transience.eu/ontologies/Variable"/>
    <rdfs:label>Final Energy|Industry|Other Sector|Gases|Biomass</rdfs:label>
    <rdfs:comment>Final energy consumption of biogas by other industry sectors</rdfs:comment>
    <ex:unit>EJ/yr</ex:unit>
  </rdf:Description>
  <rdf:Description rdf:about="http://transience.eu/ontologies/Trade_Uranium_Value">
    <rdf:type rdf:resource="http://www.w3.org/2002/07/owl#Class"/>
    <rdfs:subClassOf rdf:resource="http://transience.eu/ontologies/Variable"/>
    <rdfs:label>Trade|Uranium|Value</rdfs:label>
    <rdfs:comment>value of net exports of Uranium, at the global level these should add up to the trade losses only</rdfs:comment>
    <ex:unit>billion US$2010/yr</ex:unit>
  </rdf:Description>
  <rdf:Description rdf:about="http://transience.eu/ontologies/Trade">
    <rdf:type rdf:resource="http://www.w3.org/2002/07/owl#Class"/>
    <rdfs:subClassOf rdf:resource="http://transience.eu/ontologies/Variable"/>
    <rdfs:label>Trade</rdfs:label>
    <rdfs:comment>net exports of all goods, at the global level these should add up to the trade losses only</rdfs:comment>
    <ex:unit>billion US$2010/yr</ex:unit>
  </rdf:Description>
  <rdf:Description rdf:about="http://transience.eu/ontologies/Final_Energy_Residential_and_Commercial_Other">
    <rdf:type rdf:resource="http://www.w3.org/2002/07/owl#Class"/>
    <rdfs:subClassOf rdf:resource="http://transience.eu/ontologies/Variable"/>
    <rdfs:label>Final Energy|Residential and Commercial|Other</rdfs:label>
    <rdfs:comment>final energy consumption by the residential &amp; commercial sector of other sources that do not fit to any other category (please provide a definition of the sources in this category in the 'comments' tab)</rdfs:comment>
    <ex:unit>EJ/yr</ex:unit>
  </rdf:Description>
  <rdf:Description rdf:about="http://transience.eu/ontologies/Investment_Energy_Supply_Electricity_Geothermal">
    <rdf:type rdf:resource="http://www.w3.org/2002/07/owl#Class"/>
    <rdfs:subClassOf rdf:resource="http://transience.eu/ontologies/Variable"/>
    <rdfs:label>Investment|Energy Supply|Electricity|Geothermal</rdfs:label>
    <rdfs:comment>investments in new power generation for the specified power plant category. If the model features several sub-categories, the total investments should be reported. For plants equipped with CCS, the investment in the capturing equipment should be included but not the one on transport and storage.</rdfs:comment>
    <ex:unit>billion US$2010/yr</ex:unit>
  </rdf:Description>
  <rdf:Description rdf:about="http://transience.eu/ontologies/Production_Non-Ferrous_Metals_Aluminium_Secondary_Volume">
    <rdf:type rdf:resource="http://www.w3.org/2002/07/owl#Class"/>
    <rdfs:subClassOf rdf:resource="http://transience.eu/ontologies/Variable"/>
    <rdfs:label>Production|Non-Ferrous Metals|Aluminium|Secondary|Volume</rdfs:label>
    <rdfs:comment>production of secondary aluminum</rdfs:comment>
    <ex:unit>Mt/yr</ex:unit>
  </rdf:Description>
  <rdf:Description rdf:about="http://transience.eu/ontologies/Final_Energy_Industry_Iron_and_Steel_Solar">
    <rdf:type rdf:resource="http://www.w3.org/2002/07/owl#Class"/>
    <rdfs:subClassOf rdf:resource="http://transience.eu/ontologies/Variable"/>
    <rdfs:label>Final Energy|Industry|Iron and Steel|Solar</rdfs:label>
    <rdfs:comment>Final energy consumption of solar thermal heat by the iron and steel sector</rdfs:comment>
    <ex:unit>EJ/yr</ex:unit>
  </rdf:Description>
  <rdf:Description rdf:about="http://transience.eu/ontologies/Efficiency_Hydrogen_Biomass_w_o_CCS">
    <rdf:type rdf:resource="http://www.w3.org/2002/07/owl#Class"/>
    <rdfs:subClassOf rdf:resource="http://transience.eu/ontologies/Variable"/>
    <rdfs:label>Efficiency|Hydrogen|Biomass|w/o CCS</rdfs:label>
    <rdfs:comment>Conversion efficiency (energy content of hydrogen produced per unit of primary energy input) of a new biomass to hydrogen plant w/o CCS. The efficiency should refer to the plant type(s) for which capital costs have been reported. If capital cost for more than one plant type has been reported, modellers should report efficiency for the additional plant types by adding variables Efficiency|Hydrogen|Biomass|w/o CCS|2, ... Efficiency|Hydrogen|Biomass|w/o CCS|N (matching the assignment of plant types to technologies in the reporting of capital costs as documented in the comments sheet). </rdfs:comment>
    <ex:unit>%</ex:unit>
  </rdf:Description>
  <rdf:Description rdf:about="http://transience.eu/ontologies/Final_Energy_Commercial_Liquids_Biomass">
    <rdf:type rdf:resource="http://www.w3.org/2002/07/owl#Class"/>
    <rdfs:subClassOf rdf:resource="http://transience.eu/ontologies/Variable"/>
    <rdfs:label>Final Energy|Commercial|Liquids|Biomass</rdfs:label>
    <rdfs:comment>final energy consumption by the commercial sector of liquid biofuels</rdfs:comment>
    <ex:unit>EJ/yr</ex:unit>
  </rdf:Description>
  <rdf:Description rdf:about="http://transience.eu/ontologies/Capacity_Petrochemicals_MtA">
    <rdf:type rdf:resource="http://www.w3.org/2002/07/owl#Class"/>
    <rdfs:subClassOf rdf:resource="http://transience.eu/ontologies/Variable"/>
    <rdfs:label>Capacity|Petrochemicals|MtA</rdfs:label>
    <rdfs:comment>Capacity for aromatics production in the Methanol-to-aromatics routes; the value refers to the amount of methanol input that can be processed per year</rdfs:comment>
    <ex:unit>Mt methanol input / yr</ex:unit>
  </rdf:Description>
  <rdf:Description rdf:about="http://transience.eu/ontologies/Secondary_Energy_Gases_Electricity">
    <rdf:type rdf:resource="http://www.w3.org/2002/07/owl#Class"/>
    <rdfs:subClassOf rdf:resource="http://transience.eu/ontologies/Variable"/>
    <rdfs:label>Secondary Energy|Gases|Electricity</rdfs:label>
    <rdfs:comment>total production of gas from electricity (power to gas)</rdfs:comment>
    <ex:unit>EJ/yr</ex:unit>
  </rdf:Description>
  <rdf:Description rdf:about="http://transience.eu/ontologies/Materials_Demand_Non-metallic_minerals_Cement_Residential_and_Commercial">
    <rdf:type rdf:resource="http://www.w3.org/2002/07/owl#Class"/>
    <rdfs:subClassOf rdf:resource="http://transience.eu/ontologies/Variable"/>
    <rdfs:label>Materials Demand|Non-metallic minerals|Cement|Residential and Commercial</rdfs:label>
    <rdfs:comment>Cement requirments from a certain end-use sector</rdfs:comment>
    <ex:unit>Mt/yr</ex:unit>
  </rdf:Description>
  <rdf:Description rdf:about="http://transience.eu/ontologies/Investment_Energy_Supply_Electricity_Biomass_w_o_CCS">
    <rdf:type rdf:resource="http://www.w3.org/2002/07/owl#Class"/>
    <rdfs:subClassOf rdf:resource="http://transience.eu/ontologies/Variable"/>
    <rdfs:label>Investment|Energy Supply|Electricity|Biomass|w/o CCS</rdfs:label>
    <rdfs:comment>investments in new power generation for the specified power plant category. If the model features several sub-categories, the total investments should be reported. For plants equipped with CCS, the investment in the capturing equipment should be included but not the one on transport and storage.</rdfs:comment>
    <ex:unit>billion US$2010/yr</ex:unit>
  </rdf:Description>
  <rdf:Description rdf:about="http://transience.eu/ontologies/Final_Energy_Transportation_Gases_Biomass">
    <rdf:type rdf:resource="http://www.w3.org/2002/07/owl#Class"/>
    <rdfs:subClassOf rdf:resource="http://transience.eu/ontologies/Variable"/>
    <rdfs:label>Final Energy|Transportation|Gases|Biomass</rdfs:label>
    <rdfs:comment>final energy consumption by the transportation sector of biogas</rdfs:comment>
    <ex:unit>EJ/yr</ex:unit>
  </rdf:Description>
  <rdf:Description rdf:about="http://transience.eu/ontologies/Carbon_Capture_Storage_Industrial_Processes">
    <rdf:type rdf:resource="http://www.w3.org/2002/07/owl#Class"/>
    <rdfs:subClassOf rdf:resource="http://transience.eu/ontologies/Variable"/>
    <rdfs:label>Carbon Capture|Storage|Industrial Processes</rdfs:label>
    <rdfs:comment>total carbon dioxide emissions captured from industrial processes (e.g., cement production, but not from fossil fuel burning) use and stored in geological deposits (e.g. in depleted oil and gas fields, unmined coal seams, saline aquifers) and the deep ocean, stored amounts should be reported as positive numbers</rdfs:comment>
    <ex:unit>Mt CO2/yr</ex:unit>
  </rdf:Description>
  <rdf:Description rdf:about="http://transience.eu/ontologies/Investment_Petrochemicals_MtO_+_MtA">
    <rdf:type rdf:resource="http://www.w3.org/2002/07/owl#Class"/>
    <rdfs:subClassOf rdf:resource="http://transience.eu/ontologies/Variable"/>
    <rdfs:label>Investment|Petrochemicals|MtO + MtA</rdfs:label>
    <rdfs:comment>Investment in plants to produce HVC from methanol, including both MtO and MtA plants</rdfs:comment>
    <ex:unit>Mio â‚¬_2022/yr</ex:unit>
  </rdf:Description>
  <rdf:Description rdf:about="http://transience.eu/ontologies/Cost_Production_Steel_DRI_SAF_BOF_NG_CCS">
    <rdf:type rdf:resource="http://www.w3.org/2002/07/owl#Class"/>
    <rdfs:subClassOf rdf:resource="http://transience.eu/ontologies/Variable"/>
    <rdfs:label>Cost|Production|Steel|DRI_SAF_BOF_NG_CCS</rdfs:label>
    <rdfs:comment>Specific production cost of crude steel in DRI/Smelter/BOF route when using natural gas as reducing gas and doing CCS; including CAPEX (annuity), fixed and variable OPEX, including CO2 transport and storage costs</rdfs:comment>
    <ex:unit>Mio â‚¬_2022 / t crude steel</ex:unit>
  </rdf:Description>
  <rdf:Description rdf:about="http://transience.eu/ontologies/Capital_Cost_Electricity_Biomass_w_o_CCS">
    <rdf:type rdf:resource="http://www.w3.org/2002/07/owl#Class"/>
    <rdfs:subClassOf rdf:resource="http://transience.eu/ontologies/Variable"/>
    <rdfs:label>Capital Cost|Electricity|Biomass|w/o CCS</rdfs:label>
    <rdfs:comment>Capital cost of a new biomass power plant w/o CCS. If more than one biomass power technology is modelled, modellers should report capital costs for each represented biomass power technology by adding variables Capital Cost|Electricity|Biomass|w/o CCS|2, ... Capital Cost|Electricity|Biomass|w/o CCS|N (with N = number of represented technologies). It is modeller's choice which biomass power technologies to assign to type 1 (assigned to the variable without number suffix),2,...,N. The assignment should be documented in the comments sheet. </rdfs:comment>
    <ex:unit>US$2010/kW</ex:unit>
  </rdf:Description>
  <rdf:Description rdf:about="http://transience.eu/ontologies/Carbon_Capture_Fossil_Energy_Supply">
    <rdf:type rdf:resource="http://www.w3.org/2002/07/owl#Class"/>
    <rdfs:subClassOf rdf:resource="http://transience.eu/ontologies/Variable"/>
    <rdfs:label>Carbon Capture|Fossil|Energy|Supply</rdfs:label>
    <rdfs:comment>total carbon dioxide emissions captured from fossil fuel use in energy supply (IPCC category 1A), should be reported as positive numbers</rdfs:comment>
    <ex:unit>Mt CO2/yr</ex:unit>
  </rdf:Description>
  <rdf:Description rdf:about="http://transience.eu/ontologies/Production_Chemicals_Ethane__Volume">
    <rdf:type rdf:resource="http://www.w3.org/2002/07/owl#Class"/>
    <rdfs:subClassOf rdf:resource="http://transience.eu/ontologies/Variable"/>
    <rdfs:label>Production|Chemicals|Ethane |Volume</rdfs:label>
    <rdfs:comment>production of ethane (raw material for the production of high value chemicals, e.g. olefins)</rdfs:comment>
    <ex:unit>Mt/yr</ex:unit>
  </rdf:Description>
  <rdf:Description rdf:about="http://transience.eu/ontologies/Emissions_CO2_Industrial_Processes_Non-Metallic_Minerals_Cement">
    <rdf:type rdf:resource="http://www.w3.org/2002/07/owl#Class"/>
    <rdfs:subClassOf rdf:resource="http://transience.eu/ontologies/Variable"/>
    <rdfs:label>Emissions|CO2|Industrial Processes|Non-Metallic Minerals|Cement</rdfs:label>
    <rdfs:comment>CO2 emissions from industrial processes from cement</rdfs:comment>
    <ex:unit>Mt CO2/yr</ex:unit>
  </rdf:Description>
  <rdf:Description rdf:about="http://transience.eu/ontologies/OM_Cost_Fixed_Hydrogen_Coal_w_o_CCS">
    <rdf:type rdf:resource="http://www.w3.org/2002/07/owl#Class"/>
    <rdfs:subClassOf rdf:resource="http://transience.eu/ontologies/Variable"/>
    <rdfs:label>OM Cost|Fixed|Hydrogen|Coal|w/o CCS</rdfs:label>
    <rdfs:comment>Annual fixed operation &amp; maintainance cost of a new coal to hydrogen plant w/o CCS. If more than one coal to hydrogen technology is modelled, modellers should report fixed O&amp;M costs  for each represented coal to hydrogen technology by adding variables OM Cost|Fixed|Hydrogen|Coal|w/o CCS|2, ... OM Cost|Fixed|Hydrogen|Coal|w/o CCS|N (with N = number of represented technologies) (matching the assignment of plant types to technologies in the reporting of capital costs as documented in the comments sheet).</rdfs:comment>
    <ex:unit>US$2010/kW/yr</ex:unit>
  </rdf:Description>
  <rdf:Description rdf:about="http://transience.eu/ontologies/Primary_Energy_Fossil_w_o_CCS">
    <rdf:type rdf:resource="http://www.w3.org/2002/07/owl#Class"/>
    <rdfs:subClassOf rdf:resource="http://transience.eu/ontologies/Variable"/>
    <rdfs:label>Primary Energy|Fossil|w/o CCS</rdfs:label>
    <rdfs:comment>coal, gas, conventional and unconventional oil primary energy consumption without CCS</rdfs:comment>
    <ex:unit>EJ/yr</ex:unit>
  </rdf:Description>
  <rdf:Description rdf:about="http://transience.eu/ontologies/Trade_Secondary_Energy_Hydrogen_Value">
    <rdf:type rdf:resource="http://www.w3.org/2002/07/owl#Class"/>
    <rdfs:subClassOf rdf:resource="http://transience.eu/ontologies/Variable"/>
    <rdfs:label>Trade|Secondary Energy|Hydrogen|Value</rdfs:label>
    <rdfs:comment>value of net exports of hydrogen, at the global level these should add up to the trade losses only</rdfs:comment>
    <ex:unit>EJ/yr</ex:unit>
  </rdf:Description>
  <rdf:Description rdf:about="http://transience.eu/ontologies/Final_Energy_Industry_Pulp_and_Paper_Geothermal">
    <rdf:type rdf:resource="http://www.w3.org/2002/07/owl#Class"/>
    <rdfs:subClassOf rdf:resource="http://transience.eu/ontologies/Variable"/>
    <rdfs:label>Final Energy|Industry|Pulp and Paper|Geothermal</rdfs:label>
    <rdfs:comment>Final energy consumption of geothermal heat by the pulp and paper sector</rdfs:comment>
    <ex:unit>EJ/yr</ex:unit>
  </rdf:Description>
  <rdf:Description rdf:about="http://transience.eu/ontologies/Export_Industry_Non-Ferrous_Metals_Aluminum">
    <rdf:type rdf:resource="http://www.w3.org/2002/07/owl#Class"/>
    <rdfs:subClassOf rdf:resource="http://transience.eu/ontologies/Variable"/>
    <rdfs:label>Export|Industry|Non-Ferrous Metals|Aluminum</rdfs:label>
    <rdfs:comment>Export of aluminium measured in monetary units</rdfs:comment>
    <ex:unit>billion US$2010/yr</ex:unit>
  </rdf:Description>
  <rdf:Description rdf:about="http://transience.eu/ontologies/Final_Energy_Industry_Pulp_and_Paper_Hydrogen">
    <rdf:type rdf:resource="http://www.w3.org/2002/07/owl#Class"/>
    <rdfs:subClassOf rdf:resource="http://transience.eu/ontologies/Variable"/>
    <rdfs:label>Final Energy|Industry|Pulp and Paper|Hydrogen</rdfs:label>
    <rdfs:comment>Final energy consumption of hydrogen of the pulp and paper sector</rdfs:comment>
    <ex:unit>EJ/yr</ex:unit>
  </rdf:Description>
  <rdf:Description rdf:about="http://transience.eu/ontologies/Primary_Energy_Fossil_w__CCS">
    <rdf:type rdf:resource="http://www.w3.org/2002/07/owl#Class"/>
    <rdfs:subClassOf rdf:resource="http://transience.eu/ontologies/Variable"/>
    <rdfs:label>Primary Energy|Fossil|w/ CCS</rdfs:label>
    <rdfs:comment>coal, gas, conventional and unconventional oil primary energy consumption used in combination with CCS</rdfs:comment>
    <ex:unit>EJ/yr</ex:unit>
  </rdf:Description>
  <rdf:Description rdf:about="http://transience.eu/ontologies/Primary_Energy">
    <rdf:type rdf:resource="http://www.w3.org/2002/07/owl#Class"/>
    <rdfs:subClassOf rdf:resource="http://transience.eu/ontologies/Variable"/>
    <rdfs:label>Primary Energy</rdfs:label>
    <rdfs:comment>total primary energy consumption (direct equivalent)</rdfs:comment>
    <ex:unit>EJ/yr</ex:unit>
  </rdf:Description>
  <rdf:Description rdf:about="http://transience.eu/ontologies/Capital_Cost_Hydrogen_Coal_w_o_CCS">
    <rdf:type rdf:resource="http://www.w3.org/2002/07/owl#Class"/>
    <rdfs:subClassOf rdf:resource="http://transience.eu/ontologies/Variable"/>
    <rdfs:label>Capital Cost|Hydrogen|Coal|w/o CCS</rdfs:label>
    <rdfs:comment>Capital cost of a new coal to hydrogen plant w/o CCS. If more than one coal to hydrogen technology is modelled, modellers should report capital costs for each represented coal to hydrogen technology by adding variables Capital Cost|Hydrogen|Coal|w/o CCS|2, ... Capital Cost|Hydrogen|Coal|w/o CCS|N (with N = number of represented technologies). It is modeller's choice which coal to hydrogen technologies to assign to type 1 (assigned to the variable without number suffix),2,...,N. The assignment should be documented in the comments sheet. </rdfs:comment>
    <ex:unit>US$2010/kW</ex:unit>
  </rdf:Description>
  <rdf:Description rdf:about="http://transience.eu/ontologies/Final_Energy_Non-Energy_Use_Chemicals_Solids">
    <rdf:type rdf:resource="http://www.w3.org/2002/07/owl#Class"/>
    <rdfs:subClassOf rdf:resource="http://transience.eu/ontologies/Variable"/>
    <rdfs:label>Final Energy|Non-Energy Use|Chemicals|Solids</rdfs:label>
    <rdfs:comment>Final energy consumption of solids by the chemical sector by the non-combustion processes</rdfs:comment>
    <ex:unit>EJ/yr</ex:unit>
  </rdf:Description>
  <rdf:Description rdf:about="http://transience.eu/ontologies/Outflow_materials_Buildings_building_types">
    <rdf:type rdf:resource="http://www.w3.org/2002/07/owl#Class"/>
    <rdfs:subClassOf rdf:resource="http://transience.eu/ontologies/Variable"/>
    <rdfs:label>Outflow|[materials]|Buildings|[building types]</rdfs:label>
    <rdfs:comment>Material outflows from buildingsÂ </rdfs:comment>
    <ex:unit>kg/yr</ex:unit>
  </rdf:Description>
  <rdf:Description rdf:about="http://transience.eu/ontologies/Final_Energy_Industry_Other_Sector_Gases_Electricity">
    <rdf:type rdf:resource="http://www.w3.org/2002/07/owl#Class"/>
    <rdfs:subClassOf rdf:resource="http://transience.eu/ontologies/Variable"/>
    <rdfs:label>Final Energy|Industry|Other Sector|Gases|Electricity</rdfs:label>
    <rdfs:comment>Final energy consumption of synthetic e-fuel gas ("power-to-gas") by other industry sectors</rdfs:comment>
    <ex:unit>EJ/yr</ex:unit>
  </rdf:Description>
  <rdf:Description rdf:about="http://transience.eu/ontologies/Export_Industry_Iron_and_Steel_Volume">
    <rdf:type rdf:resource="http://www.w3.org/2002/07/owl#Class"/>
    <rdfs:subClassOf rdf:resource="http://transience.eu/ontologies/Variable"/>
    <rdfs:label>Export|Industry|Iron and Steel|Volume</rdfs:label>
    <rdfs:comment>Export of iron &amp; steel</rdfs:comment>
    <ex:unit>Mt/yr</ex:unit>
  </rdf:Description>
  <rdf:Description rdf:about="http://transience.eu/ontologies/Production_Steel_Primary_crude_steel_DRI_hydrogen_route">
    <rdf:type rdf:resource="http://www.w3.org/2002/07/owl#Class"/>
    <rdfs:subClassOf rdf:resource="http://transience.eu/ontologies/Variable"/>
    <rdfs:label>Production|Steel|Primary crude steel|DRI hydrogen route</rdfs:label>
    <rdfs:comment>Production of primary crude steel in DRI route with hydrogen as reducing gas (including both: processing of DRI into steel in EAF and in Smelter/BOF)</rdfs:comment>
    <ex:unit>Mt/yr</ex:unit>
  </rdf:Description>
  <rdf:Description rdf:about="http://transience.eu/ontologies/Final_Energy_Industry_Chemicals_Liquids_Electricity">
    <rdf:type rdf:resource="http://www.w3.org/2002/07/owl#Class"/>
    <rdfs:subClassOf rdf:resource="http://transience.eu/ontologies/Variable"/>
    <rdfs:label>Final Energy|Industry|Chemicals|Liquids|Electricity</rdfs:label>
    <rdfs:comment>Final energy consumption of synthetic liquid efuels ("power-to-liquid") by the chemicals sector</rdfs:comment>
    <ex:unit>EJ/yr</ex:unit>
  </rdf:Description>
  <rdf:Description rdf:about="http://transience.eu/ontologies/Import_Industry_Chemicals_Plastics">
    <rdf:type rdf:resource="http://www.w3.org/2002/07/owl#Class"/>
    <rdfs:subClassOf rdf:resource="http://transience.eu/ontologies/Variable"/>
    <rdfs:label>Import|Industry|Chemicals|Plastics</rdfs:label>
    <rdfs:comment>Import of plastics measured in monetary units</rdfs:comment>
    <ex:unit>billion US$2010/yr</ex:unit>
  </rdf:Description>
  <rdf:Description rdf:about="http://transience.eu/ontologies/Production_Iron_and_Steel_Sponge_Iron_Volume">
    <rdf:type rdf:resource="http://www.w3.org/2002/07/owl#Class"/>
    <rdfs:subClassOf rdf:resource="http://transience.eu/ontologies/Variable"/>
    <rdfs:label>Production|Iron and Steel|Sponge Iron|Volume</rdfs:label>
    <rdfs:comment>production of sponge iron (intermediate product for the production of primary steel)</rdfs:comment>
    <ex:unit>Mt/yr</ex:unit>
  </rdf:Description>
  <rdf:Description rdf:about="http://transience.eu/ontologies/Capital_Cost_Electricity_Solar_CSP">
    <rdf:type rdf:resource="http://www.w3.org/2002/07/owl#Class"/>
    <rdfs:subClassOf rdf:resource="http://transience.eu/ontologies/Variable"/>
    <rdfs:label>Capital Cost|Electricity|Solar|CSP</rdfs:label>
    <rdfs:comment>Capital cost of a new concentrated solar power plant. If more than one CSP technology is modelled (e.g., parabolic trough, solar power tower), modellers should report capital costs for each represented CSP technology by adding variables Capital Cost|Electricity|Solar|CSP|2, ... Capital|Cost|Electricity|Solar|CSP|N (with N = number of represented CSP technologies). It is modeller's choice which CSP technologies to assign to type 1 (assigned to the variable without number suffix),2,...,N. The assignment should be documented in the comments sheet. </rdfs:comment>
    <ex:unit>US$2010/kW</ex:unit>
  </rdf:Description>
  <rdf:Description rdf:about="http://transience.eu/ontologies/Emissions_CO2_Energy_Demand_Residential">
    <rdf:type rdf:resource="http://www.w3.org/2002/07/owl#Class"/>
    <rdfs:subClassOf rdf:resource="http://transience.eu/ontologies/Variable"/>
    <rdfs:label>Emissions|CO2|Energy|Demand|Residential</rdfs:label>
    <rdfs:comment>Fossil CO2 emissions from fuel combustion in residential (IPCC category 1A4b)</rdfs:comment>
    <ex:unit>Mt CO2/yr</ex:unit>
  </rdf:Description>
  <rdf:Description rdf:about="http://transience.eu/ontologies/Lifetime_Hydrogen_Biomass_w_o_CCS">
    <rdf:type rdf:resource="http://www.w3.org/2002/07/owl#Class"/>
    <rdfs:subClassOf rdf:resource="http://transience.eu/ontologies/Variable"/>
    <rdfs:label>Lifetime|Hydrogen|Biomass|w/o CCS</rdfs:label>
    <rdfs:comment>Lifetime of a new biomass to hydrogen plant w/o CCS. Lifetime should be calculated by summing all vintages of a  capacity unit (e.g. (1+1+0.9+0.7+0.5) * 10 years = 41 years) or by the e-folding time for exponential capacity depreciation.  The lifetime should refer to the plant type(s) for which capital costs have been reported. If capital cost for more than one plant type has been reported, modellers should report lifetime for the additional plant types by adding variables Lifetime|Hydrogen|Biomass|w/o CCS|2, ... Lifetime|Hydrogen|Biomass|w/o CCS|N (matching the assignment of plant types to technologies in the reporting of capital costs as documented in the comments sheet). </rdfs:comment>
    <ex:unit>years</ex:unit>
  </rdf:Description>
  <rdf:Description rdf:about="http://transience.eu/ontologies/Lifetime_Electricity_Gas_w__CCS">
    <rdf:type rdf:resource="http://www.w3.org/2002/07/owl#Class"/>
    <rdfs:subClassOf rdf:resource="http://transience.eu/ontologies/Variable"/>
    <rdfs:label>Lifetime|Electricity|Gas|w/ CCS</rdfs:label>
    <rdfs:comment>Lifetime of a new gas power plant with CCS. Lifetime should be calculated by summing all vintages of a  capacity unit (e.g. (1+1+0.9+0.7+0.5) * 10 years = 41 years) or by the e-folding time for exponential capacity depreciation.  The lifetime should refer to the plant type(s) for which capital costs have been reported. If capital cost for more than one plant type has been reported, modellers should report lifetime for the additional plant types by adding variables Lifetime|Electricity|Gas|w/ CCS|2, ... Lifetime|Electricity|Gas|w/ CCS|N (matching the assignment of plant types to technologies in the reporting of capital costs as documented in the comments sheet). </rdfs:comment>
    <ex:unit>years</ex:unit>
  </rdf:Description>
  <rdf:Description rdf:about="http://transience.eu/ontologies/Outflow_Plastics_Other_demand_sectors_Product_categories">
    <rdf:type rdf:resource="http://www.w3.org/2002/07/owl#Class"/>
    <rdfs:subClassOf rdf:resource="http://transience.eu/ontologies/Variable"/>
    <rdfs:label>Outflow|Plastics|Other|[demand sectors]|[Product categories]</rdfs:label>
    <rdfs:comment>Plastics outflow from other sectorsÂ </rdfs:comment>
    <ex:unit>t/yr</ex:unit>
  </rdf:Description>
  <rdf:Description rdf:about="http://transience.eu/ontologies/Final_Energy_Industry_Steel_Natural_gas">
    <rdf:type rdf:resource="http://www.w3.org/2002/07/owl#Class"/>
    <rdfs:subClassOf rdf:resource="http://transience.eu/ontologies/Variable"/>
    <rdfs:label>Final Energy|Industry|Steel|Natural gas</rdfs:label>
    <rdfs:comment>Final energy. System boundaries in line with energy accounting</rdfs:comment>
    <ex:unit>PJ/yr</ex:unit>
  </rdf:Description>
  <rdf:Description rdf:about="http://transience.eu/ontologies/Final_Energy_Industry_Other_Sector_Other">
    <rdf:type rdf:resource="http://www.w3.org/2002/07/owl#Class"/>
    <rdfs:subClassOf rdf:resource="http://transience.eu/ontologies/Variable"/>
    <rdfs:label>Final Energy|Industry|Other Sector|Other</rdfs:label>
    <rdfs:comment>Final energy consumption of other energy carriers by other industry sectors (please provide a definition of the energy carriers in this category in the 'comments' tab)</rdfs:comment>
    <ex:unit>EJ/yr</ex:unit>
  </rdf:Description>
  <rdf:Description rdf:about="http://transience.eu/ontologies/Secondary_Energy_Hydrogen">
    <rdf:type rdf:resource="http://www.w3.org/2002/07/owl#Class"/>
    <rdfs:subClassOf rdf:resource="http://transience.eu/ontologies/Variable"/>
    <rdfs:label>Secondary Energy|Hydrogen</rdfs:label>
    <rdfs:comment>total hydrogen production</rdfs:comment>
    <ex:unit>EJ/yr</ex:unit>
  </rdf:Description>
  <rdf:Description rdf:about="http://transience.eu/ontologies/Production_Clinker">
    <rdf:type rdf:resource="http://www.w3.org/2002/07/owl#Class"/>
    <rdfs:subClassOf rdf:resource="http://transience.eu/ontologies/ParameterOutput"/>
    <rdfs:label>Production|Clinker</rdfs:label>
    <rdfs:comment>Clinker productionÂ </rdfs:comment>
    <ex:unit>t/yr</ex:unit>
  </rdf:Description>
  <rdf:Description rdf:about="http://transience.eu/ontologies/Capital_Cost_Liquids_Gas_w__CCS">
    <rdf:type rdf:resource="http://www.w3.org/2002/07/owl#Class"/>
    <rdfs:subClassOf rdf:resource="http://transience.eu/ontologies/Variable"/>
    <rdfs:label>Capital Cost|Liquids|Gas|w/ CCS</rdfs:label>
    <rdfs:comment>Capital cost of a new gas to liquids plant with CCS. If more than one CCS GTL technology is modelled, modellers should report capital costs for each represented CCS GTL technology by adding variables Capital Cost|Liquids|Gas|w/ CCS|2, ... Capital Cost|Liquids|Gas|w/ CCS|N (with N = number of represented technologies). It is modeller's choice which CCS GTL technologies to assign to type 1 (assigned to the variable without number suffix),2,...,N. The assignment should be documented in the comments sheet. </rdfs:comment>
    <ex:unit>US$2010/kW</ex:unit>
  </rdf:Description>
  <rdf:Description rdf:about="http://transience.eu/ontologies/Export_Industry_Non-Ferrous_Metals">
    <rdf:type rdf:resource="http://www.w3.org/2002/07/owl#Class"/>
    <rdfs:subClassOf rdf:resource="http://transience.eu/ontologies/Variable"/>
    <rdfs:label>Export|Industry|Non-Ferrous Metals</rdfs:label>
    <rdfs:comment>Export of non-ferrous metals measured in monetary units</rdfs:comment>
    <ex:unit>billion US$2010/yr</ex:unit>
  </rdf:Description>
  <rdf:Description rdf:about="http://transience.eu/ontologies/Investment_Energy_Supply_Electricity_Gas_w_o_CCS">
    <rdf:type rdf:resource="http://www.w3.org/2002/07/owl#Class"/>
    <rdfs:subClassOf rdf:resource="http://transience.eu/ontologies/Variable"/>
    <rdfs:label>Investment|Energy Supply|Electricity|Gas|w/o CCS</rdfs:label>
    <rdfs:comment>investments in new power generation for the specified power plant category. If the model features several sub-categories, the total investments should be reported. For plants equipped with CCS, the investment in the capturing equipment should be included but not the one on transport and storage.</rdfs:comment>
    <ex:unit>billion US$2010/yr</ex:unit>
  </rdf:Description>
  <rdf:Description rdf:about="http://transience.eu/ontologies/Final_Energy_Industry_Pulp_and_Paper_Gases">
    <rdf:type rdf:resource="http://www.w3.org/2002/07/owl#Class"/>
    <rdfs:subClassOf rdf:resource="http://transience.eu/ontologies/Variable"/>
    <rdfs:label>Final Energy|Industry|Pulp and Paper|Gases</rdfs:label>
    <rdfs:comment>Final energy consumption of gases of the pulp and paper sector (natural gas, biogas, coal-gas), excluding transmission/distribution losses</rdfs:comment>
    <ex:unit>EJ/yr</ex:unit>
  </rdf:Description>
  <rdf:Description rdf:about="http://transience.eu/ontologies/Policy_Cost_Consumption_Loss">
    <rdf:type rdf:resource="http://www.w3.org/2002/07/owl#Class"/>
    <rdfs:subClassOf rdf:resource="http://transience.eu/ontologies/Variable"/>
    <rdfs:label>Policy Cost|Consumption Loss</rdfs:label>
    <rdfs:comment>consumption loss in a policy scenario compared to the corresponding baseline (losses should be reported as positive numbers)</rdfs:comment>
    <ex:unit>billion US$2010/yr</ex:unit>
  </rdf:Description>
  <rdf:Description rdf:about="http://transience.eu/ontologies/Primary_Energy_Coal_w__CCS">
    <rdf:type rdf:resource="http://www.w3.org/2002/07/owl#Class"/>
    <rdfs:subClassOf rdf:resource="http://transience.eu/ontologies/Variable"/>
    <rdfs:label>Primary Energy|Coal|w/ CCS</rdfs:label>
    <rdfs:comment>coal primary energy consumption used in combination with CCS</rdfs:comment>
    <ex:unit>EJ/yr</ex:unit>
  </rdf:Description>
  <rdf:Description rdf:about="http://transience.eu/ontologies/Price_Primary_Energy_Biomass">
    <rdf:type rdf:resource="http://www.w3.org/2002/07/owl#Class"/>
    <rdfs:subClassOf rdf:resource="http://transience.eu/ontologies/Variable"/>
    <rdfs:label>Price|Primary Energy|Biomass</rdfs:label>
    <rdfs:comment>biomass producer price</rdfs:comment>
    <ex:unit>US$2010/GJ</ex:unit>
  </rdf:Description>
  <rdf:Description rdf:about="http://transience.eu/ontologies/Capacity_Petrochemicals_Chemical_Recycling_Gasification">
    <rdf:type rdf:resource="http://www.w3.org/2002/07/owl#Class"/>
    <rdfs:subClassOf rdf:resource="http://transience.eu/ontologies/Variable"/>
    <rdfs:label>Capacity|Petrochemicals|Chemical Recycling|Gasification</rdfs:label>
    <rdfs:comment>Capacity for chemical recycling of plastic wastes via gasification; the value refers to the amount of plastic waste input that can be processed per year</rdfs:comment>
    <ex:unit>Mt plastic waste input / yr</ex:unit>
  </rdf:Description>
  <rdf:Description rdf:about="http://transience.eu/ontologies/Total_Scrap_Iron_and_Steel_Transportation">
    <rdf:type rdf:resource="http://www.w3.org/2002/07/owl#Class"/>
    <rdfs:subClassOf rdf:resource="http://transience.eu/ontologies/Variable"/>
    <rdfs:label>Total Scrap|Iron and Steel|Transportation</rdfs:label>
    <rdfs:comment>Total potential of iron &amp; steel scrap material as a result of end of life products (before collection)</rdfs:comment>
    <ex:unit>Mt/yr</ex:unit>
  </rdf:Description>
  <rdf:Description rdf:about="http://transience.eu/ontologies/Employment_Industry_Manufacturing">
    <rdf:type rdf:resource="http://www.w3.org/2002/07/owl#Class"/>
    <rdfs:subClassOf rdf:resource="http://transience.eu/ontologies/Variable"/>
    <rdfs:label>Employment|Industry|Manufacturing</rdfs:label>
    <rdfs:comment>Number of employed inhabitants (payrolls) in manufacturing industries (based on ILO classification)</rdfs:comment>
    <ex:unit>million</ex:unit>
  </rdf:Description>
  <rdf:Description rdf:about="http://transience.eu/ontologies/Cost_Production_Steel_DRI_EAF_BECCS">
    <rdf:type rdf:resource="http://www.w3.org/2002/07/owl#Class"/>
    <rdfs:subClassOf rdf:resource="http://transience.eu/ontologies/Variable"/>
    <rdfs:label>Cost|Production|Steel|DRI_EAF_BECCS</rdfs:label>
    <rdfs:comment>Specific production cost of crude steel in DRI/EAF route when using biogenic syngas as reducing gas and doing CCS; including CAPEX (annuity), fixed and variable OPEX, including CO2 transport and storage costs</rdfs:comment>
    <ex:unit>Mio â‚¬_2022 / t crude steel</ex:unit>
  </rdf:Description>
  <rdf:Description rdf:about="http://transience.eu/ontologies/Conversion_Input_Hydrogen_Liquids">
    <rdf:type rdf:resource="http://www.w3.org/2002/07/owl#Class"/>
    <rdfs:subClassOf rdf:resource="http://transience.eu/ontologies/Variable"/>
    <rdfs:label>Conversion Input|Hydrogen|Liquids</rdfs:label>
    <rdfs:comment>secondary energy consumption of hydrogen for the production of liquids (synfuels)</rdfs:comment>
    <ex:unit>EJ/yr</ex:unit>
  </rdf:Description>
  <rdf:Description rdf:about="http://transience.eu/ontologies/Import_Industry_Non-Ferrous_Metals_Aluminum">
    <rdf:type rdf:resource="http://www.w3.org/2002/07/owl#Class"/>
    <rdfs:subClassOf rdf:resource="http://transience.eu/ontologies/Variable"/>
    <rdfs:label>Import|Industry|Non-Ferrous Metals|Aluminum</rdfs:label>
    <rdfs:comment>Import of aluminium measured in monetary units</rdfs:comment>
    <ex:unit>billion US$2010/yr</ex:unit>
  </rdf:Description>
  <rdf:Description rdf:about="http://transience.eu/ontologies/Final_Energy_Commercial">
    <rdf:type rdf:resource="http://www.w3.org/2002/07/owl#Class"/>
    <rdfs:subClassOf rdf:resource="http://transience.eu/ontologies/Variable"/>
    <rdfs:label>Final Energy|Commercial</rdfs:label>
    <rdfs:comment>final energy consumed in the commercial sector</rdfs:comment>
    <ex:unit>EJ/yr</ex:unit>
  </rdf:Description>
  <rdf:Description rdf:about="http://transience.eu/ontologies/Energy_Service_Transportation_Freight_Domestic_Navigation">
    <rdf:type rdf:resource="http://www.w3.org/2002/07/owl#Class"/>
    <rdfs:subClassOf rdf:resource="http://transience.eu/ontologies/Variable"/>
    <rdfs:label>Energy Service|Transportation|Freight|Domestic Navigation</rdfs:label>
    <rdfs:comment>energy service demand for freight transport on domestic ships</rdfs:comment>
    <ex:unit>bn tkm/yr</ex:unit>
  </rdf:Description>
  <rdf:Description rdf:about="http://transience.eu/ontologies/Final_Energy_Commercial_Gases">
    <rdf:type rdf:resource="http://www.w3.org/2002/07/owl#Class"/>
    <rdfs:subClassOf rdf:resource="http://transience.eu/ontologies/Variable"/>
    <rdfs:label>Final Energy|Commercial|Gases</rdfs:label>
    <rdfs:comment>final energy consumption by the commercial sector of gases (natural gas, biogas, coal-gas), excluding transmission/distribution losses</rdfs:comment>
    <ex:unit>EJ/yr</ex:unit>
  </rdf:Description>
  <rdf:Description rdf:about="http://transience.eu/ontologies/Carbon_Capture_Storage_Biomass_Energy_Supply_Other">
    <rdf:type rdf:resource="http://www.w3.org/2002/07/owl#Class"/>
    <rdfs:subClassOf rdf:resource="http://transience.eu/ontologies/Variable"/>
    <rdfs:label>Carbon Capture|Storage|Biomass|Energy|Supply|Other</rdfs:label>
    <rdfs:comment>total carbon dioxide emissions captured from bioenergy use in other energy supply (part of IPCC category 1A) and stored in geological deposits (e.g. in depleted oil and gas fields, unmined coal seams, saline aquifers) and the deep ocean, stored amounts should be reported as positive numbers</rdfs:comment>
    <ex:unit>Mt CO2/yr</ex:unit>
  </rdf:Description>
  <rdf:Description rdf:about="http://transience.eu/ontologies/Secondary_Energy_Electricity_Gas_w_o_CCS">
    <rdf:type rdf:resource="http://www.w3.org/2002/07/owl#Class"/>
    <rdfs:subClassOf rdf:resource="http://transience.eu/ontologies/Variable"/>
    <rdfs:label>Secondary Energy|Electricity|Gas|w/o CCS</rdfs:label>
    <rdfs:comment>net electricity production from natural gas with freely vented CO2 emissions</rdfs:comment>
    <ex:unit>EJ/yr</ex:unit>
  </rdf:Description>
  <rdf:Description rdf:about="http://transience.eu/ontologies/Secondary_Energy_Liquids_Biomass_Energy_Crops">
    <rdf:type rdf:resource="http://www.w3.org/2002/07/owl#Class"/>
    <rdfs:subClassOf rdf:resource="http://transience.eu/ontologies/Variable"/>
    <rdfs:label>Secondary Energy|Liquids|Biomass|Energy Crops</rdfs:label>
    <rdfs:comment>liquid biofuels production from energy crops</rdfs:comment>
    <ex:unit>EJ/yr</ex:unit>
  </rdf:Description>
  <rdf:Description rdf:about="http://transience.eu/ontologies/Final_Energy_Non-Energy_Use_Liquids_Biomass">
    <rdf:type rdf:resource="http://www.w3.org/2002/07/owl#Class"/>
    <rdfs:subClassOf rdf:resource="http://transience.eu/ontologies/Variable"/>
    <rdfs:label>Final Energy|Non-Energy Use|Liquids|Biomass</rdfs:label>
    <rdfs:comment>Final energy consumption of liquid biofuels by the non-combustion processes</rdfs:comment>
    <ex:unit>EJ/yr</ex:unit>
  </rdf:Description>
  <rdf:Description rdf:about="http://transience.eu/ontologies/Investment_Infrastructure">
    <rdf:type rdf:resource="http://www.w3.org/2002/07/owl#Class"/>
    <rdfs:subClassOf rdf:resource="http://transience.eu/ontologies/Variable"/>
    <rdfs:label>Investment|Infrastructure</rdfs:label>
    <rdfs:comment>investment into infrastrucutre</rdfs:comment>
    <ex:unit>billion US$2010/yr</ex:unit>
  </rdf:Description>
  <rdf:Description rdf:about="http://transience.eu/ontologies/Primary_Energy_Biomass_Traditional">
    <rdf:type rdf:resource="http://www.w3.org/2002/07/owl#Class"/>
    <rdfs:subClassOf rdf:resource="http://transience.eu/ontologies/Variable"/>
    <rdfs:label>Primary Energy|Biomass|Traditional</rdfs:label>
    <rdfs:comment>traditional biomass primary energy consumption</rdfs:comment>
    <ex:unit>EJ/yr</ex:unit>
  </rdf:Description>
  <rdf:Description rdf:about="http://transience.eu/ontologies/Production_Petrochemicals_Polymers">
    <rdf:type rdf:resource="http://www.w3.org/2002/07/owl#Class"/>
    <rdfs:subClassOf rdf:resource="http://transience.eu/ontologies/Variable"/>
    <rdfs:label>Production|Petrochemicals|Polymers</rdfs:label>
    <rdfs:comment>Production of Polymers</rdfs:comment>
    <ex:unit>Mt/yr</ex:unit>
  </rdf:Description>
  <rdf:Description rdf:about="http://transience.eu/ontologies/Export_Agriculture">
    <rdf:type rdf:resource="http://www.w3.org/2002/07/owl#Class"/>
    <rdfs:subClassOf rdf:resource="http://transience.eu/ontologies/Variable"/>
    <rdfs:label>Export|Agriculture</rdfs:label>
    <rdfs:comment>export of agricultural commodities measured in monetary units.</rdfs:comment>
    <ex:unit>billion US$2010/yr</ex:unit>
  </rdf:Description>
  <rdf:Description rdf:about="http://transience.eu/ontologies/Investment_Energy_Supply_Electricity_Coal_w_o_CCS">
    <rdf:type rdf:resource="http://www.w3.org/2002/07/owl#Class"/>
    <rdfs:subClassOf rdf:resource="http://transience.eu/ontologies/Variable"/>
    <rdfs:label>Investment|Energy Supply|Electricity|Coal|w/o CCS</rdfs:label>
    <rdfs:comment>investments in new power generation for the specified power plant category. If the model features several sub-categories, the total investments should be reported. For plants equipped with CCS, the investment in the capturing equipment should be included but not the one on transport and storage.</rdfs:comment>
    <ex:unit>billion US$2010/yr</ex:unit>
  </rdf:Description>
  <rdf:Description rdf:about="http://transience.eu/ontologies/OM_Cost_Fixed_Electricity_Solar_CSP">
    <rdf:type rdf:resource="http://www.w3.org/2002/07/owl#Class"/>
    <rdfs:subClassOf rdf:resource="http://transience.eu/ontologies/Variable"/>
    <rdfs:label>OM Cost|Fixed|Electricity|Solar|CSP</rdfs:label>
    <rdfs:comment>Annual fixed operation &amp; maintainance cost of a new concentrated solar power plant. If more than one CSP technology is modelled (e.g., parabolic trough, solar power tower), modellers should report fixed O&amp;M costs  for each represented CSP technology by adding variables OM Cost|Fixed|Electricity|Solar|CSP|2, ... Capital|Cost|Electricity|Solar|CSP|N (with N = number of represented CSP technologies) (matching the assignment of plant types to technologies in the reporting of capital costs as documented in the comments sheet).</rdfs:comment>
    <ex:unit>US$2010/kW/yr</ex:unit>
  </rdf:Description>
  <rdf:Description rdf:about="http://transience.eu/ontologies/Import_Industry_Non-Ferrous_Metals">
    <rdf:type rdf:resource="http://www.w3.org/2002/07/owl#Class"/>
    <rdfs:subClassOf rdf:resource="http://transience.eu/ontologies/Variable"/>
    <rdfs:label>Import|Industry|Non-Ferrous Metals</rdfs:label>
    <rdfs:comment>Import of non-ferrous metals measured in monetary units</rdfs:comment>
    <ex:unit>billion US$2010/yr</ex:unit>
  </rdf:Description>
  <rdf:Description rdf:about="http://transience.eu/ontologies/Carbon_Capture_Industry_Electricity">
    <rdf:type rdf:resource="http://www.w3.org/2002/07/owl#Class"/>
    <rdfs:subClassOf rdf:resource="http://transience.eu/ontologies/Variable"/>
    <rdfs:label>Carbon Capture|Industry|Electricity</rdfs:label>
    <rdfs:comment>total carbon dioxide emissions from hydrogen or synthetic fuel use captured in industry sector</rdfs:comment>
    <ex:unit>Mt CO2/yr</ex:unit>
  </rdf:Description>
  <rdf:Description rdf:about="http://transience.eu/ontologies/Final_Energy_Industry_Iron_and_Steel_Solids">
    <rdf:type rdf:resource="http://www.w3.org/2002/07/owl#Class"/>
    <rdfs:subClassOf rdf:resource="http://transience.eu/ontologies/Variable"/>
    <rdfs:label>Final Energy|Industry|Iron and Steel|Solids</rdfs:label>
    <rdfs:comment>Final energy solid fuel consumption by the iron and steel sector (including coal and solid biomass)</rdfs:comment>
    <ex:unit>EJ/yr</ex:unit>
  </rdf:Description>
  <rdf:Description rdf:about="http://transience.eu/ontologies/Final_Energy_Transportation_Liquids_Electricity">
    <rdf:type rdf:resource="http://www.w3.org/2002/07/owl#Class"/>
    <rdfs:subClassOf rdf:resource="http://transience.eu/ontologies/Variable"/>
    <rdfs:label>Final Energy|Transportation|Liquids|Electricity</rdfs:label>
    <rdfs:comment>final energy consumption by the transportation sector of synthetic liquid efuels</rdfs:comment>
    <ex:unit>EJ/yr</ex:unit>
  </rdf:Description>
  <rdf:Description rdf:about="http://transience.eu/ontologies/Carbon_Capture_Storage_Biomass_Energy_Supply">
    <rdf:type rdf:resource="http://www.w3.org/2002/07/owl#Class"/>
    <rdfs:subClassOf rdf:resource="http://transience.eu/ontologies/Variable"/>
    <rdfs:label>Carbon Capture|Storage|Biomass|Energy|Supply</rdfs:label>
    <rdfs:comment>total carbon dioxide emissions captured  from bioenergy use and stored in geological deposits (e.g. in depleted oil and gas fields, unmined coal seams, saline aquifers) and the deep ocean, stored amounts should be reported as positive numbers</rdfs:comment>
    <ex:unit>Mt CO2/yr</ex:unit>
  </rdf:Description>
  <rdf:Description rdf:about="http://transience.eu/ontologies/Capital_Cost_Electricity_Solar_PV">
    <rdf:type rdf:resource="http://www.w3.org/2002/07/owl#Class"/>
    <rdfs:subClassOf rdf:resource="http://transience.eu/ontologies/Variable"/>
    <rdfs:label>Capital Cost|Electricity|Solar|PV</rdfs:label>
    <rdfs:comment>Capital cost of a new solar PV units. If more than one PV technology is modelled (e.g., centralized PV plant, distributed (rooftop) PV, crystalline SI PV, thin-film PV), modellers should report capital costs for each represented PV technology by adding variables Capital Cost|Electricity|Solar|PV|2, ... Capital|Cost|Electricity|Solar|PV|N (with N = number of represented PV technologies). It is modeller's choice which PV technologies to assign to type 1 (assigned to the variable without number suffix),2,...,N. The assignment should be documented in the comments sheet. </rdfs:comment>
    <ex:unit>US$2010/kW</ex:unit>
  </rdf:Description>
  <rdf:Description rdf:about="http://transience.eu/ontologies/Carbon_Capture_Storage_Fossil_Energy_Supply_Gases">
    <rdf:type rdf:resource="http://www.w3.org/2002/07/owl#Class"/>
    <rdfs:subClassOf rdf:resource="http://transience.eu/ontologies/Variable"/>
    <rdfs:label>Carbon Capture|Storage|Fossil|Energy|Supply|Gases</rdfs:label>
    <rdfs:comment>total carbon dioxide emissions captured from fossil fuel use in gaseous fuel production, excl. hydrogen (part of IPCC category 1A) and stored in geological deposits (e.g. in depleted oil and gas fields, unmined coal seams, saline aquifers) and the deep ocean, stored amounts should be reported as positive numbers</rdfs:comment>
    <ex:unit>Mt CO2/yr</ex:unit>
  </rdf:Description>
  <rdf:Description rdf:about="http://transience.eu/ontologies/Capital_Cost_Electricity_Gas_w_o_CCS">
    <rdf:type rdf:resource="http://www.w3.org/2002/07/owl#Class"/>
    <rdfs:subClassOf rdf:resource="http://transience.eu/ontologies/Variable"/>
    <rdfs:label>Capital Cost|Electricity|Gas|w/o CCS</rdfs:label>
    <rdfs:comment>Capital cost of a new gas power plant w/o CCS. If more than one gas power technology is modelled, modellers should report capital costs for each represented gas power technology by adding variables Capital Cost|Electricity|Gas|w/o CCS|2, ... Capital Cost|Electricity|Gas|w/o CCS|N (with N = number of represented technologies). It is modeller's choice which gas power technologies to assign to type 1 (assigned to the variable without number suffix),2,...,N. The assignment should be documented in the comments sheet. </rdfs:comment>
    <ex:unit>US$2010/kW</ex:unit>
  </rdf:Description>
  <rdf:Description rdf:about="http://transience.eu/ontologies/Investment_Energy_Supply_Electricity_Gas">
    <rdf:type rdf:resource="http://www.w3.org/2002/07/owl#Class"/>
    <rdfs:subClassOf rdf:resource="http://transience.eu/ontologies/Variable"/>
    <rdfs:label>Investment|Energy Supply|Electricity|Gas</rdfs:label>
    <rdfs:comment>investments in new power generation for the specified power plant category. If the model features several sub-categories, the total investments should be reported. For plants equipped with CCS, the investment in the capturing equipment should be included but not the one on transport and storage.</rdfs:comment>
    <ex:unit>billion US$2010/yr</ex:unit>
  </rdf:Description>
  <rdf:Description rdf:about="http://transience.eu/ontologies/Carbon_Capture_Usage_Materials_Short-lived">
    <rdf:type rdf:resource="http://www.w3.org/2002/07/owl#Class"/>
    <rdfs:subClassOf rdf:resource="http://transience.eu/ontologies/Variable"/>
    <rdfs:label>Carbon Capture|Usage|Materials|Short-lived</rdfs:label>
    <rdfs:comment>total carbon dioxide captured and used in short-lived materials (e.g. plastics)</rdfs:comment>
    <ex:unit>Mt CO2/yr</ex:unit>
  </rdf:Description>
  <rdf:Description rdf:about="http://transience.eu/ontologies/Secondary_Energy_Electricity_Solar_CSP">
    <rdf:type rdf:resource="http://www.w3.org/2002/07/owl#Class"/>
    <rdfs:subClassOf rdf:resource="http://transience.eu/ontologies/Variable"/>
    <rdfs:label>Secondary Energy|Electricity|Solar|CSP</rdfs:label>
    <rdfs:comment>net electricity production from concentrating solar power (CSP)</rdfs:comment>
    <ex:unit>EJ/yr</ex:unit>
  </rdf:Description>
  <rdf:Description rdf:about="http://transience.eu/ontologies/Primary_Energy_Gas_Electricity_w_o_CCS">
    <rdf:type rdf:resource="http://www.w3.org/2002/07/owl#Class"/>
    <rdfs:subClassOf rdf:resource="http://transience.eu/ontologies/Variable"/>
    <rdfs:label>Primary Energy|Gas|Electricity|w/o CCS</rdfs:label>
    <rdfs:comment>gas primary energy input to electricity generation without CCS</rdfs:comment>
    <ex:unit>EJ/yr</ex:unit>
  </rdf:Description>
  <rdf:Description rdf:about="http://transience.eu/ontologies/Collected_Scrap_Non-Ferrous_Metals">
    <rdf:type rdf:resource="http://www.w3.org/2002/07/owl#Class"/>
    <rdfs:subClassOf rdf:resource="http://transience.eu/ontologies/Variable"/>
    <rdfs:label>Collected Scrap|Non-Ferrous Metals</rdfs:label>
    <rdfs:comment>Collected non-ferrou metals scrap</rdfs:comment>
    <ex:unit>Mt/yr</ex:unit>
  </rdf:Description>
  <rdf:Description rdf:about="http://transience.eu/ontologies/OM_Cost_Fixed_Gases_Biomass_w__CCS">
    <rdf:type rdf:resource="http://www.w3.org/2002/07/owl#Class"/>
    <rdfs:subClassOf rdf:resource="http://transience.eu/ontologies/Variable"/>
    <rdfs:label>OM Cost|Fixed|Gases|Biomass|w/ CCS</rdfs:label>
    <rdfs:comment>Annual fixed operation &amp; maintainance cost of a new biomass to gas plant with CCS. If more than one CCS biomass to gas technology is modelled, modellers should report fixed O&amp;M costs  for each represented CCS biomass to  gas technology by adding variables OM Cost|Fixed|Gases|Biomass|w/ CCS|2, ... OM Cost|Fixed|Gases|Biomass|w/ CCS|N (with N = number of represented technologies). (matching the assignment of plant types to technologies in the reporting of capital costs as documented in the comments sheet).</rdfs:comment>
    <ex:unit>US$2010/kW/yr</ex:unit>
  </rdf:Description>
  <rdf:Description rdf:about="http://transience.eu/ontologies/Secondary_Energy_Hydrogen_Fossil">
    <rdf:type rdf:resource="http://www.w3.org/2002/07/owl#Class"/>
    <rdfs:subClassOf rdf:resource="http://transience.eu/ontologies/Variable"/>
    <rdfs:label>Secondary Energy|Hydrogen|Fossil</rdfs:label>
    <rdfs:comment>hydrogen production from fossil fuels</rdfs:comment>
    <ex:unit>EJ/yr</ex:unit>
  </rdf:Description>
  <rdf:Description rdf:about="http://transience.eu/ontologies/Price_Secondary_Energy_Hydrogen">
    <rdf:type rdf:resource="http://www.w3.org/2002/07/owl#Class"/>
    <rdfs:subClassOf rdf:resource="http://transience.eu/ontologies/Variable"/>
    <rdfs:label>Price|Secondary Energy|Hydrogen</rdfs:label>
    <rdfs:comment>hydrogen price at the secondary level. Prices should include the effect of carbon prices</rdfs:comment>
    <ex:unit>US$2010/GJ</ex:unit>
  </rdf:Description>
  <rdf:Description rdf:about="http://transience.eu/ontologies/Primary_Energy_Nuclear">
    <rdf:type rdf:resource="http://www.w3.org/2002/07/owl#Class"/>
    <rdfs:subClassOf rdf:resource="http://transience.eu/ontologies/Variable"/>
    <rdfs:label>Primary Energy|Nuclear</rdfs:label>
    <rdfs:comment>nuclear primary energy consumption (direct equivalent, includes electricity, heat and hydrogen production from nuclear energy)</rdfs:comment>
    <ex:unit>EJ/yr</ex:unit>
  </rdf:Description>
  <rdf:Description rdf:about="http://transience.eu/ontologies/Lifetime_Hydrogen_Gas_w_o_CCS">
    <rdf:type rdf:resource="http://www.w3.org/2002/07/owl#Class"/>
    <rdfs:subClassOf rdf:resource="http://transience.eu/ontologies/Variable"/>
    <rdfs:label>Lifetime|Hydrogen|Gas|w/o CCS</rdfs:label>
    <rdfs:comment>Lifetime of a new gas to hydrogen plant w/o CCS. Lifetime should be calculated by summing all vintages of a  capacity unit (e.g. (1+1+0.9+0.7+0.5) * 10 years = 41 years) or by the e-folding time for exponential capacity depreciation.  The lifetime should refer to the plant type(s) for which capital costs have been reported. If capital cost for more than one plant type has been reported, modellers should report lifetime for the additional plant types by adding variables Lifetime|Hydrogen|Gas|w/o CCS|2, ... Lifetime|Hydrogen|Gas|w/o CCS|N (matching the assignment of plant types to technologies in the reporting of capital costs as documented in the comments sheet). </rdfs:comment>
    <ex:unit>years</ex:unit>
  </rdf:Description>
  <rdf:Description rdf:about="http://transience.eu/ontologies/Efficiency_Electricity_Coal_w__CCS">
    <rdf:type rdf:resource="http://www.w3.org/2002/07/owl#Class"/>
    <rdfs:subClassOf rdf:resource="http://transience.eu/ontologies/Variable"/>
    <rdfs:label>Efficiency|Electricity|Coal|w/ CCS</rdfs:label>
    <rdfs:comment>Conversion efficiency (electricity produced per unit of primary energy input) of a new coal power plant with CCS. The efficiency should refer to the plant type(s) for which capital costs have been reported. If capital cost for more than one plant type has been reported, modellers should report efficiency for the additional plant types by adding variables Efficiency|Electricity|Coal|w/ CCS|2, ... Efficiency|Electricity|Coal|w/ CCS|N (matching the assignment of plant types to technologies in the reporting of capital costs as documented in the comments sheet). </rdfs:comment>
    <ex:unit>%</ex:unit>
  </rdf:Description>
  <rdf:Description rdf:about="http://transience.eu/ontologies/Secondary_Energy_Liquids_Biomass_w_o_CCS">
    <rdf:type rdf:resource="http://www.w3.org/2002/07/owl#Class"/>
    <rdfs:subClassOf rdf:resource="http://transience.eu/ontologies/Variable"/>
    <rdfs:label>Secondary Energy|Liquids|Biomass|w/o CCS</rdfs:label>
    <rdfs:comment>total production of liquid biofuels from facilities without CCS</rdfs:comment>
    <ex:unit>EJ/yr</ex:unit>
  </rdf:Description>
  <rdf:Description rdf:about="http://transience.eu/ontologies/Tariffs_Average">
    <rdf:type rdf:resource="http://www.w3.org/2002/07/owl#Class"/>
    <rdfs:subClassOf rdf:resource="http://transience.eu/ontologies/Variable"/>
    <rdfs:label>Tariffs|Average</rdfs:label>
    <rdfs:comment>Weighted trade tariff-average (regional and global indicator relevant)</rdfs:comment>
    <ex:unit>%</ex:unit>
  </rdf:Description>
  <rdf:Description rdf:about="http://transience.eu/ontologies/Final_Energy_Industry_Chemicals_Liquids_Fossil">
    <rdf:type rdf:resource="http://www.w3.org/2002/07/owl#Class"/>
    <rdfs:subClassOf rdf:resource="http://transience.eu/ontologies/Variable"/>
    <rdfs:label>Final Energy|Industry|Chemicals|Liquids|Fossil</rdfs:label>
    <rdfs:comment>Final energy consumption of liquids of fossil origin by the chemicals sector</rdfs:comment>
    <ex:unit>EJ/yr</ex:unit>
  </rdf:Description>
  <rdf:Description rdf:about="http://transience.eu/ontologies/Efficiency_Hydrogen_Gas_w__CCS">
    <rdf:type rdf:resource="http://www.w3.org/2002/07/owl#Class"/>
    <rdfs:subClassOf rdf:resource="http://transience.eu/ontologies/Variable"/>
    <rdfs:label>Efficiency|Hydrogen|Gas|w/ CCS</rdfs:label>
    <rdfs:comment>Conversion efficiency (energy content of hydrogen produced per unit of primary energy input) of a new gas to hydrogen plant with CCS. The efficiency should refer to the plant type(s) for which capital costs have been reported. If capital cost for more than one plant type has been reported, modellers should report efficiency for the additional plant types by adding variables Efficiency|Hydrogen|Gas|w/ CCS|2, ... Efficiency|Hydrogen|Gas|w/ CCS|N (matching the assignment of plant types to technologies in the reporting of capital costs as documented in the comments sheet). </rdfs:comment>
    <ex:unit>%</ex:unit>
  </rdf:Description>
  <rdf:Description rdf:about="http://transience.eu/ontologies/Trade_Secondary_Energy_Liquids_Gas_Volume">
    <rdf:type rdf:resource="http://www.w3.org/2002/07/owl#Class"/>
    <rdfs:subClassOf rdf:resource="http://transience.eu/ontologies/Variable"/>
    <rdfs:label>Trade|Secondary Energy|Liquids|Gas|Volume</rdfs:label>
    <rdfs:comment>net exports of fossil liquid synfuels from gas-to-liquids (GTL) technologies, at the global level these should add up to the trade losses only</rdfs:comment>
    <ex:unit>EJ/yr</ex:unit>
  </rdf:Description>
  <rdf:Description rdf:about="http://transience.eu/ontologies/Efficiency_Liquids_Coal_w_o_CCS">
    <rdf:type rdf:resource="http://www.w3.org/2002/07/owl#Class"/>
    <rdfs:subClassOf rdf:resource="http://transience.eu/ontologies/Variable"/>
    <rdfs:label>Efficiency|Liquids|Coal|w/o CCS</rdfs:label>
    <rdfs:comment>Conversion efficiency (energy content of liquids produced per unit of primary energy input) of a new coal to liquids plant w/o CCS. The efficiency should refer to the plant type(s) for which capital costs have been reported. If capital cost for more than one plant type has been reported, modellers should report efficiency for the additional plant types by adding variables Efficiency|Liquids|Coal|w/o CCS|2, ... Efficiency|Liquids|Coal|w/o CCS|N (matching the assignment of plant types to technologies in the reporting of capital costs as documented in the comments sheet). </rdfs:comment>
    <ex:unit>%</ex:unit>
  </rdf:Description>
  <rdf:Description rdf:about="http://transience.eu/ontologies/Primary_Energy_Industry_Steel_Biomass">
    <rdf:type rdf:resource="http://www.w3.org/2002/07/owl#Class"/>
    <rdfs:subClassOf rdf:resource="http://transience.eu/ontologies/Variable"/>
    <rdfs:label>Primary Energy|Industry|Steel|Biomass</rdfs:label>
    <rdfs:comment>Energy demand including own coke ovens and autoproduction of electricity</rdfs:comment>
    <ex:unit>PJ/yr</ex:unit>
  </rdf:Description>
</rdf:RDF>
